@prefix bibo:     <http://purl.org/ontology/bibo/> .
@prefix data:     <http://advworks.example.org/data/> .
@prefix dcat:     <http://www.w3.org/ns/dcat#> .
@prefix dcmitype: <http://purl.org/dc/dcmitype/> .
@prefix dct:      <http://purl.org/dc/terms/> .
@prefix foaf:     <http://xmlns.com/foaf/0.1/> .
@prefix geo:      <http://www.opengis.net/ont/geosparql#> .
@prefix owl:      <http://www.w3.org/2002/07/owl#> .
@prefix rdf:      <http://www.w3.org/1999/02/22-rdf-syntax-ns#> .
@prefix rdfs:     <http://www.w3.org/2000/01/rdf-schema#> .
@prefix schema:   <http://schema.org/> .
@prefix skos:     <http://www.w3.org/2004/02/skos/core#> .
@prefix voc:      <http://advworks.example.org/voc/> .
@prefix void:     <http://rdfs.org/ns/void#> .
@prefix xsd:      <http://www.w3.org/2001/XMLSchema#> .

schema:Sculpture  rdf:type  rdfs:Class ;
        rdfs:comment     "A piece of sculpture." ;
        rdfs:label       "Sculpture" ;
        rdfs:subClassOf  schema:CreativeWork .

schema:contentRating  rdf:type  rdf:Property ;
        rdfs:comment  "Official rating of a piece of content&#x2014;for example,'MPAA PG-13'." ;
        rdfs:label    "contentRating" .

schema:Recipe  rdf:type  rdfs:Class ;
        rdfs:comment     "A recipe. For dietary restrictions covered by the recipe, a few common restrictions are enumerated via [[suitableForDiet]]. The [[keywords]] property can also be used to add more detail." ;
        rdfs:label       "Recipe" ;
        rdfs:subClassOf  schema:HowTo .

schema:Brand  rdf:type   rdfs:Class ;
        rdfs:comment     "A brand is a name used by an organization or business person for labeling a product, product group, or similar." ;
        rdfs:label       "Brand" ;
        rdfs:subClassOf  schema:Intangible .

schema:creator  rdf:type  rdf:Property ;
        rdfs:comment  "The creator/author of this CreativeWork. This is the same as the Author property for CreativeWork." ;
        rdfs:label    "creator" .

schema:Barcode  rdf:type  rdfs:Class ;
        rdfs:comment     "An image of a visual machine-readable code such as a barcode or QR code." ;
        rdfs:label       "Barcode" ;
        rdfs:subClassOf  schema:ImageObject .

schema:ReturnAction  rdf:type  rdfs:Class ;
        rdfs:comment     "The act of returning to the origin that which was previously received (concrete objects) or taken (ownership)." ;
        rdfs:label       "ReturnAction" ;
        rdfs:subClassOf  schema:TransferAction .

schema:departureStation
        rdf:type      rdf:Property ;
        rdfs:comment  "The station from which the train departs." ;
        rdfs:label    "departureStation" .

schema:PathologyTest  rdf:type  rdfs:Class ;
        rdfs:comment     "A medical test performed by a laboratory that typically involves examination of a tissue sample by a pathologist." ;
        rdfs:label       "PathologyTest" ;
        rdfs:subClassOf  schema:MedicalTest .

schema:Nerve  rdf:type   rdfs:Class ;
        rdfs:comment     "A common pathway for the electrochemical nerve impulses that are transmitted along each of the axons." ;
        rdfs:label       "Nerve" ;
        rdfs:subClassOf  schema:AnatomicalStructure .

schema:sdPublisher  rdf:type  rdf:Property ;
        rdfs:comment  "Indicates the party responsible for generating and publishing the current structured data markup, typically in cases where the structured data is derived automatically from existing published content but published on a different site. For example, student projects and open data initiatives often re-publish existing content with more explicitly structured metadata. The\n[[sdPublisher]] property helps make such practices more explicit." ;
        rdfs:label    "sdPublisher" .

schema:trackingUrl  rdf:type  rdf:Property ;
        rdfs:comment  "Tracking url for the parcel delivery." ;
        rdfs:label    "trackingUrl" .

schema:suitableForDiet
        rdf:type      rdf:Property ;
        rdfs:comment  "Indicates a dietary restriction or guideline for which this recipe or menu item is suitable, e.g. diabetic, halal etc." ;
        rdfs:label    "suitableForDiet" .

schema:linkRelationship
        rdf:type      rdf:Property ;
        rdfs:comment  "Indicates the relationship type of a Web link. " ;
        rdfs:label    "linkRelationship" .

schema:foodEvent  rdf:type  rdf:Property ;
        rdfs:comment        "A sub property of location. The specific food event where the action occurred." ;
        rdfs:label          "foodEvent" ;
        rdfs:subPropertyOf  schema:location .

schema:course  rdf:type     rdf:Property ;
        rdfs:comment        "A sub property of location. The course where this action was taken." ;
        rdfs:label          "course" ;
        rdfs:subPropertyOf  schema:location .

schema:Optometric  rdf:type  rdfs:Class ;
        rdfs:comment     "The science or practice of testing visual acuity and prescribing corrective lenses." ;
        rdfs:label       "Optometric" ;
        rdfs:subClassOf  schema:MedicalBusiness .

schema:CookAction  rdf:type  rdfs:Class ;
        rdfs:comment     "The act of producing/preparing food." ;
        rdfs:label       "CookAction" ;
        rdfs:subClassOf  schema:CreateAction .

schema:maximumAttendeeCapacity
        rdf:type      rdf:Property ;
        rdfs:comment  "The total number of individuals that may attend an event or venue." ;
        rdfs:label    "maximumAttendeeCapacity" .

schema:ViewAction  rdf:type  rdfs:Class ;
        rdfs:comment     "The act of consuming static visual content." ;
        rdfs:label       "ViewAction" ;
        rdfs:subClassOf  schema:ConsumeAction .

schema:firstPerformance
        rdf:type      rdf:Property ;
        rdfs:comment  "The date and place the work was first performed." ;
        rdfs:label    "firstPerformance" .

schema:bitrate  rdf:type  rdf:Property ;
        rdfs:comment  "The bitrate of the media object." ;
        rdfs:label    "bitrate" .

schema:MusicVideoObject
        rdf:type         rdfs:Class ;
        rdfs:comment     "A music video file." ;
        rdfs:label       "MusicVideoObject" ;
        rdfs:subClassOf  schema:MediaObject .

schema:paymentStatus  rdf:type  rdf:Property ;
        rdfs:comment  "The status of payment; whether the invoice has been paid or not." ;
        rdfs:label    "paymentStatus" .

schema:manufacturer  rdf:type  rdf:Property ;
        rdfs:comment  "The manufacturer of the product." ;
        rdfs:label    "manufacturer" .

schema:Dermatology  rdf:type  rdfs:Class ;
        rdfs:comment     "A specific branch of medical science that pertains to diagnosis and treatment of disorders of skin." ;
        rdfs:label       "Dermatology" ;
        rdfs:subClassOf  schema:MedicalBusiness .

schema:author  rdf:type  rdf:Property ;
        rdfs:comment  "The author of this content or rating. Please note that author is special in that HTML 5 provides a special mechanism for indicating authorship via the rel tag. That is equivalent to this and may be used interchangeably." ;
        rdfs:label    "author" .

schema:ReviewNewsArticle
        rdf:type         rdfs:Class ;
        rdfs:comment     "A [[NewsArticle]] and [[CriticReview]] providing a professional critic's assessment of a service, product, performance, or artistic or literary work." ;
        rdfs:label       "ReviewNewsArticle" ;
        rdfs:subClassOf  schema:CriticReview , schema:NewsArticle .

schema:AmpStory  rdf:type  rdfs:Class ;
        rdfs:comment     "A creative work with a visual storytelling format intended to be viewed online, particularly on mobile devices." ;
        rdfs:label       "AmpStory" ;
        rdfs:subClassOf  schema:CreativeWork .

schema:UserInteraction
        rdf:type         rdfs:Class ;
        rdfs:comment     "UserInteraction and its subtypes is an old way of talking about users interacting with pages. It is generally better to use [[Action]]-based vocabulary, alongside types such as [[Comment]]." ;
        rdfs:label       "UserInteraction" ;
        rdfs:subClassOf  schema:Event .

schema:OrderStatus  rdf:type  rdfs:Class ;
        rdfs:comment     "Enumerated status values for Order." ;
        rdfs:label       "OrderStatus" ;
        rdfs:subClassOf  schema:StatusEnumeration .

schema:nonEqual  rdf:type  rdf:Property ;
        rdfs:comment  "This ordering relation for qualitative values indicates that the subject is not equal to the object." ;
        rdfs:label    "nonEqual" .

schema:School  rdf:type  rdfs:Class ;
        rdfs:comment     "A school." ;
        rdfs:label       "School" ;
        rdfs:subClassOf  schema:EducationalOrganization .

schema:BusinessFunction
        rdf:type         rdfs:Class ;
        rdfs:comment     "The business function specifies the type of activity or access (i.e., the bundle of rights) offered by the organization or business person through the offer. Typical are sell, rental or lease, maintenance or repair, manufacture / produce, recycle / dispose, engineering / construction, or installation. Proprietary specifications of access rights are also instances of this class.\\n\\nCommonly used values:\\n\\n* http://purl.org/goodrelations/v1#ConstructionInstallation\\n* http://purl.org/goodrelations/v1#Dispose\\n* http://purl.org/goodrelations/v1#LeaseOut\\n* http://purl.org/goodrelations/v1#Maintain\\n* http://purl.org/goodrelations/v1#ProvideService\\n* http://purl.org/goodrelations/v1#Repair\\n* http://purl.org/goodrelations/v1#Sell\\n* http://purl.org/goodrelations/v1#Buy\n        " ;
        rdfs:label       "BusinessFunction" ;
        rdfs:subClassOf  schema:Enumeration .

schema:recipient  rdf:type  rdf:Property ;
        rdfs:comment        "A sub property of participant. The participant who is at the receiving end of the action." ;
        rdfs:label          "recipient" ;
        rdfs:subPropertyOf  schema:participant .

schema:reviewAspect  rdf:type  rdf:Property ;
        rdfs:comment  "This Review or Rating is relevant to this part or facet of the itemReviewed." ;
        rdfs:label    "reviewAspect" .

schema:step  rdf:type  rdf:Property ;
        rdfs:comment  "A single step item (as HowToStep, text, document, video, etc.) or a HowToSection." ;
        rdfs:label    "step" .

schema:children  rdf:type  rdf:Property ;
        rdfs:comment  "A child of the person." ;
        rdfs:label    "children" .

schema:proteinContent
        rdf:type      rdf:Property ;
        rdfs:comment  "The number of grams of protein." ;
        rdfs:label    "proteinContent" .

schema:applicantLocationRequirements
        rdf:type      rdf:Property ;
        rdfs:comment  "The location(s) applicants can apply from. This is usually used for telecommuting jobs where the applicant does not need to be in a physical office. Note: This should not be used for citizenship or work visa requirements." ;
        rdfs:label    "applicantLocationRequirements" .

schema:RegisterAction
        rdf:type         rdfs:Class ;
        rdfs:comment     "The act of registering to be a user of a service, product or web page.\\n\\nRelated actions:\\n\\n* [[JoinAction]]: Unlike JoinAction, RegisterAction implies you are registering to be a user of a service, *not* a group/team of people.\\n* [FollowAction]]: Unlike FollowAction, RegisterAction doesn't imply that the agent is expecting to poll for updates from the object.\\n* [[SubscribeAction]]: Unlike SubscribeAction, RegisterAction doesn't imply that the agent is expecting updates from the object." ;
        rdfs:label       "RegisterAction" ;
        rdfs:subClassOf  schema:InteractAction .

schema:WarrantyPromise
        rdf:type         rdfs:Class ;
        rdfs:comment     "A structured value representing the duration and scope of services that will be provided to a customer free of charge in case of a defect or malfunction of a product." ;
        rdfs:label       "WarrantyPromise" ;
        rdfs:subClassOf  schema:StructuredValue .

schema:Guide  rdf:type   rdfs:Class ;
        rdfs:comment     "[[Guide]] is a page or article that recommend specific products or services, or aspects of a thing for a user to consider. A [[Guide]] may represent a Buying Guide and detail aspects of products or services for a user to consider. A [[Guide]] may represent a Product Guide and recommend specific products or services. A [[Guide]] may represent a Ranked List and recommend specific products or services with ranking." ;
        rdfs:label       "Guide" ;
        rdfs:subClassOf  schema:CreativeWork .

schema:roleName  rdf:type  rdf:Property ;
        rdfs:comment  "A role played, performed or filled by a person or organization. For example, the team of creators for a comic book might fill the roles named 'inker', 'penciller', and 'letterer'; or an athlete in a SportsTeam might play in the position named 'Quarterback'." ;
        rdfs:label    "roleName" .

schema:AssessAction  rdf:type  rdfs:Class ;
        rdfs:comment     "The act of forming one's opinion, reaction or sentiment." ;
        rdfs:label       "AssessAction" ;
        rdfs:subClassOf  schema:Action .

schema:contactPoints  rdf:type  rdf:Property ;
        rdfs:comment  "A contact point for a person or organization." ;
        rdfs:label    "contactPoints" .

schema:ReturnFeesEnumeration
        rdf:type         rdfs:Class ;
        rdfs:comment     "ReturnFeesEnumeration expresses policies for return fees." ;
        rdfs:label       "ReturnFeesEnumeration" ;
        rdfs:subClassOf  schema:Enumeration .

schema:BikeStore  rdf:type  rdfs:Class ;
        rdfs:comment     "A bike store." ;
        rdfs:label       "BikeStore" ;
        rdfs:subClassOf  schema:Store .

schema:DrawAction  rdf:type  rdfs:Class ;
        rdfs:comment     "The act of producing a visual/graphical representation of an object, typically with a pen/pencil and paper as instruments." ;
        rdfs:label       "DrawAction" ;
        rdfs:subClassOf  schema:CreateAction .

schema:yearlyRevenue  rdf:type  rdf:Property ;
        rdfs:comment  "The size of the business in annual revenue." ;
        rdfs:label    "yearlyRevenue" .

schema:PropertyValueSpecification
        rdf:type         rdfs:Class ;
        rdfs:comment     "A Property value specification." ;
        rdfs:label       "PropertyValueSpecification" ;
        rdfs:subClassOf  schema:Intangible .

schema:vatID  rdf:type  rdf:Property ;
        rdfs:comment  "The Value-added Tax ID of the organization or person." ;
        rdfs:label    "vatID" .

schema:MedicalIntangible
        rdf:type         rdfs:Class ;
        rdfs:comment     "A utility class that serves as the umbrella for a number of 'intangible' things in the medical space." ;
        rdfs:label       "MedicalIntangible" ;
        rdfs:subClassOf  schema:MedicalEntity .

schema:broadcastSignalModulation
        rdf:type      rdf:Property ;
        rdfs:comment  "The modulation (e.g. FM, AM, etc) used by a particular broadcast service." ;
        rdfs:label    "broadcastSignalModulation" .

schema:workHours  rdf:type  rdf:Property ;
        rdfs:comment  "The typical working hours for this job (e.g. 1st shift, night shift, 8am-5pm)." ;
        rdfs:label    "workHours" .

schema:EndorseAction  rdf:type  rdfs:Class ;
        rdfs:comment     "An agent approves/certifies/likes/supports/sanction an object." ;
        rdfs:label       "EndorseAction" ;
        rdfs:subClassOf  schema:ReactAction .

schema:HinduTemple  rdf:type  rdfs:Class ;
        rdfs:comment     "A Hindu temple." ;
        rdfs:label       "HinduTemple" ;
        rdfs:subClassOf  schema:PlaceOfWorship .

schema:commentText  rdf:type  rdf:Property ;
        rdfs:comment  "The text of the UserComment." ;
        rdfs:label    "commentText" .

schema:contentType  rdf:type  rdf:Property ;
        rdfs:comment  "The supported content type(s) for an EntryPoint response." ;
        rdfs:label    "contentType" .

schema:requiredMinAge
        rdf:type      rdf:Property ;
        rdfs:comment  "Audiences defined by a person's minimum age." ;
        rdfs:label    "requiredMinAge" .

schema:DanceEvent  rdf:type  rdfs:Class ;
        rdfs:comment     "Event type: A social dance." ;
        rdfs:label       "DanceEvent" ;
        rdfs:subClassOf  schema:Event .

schema:honorificSuffix
        rdf:type      rdf:Property ;
        rdfs:comment  "An honorific suffix following a Person's name such as M.D. /PhD/MSCSW." ;
        rdfs:label    "honorificSuffix" .

schema:WatchAction  rdf:type  rdfs:Class ;
        rdfs:comment     "The act of consuming dynamic/moving visual content." ;
        rdfs:label       "WatchAction" ;
        rdfs:subClassOf  schema:ConsumeAction .

schema:domiciledMortgage
        rdf:type      rdf:Property ;
        rdfs:comment  "Whether borrower is a resident of the jurisdiction where the property is located." ;
        rdfs:label    "domiciledMortgage" .

schema:productionCompany
        rdf:type      rdf:Property ;
        rdfs:comment  "The production company or studio responsible for the item e.g. series, video game, episode etc." ;
        rdfs:label    "productionCompany" .

schema:typeOfBed  rdf:type  rdf:Property ;
        rdfs:comment  "The type of bed to which the BedDetail refers, i.e. the type of bed available in the quantity indicated by quantity." ;
        rdfs:label    "typeOfBed" .

schema:SportsActivityLocation
        rdf:type         rdfs:Class ;
        rdfs:comment     "A sports location, such as a playing field." ;
        rdfs:label       "SportsActivityLocation" ;
        rdfs:subClassOf  schema:LocalBusiness .

schema:sampleType  rdf:type  rdf:Property ;
        rdfs:comment  "What type of code sample: full (compile ready) solution, code snippet, inline code, scripts, template." ;
        rdfs:label    "sampleType" .

schema:RealEstateAgent
        rdf:type         rdfs:Class ;
        rdfs:comment     "A real-estate agent." ;
        rdfs:label       "RealEstateAgent" ;
        rdfs:subClassOf  schema:LocalBusiness .

schema:TextDigitalDocument
        rdf:type         rdfs:Class ;
        rdfs:comment     "A file composed primarily of text." ;
        rdfs:label       "TextDigitalDocument" ;
        rdfs:subClassOf  schema:DigitalDocument .

schema:payload  rdf:type  rdf:Property ;
        rdfs:comment  "The permitted weight of passengers and cargo, EXCLUDING the weight of the empty vehicle.\\n\\nTypical unit code(s): KGM for kilogram, LBR for pound\\n\\n* Note 1: Many databases specify the permitted TOTAL weight instead, which is the sum of [[weight]] and [[payload]]\\n* Note 2: You can indicate additional information in the [[name]] of the [[QuantitativeValue]] node.\\n* Note 3: You may also link to a [[QualitativeValue]] node that provides additional information using [[valueReference]].\\n* Note 4: Note that you can use [[minValue]] and [[maxValue]] to indicate ranges." ;
        rdfs:label    "payload" .

schema:broadcastOfEvent
        rdf:type      rdf:Property ;
        rdfs:comment  "The event being broadcast such as a sporting event or awards ceremony." ;
        rdfs:label    "broadcastOfEvent" .

schema:LegislationObject
        rdf:type         rdfs:Class ;
        rdfs:comment     "A specific object or file containing a Legislation. Note that the same Legislation can be published in multiple files. For example, a digitally signed PDF, a plain PDF and an HTML version." ;
        rdfs:label       "LegislationObject" ;
        rdfs:subClassOf  schema:MediaObject , schema:Legislation .

schema:departureBusStop
        rdf:type      rdf:Property ;
        rdfs:comment  "The stop or station from which the bus departs." ;
        rdfs:label    "departureBusStop" .

schema:numTracks  rdf:type  rdf:Property ;
        rdfs:comment  "The number of tracks in this album or playlist." ;
        rdfs:label    "numTracks" .

schema:percentile25  rdf:type  rdf:Property ;
        rdfs:comment  "The 25th percentile value." ;
        rdfs:label    "percentile25" .

schema:suggestedMaxAge
        rdf:type      rdf:Property ;
        rdfs:comment  "Maximum recommended age in years for the audience or user." ;
        rdfs:label    "suggestedMaxAge" .

schema:tocEntry  rdf:type   rdf:Property ;
        rdfs:comment        "Indicates a [[HyperTocEntry]] in a [[HyperToc]]." ;
        rdfs:label          "tocEntry" ;
        rdfs:subPropertyOf  schema:hasPart .

schema:hasCategoryCode
        rdf:type            rdf:Property ;
        rdfs:comment        "A Category code contained in this code set." ;
        rdfs:label          "hasCategoryCode" ;
        rdfs:subPropertyOf  schema:hasDefinedTerm .

schema:partOfTVSeries
        rdf:type            rdf:Property ;
        rdfs:comment        "The TV series to which this episode or season belongs." ;
        rdfs:label          "partOfTVSeries" ;
        rdfs:subPropertyOf  schema:isPartOf .

schema:ParkingFacility
        rdf:type         rdfs:Class ;
        rdfs:comment     "A parking lot or other parking facility." ;
        rdfs:label       "ParkingFacility" ;
        rdfs:subClassOf  schema:CivicStructure .

skos:changeNote  rdf:type   rdf:Property ;
        rdfs:label          "change note"@en ;
        rdfs:subPropertyOf  skos:note .

schema:softwareVersion
        rdf:type      rdf:Property ;
        rdfs:comment  "Version of the software instance." ;
        rdfs:label    "softwareVersion" .

schema:study  rdf:type  rdf:Property ;
        rdfs:comment  "A medical study or trial related to this entity." ;
        rdfs:label    "study" .

schema:inverseOf  rdf:type  rdf:Property ;
        rdfs:comment  "Relates a property to a property that is its inverse. Inverse properties relate the same pairs of items to each other, but in reversed direction. For example, the 'alumni' and 'alumniOf' properties are inverseOf each other. Some properties don't have explicit inverses; in these situations RDFa and JSON-LD syntax for reverse properties can be used." ;
        rdfs:label    "inverseOf" .

schema:referenceQuantity
        rdf:type      rdf:Property ;
        rdfs:comment  "The reference quantity for which a certain price applies, e.g. 1 EUR per 4 kWh of electricity. This property is a replacement for unitOfMeasurement for the advanced cases where the price does not relate to a standard unit." ;
        rdfs:label    "referenceQuantity" .

schema:RadioClip  rdf:type  rdfs:Class ;
        rdfs:comment     "A short radio program or a segment/part of a radio program." ;
        rdfs:label       "RadioClip" ;
        rdfs:subClassOf  schema:Clip .

schema:healthPlanCopayOption
        rdf:type      rdf:Property ;
        rdfs:comment  "Whether the copay is before or after deductible, etc. TODO: Is this a closed set?" ;
        rdfs:label    "healthPlanCopayOption" .

schema:VisualArtwork  rdf:type  rdfs:Class ;
        rdfs:comment     "A work of art that is primarily visual in character." ;
        rdfs:label       "VisualArtwork" ;
        rdfs:subClassOf  schema:CreativeWork .

schema:membershipNumber
        rdf:type      rdf:Property ;
        rdfs:comment  "A unique identifier for the membership." ;
        rdfs:label    "membershipNumber" .

schema:byMonthWeek  rdf:type  rdf:Property ;
        rdfs:comment  "Defines the week(s) of the month on which a recurring Event takes place. Specified as an Integer between 1-5. For clarity, byMonthWeek is best used in conjunction with byDay to indicate concepts like the first and third Mondays of a month." ;
        rdfs:label    "byMonthWeek" .

schema:monthsOfExperience
        rdf:type      rdf:Property ;
        rdfs:comment  "Indicates the minimal number of months of experience required for a position." ;
        rdfs:label    "monthsOfExperience" .

schema:DiscussionForumPosting
        rdf:type         rdfs:Class ;
        rdfs:comment     "A posting to a discussion forum." ;
        rdfs:label       "DiscussionForumPosting" ;
        rdfs:subClassOf  schema:SocialMediaPosting .

schema:ticketToken  rdf:type  rdf:Property ;
        rdfs:comment  "Reference to an asset (e.g., Barcode, QR code image or PDF) usable for entrance." ;
        rdfs:label    "ticketToken" .

schema:numberOfBathroomsTotal
        rdf:type      rdf:Property ;
        rdfs:comment  "The total integer number of bathrooms in a some [[Accommodation]], following real estate conventions as [documented in RESO](https://ddwiki.reso.org/display/DDW17/BathroomsTotalInteger+Field): \"The simple sum of the number of bathrooms. For example for a property with two Full Bathrooms and one Half Bathroom, the Bathrooms Total Integer will be 3.\". See also [[numberOfRooms]]." ;
        rdfs:label    "numberOfBathroomsTotal" .

schema:restPeriods  rdf:type  rdf:Property ;
        rdfs:comment  "How often one should break from the activity." ;
        rdfs:label    "restPeriods" .

schema:salaryCurrency
        rdf:type      rdf:Property ;
        rdfs:comment  "The currency (coded using [ISO 4217](http://en.wikipedia.org/wiki/ISO_4217) ) used for the main salary information in this job posting or for this employee." ;
        rdfs:label    "salaryCurrency" .

schema:numberOfItems  rdf:type  rdf:Property ;
        rdfs:comment  "The number of items in an ItemList. Note that some descriptions might not fully describe all items in a list (e.g., multi-page pagination); in such cases, the numberOfItems would be for the entire list." ;
        rdfs:label    "numberOfItems" .

schema:doseUnit  rdf:type  rdf:Property ;
        rdfs:comment  "The unit of the dose, e.g. 'mg'." ;
        rdfs:label    "doseUnit" .

schema:LifestyleModification
        rdf:type         rdfs:Class ;
        rdfs:comment     "A process of care involving exercise, changes to diet, fitness routines, and other lifestyle changes aimed at improving a health condition." ;
        rdfs:label       "LifestyleModification" ;
        rdfs:subClassOf  schema:MedicalEntity .

schema:memoryRequirements
        rdf:type      rdf:Property ;
        rdfs:comment  "Minimum memory requirements." ;
        rdfs:label    "memoryRequirements" .

schema:sku  rdf:type        rdf:Property ;
        rdfs:comment        "The Stock Keeping Unit (SKU), i.e. a merchant-specific identifier for a product or service, or the product to which the offer refers." ;
        rdfs:label          "sku" ;
        rdfs:subPropertyOf  schema:identifier .

schema:height  rdf:type  rdf:Property ;
        rdfs:comment  "The height of the item." ;
        rdfs:label    "height" .

schema:cvdNumBeds  rdf:type  rdf:Property ;
        rdfs:comment  "numbeds - HOSPITAL INPATIENT BEDS: Inpatient beds, including all staffed, licensed, and overflow (surge) beds used for inpatients." ;
        rdfs:label    "cvdNumBeds" .

schema:operatingSystem
        rdf:type      rdf:Property ;
        rdfs:comment  "Operating systems supported (Windows 7, OSX 10.6, Android 1.6)." ;
        rdfs:label    "operatingSystem" .

schema:geoCoveredBy  rdf:type  rdf:Property ;
        rdfs:comment  "Represents a relationship between two geometries (or the places they represent), relating a geometry to another that covers it. As defined in [DE-9IM](https://en.wikipedia.org/wiki/DE-9IM)." ;
        rdfs:label    "geoCoveredBy" .

schema:Park  rdf:type    rdfs:Class ;
        rdfs:comment     "A park." ;
        rdfs:label       "Park" ;
        rdfs:subClassOf  schema:CivicStructure .

schema:costPerUnit  rdf:type  rdf:Property ;
        rdfs:comment  "The cost per unit of the drug." ;
        rdfs:label    "costPerUnit" .

schema:educationalProgramMode
        rdf:type      rdf:Property ;
        rdfs:comment  "Similar to courseMode, The medium or means of delivery of the program as a whole. The value may either be a text label (e.g. \"online\", \"onsite\" or \"blended\"; \"synchronous\" or \"asynchronous\"; \"full-time\" or \"part-time\") or a URL reference to a term from a controlled vocabulary (e.g. https://ceds.ed.gov/element/001311#Asynchronous )." ;
        rdfs:label    "educationalProgramMode" .

schema:AutomotiveBusiness
        rdf:type         rdfs:Class ;
        rdfs:comment     "Car repair, sales, or parts." ;
        rdfs:label       "AutomotiveBusiness" ;
        rdfs:subClassOf  schema:LocalBusiness .

schema:BoatTerminal  rdf:type  rdfs:Class ;
        rdfs:comment     "A terminal for boats, ships, and other water vessels." ;
        rdfs:label       "BoatTerminal" ;
        rdfs:subClassOf  schema:CivicStructure .

schema:relatedTherapy
        rdf:type      rdf:Property ;
        rdfs:comment  "A medical therapy related to this anatomy." ;
        rdfs:label    "relatedTherapy" .

schema:speechToTextMarkup
        rdf:type      rdf:Property ;
        rdfs:comment  "Form of markup used. eg. [SSML](https://www.w3.org/TR/speech-synthesis11) or [IPA](https://www.wikidata.org/wiki/Property:P898)." ;
        rdfs:label    "speechToTextMarkup" .

schema:character  rdf:type  rdf:Property ;
        rdfs:comment  "Fictional person connected with a creative work." ;
        rdfs:label    "character" .

schema:subStructure  rdf:type  rdf:Property ;
        rdfs:comment  "Component (sub-)structure(s) that comprise this anatomical structure." ;
        rdfs:label    "subStructure" .

schema:actionableFeedbackPolicy
        rdf:type            rdf:Property ;
        rdfs:comment        "For a [[NewsMediaOrganization]] or other news-related [[Organization]], a statement about public engagement activities (for news media, the newsroom’s), including involving the public - digitally or otherwise -- in coverage decisions, reporting and activities after publication." ;
        rdfs:label          "actionableFeedbackPolicy" ;
        rdfs:subPropertyOf  schema:publishingPrinciples .

schema:brand  rdf:type  rdf:Property ;
        rdfs:comment  "The brand(s) associated with a product or service, or the brand(s) maintained by an organization or business person." ;
        rdfs:label    "brand" .

schema:FinancialService
        rdf:type         rdfs:Class ;
        rdfs:comment     "Financial services business." ;
        rdfs:label       "FinancialService" ;
        rdfs:subClassOf  schema:LocalBusiness .

schema:enginePower  rdf:type  rdf:Property ;
        rdfs:comment  "The power of the vehicle's engine.\n    Typical unit code(s): KWT for kilowatt, BHP for brake horsepower, N12 for metric horsepower (PS, with 1 PS = 735,49875 W)\\n\\n* Note 1: There are many different ways of measuring an engine's power. For an overview, see  [http://en.wikipedia.org/wiki/Horsepower#Engine_power_test_codes](http://en.wikipedia.org/wiki/Horsepower#Engine_power_test_codes).\\n* Note 2: You can link to information about how the given value has been determined using the [[valueReference]] property.\\n* Note 3: You can use [[minValue]] and [[maxValue]] to indicate ranges." ;
        rdfs:label    "enginePower" .

schema:SizeSystemEnumeration
        rdf:type         rdfs:Class ;
        rdfs:comment     "Enumerates common size systems for different categories of products, for example \"EN-13402\" or \"UK\" for wearables or \"Imperial\" for screws." ;
        rdfs:label       "SizeSystemEnumeration" ;
        rdfs:subClassOf  schema:Enumeration .

schema:NGO  rdf:type     rdfs:Class ;
        rdfs:comment     "Organization: Non-governmental Organization." ;
        rdfs:label       "NGO" ;
        rdfs:subClassOf  schema:Organization .

schema:GeoShape  rdf:type  rdfs:Class ;
        rdfs:comment     "The geographic shape of a place. A GeoShape can be described using several properties whose values are based on latitude/longitude pairs. Either whitespace or commas can be used to separate latitude and longitude; whitespace should be used when writing a list of several such points." ;
        rdfs:label       "GeoShape" ;
        rdfs:subClassOf  schema:StructuredValue .

schema:Mosque  rdf:type  rdfs:Class ;
        rdfs:comment     "A mosque." ;
        rdfs:label       "Mosque" ;
        rdfs:subClassOf  schema:PlaceOfWorship .

schema:originAddress  rdf:type  rdf:Property ;
        rdfs:comment  "Shipper's address." ;
        rdfs:label    "originAddress" .

schema:nerve  rdf:type  rdf:Property ;
        rdfs:comment  "The underlying innervation associated with the muscle." ;
        rdfs:label    "nerve" .

schema:MusicAlbumProductionType
        rdf:type         rdfs:Class ;
        rdfs:comment     "Classification of the album by it's type of content: soundtrack, live album, studio album, etc." ;
        rdfs:label       "MusicAlbumProductionType" ;
        rdfs:subClassOf  schema:Enumeration .

schema:maintainer  rdf:type  rdf:Property ;
        rdfs:comment  "A maintainer of a [[Dataset]], software package ([[SoftwareApplication]]), or other [[Project]]. A maintainer is a [[Person]] or [[Organization]] that manages contributions to, and/or publication of, some (typically complex) artifact. It is common for distributions of software and data to be based on \"upstream\" sources. When [[maintainer]] is applied to a specific version of something e.g. a particular version or packaging of a [[Dataset]], it is always  possible that the upstream source has a different maintainer. The [[isBasedOn]] property can be used to indicate such relationships between datasets to make the different maintenance roles clear. Similarly in the case of software, a package may have dedicated maintainers working on integration into software distributions such as Ubuntu, as well as upstream maintainers of the underlying work.\n      " ;
        rdfs:label    "maintainer" .

schema:programName  rdf:type  rdf:Property ;
        rdfs:comment  "The program providing the membership." ;
        rdfs:label    "programName" .

schema:result  rdf:type  rdf:Property ;
        rdfs:comment  "The result produced in the action. e.g. John wrote *a book*." ;
        rdfs:label    "result" .

schema:MotorizedBicycle
        rdf:type         rdfs:Class ;
        rdfs:comment     "A motorized bicycle is a bicycle with an attached motor used to power the vehicle, or to assist with pedaling." ;
        rdfs:label       "MotorizedBicycle" ;
        rdfs:subClassOf  schema:Vehicle .

schema:validUntil  rdf:type  rdf:Property ;
        rdfs:comment  "The date when the item is no longer valid." ;
        rdfs:label    "validUntil" .

schema:partOfInvoice  rdf:type  rdf:Property ;
        rdfs:comment  "The order is being paid as part of the referenced Invoice." ;
        rdfs:label    "partOfInvoice" .

schema:HealthTopicContent
        rdf:type         rdfs:Class ;
        rdfs:comment     "[[HealthTopicContent]] is [[WebContent]] that is about some aspect of a health topic, e.g. a condition, its symptoms or treatments. Such content may be comprised of several parts or sections and use different types of media. Multiple instances of [[WebContent]] (and hence [[HealthTopicContent]]) can be related using [[hasPart]] / [[isPartOf]] where there is some kind of content hierarchy, and their content described with [[about]] and [[mentions]] e.g. building upon the existing [[MedicalCondition]] vocabulary.\n  " ;
        rdfs:label       "HealthTopicContent" ;
        rdfs:subClassOf  schema:WebContent .

schema:Hotel  rdf:type   rdfs:Class ;
        rdfs:comment     "A hotel is an establishment that provides lodging paid on a short-term basis (Source: Wikipedia, the free encyclopedia, see http://en.wikipedia.org/wiki/Hotel).\n<br /><br />\nSee also the <a href=\"/docs/hotels.html\">dedicated document on the use of schema.org for marking up hotels and other forms of accommodations</a>.\n" ;
        rdfs:label       "Hotel" ;
        rdfs:subClassOf  schema:LodgingBusiness .

schema:AskPublicNewsArticle
        rdf:type         rdfs:Class ;
        rdfs:comment     "A [[NewsArticle]] expressing an open call by a [[NewsMediaOrganization]] asking the public for input, insights, clarifications, anecdotes, documentation, etc., on an issue, for reporting purposes." ;
        rdfs:label       "AskPublicNewsArticle" ;
        rdfs:subClassOf  schema:NewsArticle .

schema:status  rdf:type  rdf:Property ;
        rdfs:comment  "The status of the study (enumerated)." ;
        rdfs:label    "status" .

schema:translator  rdf:type  rdf:Property ;
        rdfs:comment  "Organization or person who adapts a creative work to different languages, regional differences and technical requirements of a target market, or that translates during some event." ;
        rdfs:label    "translator" .

schema:modifiedTime  rdf:type  rdf:Property ;
        rdfs:comment  "The date and time the reservation was modified." ;
        rdfs:label    "modifiedTime" .

schema:mpn  rdf:type  rdf:Property ;
        rdfs:comment  "The Manufacturer Part Number (MPN) of the product, or the product to which the offer refers." ;
        rdfs:label    "mpn" .

schema:GroceryStore  rdf:type  rdfs:Class ;
        rdfs:comment     "A grocery store." ;
        rdfs:label       "GroceryStore" ;
        rdfs:subClassOf  schema:Store .

schema:subTest  rdf:type  rdf:Property ;
        rdfs:comment  "A component test of the panel." ;
        rdfs:label    "subTest" .

schema:publisherImprint
        rdf:type      rdf:Property ;
        rdfs:comment  "The publishing division which published the comic." ;
        rdfs:label    "publisherImprint" .

schema:geoRadius  rdf:type  rdf:Property ;
        rdfs:comment  "Indicates the approximate radius of a GeoCircle (metres unless indicated otherwise via Distance notation)." ;
        rdfs:label    "geoRadius" .

schema:startTime  rdf:type  rdf:Property ;
        rdfs:comment  "The startTime of something. For a reserved event or service (e.g. FoodEstablishmentReservation), the time that it is expected to start. For actions that span a period of time, when the action was performed. e.g. John wrote a book from *January* to December. For media, including audio and video, it's the time offset of the start of a clip within a larger file.\\n\\nNote that Event uses startDate/endDate instead of startTime/endTime, even when describing dates with times. This situation may be clarified in future revisions." ;
        rdfs:label    "startTime" .

schema:exampleOfWork  rdf:type  rdf:Property ;
        rdfs:comment  "A creative work that this work is an example/instance/realization/derivation of." ;
        rdfs:label    "exampleOfWork" .

schema:Gynecologic  rdf:type  rdfs:Class ;
        rdfs:comment     "A specific branch of medical science that pertains to the health care of women, particularly in the diagnosis and treatment of disorders affecting the female reproductive system." ;
        rdfs:label       "Gynecologic" ;
        rdfs:subClassOf  schema:MedicalBusiness .

schema:childMaxAge  rdf:type  rdf:Property ;
        rdfs:comment  "Maximal age of the child." ;
        rdfs:label    "childMaxAge" .

schema:DrugPregnancyCategory
        rdf:type         rdfs:Class ;
        rdfs:comment     "Categories that represent an assessment of the risk of fetal injury due to a drug or pharmaceutical used as directed by the mother during pregnancy." ;
        rdfs:label       "DrugPregnancyCategory" ;
        rdfs:subClassOf  schema:MedicalEnumeration .

schema:MedicalSignOrSymptom
        rdf:type         rdfs:Class ;
        rdfs:comment     "Any feature associated or not with a medical condition. In medicine a symptom is generally subjective while a sign is objective." ;
        rdfs:label       "MedicalSignOrSymptom" ;
        rdfs:subClassOf  schema:MedicalCondition .

schema:polygon  rdf:type  rdf:Property ;
        rdfs:comment  "A polygon is the area enclosed by a point-to-point path for which the starting and ending points are the same. A polygon is expressed as a series of four or more space delimited points where the first and final points are identical." ;
        rdfs:label    "polygon" .

schema:installUrl  rdf:type  rdf:Property ;
        rdfs:comment  "URL at which the app may be installed, if different from the URL of the item." ;
        rdfs:label    "installUrl" .

schema:legislationJurisdiction
        rdf:type            rdf:Property ;
        rdfs:comment        "The jurisdiction from which the legislation originates." ;
        rdfs:label          "legislationJurisdiction" ;
        rdfs:subPropertyOf  schema:spatialCoverage , schema:jurisdiction .

schema:distinguishingSign
        rdf:type      rdf:Property ;
        rdfs:comment  "One of a set of signs and symptoms that can be used to distinguish this diagnosis from others in the differential diagnosis." ;
        rdfs:label    "distinguishingSign" .

schema:diet  rdf:type       rdf:Property ;
        rdfs:comment        "A sub property of instrument. The diet used in this action." ;
        rdfs:label          "diet" ;
        rdfs:subPropertyOf  schema:instrument .

schema:orderItemNumber
        rdf:type      rdf:Property ;
        rdfs:comment  "The identifier of the order item." ;
        rdfs:label    "orderItemNumber" .

schema:EntryPoint  rdf:type  rdfs:Class ;
        rdfs:comment     "An entry point, within some Web-based protocol." ;
        rdfs:label       "EntryPoint" ;
        rdfs:subClassOf  schema:Intangible .

schema:AssignAction  rdf:type  rdfs:Class ;
        rdfs:comment     "The act of allocating an action/event/task to some destination (someone or something)." ;
        rdfs:label       "AssignAction" ;
        rdfs:subClassOf  schema:AllocateAction .

schema:Drug  rdf:type    rdfs:Class ;
        rdfs:comment     "A chemical or biologic substance, used as a medical therapy, that has a physiological effect on an organism. Here the term drug is used interchangeably with the term medicine although clinical knowledge make a clear difference between them." ;
        rdfs:label       "Drug" ;
        rdfs:subClassOf  schema:Substance .

schema:LoanOrCredit  rdf:type  rdfs:Class ;
        rdfs:comment     "A financial product for the loaning of an amount of money, or line of credit, under agreed terms and charges." ;
        rdfs:label       "LoanOrCredit" ;
        rdfs:subClassOf  schema:FinancialProduct .

schema:dateModified  rdf:type  rdf:Property ;
        rdfs:comment  "The date on which the CreativeWork was most recently modified or when the item's entry was modified within a DataFeed." ;
        rdfs:label    "dateModified" .

schema:workLocation  rdf:type  rdf:Property ;
        rdfs:comment        "A contact location for a person's place of work." ;
        rdfs:label          "workLocation" ;
        rdfs:subPropertyOf  schema:location .

schema:Vessel  rdf:type  rdfs:Class ;
        rdfs:comment     "A component of the human body circulatory system comprised of an intricate network of hollow tubes that transport blood throughout the entire body." ;
        rdfs:label       "Vessel" ;
        rdfs:subClassOf  schema:AnatomicalStructure .

schema:ComedyClub  rdf:type  rdfs:Class ;
        rdfs:comment     "A comedy club." ;
        rdfs:label       "ComedyClub" ;
        rdfs:subClassOf  schema:EntertainmentBusiness .

schema:colorist  rdf:type  rdf:Property ;
        rdfs:comment  "The individual who adds color to inked drawings." ;
        rdfs:label    "colorist" .

schema:availableThrough
        rdf:type      rdf:Property ;
        rdfs:comment  "After this date, the item will no longer be available for pickup." ;
        rdfs:label    "availableThrough" .

schema:responsibilities
        rdf:type      rdf:Property ;
        rdfs:comment  "Responsibilities associated with this role or Occupation." ;
        rdfs:label    "responsibilities" .

schema:LiteraryEvent  rdf:type  rdfs:Class ;
        rdfs:comment     "Event type: Literary event." ;
        rdfs:label       "LiteraryEvent" ;
        rdfs:subClassOf  schema:Event .

schema:season  rdf:type     rdf:Property ;
        rdfs:comment        "A season in a media series." ;
        rdfs:label          "season" ;
        rdfs:subPropertyOf  schema:hasPart .

schema:ShoeStore  rdf:type  rdfs:Class ;
        rdfs:comment     "A shoe store." ;
        rdfs:label       "ShoeStore" ;
        rdfs:subClassOf  schema:Store .

schema:HowToSection  rdf:type  rdfs:Class ;
        rdfs:comment     "A sub-grouping of steps in the instructions for how to achieve a result (e.g. steps for making a pie crust within a pie recipe)." ;
        rdfs:label       "HowToSection" ;
        rdfs:subClassOf  schema:ListItem , schema:ItemList , schema:CreativeWork .

schema:LocalBusiness  rdf:type  rdfs:Class ;
        rdfs:comment     "A particular physical business or branch of an organization. Examples of LocalBusiness include a restaurant, a particular branch of a restaurant chain, a branch of a bank, a medical practice, a club, a bowling alley, etc." ;
        rdfs:label       "LocalBusiness" ;
        rdfs:subClassOf  schema:Place , schema:Organization .

schema:UserReview  rdf:type  rdfs:Class ;
        rdfs:comment     "A review created by an end-user (e.g. consumer, purchaser, attendee etc.), in contrast with [[CriticReview]]." ;
        rdfs:label       "UserReview" ;
        rdfs:subClassOf  schema:Review .

schema:isAccessoryOrSparePartFor
        rdf:type      rdf:Property ;
        rdfs:comment  "A pointer to another product (or multiple products) for which this product is an accessory or spare part." ;
        rdfs:label    "isAccessoryOrSparePartFor" .

schema:foundingLocation
        rdf:type      rdf:Property ;
        rdfs:comment  "The place where the Organization was founded." ;
        rdfs:label    "foundingLocation" .

schema:deliveryTime  rdf:type  rdf:Property ;
        rdfs:comment  "The total delay between the receipt of the order and the goods reaching the final customer." ;
        rdfs:label    "deliveryTime" .

schema:employee  rdf:type  rdf:Property ;
        rdfs:comment  "Someone working for this organization." ;
        rdfs:label    "employee" .

schema:cssSelector  rdf:type  rdf:Property ;
        rdfs:comment  "A CSS selector, e.g. of a [[SpeakableSpecification]] or [[WebPageElement]]. In the latter case, multiple matches within a page can constitute a single conceptual \"Web page element\"." ;
        rdfs:label    "cssSelector" .

schema:legislationChanges
        rdf:type      rdf:Property ;
        rdfs:comment  "Another legislation that this legislation changes. This encompasses the notions of amendment, replacement, correction, repeal, or other types of change. This may be a direct change (textual or non-textual amendment) or a consequential or indirect change. The property is to be used to express the existence of a change relationship between two acts rather than the existence of a consolidated version of the text that shows the result of the change. For consolidation relationships, use the <a href=\"/legislationConsolidates\">legislationConsolidates</a> property." ;
        rdfs:label    "legislationChanges" .

schema:followup  rdf:type  rdf:Property ;
        rdfs:comment  "Typical or recommended followup care after the procedure is performed." ;
        rdfs:label    "followup" .

schema:reservedTicket
        rdf:type      rdf:Property ;
        rdfs:comment  "A ticket associated with the reservation." ;
        rdfs:label    "reservedTicket" .

schema:procedure  rdf:type  rdf:Property ;
        rdfs:comment  "A description of the procedure involved in setting up, using, and/or installing the device." ;
        rdfs:label    "procedure" .

schema:borrower  rdf:type   rdf:Property ;
        rdfs:comment        "A sub property of participant. The person that borrows the object being lent." ;
        rdfs:label          "borrower" ;
        rdfs:subPropertyOf  schema:participant .

schema:workload  rdf:type  rdf:Property ;
        rdfs:comment  "Quantitative measure of the physiologic output of the exercise; also referred to as energy expenditure." ;
        rdfs:label    "workload" .

schema:Muscle  rdf:type  rdfs:Class ;
        rdfs:comment     "A muscle is an anatomical structure consisting of a contractile form of tissue that animals use to effect movement." ;
        rdfs:label       "Muscle" ;
        rdfs:subClassOf  schema:AnatomicalStructure .

schema:containedIn  rdf:type  rdf:Property ;
        rdfs:comment  "The basic containment relation between a place and one that contains it." ;
        rdfs:label    "containedIn" .

schema:bodyLocation  rdf:type  rdf:Property ;
        rdfs:comment  "Location in the body of the anatomical structure." ;
        rdfs:label    "bodyLocation" .

schema:callSign  rdf:type   rdf:Property ;
        rdfs:comment        "A [callsign](https://en.wikipedia.org/wiki/Call_sign), as used in broadcasting and radio communications to identify people, radio and TV stations, or vehicles." ;
        rdfs:label          "callSign" ;
        rdfs:subPropertyOf  schema:identifier .

schema:DeliveryEvent  rdf:type  rdfs:Class ;
        rdfs:comment     "An event involving the delivery of an item." ;
        rdfs:label       "DeliveryEvent" ;
        rdfs:subClassOf  schema:Event .

schema:HowToItem  rdf:type  rdfs:Class ;
        rdfs:comment     "An item used as either a tool or supply when performing the instructions for how to to achieve a result." ;
        rdfs:label       "HowToItem" ;
        rdfs:subClassOf  schema:ListItem .

schema:SomeProducts  rdf:type  rdfs:Class ;
        rdfs:comment     "A placeholder for multiple similar products of the same kind." ;
        rdfs:label       "SomeProducts" ;
        rdfs:subClassOf  schema:Product .

schema:processingTime
        rdf:type      rdf:Property ;
        rdfs:comment  "Estimated processing time for the service using this channel." ;
        rdfs:label    "processingTime" .

schema:trainName  rdf:type  rdf:Property ;
        rdfs:comment  "The name of the train (e.g. The Orient Express)." ;
        rdfs:label    "trainName" .

schema:pagination  rdf:type  rdf:Property ;
        rdfs:comment  "Any description of pages that is not separated into pageStart and pageEnd; for example, \"1-6, 9, 55\" or \"10-12, 46-49\"." ;
        rdfs:label    "pagination" .

schema:ownedFrom  rdf:type  rdf:Property ;
        rdfs:comment  "The date and time of obtaining the product." ;
        rdfs:label    "ownedFrom" .

schema:AutoWash  rdf:type  rdfs:Class ;
        rdfs:comment     "A car wash business." ;
        rdfs:label       "AutoWash" ;
        rdfs:subClassOf  schema:AutomotiveBusiness .

schema:MedicalTrial  rdf:type  rdfs:Class ;
        rdfs:comment     "A medical trial is a type of medical study that uses scientific process used to compare the safety and efficacy of medical therapies or medical procedures. In general, medical trials are controlled and subjects are allocated at random to the different treatment and/or control groups." ;
        rdfs:label       "MedicalTrial" ;
        rdfs:subClassOf  schema:MedicalStudy .

schema:text  rdf:type  rdf:Property ;
        rdfs:comment  "The textual content of this CreativeWork." ;
        rdfs:label    "text" .

schema:opens  rdf:type  rdf:Property ;
        rdfs:comment  "The opening hour of the place or service on the given day(s) of the week." ;
        rdfs:label    "opens" .

schema:foodWarning  rdf:type  rdf:Property ;
        rdfs:comment  "Any precaution, guidance, contraindication, etc. related to consumption of specific foods while taking this drug." ;
        rdfs:label    "foodWarning" .

schema:Observation  rdf:type  rdfs:Class ;
        rdfs:comment     "Instances of the class [[Observation]] are used to specify observations about an entity (which may or may not be an instance of a [[StatisticalPopulation]]), at a particular time. The principal properties of an [[Observation]] are [[observedNode]], [[measuredProperty]], [[measuredValue]] (or [[median]], etc.) and [[observationDate]] ([[measuredProperty]] properties can, but need not always, be W3C RDF Data Cube \"measure properties\", as in the [lifeExpectancy example](https://www.w3.org/TR/vocab-data-cube/#dsd-example)).\nSee also [[StatisticalPopulation]], and the [data and datasets](/docs/data-and-datasets.html) overview for more details.\n  " ;
        rdfs:label       "Observation" ;
        rdfs:subClassOf  schema:Intangible .

schema:BoatReservation
        rdf:type         rdfs:Class ;
        rdfs:comment     "A reservation for boat travel.\n\nNote: This type is for information about actual reservations, e.g. in confirmation emails or HTML pages with individual confirmations of reservations. For offers of tickets, use [[Offer]]." ;
        rdfs:label       "BoatReservation" ;
        rdfs:subClassOf  schema:Reservation .

schema:MonetaryAmount
        rdf:type         rdfs:Class ;
        rdfs:comment     "A monetary value or range. This type can be used to describe an amount of money such as $50 USD, or a range as in describing a bank account being suitable for a balance between £1,000 and £1,000,000 GBP, or the value of a salary, etc. It is recommended to use [[PriceSpecification]] Types to describe the price of an Offer, Invoice, etc." ;
        rdfs:label       "MonetaryAmount" ;
        rdfs:subClassOf  schema:StructuredValue .

schema:TaxiService  rdf:type  rdfs:Class ;
        rdfs:comment     "A service for a vehicle for hire with a driver for local travel. Fares are usually calculated based on distance traveled." ;
        rdfs:label       "TaxiService" ;
        rdfs:subClassOf  schema:Service .

schema:numberOfForwardGears
        rdf:type      rdf:Property ;
        rdfs:comment  "The total number of forward gears available for the transmission system of the vehicle.\\n\\nTypical unit code(s): C62" ;
        rdfs:label    "numberOfForwardGears" .

schema:valueMaxLength
        rdf:type      rdf:Property ;
        rdfs:comment  "Specifies the allowed range for number of characters in a literal value." ;
        rdfs:label    "valueMaxLength" .

schema:awards  rdf:type  rdf:Property ;
        rdfs:comment  "Awards won by or for this item." ;
        rdfs:label    "awards" .

schema:containedInPlace
        rdf:type      rdf:Property ;
        rdfs:comment  "The basic containment relation between a place and one that contains it." ;
        rdfs:label    "containedInPlace" .

schema:ratingCount  rdf:type  rdf:Property ;
        rdfs:comment  "The count of total number of ratings." ;
        rdfs:label    "ratingCount" .

schema:owns  rdf:type  rdf:Property ;
        rdfs:comment  "Products owned by the organization or person." ;
        rdfs:label    "owns" .

schema:suggestedAge  rdf:type  rdf:Property ;
        rdfs:comment  "The age or age range for the intended audience or person, for example 3-12 months for infants, 1-5 years for toddlers." ;
        rdfs:label    "suggestedAge" .

schema:phoneticText  rdf:type  rdf:Property ;
        rdfs:comment  "Representation of a text [[textValue]] using the specified [[speechToTextMarkup]]. For example the city name of Houston in IPA: /ˈhjuːstən/." ;
        rdfs:label    "phoneticText" .

schema:clipNumber  rdf:type  rdf:Property ;
        rdfs:comment        "Position of the clip within an ordered group of clips." ;
        rdfs:label          "clipNumber" ;
        rdfs:subPropertyOf  schema:position .

schema:HealthInsurancePlan
        rdf:type         rdfs:Class ;
        rdfs:comment     "A US-style health insurance plan, including PPOs, EPOs, and HMOs. " ;
        rdfs:label       "HealthInsurancePlan" ;
        rdfs:subClassOf  schema:Intangible .

schema:browserRequirements
        rdf:type      rdf:Property ;
        rdfs:comment  "Specifies browser requirements in human-readable text. For example, 'requires HTML5 support'." ;
        rdfs:label    "browserRequirements" .

schema:foundingDate  rdf:type  rdf:Property ;
        rdfs:comment  "The date that this organization was founded." ;
        rdfs:label    "foundingDate" .

schema:AutoRental  rdf:type  rdfs:Class ;
        rdfs:comment     "A car rental business." ;
        rdfs:label       "AutoRental" ;
        rdfs:subClassOf  schema:AutomotiveBusiness .

schema:educationalUse
        rdf:type      rdf:Property ;
        rdfs:comment  "The purpose of a work in the context of education; for example, 'assignment', 'group work'." ;
        rdfs:label    "educationalUse" .

schema:MedicalTrialDesign
        rdf:type         rdfs:Class ;
        rdfs:comment     "Design models for medical trials. Enumerated type." ;
        rdfs:label       "MedicalTrialDesign" ;
        rdfs:subClassOf  schema:MedicalEnumeration .

schema:audience  rdf:type  rdf:Property ;
        rdfs:comment  "An intended audience, i.e. a group for whom something was created." ;
        rdfs:label    "audience" .

schema:Answer  rdf:type  rdfs:Class ;
        rdfs:comment     "An answer offered to a question; perhaps correct, perhaps opinionated or wrong." ;
        rdfs:label       "Answer" ;
        rdfs:subClassOf  schema:Comment .

skos:narrowMatch  rdf:type  owl:ObjectProperty ;
        rdfs:label          "has narrower match"@en ;
        rdfs:subPropertyOf  skos:narrower , skos:mappingRelation ;
        owl:inverseOf       skos:broadMatch .

schema:afterMedia  rdf:type  rdf:Property ;
        rdfs:comment  "A media object representing the circumstances after performing this direction." ;
        rdfs:label    "afterMedia" .

schema:cashBack  rdf:type  rdf:Property ;
        rdfs:comment  "A cardholder benefit that pays the cardholder a small percentage of their net expenditures." ;
        rdfs:label    "cashBack" .

schema:parent  rdf:type  rdf:Property ;
        rdfs:comment  "A parent of this person." ;
        rdfs:label    "parent" .

schema:InfectiousAgentClass
        rdf:type         rdfs:Class ;
        rdfs:comment     "Classes of agents or pathogens that transmit infectious diseases. Enumerated type." ;
        rdfs:label       "InfectiousAgentClass" ;
        rdfs:subClassOf  schema:MedicalEnumeration .

schema:image  rdf:type  rdf:Property ;
        rdfs:comment  "An image of the item. This can be a [[URL]] or a fully described [[ImageObject]]." ;
        rdfs:label    "image" .

schema:infectiousAgent
        rdf:type      rdf:Property ;
        rdfs:comment  "The actual infectious agent, such as a specific bacterium." ;
        rdfs:label    "infectiousAgent" .

schema:RepaymentSpecification
        rdf:type         rdfs:Class ;
        rdfs:comment     "A structured value representing repayment." ;
        rdfs:label       "RepaymentSpecification" ;
        rdfs:subClassOf  schema:StructuredValue .

schema:CreateAction  rdf:type  rdfs:Class ;
        rdfs:comment     "The act of deliberately creating/producing/generating/building a result out of the agent." ;
        rdfs:label       "CreateAction" ;
        rdfs:subClassOf  schema:Action .

voc:SalesReasonCategory
        rdf:type         rdfs:Class ;
        rdfs:subClassOf  skos:Concept .

schema:greater  rdf:type  rdf:Property ;
        rdfs:comment  "This ordering relation for qualitative values indicates that the subject is greater than the object." ;
        rdfs:label    "greater" .

schema:measurementTechnique
        rdf:type      rdf:Property ;
        rdfs:comment  "A technique or technology used in a [[Dataset]] (or [[DataDownload]], [[DataCatalog]]),\ncorresponding to the method used for measuring the corresponding variable(s) (described using [[variableMeasured]]). This is oriented towards scientific and scholarly dataset publication but may have broader applicability; it is not intended as a full representation of measurement, but rather as a high level summary for dataset discovery.\n\nFor example, if [[variableMeasured]] is: molecule concentration, [[measurementTechnique]] could be: \"mass spectrometry\" or \"nmr spectroscopy\" or \"colorimetry\" or \"immunofluorescence\".\n\nIf the [[variableMeasured]] is \"depression rating\", the [[measurementTechnique]] could be \"Zung Scale\" or \"HAM-D\" or \"Beck Depression Inventory\".\n\nIf there are several [[variableMeasured]] properties recorded for some given data object, use a [[PropertyValue]] for each [[variableMeasured]] and attach the corresponding [[measurementTechnique]].\n      " ;
        rdfs:label    "measurementTechnique" .

schema:dayOfWeek  rdf:type  rdf:Property ;
        rdfs:comment  "The day of the week for which these opening hours are valid." ;
        rdfs:label    "dayOfWeek" .

schema:targetPopulation
        rdf:type      rdf:Property ;
        rdfs:comment  "Characteristics of the population for which this is intended, or which typically uses it, e.g. 'adults'." ;
        rdfs:label    "targetPopulation" .

schema:director  rdf:type  rdf:Property ;
        rdfs:comment  "A director of e.g. tv, radio, movie, video gaming etc. content, or of an event. Directors can be associated with individual items or with a series, episode, clip." ;
        rdfs:label    "director" .

schema:paymentDue  rdf:type  rdf:Property ;
        rdfs:comment  "The date that payment is due." ;
        rdfs:label    "paymentDue" .

schema:broadcastFrequencyValue
        rdf:type      rdf:Property ;
        rdfs:comment  "The frequency in MHz for a particular broadcast." ;
        rdfs:label    "broadcastFrequencyValue" .

schema:identifier  rdf:type  rdf:Property ;
        rdfs:comment  "The identifier property represents any kind of identifier for any kind of [[Thing]], such as ISBNs, GTIN codes, UUIDs etc. Schema.org provides dedicated properties for representing many of these, either as textual strings or as URL (URI) links. See [background notes](/docs/datamodel.html#identifierBg) for more details.\n        " ;
        rdfs:label    "identifier" .

skos:hiddenLabel  rdf:type  rdf:Property ;
        rdfs:comment        "skos:prefLabel, skos:altLabel and skos:hiddenLabel are pairwise disjoint properties."@en , "The range of skos:hiddenLabel is the class of RDF plain literals."@en ;
        rdfs:label          "hidden label"@en ;
        rdfs:subPropertyOf  rdfs:label .

schema:repetitions  rdf:type  rdf:Property ;
        rdfs:comment  "Number of times one should repeat the activity." ;
        rdfs:label    "repetitions" .

schema:MediaSubscription
        rdf:type         rdfs:Class ;
        rdfs:comment     "A subscription which allows a user to access media including audio, video, books, etc." ;
        rdfs:label       "MediaSubscription" ;
        rdfs:subClassOf  schema:Intangible .

schema:doseSchedule  rdf:type  rdf:Property ;
        rdfs:comment  "A dosing schedule for the drug for a given population, either observed, recommended, or maximum dose based on the type used." ;
        rdfs:label    "doseSchedule" .

schema:candidate  rdf:type  rdf:Property ;
        rdfs:comment        "A sub property of object. The candidate subject of this action." ;
        rdfs:label          "candidate" ;
        rdfs:subPropertyOf  schema:object .

schema:OceanBodyOfWater
        rdf:type         rdfs:Class ;
        rdfs:comment     "An ocean (for example, the Pacific)." ;
        rdfs:label       "OceanBodyOfWater" ;
        rdfs:subClassOf  schema:BodyOfWater .

schema:ReplaceAction  rdf:type  rdfs:Class ;
        rdfs:comment     "The act of editing a recipient by replacing an old object with a new object." ;
        rdfs:label       "ReplaceAction" ;
        rdfs:subClassOf  schema:UpdateAction .

schema:governmentBenefitsInfo
        rdf:type      rdf:Property ;
        rdfs:comment  "governmentBenefitsInfo provides information about government benefits associated with a SpecialAnnouncement." ;
        rdfs:label    "governmentBenefitsInfo" .

schema:runsTo  rdf:type  rdf:Property ;
        rdfs:comment  "The vasculature the lymphatic structure runs, or efferents, to." ;
        rdfs:label    "runsTo" .

schema:educationalCredentialAwarded
        rdf:type      rdf:Property ;
        rdfs:comment  "A description of the qualification, award, certificate, diploma or other educational credential awarded as a consequence of successful completion of this course or program." ;
        rdfs:label    "educationalCredentialAwarded" .

schema:Series  rdf:type  rdfs:Class ;
        rdfs:comment     "A Series in schema.org is a group of related items, typically but not necessarily of the same kind. See also [[CreativeWorkSeries]], [[EventSeries]]." ;
        rdfs:label       "Series" ;
        rdfs:subClassOf  schema:Intangible .

schema:previousStartDate
        rdf:type      rdf:Property ;
        rdfs:comment  "Used in conjunction with eventStatus for rescheduled or cancelled events. This property contains the previously scheduled start date. For rescheduled events, the startDate property should be used for the newly scheduled start date. In the (rare) case of an event that has been postponed and rescheduled multiple times, this field may be repeated." ;
        rdfs:label    "previousStartDate" .

schema:AllocateAction
        rdf:type         rdfs:Class ;
        rdfs:comment     "The act of organizing tasks/objects/events by associating resources to it." ;
        rdfs:label       "AllocateAction" ;
        rdfs:subClassOf  schema:OrganizeAction .

schema:musicArrangement
        rdf:type      rdf:Property ;
        rdfs:comment  "An arrangement derived from the composition." ;
        rdfs:label    "musicArrangement" .

schema:BusinessAudience
        rdf:type         rdfs:Class ;
        rdfs:comment     "A set of characteristics belonging to businesses, e.g. who compose an item's target audience." ;
        rdfs:label       "BusinessAudience" ;
        rdfs:subClassOf  schema:Audience .

schema:sensoryUnit  rdf:type  rdf:Property ;
        rdfs:comment  "The neurological pathway extension that inputs and sends information to the brain or spinal cord." ;
        rdfs:label    "sensoryUnit" .

schema:GovernmentService
        rdf:type         rdfs:Class ;
        rdfs:comment     "A service provided by a government organization, e.g. food stamps, veterans benefits, etc." ;
        rdfs:label       "GovernmentService" ;
        rdfs:subClassOf  schema:Service .

skos:ConceptScheme  rdf:type  rdfs:Class ;
        rdfs:label  "Concept Scheme"@en .

schema:RiverBodyOfWater
        rdf:type         rdfs:Class ;
        rdfs:comment     "A river (for example, the broad majestic Shannon)." ;
        rdfs:label       "RiverBodyOfWater" ;
        rdfs:subClassOf  schema:BodyOfWater .

schema:referencesOrder
        rdf:type      rdf:Property ;
        rdfs:comment  "The Order(s) related to this Invoice. One or more Orders may be combined into a single Invoice." ;
        rdfs:label    "referencesOrder" .

schema:loanType  rdf:type  rdf:Property ;
        rdfs:comment  "The type of a loan or credit." ;
        rdfs:label    "loanType" .

schema:MedicalTherapy
        rdf:type         rdfs:Class ;
        rdfs:comment     "Any medical intervention designed to prevent, treat, and cure human diseases and medical conditions, including both curative and palliative therapies. Medical therapies are typically processes of care relying upon pharmacotherapy, behavioral therapy, supportive therapy (with fluid or nutrition for example), or detoxification (e.g. hemodialysis) aimed at improving or preventing a health condition." ;
        rdfs:label       "MedicalTherapy" ;
        rdfs:subClassOf  schema:TherapeuticProcedure .

schema:BookmarkAction
        rdf:type         rdfs:Class ;
        rdfs:comment     "An agent bookmarks/flags/labels/tags/marks an object." ;
        rdfs:label       "BookmarkAction" ;
        rdfs:subClassOf  schema:OrganizeAction .

schema:modelDate  rdf:type  rdf:Property ;
        rdfs:comment  "The release date of a vehicle model (often used to differentiate versions of the same make and model)." ;
        rdfs:label    "modelDate" .

schema:programType  rdf:type  rdf:Property ;
        rdfs:comment  "The type of educational or occupational program. For example, classroom, internship, alternance, etc.." ;
        rdfs:label    "programType" .

schema:SaleEvent  rdf:type  rdfs:Class ;
        rdfs:comment     "Event type: Sales event." ;
        rdfs:label       "SaleEvent" ;
        rdfs:subClassOf  schema:Event .

schema:travelBans  rdf:type  rdf:Property ;
        rdfs:comment  "Information about travel bans, e.g. in the context of a pandemic." ;
        rdfs:label    "travelBans" .

schema:coursePrerequisites
        rdf:type      rdf:Property ;
        rdfs:comment  "Requirements for taking the Course. May be completion of another [[Course]] or a textual description like \"permission of instructor\". Requirements may be a pre-requisite competency, referenced using [[AlignmentObject]]." ;
        rdfs:label    "coursePrerequisites" .

schema:EmergencyService
        rdf:type         rdfs:Class ;
        rdfs:comment     "An emergency service, such as a fire station or ER." ;
        rdfs:label       "EmergencyService" ;
        rdfs:subClassOf  schema:LocalBusiness .

schema:quest  rdf:type  rdf:Property ;
        rdfs:comment  "The task that a player-controlled character, or group of characters may complete in order to gain a reward." ;
        rdfs:label    "quest" .

schema:Occupation  rdf:type  rdfs:Class ;
        rdfs:comment     "A profession, may involve prolonged training and/or a formal qualification." ;
        rdfs:label       "Occupation" ;
        rdfs:subClassOf  schema:Intangible .

schema:CafeOrCoffeeShop
        rdf:type         rdfs:Class ;
        rdfs:comment     "A cafe or coffee shop." ;
        rdfs:label       "CafeOrCoffeeShop" ;
        rdfs:subClassOf  schema:FoodEstablishment .

schema:runtimePlatform
        rdf:type      rdf:Property ;
        rdfs:comment  "Runtime platform or script interpreter dependencies (Example - Java v1, Python2.3, .Net Framework 3.0)." ;
        rdfs:label    "runtimePlatform" .

schema:accommodationFloorPlan
        rdf:type      rdf:Property ;
        rdfs:comment  "A floorplan of some [[Accommodation]]." ;
        rdfs:label    "accommodationFloorPlan" .

schema:copyrightNotice
        rdf:type      rdf:Property ;
        rdfs:comment  "Text of a notice appropriate for describing the copyright aspects of this Creative Work, ideally indicating the owner of the copyright for the Work." ;
        rdfs:label    "copyrightNotice" .

schema:LendAction  rdf:type  rdfs:Class ;
        rdfs:comment     "The act of providing an object under an agreement that it will be returned at a later date. Reciprocal of BorrowAction.\\n\\nRelated actions:\\n\\n* [[BorrowAction]]: Reciprocal of LendAction." ;
        rdfs:label       "LendAction" ;
        rdfs:subClassOf  schema:TransferAction .

schema:TaxiStand  rdf:type  rdfs:Class ;
        rdfs:comment     "A taxi stand." ;
        rdfs:label       "TaxiStand" ;
        rdfs:subClassOf  schema:CivicStructure .

schema:QuantitativeValue
        rdf:type         rdfs:Class ;
        rdfs:comment     " A point value or interval for product characteristics and other purposes." ;
        rdfs:label       "QuantitativeValue" ;
        rdfs:subClassOf  schema:StructuredValue .

schema:AutomatedTeller
        rdf:type         rdfs:Class ;
        rdfs:comment     "ATM/cash machine." ;
        rdfs:label       "AutomatedTeller" ;
        rdfs:subClassOf  schema:FinancialService .

schema:expires  rdf:type  rdf:Property ;
        rdfs:comment  "Date the content expires and is no longer useful or available. For example a [[VideoObject]] or [[NewsArticle]] whose availability or relevance is time-limited, or a [[ClaimReview]] fact check whose publisher wants to indicate that it may no longer be relevant (or helpful to highlight) after some date." ;
        rdfs:label    "expires" .

schema:abstract  rdf:type  rdf:Property ;
        rdfs:comment  "An abstract is a short description that summarizes a [[CreativeWork]]." ;
        rdfs:label    "abstract" .

schema:availableChannel
        rdf:type      rdf:Property ;
        rdfs:comment  "A means of accessing the service (e.g. a phone bank, a web site, a location, etc.)." ;
        rdfs:label    "availableChannel" .

schema:roofLoad  rdf:type  rdf:Property ;
        rdfs:comment  "The permitted total weight of cargo and installations (e.g. a roof rack) on top of the vehicle.\\n\\nTypical unit code(s): KGM for kilogram, LBR for pound\\n\\n* Note 1: You can indicate additional information in the [[name]] of the [[QuantitativeValue]] node.\\n* Note 2: You may also link to a [[QualitativeValue]] node that provides additional information using [[valueReference]]\\n* Note 3: Note that you can use [[minValue]] and [[maxValue]] to indicate ranges." ;
        rdfs:label    "roofLoad" .

schema:Synagogue  rdf:type  rdfs:Class ;
        rdfs:comment     "A synagogue." ;
        rdfs:label       "Synagogue" ;
        rdfs:subClassOf  schema:PlaceOfWorship .

schema:availableDeliveryMethod
        rdf:type      rdf:Property ;
        rdfs:comment  "The delivery method(s) available for this offer." ;
        rdfs:label    "availableDeliveryMethod" .

schema:acceptedOffer  rdf:type  rdf:Property ;
        rdfs:comment  "The offer(s) -- e.g., product, quantity and price combinations -- included in the order." ;
        rdfs:label    "acceptedOffer" .

schema:broadcastSubChannel
        rdf:type      rdf:Property ;
        rdfs:comment  "The subchannel used for the broadcast." ;
        rdfs:label    "broadcastSubChannel" .

schema:ComicSeries  rdf:type  rdfs:Class ;
        rdfs:comment     "A sequential publication of comic stories under a\n    \tunifying title, for example \"The Amazing Spider-Man\" or \"Groo the\n    \tWanderer\"." ;
        rdfs:label       "ComicSeries" ;
        rdfs:subClassOf  schema:Periodical .

schema:ParentAudience
        rdf:type         rdfs:Class ;
        rdfs:comment     "A set of characteristics describing parents, who can be interested in viewing some content." ;
        rdfs:label       "ParentAudience" ;
        rdfs:subClassOf  schema:PeopleAudience .

schema:departureBoatTerminal
        rdf:type      rdf:Property ;
        rdfs:comment  "The terminal or port from which the boat departs." ;
        rdfs:label    "departureBoatTerminal" .

schema:lodgingUnitDescription
        rdf:type      rdf:Property ;
        rdfs:comment  "A full description of the lodging unit." ;
        rdfs:label    "lodgingUnitDescription" .

schema:numberedPosition
        rdf:type      rdf:Property ;
        rdfs:comment  "A number associated with a role in an organization, for example, the number on an athlete's jersey." ;
        rdfs:label    "numberedPosition" .

schema:carrier  rdf:type  rdf:Property ;
        rdfs:comment  "'carrier' is an out-dated term indicating the 'provider' for parcel delivery and flights." ;
        rdfs:label    "carrier" .

schema:catalogNumber  rdf:type  rdf:Property ;
        rdfs:comment  "The catalog number for the release." ;
        rdfs:label    "catalogNumber" .

schema:Chapter  rdf:type  rdfs:Class ;
        rdfs:comment     "One of the sections into which a book is divided. A chapter usually has a section number or a name." ;
        rdfs:label       "Chapter" ;
        rdfs:subClassOf  schema:CreativeWork .

schema:hasPart  rdf:type  rdf:Property ;
        rdfs:comment  "Indicates an item or CreativeWork that is part of this item, or CreativeWork (in some sense)." ;
        rdfs:label    "hasPart" .

schema:target  rdf:type  rdf:Property ;
        rdfs:comment  "Indicates a target EntryPoint for an Action." ;
        rdfs:label    "target" .

schema:departureTime  rdf:type  rdf:Property ;
        rdfs:comment  "The expected departure time." ;
        rdfs:label    "departureTime" .

schema:Course  rdf:type  rdfs:Class ;
        rdfs:comment     "A description of an educational course which may be offered as distinct instances at which take place at different times or take place at different locations, or be offered through different media or modes of study. An educational course is a sequence of one or more educational events and/or creative works which aims to build knowledge, competence or ability of learners." ;
        rdfs:label       "Course" ;
        rdfs:subClassOf  schema:LearningResource , schema:CreativeWork .

schema:feesAndCommissionsSpecification
        rdf:type      rdf:Property ;
        rdfs:comment  "Description of fees, commissions, and other terms applied either to a class of financial product, or by a financial service organization." ;
        rdfs:label    "feesAndCommissionsSpecification" .

schema:BefriendAction
        rdf:type         rdfs:Class ;
        rdfs:comment     "The act of forming a personal connection with someone (object) mutually/bidirectionally/symmetrically.\\n\\nRelated actions:\\n\\n* [[FollowAction]]: Unlike FollowAction, BefriendAction implies that the connection is reciprocal." ;
        rdfs:label       "BefriendAction" ;
        rdfs:subClassOf  schema:InteractAction .

schema:Bridge  rdf:type  rdfs:Class ;
        rdfs:comment     "A bridge." ;
        rdfs:label       "Bridge" ;
        rdfs:subClassOf  schema:CivicStructure .

skos:member  rdf:type  owl:ObjectProperty ;
        rdfs:domain  skos:Collection ;
        rdfs:label   "has member"@en .

schema:FAQPage  rdf:type  rdfs:Class ;
        rdfs:comment     "A [[FAQPage]] is a [[WebPage]] presenting one or more \"[Frequently asked questions](https://en.wikipedia.org/wiki/FAQ)\" (see also [[QAPage]])." ;
        rdfs:label       "FAQPage" ;
        rdfs:subClassOf  schema:WebPage .

schema:sizeGroup  rdf:type  rdf:Property ;
        rdfs:comment  "The size group (also known as \"size type\") for a product's size. Size groups are common in the fashion industry to define size segments and suggested audiences for wearable products. Multiple values can be combined, for example \"men's big and tall\", \"petite maternity\" or \"regular\"" ;
        rdfs:label    "sizeGroup" .

schema:ProductGroup  rdf:type  rdfs:Class ;
        rdfs:comment     "A ProductGroup represents a group of [[Product]]s that vary only in certain well-described ways, such as by [[size]], [[color]], [[material]] etc.\n\nWhile a ProductGroup itself is not directly offered for sale, the various varying products that it represents can be. The ProductGroup serves as a prototype or template, standing in for all of the products who have an [[isVariantOf]] relationship to it. As such, properties (including additional types) can be applied to the ProductGroup to represent characteristics shared by each of the (possibly very many) variants. Properties that reference a ProductGroup are not included in this mechanism; neither are the following specific properties [[variesBy]], [[hasVariant]], [[url]]. " ;
        rdfs:label       "ProductGroup" ;
        rdfs:subClassOf  schema:Product .

schema:albumRelease  rdf:type  rdf:Property ;
        rdfs:comment  "A release of this album." ;
        rdfs:label    "albumRelease" .

schema:clinicalPharmacology
        rdf:type      rdf:Property ;
        rdfs:comment  "Description of the absorption and elimination of drugs, including their concentration (pharmacokinetics, pK) and biological effects (pharmacodynamics, pD)." ;
        rdfs:label    "clinicalPharmacology" .

schema:prescribingInfo
        rdf:type      rdf:Property ;
        rdfs:comment  "Link to prescribing information for the drug." ;
        rdfs:label    "prescribingInfo" .

schema:commentCount  rdf:type  rdf:Property ;
        rdfs:comment  "The number of comments this CreativeWork (e.g. Article, Question or Answer) has received. This is most applicable to works published in Web sites with commenting system; additional comments may exist elsewhere." ;
        rdfs:label    "commentCount" .

schema:width  rdf:type  rdf:Property ;
        rdfs:comment  "The width of the item." ;
        rdfs:label    "width" .

schema:itemLocation  rdf:type  rdf:Property ;
        rdfs:comment        "Current location of the item."@en ;
        rdfs:label          "itemLocation"@en ;
        rdfs:subPropertyOf  schema:location .

schema:VideoGameClip  rdf:type  rdfs:Class ;
        rdfs:comment     "A short segment/part of a video game." ;
        rdfs:label       "VideoGameClip" ;
        rdfs:subClassOf  schema:Clip .

schema:Movie  rdf:type   rdfs:Class ;
        rdfs:comment     "A movie." ;
        rdfs:label       "Movie" ;
        rdfs:subClassOf  schema:CreativeWork .

schema:PhotographAction
        rdf:type         rdfs:Class ;
        rdfs:comment     "The act of capturing still images of objects using a camera." ;
        rdfs:label       "PhotographAction" ;
        rdfs:subClassOf  schema:CreateAction .

schema:DigitalDocumentPermission
        rdf:type         rdfs:Class ;
        rdfs:comment     "A permission for a particular person or group to access a particular file." ;
        rdfs:label       "DigitalDocumentPermission" ;
        rdfs:subClassOf  schema:Intangible .

schema:Emergency  rdf:type  rdfs:Class ;
        rdfs:comment     "A specific branch of medical science that deals with the evaluation and initial treatment of medical conditions caused by trauma or sudden illness." ;
        rdfs:label       "Emergency" ;
        rdfs:subClassOf  schema:MedicalBusiness .

schema:ListItem  rdf:type  rdfs:Class ;
        rdfs:comment     "An list item, e.g. a step in a checklist or how-to description." ;
        rdfs:label       "ListItem" ;
        rdfs:subClassOf  schema:Intangible .

schema:startDate  rdf:type  rdf:Property ;
        rdfs:comment  "The start date and time of the item (in [ISO 8601 date format](http://en.wikipedia.org/wiki/ISO_8601))." ;
        rdfs:label    "startDate" .

schema:servesCuisine  rdf:type  rdf:Property ;
        rdfs:comment  "The cuisine of the restaurant." ;
        rdfs:label    "servesCuisine" .

schema:replacee  rdf:type   rdf:Property ;
        rdfs:comment        "A sub property of object. The object that is being replaced." ;
        rdfs:label          "replacee" ;
        rdfs:subPropertyOf  schema:object .

schema:dosageForm  rdf:type  rdf:Property ;
        rdfs:comment  "A dosage form in which this drug/supplement is available, e.g. 'tablet', 'suspension', 'injection'." ;
        rdfs:label    "dosageForm" .

schema:variesBy  rdf:type  rdf:Property ;
        rdfs:comment  "Indicates the property or properties by which the variants in a [[ProductGroup]] vary, e.g. their size, color etc. Schema.org properties can be referenced by their short name e.g. \"color\"; terms defined elsewhere can be referenced with their URIs." ;
        rdfs:label    "variesBy" .

schema:experienceInPlaceOfEducation
        rdf:type      rdf:Property ;
        rdfs:comment  "Indicates whether a [[JobPosting]] will accept experience (as indicated by [[OccupationalExperienceRequirements]]) in place of its formal educational qualifications (as indicated by [[educationRequirements]]). If true, indicates that satisfying one of these requirements is sufficient." ;
        rdfs:label    "experienceInPlaceOfEducation" .

schema:description  rdf:type  rdf:Property ;
        rdfs:comment  "A description of the item." ;
        rdfs:label    "description" .

schema:prescriptionStatus
        rdf:type      rdf:Property ;
        rdfs:comment  "Indicates the status of drug prescription eg. local catalogs classifications or whether the drug is available by prescription or over-the-counter, etc." ;
        rdfs:label    "prescriptionStatus" .

schema:maximumEnrollment
        rdf:type      rdf:Property ;
        rdfs:comment  "The maximum number of students who may be enrolled in the program." ;
        rdfs:label    "maximumEnrollment" .

schema:availableIn  rdf:type  rdf:Property ;
        rdfs:comment  "The location in which the strength is available." ;
        rdfs:label    "availableIn" .

schema:Project  rdf:type  rdfs:Class ;
        rdfs:comment     "An enterprise (potentially individual but typically collaborative), planned to achieve a particular aim.\nUse properties from [[Organization]], [[subOrganization]]/[[parentOrganization]] to indicate project sub-structures. \n   " ;
        rdfs:label       "Project" ;
        rdfs:subClassOf  schema:Organization .

schema:Conversation  rdf:type  rdfs:Class ;
        rdfs:comment     "One or more messages between organizations or people on a particular topic. Individual messages can be linked to the conversation with isPartOf or hasPart properties." ;
        rdfs:label       "Conversation" ;
        rdfs:subClassOf  schema:CreativeWork .

schema:isbn  rdf:type       rdf:Property ;
        rdfs:comment        "The ISBN of the book." ;
        rdfs:label          "isbn" ;
        rdfs:subPropertyOf  schema:identifier .

schema:paymentUrl  rdf:type  rdf:Property ;
        rdfs:comment  "The URL for sending a payment." ;
        rdfs:label    "paymentUrl" .

schema:ReviewAction  rdf:type  rdfs:Class ;
        rdfs:comment     "The act of producing a balanced opinion about the object for an audience. An agent reviews an object with participants resulting in a review." ;
        rdfs:label       "ReviewAction" ;
        rdfs:subClassOf  schema:AssessAction .

schema:accessibilityHazard
        rdf:type      rdf:Property ;
        rdfs:comment  "A characteristic of the described resource that is physiologically dangerous to some users. Related to WCAG 2.0 guideline 2.3 ([WebSchemas wiki lists possible values](http://www.w3.org/wiki/WebSchemas/Accessibility))." ;
        rdfs:label    "accessibilityHazard" .

schema:timeToComplete
        rdf:type      rdf:Property ;
        rdfs:comment  "The expected length of time to complete the program if attending full-time." ;
        rdfs:label    "timeToComplete" .

schema:Ligament  rdf:type  rdfs:Class ;
        rdfs:comment     "A short band of tough, flexible, fibrous connective tissue that functions to connect multiple bones, cartilages, and structurally support joints." ;
        rdfs:label       "Ligament" ;
        rdfs:subClassOf  schema:AnatomicalStructure .

schema:OnDemandEvent  rdf:type  rdfs:Class ;
        rdfs:comment     "A publication event e.g. catch-up TV or radio podcast, during which a program is available on-demand." ;
        rdfs:label       "OnDemandEvent" ;
        rdfs:subClassOf  schema:PublicationEvent .

schema:priceValidUntil
        rdf:type      rdf:Property ;
        rdfs:comment  "The date after which the price is no longer available." ;
        rdfs:label    "priceValidUntil" .

schema:percentile75  rdf:type  rdf:Property ;
        rdfs:comment  "The 75th percentile value." ;
        rdfs:label    "percentile75" .

schema:TheaterEvent  rdf:type  rdfs:Class ;
        rdfs:comment     "Event type: Theater performance." ;
        rdfs:label       "TheaterEvent" ;
        rdfs:subClassOf  schema:Event .

schema:homeLocation  rdf:type  rdf:Property ;
        rdfs:comment        "A contact location for a person's residence." ;
        rdfs:label          "homeLocation" ;
        rdfs:subPropertyOf  schema:location .

schema:occupationalCredentialAwarded
        rdf:type      rdf:Property ;
        rdfs:comment  "A description of the qualification, award, certificate, diploma or other occupational credential awarded as a consequence of successful completion of this course or program." ;
        rdfs:label    "occupationalCredentialAwarded" .

schema:agent  rdf:type  rdf:Property ;
        rdfs:comment  "The direct performer or driver of the action (animate or inanimate). e.g. *John* wrote a book." ;
        rdfs:label    "agent" .

schema:AdministrativeArea
        rdf:type         rdfs:Class ;
        rdfs:comment     "A geographical region, typically under the jurisdiction of a particular government." ;
        rdfs:label       "AdministrativeArea" ;
        rdfs:subClassOf  schema:Place .

schema:defaultValue  rdf:type  rdf:Property ;
        rdfs:comment  "The default value of the input.  For properties that expect a literal, the default is a literal value, for properties that expect an object, it's an ID reference to one of the current values." ;
        rdfs:label    "defaultValue" .

schema:colleagues  rdf:type  rdf:Property ;
        rdfs:comment  "A colleague of the person." ;
        rdfs:label    "colleagues" .

schema:numConstraints
        rdf:type      rdf:Property ;
        rdfs:comment  "Indicates the number of constraints (not counting [[populationType]]) defined for a particular [[StatisticalPopulation]]. This helps applications understand if they have access to a sufficiently complete description of a [[StatisticalPopulation]]." ;
        rdfs:label    "numConstraints" .

skos:definition  rdf:type   rdf:Property ;
        rdfs:label          "definition"@en ;
        rdfs:subPropertyOf  skos:note .

schema:frequency  rdf:type  rdf:Property ;
        rdfs:comment  "How often the dose is taken, e.g. 'daily'." ;
        rdfs:label    "frequency" .

schema:isAccessibleForFree
        rdf:type      rdf:Property ;
        rdfs:comment  "A flag to signal that the item, event, or place is accessible for free." ;
        rdfs:label    "isAccessibleForFree" .

schema:MediaManipulationRatingEnumeration
        rdf:type         rdfs:Class ;
        rdfs:comment     " Codes for use with the [[mediaAuthenticityCategory]] property, indicating the authenticity of a media object (in the context of how it was published or shared). In general these codes are not mutually exclusive, although some combinations (such as 'original' versus 'transformed', 'edited' and 'staged') would be contradictory if applied in the same [[MediaReview]]. Note that the application of these codes is with regard to a piece of media shared or published in a particular context." ;
        rdfs:label       "MediaManipulationRatingEnumeration" ;
        rdfs:subClassOf  schema:Enumeration .

schema:numberOfFullBathrooms
        rdf:type      rdf:Property ;
        rdfs:comment  "Number of full bathrooms - The total number of full and ¾ bathrooms in an [[Accommodation]]. This corresponds to the [BathroomsFull field in RESO](https://ddwiki.reso.org/display/DDW17/BathroomsFull+Field)." ;
        rdfs:label    "numberOfFullBathrooms" .

schema:Preschool  rdf:type  rdfs:Class ;
        rdfs:comment     "A preschool." ;
        rdfs:label       "Preschool" ;
        rdfs:subClassOf  schema:EducationalOrganization .

schema:ItemList  rdf:type  rdfs:Class ;
        rdfs:comment     "A list of items of any sort&#x2014;for example, Top 10 Movies About Weathermen, or Top 100 Party Songs. Not to be confused with HTML lists, which are often used only for formatting." ;
        rdfs:label       "ItemList" ;
        rdfs:subClassOf  schema:Intangible .

schema:SocialEvent  rdf:type  rdfs:Class ;
        rdfs:comment     "Event type: Social event." ;
        rdfs:label       "SocialEvent" ;
        rdfs:subClassOf  schema:Event .

schema:ExhibitionEvent
        rdf:type         rdfs:Class ;
        rdfs:comment     "Event type: Exhibition event, e.g. at a museum, library, archive, tradeshow, ..." ;
        rdfs:label       "ExhibitionEvent" ;
        rdfs:subClassOf  schema:Event .

schema:ArchiveOrganization
        rdf:type         rdfs:Class ;
        rdfs:comment     "An organization with archival holdings. An organization which keeps and preserves archival material and typically makes it accessible to the public."@en ;
        rdfs:label       "ArchiveOrganization"@en ;
        rdfs:subClassOf  schema:LocalBusiness .

schema:engineType  rdf:type  rdf:Property ;
        rdfs:comment  "The type of engine or engines powering the vehicle." ;
        rdfs:label    "engineType" .

schema:FlightReservation
        rdf:type         rdfs:Class ;
        rdfs:comment     "A reservation for air travel.\\n\\nNote: This type is for information about actual reservations, e.g. in confirmation emails or HTML pages with individual confirmations of reservations. For offers of tickets, use [[Offer]]." ;
        rdfs:label       "FlightReservation" ;
        rdfs:subClassOf  schema:Reservation .

schema:sportsTeam  rdf:type  rdf:Property ;
        rdfs:comment        "A sub property of participant. The sports team that participated on this action." ;
        rdfs:label          "sportsTeam" ;
        rdfs:subPropertyOf  schema:participant .

schema:availableFrom  rdf:type  rdf:Property ;
        rdfs:comment  "When the item is available for pickup from the store, locker, etc." ;
        rdfs:label    "availableFrom" .

schema:MedicalDevicePurpose
        rdf:type         rdfs:Class ;
        rdfs:comment     "Categories of medical devices, organized by the purpose or intended use of the device." ;
        rdfs:label       "MedicalDevicePurpose" ;
        rdfs:subClassOf  schema:MedicalEnumeration .

schema:TechArticle  rdf:type  rdfs:Class ;
        rdfs:comment     "A technical article - Example: How-to (task) topics, step-by-step, procedural troubleshooting, specifications, etc." ;
        rdfs:label       "TechArticle" ;
        rdfs:subClassOf  schema:Article .

schema:code  rdf:type  rdf:Property ;
        rdfs:comment  "A medical code for the entity, taken from a controlled vocabulary or ontology such as ICD-9, DiseasesDB, MeSH, SNOMED-CT, RxNorm, etc." ;
        rdfs:label    "code" .

schema:InvestmentOrDeposit
        rdf:type         rdfs:Class ;
        rdfs:comment     "A type of financial product that typically requires the client to transfer funds to a financial service in return for potential beneficial financial return." ;
        rdfs:label       "InvestmentOrDeposit" ;
        rdfs:subClassOf  schema:FinancialProduct .

schema:valueName  rdf:type  rdf:Property ;
        rdfs:comment  "Indicates the name of the PropertyValueSpecification to be used in URL templates and form encoding in a manner analogous to HTML's input@name." ;
        rdfs:label    "valueName" .

schema:diseasePreventionInfo
        rdf:type      rdf:Property ;
        rdfs:comment  "Information about disease prevention." ;
        rdfs:label    "diseasePreventionInfo" .

schema:normalRange  rdf:type  rdf:Property ;
        rdfs:comment  "Range of acceptable values for a typical patient, when applicable." ;
        rdfs:label    "normalRange" .

skos:related  rdf:type      owl:ObjectProperty ;
        rdfs:comment        "skos:related is disjoint with skos:broaderTransitive"@en ;
        rdfs:label          "has related"@en ;
        rdfs:subPropertyOf  skos:semanticRelation .

schema:SoftwareApplication
        rdf:type         rdfs:Class ;
        rdfs:comment     "A software application." ;
        rdfs:label       "SoftwareApplication" ;
        rdfs:subClassOf  schema:CreativeWork .

schema:PublicToilet  rdf:type  rdfs:Class ;
        rdfs:comment     "A public toilet is a room or small building containing one or more toilets (and possibly also urinals) which is available for use by the general public, or by customers or employees of certain businesses." ;
        rdfs:label       "PublicToilet" ;
        rdfs:subClassOf  schema:CivicStructure .

schema:alumni  rdf:type  rdf:Property ;
        rdfs:comment  "Alumni of an organization." ;
        rdfs:label    "alumni" .

schema:billingStart  rdf:type  rdf:Property ;
        rdfs:comment  "Specifies after how much time this price (or price component) becomes valid and billing starts. Can be used, for example, to model a price increase after the first year of a subscription. The unit of measurement is specified by the unitCode property." ;
        rdfs:label    "billingStart" .

schema:publisher  rdf:type  rdf:Property ;
        rdfs:comment  "The publisher of the creative work." ;
        rdfs:label    "publisher" .

schema:totalJobOpenings
        rdf:type      rdf:Property ;
        rdfs:comment  "The number of positions open for this job posting. Use a positive integer. Do not use if the number of positions is unclear or not known." ;
        rdfs:label    "totalJobOpenings" .

schema:globalLocationNumber
        rdf:type            rdf:Property ;
        rdfs:comment        "The [Global Location Number](http://www.gs1.org/gln) (GLN, sometimes also referred to as International Location Number or ILN) of the respective organization, person, or place. The GLN is a 13-digit number used to identify parties and physical locations." ;
        rdfs:label          "globalLocationNumber" ;
        rdfs:subPropertyOf  schema:identifier .

schema:Schedule  rdf:type  rdfs:Class ;
        rdfs:comment     "A schedule defines a repeating time period used to describe a regularly occurring [[Event]]. At a minimum a schedule will specify [[repeatFrequency]] which describes the interval between occurences of the event. Additional information can be provided to specify the schedule more precisely.\n      This includes identifying the day(s) of the week or month when the recurring event will take place, in addition to its start and end time. Schedules may also\n      have start and end dates to indicate when they are active, e.g. to define a limited calendar of events." ;
        rdfs:label       "Schedule" ;
        rdfs:subClassOf  schema:Intangible .

schema:CreativeWorkSeason
        rdf:type         rdfs:Class ;
        rdfs:comment     "A media season e.g. tv, radio, video game etc." ;
        rdfs:label       "CreativeWorkSeason" ;
        rdfs:subClassOf  schema:CreativeWork .

schema:termDuration  rdf:type  rdf:Property ;
        rdfs:comment  "The amount of time in a term as defined by the institution. A term is a length of time where students take one or more classes. Semesters and quarters are common units for term." ;
        rdfs:label    "termDuration" .

schema:MedicalEntity  rdf:type  rdfs:Class ;
        rdfs:comment     "The most generic type of entity related to health and the practice of medicine." ;
        rdfs:label       "MedicalEntity" ;
        rdfs:subClassOf  schema:Thing .

schema:productGroupID
        rdf:type      rdf:Property ;
        rdfs:comment  "Indicates a textual identifier for a ProductGroup." ;
        rdfs:label    "productGroupID" .

schema:ticketNumber  rdf:type  rdf:Property ;
        rdfs:comment  "The unique identifier for the ticket." ;
        rdfs:label    "ticketNumber" .

schema:Diet  rdf:type    rdfs:Class ;
        rdfs:comment     "A strategy of regulating the intake of food to achieve or maintain a specific health-related goal." ;
        rdfs:label       "Diet" ;
        rdfs:subClassOf  schema:LifestyleModification , schema:CreativeWork .

schema:isrcCode  rdf:type  rdf:Property ;
        rdfs:comment  "The International Standard Recording Code for the recording." ;
        rdfs:label    "isrcCode" .

schema:Map  rdf:type     rdfs:Class ;
        rdfs:comment     "A map." ;
        rdfs:label       "Map" ;
        rdfs:subClassOf  schema:CreativeWork .

schema:legislationLegalValue
        rdf:type      rdf:Property ;
        rdfs:comment  "The legal value of this legislation file. The same legislation can be written in multiple files with different legal values. Typically a digitally signed PDF have a \"stronger\" legal value than the HTML file of the same act." ;
        rdfs:label    "legislationLegalValue" .

schema:BusStop  rdf:type  rdfs:Class ;
        rdfs:comment     "A bus stop." ;
        rdfs:label       "BusStop" ;
        rdfs:subClassOf  schema:CivicStructure .

schema:Midwifery  rdf:type  rdfs:Class ;
        rdfs:comment     "A nurse-like health profession that deals with pregnancy, childbirth, and the postpartum period (including care of the newborn), besides sexual and reproductive health of women throughout their lives." ;
        rdfs:label       "Midwifery" ;
        rdfs:subClassOf  schema:MedicalBusiness .

schema:Courthouse  rdf:type  rdfs:Class ;
        rdfs:comment     "A courthouse." ;
        rdfs:label       "Courthouse" ;
        rdfs:subClassOf  schema:GovernmentBuilding .

schema:PerformAction  rdf:type  rdfs:Class ;
        rdfs:comment     "The act of participating in performance arts." ;
        rdfs:label       "PerformAction" ;
        rdfs:subClassOf  schema:PlayAction .

schema:ElementarySchool
        rdf:type         rdfs:Class ;
        rdfs:comment     "An elementary school." ;
        rdfs:label       "ElementarySchool" ;
        rdfs:subClassOf  schema:EducationalOrganization .

schema:recipeYield  rdf:type  rdf:Property ;
        rdfs:comment        "The quantity produced by the recipe (for example, number of people served, number of servings, etc)." ;
        rdfs:label          "recipeYield" ;
        rdfs:subPropertyOf  schema:yield .

schema:containsSeason
        rdf:type            rdf:Property ;
        rdfs:comment        "A season that is part of the media series." ;
        rdfs:label          "containsSeason" ;
        rdfs:subPropertyOf  schema:hasPart .

schema:sourcedFrom  rdf:type  rdf:Property ;
        rdfs:comment  "The neurological pathway that originates the neurons." ;
        rdfs:label    "sourcedFrom" .

schema:downPayment  rdf:type  rdf:Property ;
        rdfs:comment  "a type of payment made in cash during the onset of the purchase of an expensive good/service. The payment typically represents only a percentage of the full purchase price." ;
        rdfs:label    "downPayment" .

schema:shippingDetails
        rdf:type      rdf:Property ;
        rdfs:comment  "Indicates information about the shipping policies and options associated with an [[Offer]]." ;
        rdfs:label    "shippingDetails" .

schema:softwareAddOn  rdf:type  rdf:Property ;
        rdfs:comment  "Additional content for a software application." ;
        rdfs:label    "softwareAddOn" .

schema:MedicalImagingTechnique
        rdf:type         rdfs:Class ;
        rdfs:comment     "Any medical imaging modality typically used for diagnostic purposes. Enumerated type." ;
        rdfs:label       "MedicalImagingTechnique" ;
        rdfs:subClassOf  schema:MedicalEnumeration .

schema:trialDesign  rdf:type  rdf:Property ;
        rdfs:comment  "Specifics about the trial design (enumerated)." ;
        rdfs:label    "trialDesign" .

schema:WPFooter  rdf:type  rdfs:Class ;
        rdfs:comment     "The footer section of the page." ;
        rdfs:label       "WPFooter" ;
        rdfs:subClassOf  schema:WebPageElement .

schema:merchantReturnLink
        rdf:type      rdf:Property ;
        rdfs:comment  "Indicates a Web page or service by URL, for product return." ;
        rdfs:label    "merchantReturnLink" .

schema:targetPlatform
        rdf:type      rdf:Property ;
        rdfs:comment  "Type of app development: phone, Metro style, desktop, XBox, etc." ;
        rdfs:label    "targetPlatform" .

schema:DrugStrength  rdf:type  rdfs:Class ;
        rdfs:comment     "A specific strength in which a medical drug is available in a specific country." ;
        rdfs:label       "DrugStrength" ;
        rdfs:subClassOf  schema:MedicalIntangible .

schema:ToyStore  rdf:type  rdfs:Class ;
        rdfs:comment     "A toy store." ;
        rdfs:label       "ToyStore" ;
        rdfs:subClassOf  schema:Store .

schema:encoding  rdf:type  rdf:Property ;
        rdfs:comment  "A media object that encodes this CreativeWork. This property is a synonym for associatedMedia." ;
        rdfs:label    "encoding" .

schema:VitalSign  rdf:type  rdfs:Class ;
        rdfs:comment     "Vital signs are measures of various physiological functions in order to assess the most basic body functions." ;
        rdfs:label       "VitalSign" ;
        rdfs:subClassOf  schema:MedicalSign .

schema:beneficiaryBank
        rdf:type      rdf:Property ;
        rdfs:comment  "A bank or bank’s branch, financial institution or international financial institution operating the beneficiary’s bank account or releasing funds for the beneficiary." ;
        rdfs:label    "beneficiaryBank" .

schema:saturatedFatContent
        rdf:type      rdf:Property ;
        rdfs:comment  "The number of grams of saturated fat." ;
        rdfs:label    "saturatedFatContent" .

schema:smokingAllowed
        rdf:type      rdf:Property ;
        rdfs:comment  "Indicates whether it is allowed to smoke in the place, e.g. in the restaurant, hotel or hotel room." ;
        rdfs:label    "smokingAllowed" .

schema:TakeAction  rdf:type  rdfs:Class ;
        rdfs:comment     "The act of gaining ownership of an object from an origin. Reciprocal of GiveAction.\\n\\nRelated actions:\\n\\n* [[GiveAction]]: The reciprocal of TakeAction.\\n* [[ReceiveAction]]: Unlike ReceiveAction, TakeAction implies that ownership has been transfered." ;
        rdfs:label       "TakeAction" ;
        rdfs:subClassOf  schema:TransferAction .

schema:GeoCircle  rdf:type  rdfs:Class ;
        rdfs:comment     "A GeoCircle is a GeoShape representing a circular geographic area. As it is a GeoShape\n          it provides the simple textual property 'circle', but also allows the combination of postalCode alongside geoRadius.\n          The center of the circle can be indicated via the 'geoMidpoint' property, or more approximately using 'address', 'postalCode'.\n       " ;
        rdfs:label       "GeoCircle" ;
        rdfs:subClassOf  schema:GeoShape .

schema:HealthClub  rdf:type  rdfs:Class ;
        rdfs:comment     "A health club." ;
        rdfs:label       "HealthClub" ;
        rdfs:subClassOf  schema:SportsActivityLocation , schema:HealthAndBeautyBusiness .

schema:insertion  rdf:type  rdf:Property ;
        rdfs:comment  "The place of attachment of a muscle, or what the muscle moves." ;
        rdfs:label    "insertion" .

schema:founders  rdf:type  rdf:Property ;
        rdfs:comment  "A person who founded this organization." ;
        rdfs:label    "founders" .

schema:familyName  rdf:type  rdf:Property ;
        rdfs:comment  "Family name. In the U.S., the last name of a Person." ;
        rdfs:label    "familyName" .

schema:Text  rdf:type  rdfs:Class ;
        rdfs:comment  "Data type: Text." ;
        rdfs:label    "Text" .

schema:mechanismOfAction
        rdf:type      rdf:Property ;
        rdfs:comment  "The specific biochemical interaction through which this drug or supplement produces its pharmacological effect." ;
        rdfs:label    "mechanismOfAction" .

schema:playerType  rdf:type  rdf:Property ;
        rdfs:comment  "Player type required&#x2014;for example, Flash or Silverlight." ;
        rdfs:label    "playerType" .

skos:altLabel  rdf:type     rdf:Property ;
        rdfs:comment        "skos:prefLabel, skos:altLabel and skos:hiddenLabel are pairwise disjoint properties."@en , "The range of skos:altLabel is the class of RDF plain literals."@en ;
        rdfs:label          "alternative label"@en ;
        rdfs:subPropertyOf  rdfs:label .

schema:Offer  rdf:type   rdfs:Class ;
        rdfs:comment     "An offer to transfer some rights to an item or to provide a service — for example, an offer to sell tickets to an event, to rent the DVD of a movie, to stream a TV show over the internet, to repair a motorcycle, or to loan a book.\\n\\nNote: As the [[businessFunction]] property, which identifies the form of offer (e.g. sell, lease, repair, dispose), defaults to http://purl.org/goodrelations/v1#Sell; an Offer without a defined businessFunction value can be assumed to be an offer to sell.\\n\\nFor [GTIN](http://www.gs1.org/barcodes/technical/idkeys/gtin)-related fields, see [Check Digit calculator](http://www.gs1.org/barcodes/support/check_digit_calculator) and [validation guide](http://www.gs1us.org/resources/standards/gtin-validation-guide) from [GS1](http://www.gs1.org/)." ;
        rdfs:label       "Offer" ;
        rdfs:subClassOf  schema:Intangible .

schema:ActionStatusType
        rdf:type         rdfs:Class ;
        rdfs:comment     "The status of an Action." ;
        rdfs:label       "ActionStatusType" ;
        rdfs:subClassOf  schema:StatusEnumeration .

schema:populationType
        rdf:type      rdf:Property ;
        rdfs:comment  "Indicates the populationType common to all members of a [[StatisticalPopulation]]." ;
        rdfs:label    "populationType" .

schema:WebSite  rdf:type  rdfs:Class ;
        rdfs:comment     "A WebSite is a set of related web pages and other items typically served from a single web domain and accessible via URLs." ;
        rdfs:label       "WebSite" ;
        rdfs:subClassOf  schema:CreativeWork .

schema:RespiratoryTherapy
        rdf:type         rdfs:Class ;
        rdfs:comment     "The therapy that is concerned with the maintenance or improvement of respiratory function (as in patients with pulmonary disease)." ;
        rdfs:label       "RespiratoryTherapy" ;
        rdfs:subClassOf  schema:MedicalTherapy .

schema:healthPlanMarketingUrl
        rdf:type      rdf:Property ;
        rdfs:comment  "The URL that goes directly to the plan brochure for the specific standard plan or plan variation." ;
        rdfs:label    "healthPlanMarketingUrl" .

schema:itemReviewed  rdf:type  rdf:Property ;
        rdfs:comment  "The item that is being reviewed/rated." ;
        rdfs:label    "itemReviewed" .

schema:MedicalStudy  rdf:type  rdfs:Class ;
        rdfs:comment     "A medical study is an umbrella type covering all kinds of research studies relating to human medicine or health, including observational studies and interventional trials and registries, randomized, controlled or not. When the specific type of study is known, use one of the extensions of this type, such as MedicalTrial or MedicalObservationalStudy. Also, note that this type should be used to mark up data that describes the study itself; to tag an article that publishes the results of a study, use MedicalScholarlyArticle. Note: use the code property of MedicalEntity to store study IDs, e.g. clinicaltrials.gov ID." ;
        rdfs:label       "MedicalStudy" ;
        rdfs:subClassOf  schema:MedicalEntity .

schema:CreativeWork  rdf:type  rdfs:Class ;
        rdfs:comment     "The most generic kind of creative work, including books, movies, photographs, software programs, etc." ;
        rdfs:label       "CreativeWork" ;
        rdfs:subClassOf  schema:Thing .

schema:iataCode  rdf:type  rdf:Property ;
        rdfs:comment  "IATA identifier for an airline or airport." ;
        rdfs:label    "iataCode" .

schema:MusicGroup  rdf:type  rdfs:Class ;
        rdfs:comment     "A musical group, such as a band, an orchestra, or a choir. Can also be a solo musician." ;
        rdfs:label       "MusicGroup" ;
        rdfs:subClassOf  schema:PerformingGroup .

bibo:Issue  rdf:type  rdfs:Class .

schema:orderQuantity  rdf:type  rdf:Property ;
        rdfs:comment  "The number of the item ordered. If the property is not set, assume the quantity is one." ;
        rdfs:label    "orderQuantity" .

schema:includedInHealthInsurancePlan
        rdf:type      rdf:Property ;
        rdfs:comment  "The insurance plans that cover this drug." ;
        rdfs:label    "includedInHealthInsurancePlan" .

schema:Embassy  rdf:type  rdfs:Class ;
        rdfs:comment     "An embassy." ;
        rdfs:label       "Embassy" ;
        rdfs:subClassOf  schema:GovernmentBuilding .

schema:nsn  rdf:type        rdf:Property ;
        rdfs:comment        "Indicates the [NATO stock number](https://en.wikipedia.org/wiki/NATO_Stock_Number) (nsn) of a [[Product]]. " ;
        rdfs:label          "nsn" ;
        rdfs:subPropertyOf  schema:identifier .

schema:reviewedBy  rdf:type  rdf:Property ;
        rdfs:comment  "People or organizations that have reviewed the content on this web page for accuracy and/or completeness." ;
        rdfs:label    "reviewedBy" .

schema:itemListOrder  rdf:type  rdf:Property ;
        rdfs:comment  "Type of ordering (e.g. Ascending, Descending, Unordered)." ;
        rdfs:label    "itemListOrder" .

schema:ReactAction  rdf:type  rdfs:Class ;
        rdfs:comment     "The act of responding instinctively and emotionally to an object, expressing a sentiment." ;
        rdfs:label       "ReactAction" ;
        rdfs:subClassOf  schema:AssessAction .

schema:EventStatusType
        rdf:type         rdfs:Class ;
        rdfs:comment     "EventStatusType is an enumeration type whose instances represent several states that an Event may be in." ;
        rdfs:label       "EventStatusType" ;
        rdfs:subClassOf  schema:StatusEnumeration .

schema:dateIssued  rdf:type  rdf:Property ;
        rdfs:comment  "The date the ticket was issued." ;
        rdfs:label    "dateIssued" .

schema:processorRequirements
        rdf:type      rdf:Property ;
        rdfs:comment  "Processor architecture required to run the application (e.g. IA64)." ;
        rdfs:label    "processorRequirements" .

schema:seatingType  rdf:type  rdf:Property ;
        rdfs:comment  "The type/class of the seat." ;
        rdfs:label    "seatingType" .

schema:MapCategoryType
        rdf:type         rdfs:Class ;
        rdfs:comment     "An enumeration of several kinds of Map." ;
        rdfs:label       "MapCategoryType" ;
        rdfs:subClassOf  schema:Enumeration .

schema:maximumIntake  rdf:type  rdf:Property ;
        rdfs:comment  "Recommended intake of this supplement for a given population as defined by a specific recommending authority." ;
        rdfs:label    "maximumIntake" .

schema:Room  rdf:type    rdfs:Class ;
        rdfs:comment     "A room is a distinguishable space within a structure, usually separated from other spaces by interior walls. (Source: Wikipedia, the free encyclopedia, see <a href=\"http://en.wikipedia.org/wiki/Room\">http://en.wikipedia.org/wiki/Room</a>).\n<br /><br />\nSee also the <a href=\"/docs/hotels.html\">dedicated document on the use of schema.org for marking up hotels and other forms of accommodations</a>.\n" ;
        rdfs:label       "Room" ;
        rdfs:subClassOf  schema:Accommodation .

schema:torque  rdf:type  rdf:Property ;
        rdfs:comment  "The torque (turning force) of the vehicle's engine.\\n\\nTypical unit code(s): NU for newton metre (N m), F17 for pound-force per foot, or F48 for pound-force per inch\\n\\n* Note 1: You can link to information about how the given value has been determined (e.g. reference RPM) using the [[valueReference]] property.\\n* Note 2: You can use [[minValue]] and [[maxValue]] to indicate ranges." ;
        rdfs:label    "torque" .

schema:geoContains  rdf:type  rdf:Property ;
        rdfs:comment  "Represents a relationship between two geometries (or the places they represent), relating a containing geometry to a contained geometry. \"a contains b iff no points of b lie in the exterior of a, and at least one point of the interior of b lies in the interior of a\". As defined in [DE-9IM](https://en.wikipedia.org/wiki/DE-9IM)." ;
        rdfs:label    "geoContains" .

schema:GovernmentBuilding
        rdf:type         rdfs:Class ;
        rdfs:comment     "A government building." ;
        rdfs:label       "GovernmentBuilding" ;
        rdfs:subClassOf  schema:CivicStructure .

schema:FoodService  rdf:type  rdfs:Class ;
        rdfs:comment     "A food service, like breakfast, lunch, or dinner." ;
        rdfs:label       "FoodService" ;
        rdfs:subClassOf  schema:Service .

skos:scopeNote  rdf:type    rdf:Property ;
        rdfs:label          "scope note"@en ;
        rdfs:subPropertyOf  skos:note .

schema:ReserveAction  rdf:type  rdfs:Class ;
        rdfs:comment     "Reserving a concrete object.\\n\\nRelated actions:\\n\\n* [[ScheduleAction]]: Unlike ScheduleAction, ReserveAction reserves concrete objects (e.g. a table, a hotel) towards a time slot / spatial allocation." ;
        rdfs:label       "ReserveAction" ;
        rdfs:subClassOf  schema:PlanAction .

schema:ArtGallery  rdf:type  rdfs:Class ;
        rdfs:comment     "An art gallery." ;
        rdfs:label       "ArtGallery" ;
        rdfs:subClassOf  schema:EntertainmentBusiness .

schema:GeneralContractor
        rdf:type         rdfs:Class ;
        rdfs:comment     "A general contractor." ;
        rdfs:label       "GeneralContractor" ;
        rdfs:subClassOf  schema:HomeAndConstructionBusiness .

schema:termsPerYear  rdf:type  rdf:Property ;
        rdfs:comment  "The number of times terms of study are offered per year. Semesters and quarters are common units for term. For example, if the student can only take 2 semesters for the program in one year, then termsPerYear should be 2." ;
        rdfs:label    "termsPerYear" .

schema:FloorPlan  rdf:type  rdfs:Class ;
        rdfs:comment     "A FloorPlan is an explicit representation of a collection of similar accommodations, allowing the provision of common information (room counts, sizes, layout diagrams) and offers for rental or sale. In typical use, some [[ApartmentComplex]] has an [[accommodationFloorPlan]] which is a [[FloorPlan]].  A FloorPlan is always in the context of a particular place, either a larger [[ApartmentComplex]] or a single [[Apartment]]. The visual/spatial aspects of a floor plan (i.e. room layout, [see wikipedia](https://en.wikipedia.org/wiki/Floor_plan)) can be indicated using [[image]]. " ;
        rdfs:label       "FloorPlan" ;
        rdfs:subClassOf  schema:Intangible .

schema:healthPlanCoinsuranceRate
        rdf:type      rdf:Property ;
        rdfs:comment  "Whether The rate of coinsurance expressed as a number between 0.0 and 1.0." ;
        rdfs:label    "healthPlanCoinsuranceRate" .

schema:applicationSubCategory
        rdf:type      rdf:Property ;
        rdfs:comment  "Subcategory of the application, e.g. 'Arcade Game'." ;
        rdfs:label    "applicationSubCategory" .

schema:leiCode  rdf:type    rdf:Property ;
        rdfs:comment        "An organization identifier that uniquely identifies a legal entity as defined in ISO 17442." ;
        rdfs:label          "leiCode" ;
        rdfs:subPropertyOf  schema:identifier .

schema:cvdNumC19Died  rdf:type  rdf:Property ;
        rdfs:comment  "numc19died - DEATHS: Patients with suspected or confirmed COVID-19 who died in the hospital, ED, or any overflow location." ;
        rdfs:label    "cvdNumC19Died" .

schema:vehicleSpecialUsage
        rdf:type      rdf:Property ;
        rdfs:comment  "Indicates whether the vehicle has been used for special purposes, like commercial rental, driving school, or as a taxi. The legislation in many countries requires this information to be revealed when offering a car for sale." ;
        rdfs:label    "vehicleSpecialUsage" .

schema:functionalClass
        rdf:type      rdf:Property ;
        rdfs:comment  "The degree of mobility the joint allows." ;
        rdfs:label    "functionalClass" .

schema:countriesNotSupported
        rdf:type      rdf:Property ;
        rdfs:comment  "Countries for which the application is not supported. You can also provide the two-letter ISO 3166-1 alpha-2 country code." ;
        rdfs:label    "countriesNotSupported" .

schema:lesserOrEqual  rdf:type  rdf:Property ;
        rdfs:comment  "This ordering relation for qualitative values indicates that the subject is lesser than or equal to the object." ;
        rdfs:label    "lesserOrEqual" .

schema:Drawing  rdf:type  rdfs:Class ;
        rdfs:comment     "A picture or diagram made with a pencil, pen, or crayon rather than paint." ;
        rdfs:label       "Drawing" ;
        rdfs:subClassOf  schema:CreativeWork .

schema:Car  rdf:type     rdfs:Class ;
        rdfs:comment     "A car is a wheeled, self-powered motor vehicle used for transportation." ;
        rdfs:label       "Car" ;
        rdfs:subClassOf  schema:Vehicle .

schema:HealthAspectEnumeration
        rdf:type         rdfs:Class ;
        rdfs:comment     "HealthAspectEnumeration enumerates several aspects of health content online, each of which might be described using [[hasHealthAspect]] and [[HealthTopicContent]]." ;
        rdfs:label       "HealthAspectEnumeration" ;
        rdfs:subClassOf  schema:Enumeration .

schema:accountMinimumInflow
        rdf:type      rdf:Property ;
        rdfs:comment  "A minimum amount that has to be paid in every month." ;
        rdfs:label    "accountMinimumInflow" .

schema:articleBody  rdf:type  rdf:Property ;
        rdfs:comment  "The actual body of the article." ;
        rdfs:label    "articleBody" .

schema:arrivalPlatform
        rdf:type      rdf:Property ;
        rdfs:comment  "The platform where the train arrives." ;
        rdfs:label    "arrivalPlatform" .

schema:broadcastFrequency
        rdf:type      rdf:Property ;
        rdfs:comment  "The frequency used for over-the-air broadcasts. Numeric values or simple ranges e.g. 87-99. In addition a shortcut idiom is supported for frequences of AM and FM radio channels, e.g. \"87 FM\"." ;
        rdfs:label    "broadcastFrequency" .

schema:MortgageLoan  rdf:type  rdfs:Class ;
        rdfs:comment     "A loan in which property or real estate is used as collateral. (A loan securitized against some real estate)." ;
        rdfs:label       "MortgageLoan" ;
        rdfs:subClassOf  schema:LoanOrCredit .

schema:codingSystem  rdf:type  rdf:Property ;
        rdfs:comment  "The coding system, e.g. 'ICD-10'." ;
        rdfs:label    "codingSystem" .

schema:diversityPolicy
        rdf:type      rdf:Property ;
        rdfs:comment  "Statement on diversity policy by an [[Organization]] e.g. a [[NewsMediaOrganization]]. For a [[NewsMediaOrganization]], a statement describing the newsroom’s diversity policy on both staffing and sources, typically providing staffing data." ;
        rdfs:label    "diversityPolicy" .

schema:ShoppingCenter
        rdf:type         rdfs:Class ;
        rdfs:comment     "A shopping center or mall." ;
        rdfs:label       "ShoppingCenter" ;
        rdfs:subClassOf  schema:LocalBusiness .

schema:MonetaryGrant  rdf:type  rdfs:Class ;
        rdfs:comment     "A monetary grant." ;
        rdfs:label       "MonetaryGrant" ;
        rdfs:subClassOf  schema:Grant .

schema:OpeningHoursSpecification
        rdf:type         rdfs:Class ;
        rdfs:comment     "A structured value providing information about the opening hours of a place or a certain service inside a place.\\n\\n\nThe place is __open__ if the [[opens]] property is specified, and __closed__ otherwise.\\n\\nIf the value for the [[closes]] property is less than the value for the [[opens]] property then the hour range is assumed to span over the next day.\n      " ;
        rdfs:label       "OpeningHoursSpecification" ;
        rdfs:subClassOf  schema:StructuredValue .

schema:storageRequirements
        rdf:type      rdf:Property ;
        rdfs:comment  "Storage requirements (free space required)." ;
        rdfs:label    "storageRequirements" .

schema:EUEnergyEfficiencyEnumeration
        rdf:type         rdfs:Class ;
        rdfs:comment     "Enumerates the EU energy efficiency classes A-G as well as A+, A++, and A+++ as defined in EU directive 2017/1369." ;
        rdfs:label       "EUEnergyEfficiencyEnumeration" ;
        rdfs:subClassOf  schema:EnergyEfficiencyEnumeration .

schema:partOfEpisode  rdf:type  rdf:Property ;
        rdfs:comment        "The episode to which this clip belongs." ;
        rdfs:label          "partOfEpisode" ;
        rdfs:subPropertyOf  schema:isPartOf .

schema:PerformanceRole
        rdf:type         rdfs:Class ;
        rdfs:comment     "A PerformanceRole is a Role that some entity places with regard to a theatrical performance, e.g. in a Movie, TVSeries etc." ;
        rdfs:label       "PerformanceRole" ;
        rdfs:subClassOf  schema:Role .

schema:RestrictedDiet
        rdf:type         rdfs:Class ;
        rdfs:comment     "A diet restricted to certain foods or preparations for cultural, religious, health or lifestyle reasons. " ;
        rdfs:label       "RestrictedDiet" ;
        rdfs:subClassOf  schema:Enumeration .

schema:Newspaper  rdf:type  rdfs:Class ;
        rdfs:comment     "A publication containing information about varied topics that are pertinent to general information, a geographic area, or a specific subject matter (i.e. business, culture, education). Often published daily." ;
        rdfs:label       "Newspaper" ;
        rdfs:subClassOf  schema:Periodical .

schema:EducationalOccupationalProgram
        rdf:type         rdfs:Class ;
        rdfs:comment     "A program offered by an institution which determines the learning progress to achieve an outcome, usually a credential like a degree or certificate. This would define a discrete set of opportunities (e.g., job, courses) that together constitute a program with a clear start, end, set of requirements, and transition to a new occupational opportunity (e.g., a job), or sometimes a higher educational opportunity (e.g., an advanced degree)." ;
        rdfs:label       "EducationalOccupationalProgram" ;
        rdfs:subClassOf  schema:Intangible .

schema:cvdNumC19OFMechVentPats
        rdf:type      rdf:Property ;
        rdfs:comment  "numc19ofmechventpats - ED/OVERFLOW and VENTILATED: Patients with suspected or confirmed COVID-19 who are in the ED or any overflow location awaiting an inpatient bed and on a mechanical ventilator." ;
        rdfs:label    "cvdNumC19OFMechVentPats" .

schema:contentLocation
        rdf:type      rdf:Property ;
        rdfs:comment  "The location depicted or described in the content. For example, the location in a photograph or painting." ;
        rdfs:label    "contentLocation" .

schema:longitude  rdf:type  rdf:Property ;
        rdfs:comment  "The longitude of a location. For example ```-122.08585``` ([WGS 84](https://en.wikipedia.org/wiki/World_Geodetic_System))." ;
        rdfs:label    "longitude" .

skos:example  rdf:type      rdf:Property ;
        rdfs:label          "example"@en ;
        rdfs:subPropertyOf  skos:note .

schema:broadcastChannelId
        rdf:type      rdf:Property ;
        rdfs:comment  "The unique address by which the BroadcastService can be identified in a provider lineup. In US, this is typically a number." ;
        rdfs:label    "broadcastChannelId" .

schema:pregnancyWarning
        rdf:type      rdf:Property ;
        rdfs:comment  "Any precaution, guidance, contraindication, etc. related to this drug's use during pregnancy." ;
        rdfs:label    "pregnancyWarning" .

schema:scheduledPaymentDate
        rdf:type      rdf:Property ;
        rdfs:comment  "The date the invoice is scheduled to be paid." ;
        rdfs:label    "scheduledPaymentDate" .

schema:CurrencyConversionService
        rdf:type         rdfs:Class ;
        rdfs:comment     "A service to convert funds from one currency to another currency." ;
        rdfs:label       "CurrencyConversionService" ;
        rdfs:subClassOf  schema:FinancialProduct .

schema:OfferForPurchase
        rdf:type         rdfs:Class ;
        rdfs:comment     "An [[OfferForPurchase]] in Schema.org represents an [[Offer]] to sell something, i.e. an [[Offer]] whose\n  [[businessFunction]] is [sell](http://purl.org/goodrelations/v1#Sell.). See [Good Relations](https://en.wikipedia.org/wiki/GoodRelations) for\n  background on the underlying concepts.\n  " ;
        rdfs:label       "OfferForPurchase" ;
        rdfs:subClassOf  schema:Offer .

schema:identifyingTest
        rdf:type      rdf:Property ;
        rdfs:comment  "A diagnostic test that can identify this sign." ;
        rdfs:label    "identifyingTest" .

schema:BusStation  rdf:type  rdfs:Class ;
        rdfs:comment     "A bus station." ;
        rdfs:label       "BusStation" ;
        rdfs:subClassOf  schema:CivicStructure .

schema:baseSalary  rdf:type  rdf:Property ;
        rdfs:comment  "The base salary of the job or of an employee in an EmployeeRole." ;
        rdfs:label    "baseSalary" .

schema:Corporation  rdf:type  rdfs:Class ;
        rdfs:comment     "Organization: A business corporation." ;
        rdfs:label       "Corporation" ;
        rdfs:subClassOf  schema:Organization .

schema:MerchantReturnPolicy
        rdf:type         rdfs:Class ;
        rdfs:comment     "A MerchantReturnPolicy provides information about product return policies associated with an [[Organization]] or [[Product]]." ;
        rdfs:label       "MerchantReturnPolicy" ;
        rdfs:subClassOf  schema:Intangible .

schema:MedicalTestPanel
        rdf:type         rdfs:Class ;
        rdfs:comment     "Any collection of tests commonly ordered together." ;
        rdfs:label       "MedicalTestPanel" ;
        rdfs:subClassOf  schema:MedicalTest .

schema:priceComponentType
        rdf:type      rdf:Property ;
        rdfs:comment  "Identifies a price component (for example, a line item on an invoice), part of the total price for an offer." ;
        rdfs:label    "priceComponentType" .

schema:PhysicalActivityCategory
        rdf:type         rdfs:Class ;
        rdfs:comment     "Categories of physical activity, organized by physiologic classification." ;
        rdfs:label       "PhysicalActivityCategory" ;
        rdfs:subClassOf  schema:Enumeration .

schema:Recommendation
        rdf:type         rdfs:Class ;
        rdfs:comment     "[[Recommendation]] is a type of [[Review]] that suggests or proposes something as the best option or best course of action. Recommendations may be for products or services, or other concrete things, as in the case of a ranked list or product guide. A [[Guide]] may list multiple recommendations for different categories. For example, in a [[Guide]] about which TVs to buy, the author may have several [[Recommendation]]s." ;
        rdfs:label       "Recommendation" ;
        rdfs:subClassOf  schema:Review .

schema:tickerSymbol  rdf:type  rdf:Property ;
        rdfs:comment  "The exchange traded instrument associated with a Corporation object. The tickerSymbol is expressed as an exchange and an instrument name separated by a space character. For the exchange component of the tickerSymbol attribute, we recommend using the controlled vocabulary of Market Identifier Codes (MIC) specified in ISO15022." ;
        rdfs:label    "tickerSymbol" .

schema:creditedTo  rdf:type  rdf:Property ;
        rdfs:comment  "The group the release is credited to if different than the byArtist. For example, Red and Blue is credited to \"Stefani Germanotta Band\", but by Lady Gaga." ;
        rdfs:label    "creditedTo" .

schema:MedicalDevice  rdf:type  rdfs:Class ;
        rdfs:comment     "Any object used in a medical capacity, such as to diagnose or treat a patient." ;
        rdfs:label       "MedicalDevice" ;
        rdfs:subClassOf  schema:MedicalEntity .

schema:publicTransportClosuresInfo
        rdf:type      rdf:Property ;
        rdfs:comment  "Information about public transport closures." ;
        rdfs:label    "publicTransportClosuresInfo" .

schema:earlyPrepaymentPenalty
        rdf:type      rdf:Property ;
        rdfs:comment  "The amount to be paid as a penalty in the event of early payment of the loan." ;
        rdfs:label    "earlyPrepaymentPenalty" .

schema:Demand  rdf:type  rdfs:Class ;
        rdfs:comment     "A demand entity represents the public, not necessarily binding, not necessarily exclusive, announcement by an organization or person to seek a certain type of goods or services. For describing demand using this type, the very same properties used for Offer apply." ;
        rdfs:label       "Demand" ;
        rdfs:subClassOf  schema:Intangible .

schema:SeekToAction  rdf:type  rdfs:Class ;
        rdfs:comment     "This is the [[Action]] of navigating to a specific [[startOffset]] timestamp within a [[VideoObject]], typically represented with a URL template structure." ;
        rdfs:label       "SeekToAction" ;
        rdfs:subClassOf  schema:Action .

schema:StadiumOrArena
        rdf:type         rdfs:Class ;
        rdfs:comment     "A stadium." ;
        rdfs:label       "StadiumOrArena" ;
        rdfs:subClassOf  schema:SportsActivityLocation , schema:CivicStructure .

schema:isBasedOn  rdf:type  rdf:Property ;
        rdfs:comment  "A resource from which this work is derived or from which it is a modification or adaption." ;
        rdfs:label    "isBasedOn" .

schema:TrackAction  rdf:type  rdfs:Class ;
        rdfs:comment     "An agent tracks an object for updates.\\n\\nRelated actions:\\n\\n* [[FollowAction]]: Unlike FollowAction, TrackAction refers to the interest on the location of innanimates objects.\\n* [[SubscribeAction]]: Unlike SubscribeAction, TrackAction refers to  the interest on the location of innanimate objects." ;
        rdfs:label       "TrackAction" ;
        rdfs:subClassOf  schema:FindAction .

schema:fiberContent  rdf:type  rdf:Property ;
        rdfs:comment  "The number of grams of fiber." ;
        rdfs:label    "fiberContent" .

schema:guidelineDate  rdf:type  rdf:Property ;
        rdfs:comment  "Date on which this guideline's recommendation was made." ;
        rdfs:label    "guidelineDate" .

skos:hasTopConcept  rdf:type  owl:ObjectProperty ;
        rdfs:domain    skos:ConceptScheme ;
        rdfs:label     "has top concept"@en ;
        rdfs:range     skos:Concept ;
        owl:inverseOf  skos:topConceptOf .

schema:LinkRole  rdf:type  rdfs:Class ;
        rdfs:comment     "A Role that represents a Web link e.g. as expressed via the 'url' property. Its linkRelationship property can indicate URL-based and plain textual link types e.g. those in IANA link registry or others such as 'amphtml'. This structure provides a placeholder where details from HTML's link element can be represented outside of HTML, e.g. in JSON-LD feeds." ;
        rdfs:label       "LinkRole" ;
        rdfs:subClassOf  schema:Role .

schema:TVClip  rdf:type  rdfs:Class ;
        rdfs:comment     "A short TV program or a segment/part of a TV program." ;
        rdfs:label       "TVClip" ;
        rdfs:subClassOf  schema:Clip .

schema:ineligibleRegion
        rdf:type      rdf:Property ;
        rdfs:comment  "The ISO 3166-1 (ISO 3166-1 alpha-2) or ISO 3166-2 code, the place, or the GeoShape for the geo-political region(s) for which the offer or delivery charge specification is not valid, e.g. a region where the transaction is not allowed.\\n\\nSee also [[eligibleRegion]].\n      " ;
        rdfs:label    "ineligibleRegion" .

schema:Distillery  rdf:type  rdfs:Class ;
        rdfs:comment     "A distillery." ;
        rdfs:label       "Distillery" ;
        rdfs:subClassOf  schema:FoodEstablishment .

schema:PriceTypeEnumeration
        rdf:type         rdfs:Class ;
        rdfs:comment     "Enumerates different price types, for example list price, invoice price, and sale price." ;
        rdfs:label       "PriceTypeEnumeration" ;
        rdfs:subClassOf  schema:Enumeration .

schema:assesses  rdf:type  rdf:Property ;
        rdfs:comment  "The item being described is intended to assess the competency or learning outcome defined by the referenced term." ;
        rdfs:label    "assesses" .

schema:MedicalContraindication
        rdf:type         rdfs:Class ;
        rdfs:comment     "A condition or factor that serves as a reason to withhold a certain medical therapy. Contraindications can be absolute (there are no reasonable circumstances for undertaking a course of action) or relative (the patient is at higher risk of complications, but that these risks may be outweighed by other considerations or mitigated by other measures)." ;
        rdfs:label       "MedicalContraindication" ;
        rdfs:subClassOf  schema:MedicalEntity .

schema:numberOfEpisodes
        rdf:type      rdf:Property ;
        rdfs:comment  "The number of episodes in this season or series." ;
        rdfs:label    "numberOfEpisodes" .

dcmitype:Image  rdf:type  rdfs:Class .

schema:requirements  rdf:type  rdf:Property ;
        rdfs:comment  "Component dependency requirements for application. This includes runtime environments and shared libraries that are not included in the application distribution package, but required to run the application (Examples: DirectX, Java or .NET runtime)." ;
        rdfs:label    "requirements" .

schema:partOfOrder  rdf:type  rdf:Property ;
        rdfs:comment  "The overall order the items in this delivery were included in." ;
        rdfs:label    "partOfOrder" .

schema:seeks  rdf:type  rdf:Property ;
        rdfs:comment  "A pointer to products or services sought by the organization or person (demand)." ;
        rdfs:label    "seeks" .

schema:RadioSeries  rdf:type  rdfs:Class ;
        rdfs:comment     "CreativeWorkSeries dedicated to radio broadcast and associated online delivery." ;
        rdfs:label       "RadioSeries" ;
        rdfs:subClassOf  schema:CreativeWorkSeries .

schema:geoEquals  rdf:type  rdf:Property ;
        rdfs:comment  "Represents spatial relations in which two geometries (or the places they represent) are topologically equal, as defined in [DE-9IM](https://en.wikipedia.org/wiki/DE-9IM). \"Two geometries are topologically equal if their interiors intersect and no part of the interior or boundary of one geometry intersects the exterior of the other\" (a symmetric relationship)" ;
        rdfs:label    "geoEquals" .

schema:includesObject
        rdf:type      rdf:Property ;
        rdfs:comment  "This links to a node or nodes indicating the exact quantity of the products included in  an [[Offer]] or [[ProductCollection]]." ;
        rdfs:label    "includesObject" .

schema:FinancialProduct
        rdf:type         rdfs:Class ;
        rdfs:comment     "A product provided to consumers and businesses by financial institutions such as banks, insurance companies, brokerage firms, consumer finance companies, and investment companies which comprise the financial services industry." ;
        rdfs:label       "FinancialProduct" ;
        rdfs:subClassOf  schema:Service .

schema:RadioBroadcastService
        rdf:type         rdfs:Class ;
        rdfs:comment     "A delivery service through which radio content is provided via broadcast over the air or online." ;
        rdfs:label       "RadioBroadcastService" ;
        rdfs:subClassOf  schema:BroadcastService .

schema:cvdNumICUBedsOcc
        rdf:type      rdf:Property ;
        rdfs:comment  "numicubedsocc - ICU BED OCCUPANCY: Total number of staffed inpatient ICU beds that are occupied." ;
        rdfs:label    "cvdNumICUBedsOcc" .

schema:relevantSpecialty
        rdf:type      rdf:Property ;
        rdfs:comment  "If applicable, a medical specialty in which this entity is relevant." ;
        rdfs:label    "relevantSpecialty" .

schema:LegalForceStatus
        rdf:type         rdfs:Class ;
        rdfs:comment     "A list of possible statuses for the legal force of a legislation." ;
        rdfs:label       "LegalForceStatus" ;
        rdfs:subClassOf  schema:StatusEnumeration .

schema:AskAction  rdf:type  rdfs:Class ;
        rdfs:comment     "The act of posing a question / favor to someone.\\n\\nRelated actions:\\n\\n* [[ReplyAction]]: Appears generally as a response to AskAction." ;
        rdfs:label       "AskAction" ;
        rdfs:subClassOf  schema:CommunicateAction .

schema:doseValue  rdf:type  rdf:Property ;
        rdfs:comment  "The value of the dose, e.g. 500." ;
        rdfs:label    "doseValue" .

schema:PhysicalTherapy
        rdf:type         rdfs:Class ;
        rdfs:comment     "A process of progressive physical care and rehabilitation aimed at improving a health condition." ;
        rdfs:label       "PhysicalTherapy" ;
        rdfs:subClassOf  schema:MedicalTherapy .

schema:ApartmentComplex
        rdf:type         rdfs:Class ;
        rdfs:comment     "Residence type: Apartment complex." ;
        rdfs:label       "ApartmentComplex" ;
        rdfs:subClassOf  schema:Residence .

schema:possibleComplication
        rdf:type      rdf:Property ;
        rdfs:comment  "A possible unexpected and unfavorable evolution of a medical condition. Complications may include worsening of the signs or symptoms of the disease, extension of the condition to other organ systems, etc." ;
        rdfs:label    "possibleComplication" .

schema:ShareAction  rdf:type  rdfs:Class ;
        rdfs:comment     "The act of distributing content to people for their amusement or edification." ;
        rdfs:label       "ShareAction" ;
        rdfs:subClassOf  schema:CommunicateAction .

schema:gameServer  rdf:type  rdf:Property ;
        rdfs:comment  "The server on which  it is possible to play the game." ;
        rdfs:label    "gameServer" .

schema:cvdNumBedsOcc  rdf:type  rdf:Property ;
        rdfs:comment  "numbedsocc - HOSPITAL INPATIENT BED OCCUPANCY: Total number of staffed inpatient beds that are occupied." ;
        rdfs:label    "cvdNumBedsOcc" .

schema:releaseOf  rdf:type  rdf:Property ;
        rdfs:comment  "The album this is a release of." ;
        rdfs:label    "releaseOf" .

schema:EnergyConsumptionDetails
        rdf:type         rdfs:Class ;
        rdfs:comment     "EnergyConsumptionDetails represents information related to the energy efficiency of a product that consumes energy. The information that can be provided is based on international regulations such as for example [EU directive 2017/1369](https://eur-lex.europa.eu/eli/reg/2017/1369/oj) for energy labeling and the [Energy labeling rule](https://www.ftc.gov/enforcement/rules/rulemaking-regulatory-reform-proceedings/energy-water-use-labeling-consumer) under the Energy Policy and Conservation Act (EPCA) in the US." ;
        rdfs:label       "EnergyConsumptionDetails" ;
        rdfs:subClassOf  schema:Intangible .

schema:expectedPrognosis
        rdf:type      rdf:Property ;
        rdfs:comment  "The likely outcome in either the short term or long term of the medical condition." ;
        rdfs:label    "expectedPrognosis" .

schema:Table  rdf:type   rdfs:Class ;
        rdfs:comment     "A table on a Web page." ;
        rdfs:label       "Table" ;
        rdfs:subClassOf  schema:WebPageElement .

schema:Order  rdf:type   rdfs:Class ;
        rdfs:comment     "An order is a confirmation of a transaction (a receipt), which can contain multiple line items, each represented by an Offer that has been accepted by the customer." ;
        rdfs:label       "Order" ;
        rdfs:subClassOf  schema:Intangible .

schema:accessibilityControl
        rdf:type      rdf:Property ;
        rdfs:comment  "Identifies input methods that are sufficient to fully control the described resource ([WebSchemas wiki lists possible values](http://www.w3.org/wiki/WebSchemas/Accessibility))." ;
        rdfs:label    "accessibilityControl" .

schema:rsvpResponse  rdf:type  rdf:Property ;
        rdfs:comment  "The response (yes, no, maybe) to the RSVP." ;
        rdfs:label    "rsvpResponse" .

schema:scheduledTime  rdf:type  rdf:Property ;
        rdfs:comment  "The time the object is scheduled to." ;
        rdfs:label    "scheduledTime" .

schema:error  rdf:type  rdf:Property ;
        rdfs:comment  "For failed actions, more information on the cause of the failure." ;
        rdfs:label    "error" .

schema:eligibleCustomerType
        rdf:type      rdf:Property ;
        rdfs:comment  "The type(s) of customers for which the given offer is valid." ;
        rdfs:label    "eligibleCustomerType" .

schema:ReservationStatusType
        rdf:type         rdfs:Class ;
        rdfs:comment     "Enumerated status values for Reservation." ;
        rdfs:label       "ReservationStatusType" ;
        rdfs:subClassOf  schema:StatusEnumeration .

schema:measuredValue  rdf:type  rdf:Property ;
        rdfs:comment  "The measuredValue of an [[Observation]]." ;
        rdfs:label    "measuredValue" .

schema:totalPrice  rdf:type  rdf:Property ;
        rdfs:comment  "The total price for the reservation or ticket, including applicable taxes, shipping, etc.\\n\\nUsage guidelines:\\n\\n* Use values from 0123456789 (Unicode 'DIGIT ZERO' (U+0030) to 'DIGIT NINE' (U+0039)) rather than superficially similiar Unicode symbols.\\n* Use '.' (Unicode 'FULL STOP' (U+002E)) rather than ',' to indicate a decimal point. Avoid using these symbols as a readability separator." ;
        rdfs:label    "totalPrice" .

schema:GovernmentOrganization
        rdf:type         rdfs:Class ;
        rdfs:comment     "A governmental organization or agency." ;
        rdfs:label       "GovernmentOrganization" ;
        rdfs:subClassOf  schema:Organization .

schema:RecyclingCenter
        rdf:type         rdfs:Class ;
        rdfs:comment     "A recycling center." ;
        rdfs:label       "RecyclingCenter" ;
        rdfs:subClassOf  schema:LocalBusiness .

schema:isResizable  rdf:type  rdf:Property ;
        rdfs:comment  "Whether the 3DModel allows resizing. For example, room layout applications often do not allow 3DModel elements to be resized to reflect reality." ;
        rdfs:label    "isResizable" .

schema:tributary  rdf:type  rdf:Property ;
        rdfs:comment  "The anatomical or organ system that the vein flows into; a larger structure that the vein connects to." ;
        rdfs:label    "tributary" .

schema:deathDate  rdf:type  rdf:Property ;
        rdfs:comment  "Date of death." ;
        rdfs:label    "deathDate" .

schema:jobLocation  rdf:type  rdf:Property ;
        rdfs:comment  "A (typically single) geographic location associated with the job position." ;
        rdfs:label    "jobLocation" .

schema:PetStore  rdf:type  rdfs:Class ;
        rdfs:comment     "A pet store." ;
        rdfs:label       "PetStore" ;
        rdfs:subClassOf  schema:Store .

schema:BoardingPolicyType
        rdf:type         rdfs:Class ;
        rdfs:comment     "A type of boarding policy used by an airline." ;
        rdfs:label       "BoardingPolicyType" ;
        rdfs:subClassOf  schema:Enumeration .

schema:eligibleQuantity
        rdf:type      rdf:Property ;
        rdfs:comment  "The interval and unit of measurement of ordering quantities for which the offer or price specification is valid. This allows e.g. specifying that a certain freight charge is valid only for a certain quantity." ;
        rdfs:label    "eligibleQuantity" .

schema:DDxElement  rdf:type  rdfs:Class ;
        rdfs:comment     "An alternative, closely-related condition typically considered later in the differential diagnosis process along with the signs that are used to distinguish it." ;
        rdfs:label       "DDxElement" ;
        rdfs:subClassOf  schema:MedicalIntangible .

schema:MedicalProcedure
        rdf:type         rdfs:Class ;
        rdfs:comment     "A process of care used in either a diagnostic, therapeutic, preventive or palliative capacity that relies on invasive (surgical), non-invasive, or other techniques." ;
        rdfs:label       "MedicalProcedure" ;
        rdfs:subClassOf  schema:MedicalEntity .

schema:healthPlanCoinsuranceOption
        rdf:type      rdf:Property ;
        rdfs:comment  "Whether the coinsurance applies before or after deductible, etc. TODO: Is this a closed set?" ;
        rdfs:label    "healthPlanCoinsuranceOption" .

schema:nationality  rdf:type  rdf:Property ;
        rdfs:comment  "Nationality of the person." ;
        rdfs:label    "nationality" .

schema:printEdition  rdf:type  rdf:Property ;
        rdfs:comment  "The edition of the print product in which the NewsArticle appears." ;
        rdfs:label    "printEdition" .

schema:SheetMusic  rdf:type  rdfs:Class ;
        rdfs:comment     "Printed music, as opposed to performed or recorded music." ;
        rdfs:label       "SheetMusic" ;
        rdfs:subClassOf  schema:CreativeWork .

schema:alignmentType  rdf:type  rdf:Property ;
        rdfs:comment  "A category of alignment between the learning resource and the framework node. Recommended values include: 'requires', 'textComplexity', 'readingLevel', and 'educationalSubject'." ;
        rdfs:label    "alignmentType" .

schema:relevantOccupation
        rdf:type      rdf:Property ;
        rdfs:comment  "The Occupation for the JobPosting." ;
        rdfs:label    "relevantOccupation" .

schema:associatedPathophysiology
        rdf:type      rdf:Property ;
        rdfs:comment  "If applicable, a description of the pathophysiology associated with the anatomical system, including potential abnormal changes in the mechanical, physical, and biochemical functions of the system." ;
        rdfs:label    "associatedPathophysiology" .

schema:disambiguatingDescription
        rdf:type            rdf:Property ;
        rdfs:comment        "A sub property of description. A short description of the item used to disambiguate from other, similar items. Information from other properties (in particular, name) may be necessary for the description to be useful for disambiguation." ;
        rdfs:label          "disambiguatingDescription" ;
        rdfs:subPropertyOf  schema:description .

schema:floorLevel  rdf:type  rdf:Property ;
        rdfs:comment  "The floor level for an [[Accommodation]] in a multi-storey building. Since counting\n  systems [vary internationally](https://en.wikipedia.org/wiki/Storey#Consecutive_number_floor_designations), the local system should be used where possible." ;
        rdfs:label    "floorLevel" .

schema:HomeGoodsStore
        rdf:type         rdfs:Class ;
        rdfs:comment     "A home goods store." ;
        rdfs:label       "HomeGoodsStore" ;
        rdfs:subClassOf  schema:Store .

schema:drugClass  rdf:type  rdf:Property ;
        rdfs:comment  "The class of drug this belongs to (e.g., statins)." ;
        rdfs:label    "drugClass" .

schema:Ticket  rdf:type  rdfs:Class ;
        rdfs:comment     "Used to describe a ticket to an event, a flight, a bus ride, etc." ;
        rdfs:label       "Ticket" ;
        rdfs:subClassOf  schema:Intangible .

schema:Code  rdf:type    rdfs:Class ;
        rdfs:comment     "Computer programming source code. Example: Full (compile ready) solutions, code snippet samples, scripts, templates." ;
        rdfs:label       "Code" ;
        rdfs:subClassOf  schema:CreativeWork .

schema:significance  rdf:type  rdf:Property ;
        rdfs:comment  "The significance associated with the superficial anatomy; as an example, how characteristics of the superficial anatomy can suggest underlying medical conditions or courses of treatment." ;
        rdfs:label    "significance" .

schema:ChildCare  rdf:type  rdfs:Class ;
        rdfs:comment     "A Childcare center." ;
        rdfs:label       "ChildCare" ;
        rdfs:subClassOf  schema:LocalBusiness .

schema:MediaObject  rdf:type  rdfs:Class ;
        rdfs:comment     "A media object, such as an image, video, or audio object embedded in a web page or a downloadable dataset i.e. DataDownload. Note that a creative work may have many media objects associated with it on the same web page. For example, a page about a single song (MusicRecording) may have a music video (VideoObject), and a high and low bandwidth audio stream (2 AudioObject's)." ;
        rdfs:label       "MediaObject" ;
        rdfs:subClassOf  schema:CreativeWork .

schema:FurnitureStore
        rdf:type         rdfs:Class ;
        rdfs:comment     "A furniture store." ;
        rdfs:label       "FurnitureStore" ;
        rdfs:subClassOf  schema:Store .

schema:doorTime  rdf:type  rdf:Property ;
        rdfs:comment  "The time admission will commence." ;
        rdfs:label    "doorTime" .

schema:scheduleTimezone
        rdf:type      rdf:Property ;
        rdfs:comment  "Indicates the timezone for which the time(s) indicated in the [[Schedule]] are given. The value provided should be among those listed in the IANA Time Zone Database." ;
        rdfs:label    "scheduleTimezone" .

schema:WPSideBar  rdf:type  rdfs:Class ;
        rdfs:comment     "A sidebar section of the page." ;
        rdfs:label       "WPSideBar" ;
        rdfs:subClassOf  schema:WebPageElement .

schema:MovingCompany  rdf:type  rdfs:Class ;
        rdfs:comment     "A moving company." ;
        rdfs:label       "MovingCompany" ;
        rdfs:subClassOf  schema:HomeAndConstructionBusiness .

schema:menu  rdf:type  rdf:Property ;
        rdfs:comment  "Either the actual menu as a structured representation, as text, or a URL of the menu." ;
        rdfs:label    "menu" .

schema:Enumeration  rdf:type  rdfs:Class ;
        rdfs:comment     "Lists or enumerations—for example, a list of cuisines or music genres, etc." ;
        rdfs:label       "Enumeration" ;
        rdfs:subClassOf  schema:Intangible .

schema:artist  rdf:type  rdf:Property ;
        rdfs:comment  "The primary artist for a work\n    \tin a medium other than pencils or digital line art--for example, if the\n    \tprimary artwork is done in watercolors or digital paints." ;
        rdfs:label    "artist" .

schema:EducationalAudience
        rdf:type         rdfs:Class ;
        rdfs:comment     "An EducationalAudience." ;
        rdfs:label       "EducationalAudience" ;
        rdfs:subClassOf  schema:Audience .

schema:ConfirmAction  rdf:type  rdfs:Class ;
        rdfs:comment     "The act of notifying someone that a future event/action is going to happen as expected.\\n\\nRelated actions:\\n\\n* [[CancelAction]]: The antonym of ConfirmAction." ;
        rdfs:label       "ConfirmAction" ;
        rdfs:subClassOf  schema:InformAction .

schema:variantCover  rdf:type  rdf:Property ;
        rdfs:comment  "A description of the variant cover\n    \tfor the issue, if the issue is a variant printing. For example, \"Bryan Hitch\n    \tVariant Cover\" or \"2nd Printing Variant\"." ;
        rdfs:label    "variantCover" .

schema:contraindication
        rdf:type      rdf:Property ;
        rdfs:comment  "A contraindication for this therapy." ;
        rdfs:label    "contraindication" .

schema:PropertyValue  rdf:type  rdfs:Class ;
        rdfs:comment     "A property-value pair, e.g. representing a feature of a product or place. Use the 'name' property for the name of the property. If there is an additional human-readable version of the value, put that into the 'description' property.\\n\\n Always use specific schema.org properties when a) they exist and b) you can populate them. Using PropertyValue as a substitute will typically not trigger the same effect as using the original, specific property.\n    " ;
        rdfs:label       "PropertyValue" ;
        rdfs:subClassOf  schema:StructuredValue .

schema:isRelatedTo  rdf:type  rdf:Property ;
        rdfs:comment  "A pointer to another, somehow related product (or multiple products)." ;
        rdfs:label    "isRelatedTo" .

schema:OrganizeAction
        rdf:type         rdfs:Class ;
        rdfs:comment     "The act of manipulating/administering/supervising/controlling one or more objects." ;
        rdfs:label       "OrganizeAction" ;
        rdfs:subClassOf  schema:Action .

schema:carrierRequirements
        rdf:type      rdf:Property ;
        rdfs:comment  "Specifies specific carrier(s) requirements for the application (e.g. an application may only work on a specific carrier network)." ;
        rdfs:label    "carrierRequirements" .

schema:aircraft  rdf:type  rdf:Property ;
        rdfs:comment  "The kind of aircraft (e.g., \"Boeing 747\")." ;
        rdfs:label    "aircraft" .

schema:BackgroundNewsArticle
        rdf:type         rdfs:Class ;
        rdfs:comment     "A [[NewsArticle]] providing historical context, definition and detail on a specific topic (aka \"explainer\" or \"backgrounder\"). For example, an in-depth article or frequently-asked-questions ([FAQ](https://en.wikipedia.org/wiki/FAQ)) document on topics such as Climate Change or the European Union. Other kinds of background material from a non-news setting are often described using [[Book]] or [[Article]], in particular [[ScholarlyArticle]]. See also [[NewsArticle]] for related vocabulary from a learning/education perspective." ;
        rdfs:label       "BackgroundNewsArticle" ;
        rdfs:subClassOf  schema:NewsArticle .

schema:domainIncludes
        rdf:type      rdf:Property ;
        rdfs:comment  "Relates a property to a class that is (one of) the type(s) the property is expected to be used on." ;
        rdfs:label    "domainIncludes" .

schema:ScholarlyArticle
        rdf:type         rdfs:Class ;
        rdfs:comment     "A scholarly article." ;
        rdfs:label       "ScholarlyArticle" ;
        rdfs:subClassOf  schema:Article .

schema:BankOrCreditUnion
        rdf:type         rdfs:Class ;
        rdfs:comment     "Bank or credit union." ;
        rdfs:label       "BankOrCreditUnion" ;
        rdfs:subClassOf  schema:FinancialService .

schema:MedicalSign  rdf:type  rdfs:Class ;
        rdfs:comment     "Any physical manifestation of a person's medical condition discoverable by objective diagnostic tests or physical examination." ;
        rdfs:label       "MedicalSign" ;
        rdfs:subClassOf  schema:MedicalSignOrSymptom .

schema:orderNumber  rdf:type  rdf:Property ;
        rdfs:comment        "The identifier of the transaction." ;
        rdfs:label          "orderNumber" ;
        rdfs:subPropertyOf  schema:identifier .

schema:screenshot  rdf:type  rdf:Property ;
        rdfs:comment  "A link to a screenshot image of the app." ;
        rdfs:label    "screenshot" .

schema:TVEpisode  rdf:type  rdfs:Class ;
        rdfs:comment     "A TV episode which can be part of a series or season." ;
        rdfs:label       "TVEpisode" ;
        rdfs:subClassOf  schema:Episode .

schema:EducationEvent
        rdf:type         rdfs:Class ;
        rdfs:comment     "Event type: Education event." ;
        rdfs:label       "EducationEvent" ;
        rdfs:subClassOf  schema:Event .

schema:refundType  rdf:type  rdf:Property ;
        rdfs:comment  "A refundType, from an enumerated list." ;
        rdfs:label    "refundType" .

schema:keywords  rdf:type  rdf:Property ;
        rdfs:comment  "Keywords or tags used to describe this content. Multiple entries in a keywords list are typically delimited by commas." ;
        rdfs:label    "keywords" .

schema:GeoCoordinates
        rdf:type         rdfs:Class ;
        rdfs:comment     "The geographic coordinates of a place or event." ;
        rdfs:label       "GeoCoordinates" ;
        rdfs:subClassOf  schema:StructuredValue .

schema:seasonNumber  rdf:type  rdf:Property ;
        rdfs:comment        "Position of the season within an ordered group of seasons." ;
        rdfs:label          "seasonNumber" ;
        rdfs:subPropertyOf  schema:position .

schema:accelerationTime
        rdf:type      rdf:Property ;
        rdfs:comment  "The time needed to accelerate the vehicle from a given start velocity to a given target velocity.\\n\\nTypical unit code(s): SEC for seconds\\n\\n* Note: There are unfortunately no standard unit codes for seconds/0..100 km/h or seconds/0..60 mph. Simply use \"SEC\" for seconds and indicate the velocities in the [[name]] of the [[QuantitativeValue]], or use [[valueReference]] with a [[QuantitativeValue]] of 0..60 mph or 0..100 km/h to specify the reference speeds." ;
        rdfs:label    "accelerationTime" .

schema:Quotation  rdf:type  rdfs:Class ;
        rdfs:comment     "A quotation. Often but not necessarily from some written work, attributable to a real world author and - if associated with a fictional character - to any fictional Person. Use [[isBasedOn]] to link to source/origin. The [[recordedIn]] property can be used to reference a Quotation from an [[Event]]." ;
        rdfs:label       "Quotation" ;
        rdfs:subClassOf  schema:CreativeWork .

schema:vehicleInteriorColor
        rdf:type      rdf:Property ;
        rdfs:comment  "The color or color combination of the interior of the vehicle." ;
        rdfs:label    "vehicleInteriorColor" .

schema:dependencies  rdf:type  rdf:Property ;
        rdfs:comment  "Prerequisites needed to fulfill steps in article." ;
        rdfs:label    "dependencies" .

schema:learningResourceType
        rdf:type      rdf:Property ;
        rdfs:comment  "The predominant type or kind characterizing the learning resource. For example, 'presentation', 'handout'." ;
        rdfs:label    "learningResourceType" .

schema:DayOfWeek  rdf:type  rdfs:Class ;
        rdfs:comment     "The day of the week, e.g. used to specify to which day the opening hours of an OpeningHoursSpecification refer.\n\nOriginally, URLs from [GoodRelations](http://purl.org/goodrelations/v1) were used (for [[Monday]], [[Tuesday]], [[Wednesday]], [[Thursday]], [[Friday]], [[Saturday]], [[Sunday]] plus a special entry for [[PublicHolidays]]); these have now been integrated directly into schema.org.\n      " ;
        rdfs:label       "DayOfWeek" ;
        rdfs:subClassOf  schema:Enumeration .

schema:accessCode  rdf:type  rdf:Property ;
        rdfs:comment  "Password, PIN, or access code needed for delivery (e.g. from a locker)." ;
        rdfs:label    "accessCode" .

schema:jobImmediateStart
        rdf:type      rdf:Property ;
        rdfs:comment  "An indicator as to whether a position is available for an immediate start." ;
        rdfs:label    "jobImmediateStart" .

schema:gtin14  rdf:type     rdf:Property ;
        rdfs:comment        "The GTIN-14 code of the product, or the product to which the offer refers. See [GS1 GTIN Summary](http://www.gs1.org/barcodes/technical/idkeys/gtin) for more details." ;
        rdfs:label          "gtin14" ;
        rdfs:subPropertyOf  schema:identifier , schema:gtin .

schema:medicalAudience
        rdf:type      rdf:Property ;
        rdfs:comment  "Medical audience for page." ;
        rdfs:label    "medicalAudience" .

schema:ActivateAction
        rdf:type         rdfs:Class ;
        rdfs:comment     "The act of starting or activating a device or application (e.g. starting a timer or turning on a flashlight)." ;
        rdfs:label       "ActivateAction" ;
        rdfs:subClassOf  schema:ControlAction .

schema:applicationStartDate
        rdf:type      rdf:Property ;
        rdfs:comment  "The date at which the program begins collecting applications for the next enrollment cycle." ;
        rdfs:label    "applicationStartDate" .

schema:Quantity  rdf:type  rdfs:Class ;
        rdfs:comment     "Quantities such as distance, time, mass, weight, etc. Particular instances of say Mass are entities like '3 Kg' or '4 milligrams'." ;
        rdfs:label       "Quantity" ;
        rdfs:subClassOf  schema:Intangible .

schema:appliesToPaymentMethod
        rdf:type      rdf:Property ;
        rdfs:comment  "The payment method(s) to which the payment charge specification applies." ;
        rdfs:label    "appliesToPaymentMethod" .

schema:workExample  rdf:type  rdf:Property ;
        rdfs:comment  "Example/instance/realization/derivation of the concept of this creative work. eg. The paperback edition, first edition, or eBook." ;
        rdfs:label    "workExample" .

schema:Poster  rdf:type  rdfs:Class ;
        rdfs:comment     "A large, usually printed placard, bill, or announcement, often illustrated, that is posted to advertise or publicize something." ;
        rdfs:label       "Poster" ;
        rdfs:subClassOf  schema:CreativeWork .

schema:loser  rdf:type      rdf:Property ;
        rdfs:comment        "A sub property of participant. The loser of the action." ;
        rdfs:label          "loser" ;
        rdfs:subPropertyOf  schema:participant .

schema:dissolutionDate
        rdf:type      rdf:Property ;
        rdfs:comment  "The date that this organization was dissolved." ;
        rdfs:label    "dissolutionDate" .

schema:performTime  rdf:type  rdf:Property ;
        rdfs:comment  "The length of time it takes to perform instructions or a direction (not including time to prepare the supplies), in [ISO 8601 duration format](http://en.wikipedia.org/wiki/ISO_8601)." ;
        rdfs:label    "performTime" .

schema:Optician  rdf:type  rdfs:Class ;
        rdfs:comment     "A store that sells reading glasses and similar devices for improving vision." ;
        rdfs:label       "Optician" ;
        rdfs:subClassOf  schema:MedicalBusiness .

schema:NutritionInformation
        rdf:type         rdfs:Class ;
        rdfs:comment     "Nutritional information about the recipe." ;
        rdfs:label       "NutritionInformation" ;
        rdfs:subClassOf  schema:StructuredValue .

schema:exifData  rdf:type  rdf:Property ;
        rdfs:comment  "exif data for this object." ;
        rdfs:label    "exifData" .

schema:DownloadAction
        rdf:type         rdfs:Class ;
        rdfs:comment     "The act of downloading an object." ;
        rdfs:label       "DownloadAction" ;
        rdfs:subClassOf  schema:TransferAction .

schema:hasCredential  rdf:type  rdf:Property ;
        rdfs:comment  "A credential awarded to the Person or Organization." ;
        rdfs:label    "hasCredential" .

schema:warranty  rdf:type  rdf:Property ;
        rdfs:comment  "The warranty promise(s) included in the offer." ;
        rdfs:label    "warranty" .

schema:vehicleIdentificationNumber
        rdf:type            rdf:Property ;
        rdfs:comment        "The Vehicle Identification Number (VIN) is a unique serial number used by the automotive industry to identify individual motor vehicles." ;
        rdfs:label          "vehicleIdentificationNumber" ;
        rdfs:subPropertyOf  schema:serialNumber .

schema:Store  rdf:type   rdfs:Class ;
        rdfs:comment     "A retail good store." ;
        rdfs:label       "Store" ;
        rdfs:subClassOf  schema:LocalBusiness .

schema:industry  rdf:type  rdf:Property ;
        rdfs:comment  "The industry associated with the job position." ;
        rdfs:label    "industry" .

schema:OrderItem  rdf:type  rdfs:Class ;
        rdfs:comment     "An order item is a line of an order. It includes the quantity and shipping details of a bought offer." ;
        rdfs:label       "OrderItem" ;
        rdfs:subClassOf  schema:Intangible .

schema:eligibleDuration
        rdf:type      rdf:Property ;
        rdfs:comment  "The duration for which the given offer is valid." ;
        rdfs:label    "eligibleDuration" .

schema:MotorcycleRepair
        rdf:type         rdfs:Class ;
        rdfs:comment     "A motorcycle repair shop." ;
        rdfs:label       "MotorcycleRepair" ;
        rdfs:subClassOf  schema:AutomotiveBusiness .

schema:Playground  rdf:type  rdfs:Class ;
        rdfs:comment     "A playground." ;
        rdfs:label       "Playground" ;
        rdfs:subClassOf  schema:CivicStructure .

schema:LandmarksOrHistoricalBuildings
        rdf:type         rdfs:Class ;
        rdfs:comment     "An historical landmark or building." ;
        rdfs:label       "LandmarksOrHistoricalBuildings" ;
        rdfs:subClassOf  schema:Place .

schema:SpeakableSpecification
        rdf:type         rdfs:Class ;
        rdfs:comment     "A SpeakableSpecification indicates (typically via [[xpath]] or [[cssSelector]]) sections of a document that are highlighted as particularly [[speakable]]. Instances of this type are expected to be used primarily as values of the [[speakable]] property." ;
        rdfs:label       "SpeakableSpecification" ;
        rdfs:subClassOf  schema:Intangible .

schema:availableTest  rdf:type  rdf:Property ;
        rdfs:comment  "A diagnostic test or procedure offered by this lab." ;
        rdfs:label    "availableTest" .

schema:Mass  rdf:type    rdfs:Class ;
        rdfs:comment     "Properties that take Mass as values are of the form '&lt;Number&gt; &lt;Mass unit of measure&gt;'. E.g., '7 kg'." ;
        rdfs:label       "Mass" ;
        rdfs:subClassOf  schema:Quantity .

schema:Physician  rdf:type  rdfs:Class ;
        rdfs:comment     "A doctor's office." ;
        rdfs:label       "Physician" ;
        rdfs:subClassOf  schema:MedicalBusiness , schema:MedicalOrganization .

schema:maxValue  rdf:type  rdf:Property ;
        rdfs:comment  "The upper value of some characteristic or property." ;
        rdfs:label    "maxValue" .

schema:muscleAction  rdf:type  rdf:Property ;
        rdfs:comment  "The movement the muscle generates." ;
        rdfs:label    "muscleAction" .

schema:seasons  rdf:type  rdf:Property ;
        rdfs:comment  "A season in a media series." ;
        rdfs:label    "seasons" .

schema:alcoholWarning
        rdf:type      rdf:Property ;
        rdfs:comment  "Any precaution, guidance, contraindication, etc. related to consumption of alcohol while taking this drug." ;
        rdfs:label    "alcoholWarning" .

schema:incentiveCompensation
        rdf:type      rdf:Property ;
        rdfs:comment  "Description of bonus and commission compensation aspects of the job." ;
        rdfs:label    "incentiveCompensation" .

schema:MedicalGuidelineRecommendation
        rdf:type         rdfs:Class ;
        rdfs:comment     "A guideline recommendation that is regarded as efficacious and where quality of the data supporting the recommendation is sound." ;
        rdfs:label       "MedicalGuidelineRecommendation" ;
        rdfs:subClassOf  schema:MedicalGuideline .

schema:musicalKey  rdf:type  rdf:Property ;
        rdfs:comment  "The key, mode, or scale this composition uses." ;
        rdfs:label    "musicalKey" .

schema:naturalProgression
        rdf:type      rdf:Property ;
        rdfs:comment  "The expected progression of the condition if it is not treated and allowed to progress naturally." ;
        rdfs:label    "naturalProgression" .

schema:Hostel  rdf:type  rdfs:Class ;
        rdfs:comment     "A hostel - cheap accommodation, often in shared dormitories.\n<br /><br />\nSee also the <a href=\"/docs/hotels.html\">dedicated document on the use of schema.org for marking up hotels and other forms of accommodations</a>.\n" ;
        rdfs:label       "Hostel" ;
        rdfs:subClassOf  schema:LodgingBusiness .

schema:countryOfOrigin
        rdf:type      rdf:Property ;
        rdfs:comment  "The country of the principal offices of the production company or individual responsible for the movie or program." ;
        rdfs:label    "countryOfOrigin" .

schema:AddAction  rdf:type  rdfs:Class ;
        rdfs:comment     "The act of editing by adding an object to a collection." ;
        rdfs:label       "AddAction" ;
        rdfs:subClassOf  schema:UpdateAction .

skos:prefLabel  rdf:type    rdf:Property ;
        rdfs:comment        "skos:prefLabel, skos:altLabel and skos:hiddenLabel are pairwise\n      disjoint properties."@en , "The range of skos:prefLabel is the class of RDF plain literals."@en , "A resource has no more than one value of skos:prefLabel per language tag, and no more than one value of skos:prefLabel without language tag."@en ;
        rdfs:label          "preferred label"@en ;
        rdfs:subPropertyOf  rdfs:label .

schema:Message  rdf:type  rdfs:Class ;
        rdfs:comment     "A single message from a sender to one or more organizations or people." ;
        rdfs:label       "Message" ;
        rdfs:subClassOf  schema:CreativeWork .

schema:numberOfCredits
        rdf:type      rdf:Property ;
        rdfs:comment  "The number of credits or units awarded by a Course or required to complete an EducationalOccupationalProgram." ;
        rdfs:label    "numberOfCredits" .

schema:trailerWeight  rdf:type  rdf:Property ;
        rdfs:comment  "The permitted weight of a trailer attached to the vehicle.\\n\\nTypical unit code(s): KGM for kilogram, LBR for pound\\n* Note 1: You can indicate additional information in the [[name]] of the [[QuantitativeValue]] node.\\n* Note 2: You may also link to a [[QualitativeValue]] node that provides additional information using [[valueReference]].\\n* Note 3: Note that you can use [[minValue]] and [[maxValue]] to indicate ranges." ;
        rdfs:label    "trailerWeight" .

schema:correction  rdf:type  rdf:Property ;
        rdfs:comment  "Indicates a correction to a [[CreativeWork]], either via a [[CorrectionComment]], textually or in another document." ;
        rdfs:label    "correction" .

schema:RsvpResponseType
        rdf:type         rdfs:Class ;
        rdfs:comment     "RsvpResponseType is an enumeration type whose instances represent responding to an RSVP request." ;
        rdfs:label       "RsvpResponseType" ;
        rdfs:subClassOf  schema:Enumeration .

schema:DefinedTermSet
        rdf:type         rdfs:Class ;
        rdfs:comment     "A set of defined terms for example a set of categories or a classification scheme, a glossary, dictionary or enumeration." ;
        rdfs:label       "DefinedTermSet" ;
        rdfs:subClassOf  schema:CreativeWork .

schema:DefenceEstablishment
        rdf:type         rdfs:Class ;
        rdfs:comment     "A defence establishment, such as an army or navy base." ;
        rdfs:label       "DefenceEstablishment" ;
        rdfs:subClassOf  schema:GovernmentBuilding .

schema:schemaVersion  rdf:type  rdf:Property ;
        rdfs:comment  "Indicates (by URL or string) a particular version of a schema used in some CreativeWork. This property was created primarily to\n    indicate the use of a specific schema.org release, e.g. ```10.0``` as a simple string, or more explicitly via URL, ```http://schema.org/docs/releases.html#v10.0```. There may be situations in which other schemas might usefully be referenced this way, e.g. ```http://dublincore.org/specifications/dublin-core/dces/1999-07-02/``` but this has not been carefully explored in the community." ;
        rdfs:label    "schemaVersion" .

schema:surface  rdf:type    rdf:Property ;
        rdfs:comment        "A material used as a surface in some artwork, e.g. Canvas, Paper, Wood, Board, etc." ;
        rdfs:label          "surface" ;
        rdfs:subPropertyOf  schema:material .

schema:advanceBookingRequirement
        rdf:type      rdf:Property ;
        rdfs:comment  "The amount of time that is required between accepting the offer and the actual usage of the resource or service." ;
        rdfs:label    "advanceBookingRequirement" .

schema:hasBroadcastChannel
        rdf:type      rdf:Property ;
        rdfs:comment  "A broadcast channel of a broadcast service." ;
        rdfs:label    "hasBroadcastChannel" .

schema:includesHealthPlanNetwork
        rdf:type      rdf:Property ;
        rdfs:comment  "Networks covered by this plan." ;
        rdfs:label    "includesHealthPlanNetwork" .

schema:ItemListOrderType
        rdf:type         rdfs:Class ;
        rdfs:comment     "Enumerated for values for itemListOrder for indicating how an ordered ItemList is organized." ;
        rdfs:label       "ItemListOrderType" ;
        rdfs:subClassOf  schema:Enumeration .

schema:billingDuration
        rdf:type      rdf:Property ;
        rdfs:comment  "Specifies for how long this price (or price component) will be billed. Can be used, for example, to model the contractual duration of a subscription or payment plan. Type can be either a Duration or a Number (in which case the unit of measurement, for example month, is specified by the unitCode property)." ;
        rdfs:label    "billingDuration" .

schema:relatedLink  rdf:type  rdf:Property ;
        rdfs:comment  "A link related to this web page, for example to other related web pages." ;
        rdfs:label    "relatedLink" .

schema:discount  rdf:type  rdf:Property ;
        rdfs:comment  "Any discount applied (to an Order)." ;
        rdfs:label    "discount" .

schema:serviceLocation
        rdf:type      rdf:Property ;
        rdfs:comment  "The location (e.g. civic structure, local business, etc.) where a person can go to access the service." ;
        rdfs:label    "serviceLocation" .

schema:isAvailableGenerically
        rdf:type      rdf:Property ;
        rdfs:comment  "True if the drug is available in a generic form (regardless of name)." ;
        rdfs:label    "isAvailableGenerically" .

schema:employmentUnit
        rdf:type      rdf:Property ;
        rdfs:comment  "Indicates the department, unit and/or facility where the employee reports and/or in which the job is to be performed." ;
        rdfs:label    "employmentUnit" .

schema:applicableLocation
        rdf:type      rdf:Property ;
        rdfs:comment  "The location in which the status applies." ;
        rdfs:label    "applicableLocation" .

schema:Person  rdf:type  rdfs:Class ;
        rdfs:comment     "A person (alive, dead, undead, or fictional)." ;
        rdfs:label       "Person" ;
        rdfs:subClassOf  schema:Thing .

schema:TVSeason  rdf:type  rdfs:Class ;
        rdfs:comment     "Season dedicated to TV broadcast and associated online delivery." ;
        rdfs:label       "TVSeason" ;
        rdfs:subClassOf  schema:CreativeWorkSeason , schema:CreativeWork .

schema:PronounceableText
        rdf:type         rdfs:Class ;
        rdfs:comment     "Data type: PronounceableText." ;
        rdfs:label       "PronounceableText" ;
        rdfs:subClassOf  schema:Text .

schema:activityFrequency
        rdf:type      rdf:Property ;
        rdfs:comment  "How often one should engage in the activity." ;
        rdfs:label    "activityFrequency" .

schema:amenityFeature
        rdf:type      rdf:Property ;
        rdfs:comment  "An amenity feature (e.g. a characteristic or service) of the Accommodation. This generic property does not make a statement about whether the feature is included in an offer for the main accommodation or available at extra costs." ;
        rdfs:label    "amenityFeature" .

schema:maxPrice  rdf:type  rdf:Property ;
        rdfs:comment  "The highest price if the price is a range." ;
        rdfs:label    "maxPrice" .

schema:programMembershipUsed
        rdf:type      rdf:Property ;
        rdfs:comment  "Any membership in a frequent flyer, hotel loyalty program, etc. being applied to the reservation." ;
        rdfs:label    "programMembershipUsed" .

schema:serviceAudience
        rdf:type      rdf:Property ;
        rdfs:comment  "The audience eligible for this service." ;
        rdfs:label    "serviceAudience" .

schema:strengthUnit  rdf:type  rdf:Property ;
        rdfs:comment  "The units of an active ingredient's strength, e.g. mg." ;
        rdfs:label    "strengthUnit" .

dcat:Dataset  rdf:type  rdfs:Class .

schema:sponsor  rdf:type  rdf:Property ;
        rdfs:comment  "A person or organization that supports a thing through a pledge, promise, or financial contribution. e.g. a sponsor of a Medical Study or a corporate sponsor of an event." ;
        rdfs:label    "sponsor" .

schema:URL  rdf:type     rdfs:Class ;
        rdfs:comment     "Data type: URL." ;
        rdfs:label       "URL" ;
        rdfs:subClassOf  schema:Text .

schema:Apartment  rdf:type  rdfs:Class ;
        rdfs:comment     "An apartment (in American English) or flat (in British English) is a self-contained housing unit (a type of residential real estate) that occupies only part of a building (Source: Wikipedia, the free encyclopedia, see <a href=\"http://en.wikipedia.org/wiki/Apartment\">http://en.wikipedia.org/wiki/Apartment</a>)." ;
        rdfs:label       "Apartment" ;
        rdfs:subClassOf  schema:Accommodation .

schema:deliveryStatus
        rdf:type      rdf:Property ;
        rdfs:comment  "New entry added as the package passes through each leg of its journey (from shipment to final delivery)." ;
        rdfs:label    "deliveryStatus" .

schema:legislationConsolidates
        rdf:type      rdf:Property ;
        rdfs:comment  "Indicates another legislation taken into account in this consolidated legislation (which is usually the product of an editorial process that revises the legislation). This property should be used multiple times to refer to both the original version or the previous consolidated version, and to the legislations making the change." ;
        rdfs:label    "legislationConsolidates" .

schema:JobPosting  rdf:type  rdfs:Class ;
        rdfs:comment     "A listing that describes a job opening in a certain organization." ;
        rdfs:label       "JobPosting" ;
        rdfs:subClassOf  schema:Intangible .

schema:BusReservation
        rdf:type         rdfs:Class ;
        rdfs:comment     "A reservation for bus travel. \\n\\nNote: This type is for information about actual reservations, e.g. in confirmation emails or HTML pages with individual confirmations of reservations. For offers of tickets, use [[Offer]]." ;
        rdfs:label       "BusReservation" ;
        rdfs:subClassOf  schema:Reservation .

schema:physicalRequirement
        rdf:type      rdf:Property ;
        rdfs:comment  "A description of the types of physical activity associated with the job. Defined terms such as those in O*net may be used, but note that there is no way to specify the level of ability as well as its nature when using a defined term." ;
        rdfs:label    "physicalRequirement" .

schema:colleague  rdf:type  rdf:Property ;
        rdfs:comment  "A colleague of the person." ;
        rdfs:label    "colleague" .

schema:Duration  rdf:type  rdfs:Class ;
        rdfs:comment     "Quantity: Duration (use [ISO 8601 duration format](http://en.wikipedia.org/wiki/ISO_8601))." ;
        rdfs:label       "Duration" ;
        rdfs:subClassOf  schema:Quantity .

schema:numberOfRooms  rdf:type  rdf:Property ;
        rdfs:comment  "The number of rooms (excluding bathrooms and closets) of the accommodation or lodging business.\nTypical unit code(s): ROM for room or C62 for no unit. The type of room can be put in the unitText property of the QuantitativeValue." ;
        rdfs:label    "numberOfRooms" .

schema:TransferAction
        rdf:type         rdfs:Class ;
        rdfs:comment     "The act of transferring/moving (abstract or concrete) animate or inanimate objects from one place to another." ;
        rdfs:label       "TransferAction" ;
        rdfs:subClassOf  schema:Action .

schema:SizeSpecification
        rdf:type         rdfs:Class ;
        rdfs:comment     "Size related properties of a product, typically a size code ([[name]]) and optionally a [[sizeSystem]], [[sizeGroup]], and product measurements ([[hasMeasurement]]). In addition, the intended audience can be defined through [[suggestedAge]], [[suggestedGender]], and suggested body measurements ([[suggestedMeasurement]])." ;
        rdfs:label       "SizeSpecification" ;
        rdfs:subClassOf  schema:QualitativeValue .

schema:inCodeSet  rdf:type  rdf:Property ;
        rdfs:comment        "A [[CategoryCodeSet]] that contains this category code." ;
        rdfs:label          "inCodeSet" ;
        rdfs:subPropertyOf  schema:inDefinedTermSet .

schema:TheaterGroup  rdf:type  rdfs:Class ;
        rdfs:comment     "A theater group or company, for example, the Royal Shakespeare Company or Druid Theatre." ;
        rdfs:label       "TheaterGroup" ;
        rdfs:subClassOf  schema:PerformingGroup .

schema:pageStart  rdf:type  rdf:Property ;
        rdfs:comment  "The page on which the work starts; for example \"135\" or \"xiii\"." ;
        rdfs:label    "pageStart" .

skos:mappingRelation  rdf:type  owl:ObjectProperty ;
        rdfs:comment        "These concept mapping relations mirror semantic relations, and the data model defined below is similar (with the exception of skos:exactMatch) to the data model defined for semantic relations. A distinct vocabulary is provided for concept mapping relations, to provide a convenient way to differentiate links within a concept scheme from links between concept schemes. However, this pattern of usage is not a formal requirement of the SKOS data model, and relies on informal definitions of best practice."@en ;
        rdfs:label          "is in mapping relation with"@en ;
        rdfs:subPropertyOf  skos:semanticRelation .

schema:spatial  rdf:type  rdf:Property ;
        rdfs:comment  "The \"spatial\" property can be used in cases when more specific properties\n(e.g. [[locationCreated]], [[spatialCoverage]], [[contentLocation]]) are not known to be appropriate." ;
        rdfs:label    "spatial" .

schema:unnamedSourcesPolicy
        rdf:type            rdf:Property ;
        rdfs:comment        "For an [[Organization]] (typically a [[NewsMediaOrganization]]), a statement about policy on use of unnamed sources and the decision process required." ;
        rdfs:label          "unnamedSourcesPolicy" ;
        rdfs:subPropertyOf  schema:publishingPrinciples .

schema:additionalNumberOfGuests
        rdf:type      rdf:Property ;
        rdfs:comment  "If responding yes, the number of guests who will attend in addition to the invitee." ;
        rdfs:label    "additionalNumberOfGuests" .

schema:foodEstablishment
        rdf:type            rdf:Property ;
        rdfs:comment        "A sub property of location. The specific food establishment where the action occurred." ;
        rdfs:label          "foodEstablishment" ;
        rdfs:subPropertyOf  schema:location .

schema:fuelConsumption
        rdf:type      rdf:Property ;
        rdfs:comment  "The amount of fuel consumed for traveling a particular distance or temporal duration with the given vehicle (e.g. liters per 100 km).\\n\\n* Note 1: There are unfortunately no standard unit codes for liters per 100 km.  Use [[unitText]] to indicate the unit of measurement, e.g. L/100 km.\\n* Note 2: There are two ways of indicating the fuel consumption, [[fuelConsumption]] (e.g. 8 liters per 100 km) and [[fuelEfficiency]] (e.g. 30 miles per gallon). They are reciprocal.\\n* Note 3: Often, the absolute value is useful only when related to driving speed (\"at 80 km/h\") or usage pattern (\"city traffic\"). You can use [[valueReference]] to link the value for the fuel consumption to another value." ;
        rdfs:label    "fuelConsumption" .

schema:passengerSequenceNumber
        rdf:type      rdf:Property ;
        rdfs:comment  "The passenger's sequence number as assigned by the airline." ;
        rdfs:label    "passengerSequenceNumber" .

schema:IceCreamShop  rdf:type  rdfs:Class ;
        rdfs:comment     "An ice cream shop." ;
        rdfs:label       "IceCreamShop" ;
        rdfs:subClassOf  schema:FoodEstablishment .

schema:JoinAction  rdf:type  rdfs:Class ;
        rdfs:comment     "An agent joins an event/group with participants/friends at a location.\\n\\nRelated actions:\\n\\n* [[RegisterAction]]: Unlike RegisterAction, JoinAction refers to joining a group/team of people.\\n* [[SubscribeAction]]: Unlike SubscribeAction, JoinAction does not imply that you'll be receiving updates.\\n* [[FollowAction]]: Unlike FollowAction, JoinAction does not imply that you'll be polling for updates." ;
        rdfs:label       "JoinAction" ;
        rdfs:subClassOf  schema:InteractAction .

schema:commentTime  rdf:type  rdf:Property ;
        rdfs:comment  "The time at which the UserComment was made." ;
        rdfs:label    "commentTime" .

schema:WebPage  rdf:type  rdfs:Class ;
        rdfs:comment     "A web page. Every web page is implicitly assumed to be declared to be of type WebPage, so the various properties about that webpage, such as <code>breadcrumb</code> may be used. We recommend explicit declaration if these properties are specified, but if they are found outside of an itemscope, they will be assumed to be about the page." ;
        rdfs:label       "WebPage" ;
        rdfs:subClassOf  schema:CreativeWork .

schema:PrependAction  rdf:type  rdfs:Class ;
        rdfs:comment     "The act of inserting at the beginning if an ordered collection." ;
        rdfs:label       "PrependAction" ;
        rdfs:subClassOf  schema:InsertAction .

schema:busName  rdf:type  rdf:Property ;
        rdfs:comment  "The name of the bus (e.g. Bolt Express)." ;
        rdfs:label    "busName" .

schema:nonprofitStatus
        rdf:type      rdf:Property ;
        rdfs:comment  "nonprofit Status indicates the legal status of a non-profit organization in its primary place of business." ;
        rdfs:label    "nonprofitStatus" .

schema:deathPlace  rdf:type  rdf:Property ;
        rdfs:comment  "The place where the person died." ;
        rdfs:label    "deathPlace" .

schema:availableStrength
        rdf:type      rdf:Property ;
        rdfs:comment  "An available dosage strength for the drug." ;
        rdfs:label    "availableStrength" .

schema:isLiveBroadcast
        rdf:type      rdf:Property ;
        rdfs:comment  "True if the broadcast is of a live event." ;
        rdfs:label    "isLiveBroadcast" .

schema:studyLocation  rdf:type  rdf:Property ;
        rdfs:comment  "The location in which the study is taking/took place." ;
        rdfs:label    "studyLocation" .

schema:namedPosition  rdf:type  rdf:Property ;
        rdfs:comment  "A position played, performed or filled by a person or organization, as part of an organization. For example, an athlete in a SportsTeam might play in the position named 'Quarterback'." ;
        rdfs:label    "namedPosition" .

schema:NightClub  rdf:type  rdfs:Class ;
        rdfs:comment     "A nightclub or discotheque." ;
        rdfs:label       "NightClub" ;
        rdfs:subClassOf  schema:EntertainmentBusiness .

schema:HowToTool  rdf:type  rdfs:Class ;
        rdfs:comment     "A tool used (but not consumed) when performing instructions for how to achieve a result." ;
        rdfs:label       "HowToTool" ;
        rdfs:subClassOf  schema:HowToItem .

schema:productID  rdf:type  rdf:Property ;
        rdfs:comment        "The product identifier, such as ISBN. For example: ``` meta itemprop=\"productID\" content=\"isbn:123-456-789\" ```." ;
        rdfs:label          "productID" ;
        rdfs:subPropertyOf  schema:identifier .

schema:LikeAction  rdf:type  rdfs:Class ;
        rdfs:comment     "The act of expressing a positive sentiment about the object. An agent likes an object (a proposition, topic or theme) with participants." ;
        rdfs:label       "LikeAction" ;
        rdfs:subClassOf  schema:ReactAction .

schema:CreditCard  rdf:type  rdfs:Class ;
        rdfs:comment     "A card payment method of a particular brand or name.  Used to mark up a particular payment method and/or the financial product/service that supplies the card account.\\n\\nCommonly used values:\\n\\n* http://purl.org/goodrelations/v1#AmericanExpress\\n* http://purl.org/goodrelations/v1#DinersClub\\n* http://purl.org/goodrelations/v1#Discover\\n* http://purl.org/goodrelations/v1#JCB\\n* http://purl.org/goodrelations/v1#MasterCard\\n* http://purl.org/goodrelations/v1#VISA\n       " ;
        rdfs:label       "CreditCard" ;
        rdfs:subClassOf  schema:PaymentCard , schema:LoanOrCredit .

schema:predecessorOf  rdf:type  rdf:Property ;
        rdfs:comment  "A pointer from a previous, often discontinued variant of the product to its newer variant." ;
        rdfs:label    "predecessorOf" .

schema:offeredBy  rdf:type  rdf:Property ;
        rdfs:comment  "A pointer to the organization or person making the offer." ;
        rdfs:label    "offeredBy" .

schema:tongueWeight  rdf:type  rdf:Property ;
        rdfs:comment  "The permitted vertical load (TWR) of a trailer attached to the vehicle. Also referred to as Tongue Load Rating (TLR) or Vertical Load Rating (VLR)\\n\\nTypical unit code(s): KGM for kilogram, LBR for pound\\n\\n* Note 1: You can indicate additional information in the [[name]] of the [[QuantitativeValue]] node.\\n* Note 2: You may also link to a [[QualitativeValue]] node that provides additional information using [[valueReference]].\\n* Note 3: Note that you can use [[minValue]] and [[maxValue]] to indicate ranges." ;
        rdfs:label    "tongueWeight" .

schema:endorsers  rdf:type  rdf:Property ;
        rdfs:comment  "People or organizations that endorse the plan." ;
        rdfs:label    "endorsers" .

schema:PaymentChargeSpecification
        rdf:type         rdfs:Class ;
        rdfs:comment     "The costs of settling the payment using a particular payment method." ;
        rdfs:label       "PaymentChargeSpecification" ;
        rdfs:subClassOf  schema:PriceSpecification .

schema:timeRequired  rdf:type  rdf:Property ;
        rdfs:comment  "Approximate or typical time it takes to work with or through this learning resource for the typical intended target audience, e.g. 'PT30M', 'PT1H25M'." ;
        rdfs:label    "timeRequired" .

schema:availabilityStarts
        rdf:type      rdf:Property ;
        rdfs:comment  "The beginning of the availability of the product or service included in the offer." ;
        rdfs:label    "availabilityStarts" .

schema:PreOrderAction
        rdf:type         rdfs:Class ;
        rdfs:comment     "An agent orders a (not yet released) object/product/service to be delivered/sent." ;
        rdfs:label       "PreOrderAction" ;
        rdfs:subClassOf  schema:TradeAction .

schema:TireShop  rdf:type  rdfs:Class ;
        rdfs:comment     "A tire shop." ;
        rdfs:label       "TireShop" ;
        rdfs:subClassOf  schema:Store .

schema:APIReference  rdf:type  rdfs:Class ;
        rdfs:comment     "Reference documentation for application programming interfaces (APIs)." ;
        rdfs:label       "APIReference" ;
        rdfs:subClassOf  schema:TechArticle .

schema:ImagingTest  rdf:type  rdfs:Class ;
        rdfs:comment     "Any medical imaging modality typically used for diagnostic purposes." ;
        rdfs:label       "ImagingTest" ;
        rdfs:subClassOf  schema:MedicalTest .

schema:Clip  rdf:type    rdfs:Class ;
        rdfs:comment     "A short TV or radio program or a segment/part of a program." ;
        rdfs:label       "Clip" ;
        rdfs:subClassOf  schema:CreativeWork .

schema:DryCleaningOrLaundry
        rdf:type         rdfs:Class ;
        rdfs:comment     "A dry-cleaning business." ;
        rdfs:label       "DryCleaningOrLaundry" ;
        rdfs:subClassOf  schema:LocalBusiness .

skos:broaderTransitive
        rdf:type            owl:ObjectProperty ;
        rdfs:label          "has broader transitive"@en ;
        rdfs:subPropertyOf  skos:semanticRelation ;
        owl:inverseOf       skos:narrowerTransitive .

schema:holdingArchive
        rdf:type      rdf:Property ;
        rdfs:comment  "[[ArchiveOrganization]] that holds, keeps or maintains the [[ArchiveComponent]]."@en ;
        rdfs:label    "holdingArchive"@en .

schema:jobLocationType
        rdf:type      rdf:Property ;
        rdfs:comment  "A description of the job location (e.g TELECOMMUTE for telecommute jobs)." ;
        rdfs:label    "jobLocationType" .

schema:DataDownload  rdf:type  rdfs:Class ;
        rdfs:comment     "A dataset in downloadable form." ;
        rdfs:label       "DataDownload" ;
        rdfs:subClassOf  schema:MediaObject .

schema:CriticReview  rdf:type  rdfs:Class ;
        rdfs:comment     "A [[CriticReview]] is a more specialized form of Review written or published by a source that is recognized for its reviewing activities. These can include online columns, travel and food guides, TV and radio shows, blogs and other independent Web sites. [[CriticReview]]s are typically more in-depth and professionally written. For simpler, casually written user/visitor/viewer/customer reviews, it is more appropriate to use the [[UserReview]] type. Review aggregator sites such as Metacritic already separate out the site's user reviews from selected critic reviews that originate from third-party sources." ;
        rdfs:label       "CriticReview" ;
        rdfs:subClassOf  schema:Review .

schema:RoofingContractor
        rdf:type         rdfs:Class ;
        rdfs:comment     "A roofing contractor." ;
        rdfs:label       "RoofingContractor" ;
        rdfs:subClassOf  schema:HomeAndConstructionBusiness .

schema:StatusEnumeration
        rdf:type         rdfs:Class ;
        rdfs:comment     "Lists or enumerations dealing with status types." ;
        rdfs:label       "StatusEnumeration" ;
        rdfs:subClassOf  schema:Enumeration .

schema:isFamilyFriendly
        rdf:type      rdf:Property ;
        rdfs:comment  "Indicates whether this content is family friendly." ;
        rdfs:label    "isFamilyFriendly" .

schema:workPerformed  rdf:type  rdf:Property ;
        rdfs:comment        "A work performed in some event, for example a play performed in a TheaterEvent." ;
        rdfs:label          "workPerformed" ;
        rdfs:subPropertyOf  schema:workFeatured .

schema:leaseLength  rdf:type  rdf:Property ;
        rdfs:comment  "Length of the lease for some [[Accommodation]], either particular to some [[Offer]] or in some cases intrinsic to the property." ;
        rdfs:label    "leaseLength" .

schema:repeatCount  rdf:type  rdf:Property ;
        rdfs:comment  "Defines the number of times a recurring [[Event]] will take place" ;
        rdfs:label    "repeatCount" .

schema:exceptDate  rdf:type  rdf:Property ;
        rdfs:comment  "Defines a [[Date]] or [[DateTime]] during which a scheduled [[Event]] will not take place. The property allows exceptions to\n      a [[Schedule]] to be specified. If an exception is specified as a [[DateTime]] then only the event that would have started at that specific date and time\n      should be excluded from the schedule. If an exception is specified as a [[Date]] then any event that is scheduled for that 24 hour period should be\n      excluded from the schedule. This allows a whole day to be excluded from the schedule without having to itemise every scheduled event." ;
        rdfs:label    "exceptDate" .

schema:estimatedFlightDuration
        rdf:type      rdf:Property ;
        rdfs:comment  "The estimated time the flight will take." ;
        rdfs:label    "estimatedFlightDuration" .

schema:preparation  rdf:type  rdf:Property ;
        rdfs:comment  "Typical preparation that a patient must undergo before having the procedure performed." ;
        rdfs:label    "preparation" .

schema:dropoffLocation
        rdf:type      rdf:Property ;
        rdfs:comment  "Where a rental car can be dropped off." ;
        rdfs:label    "dropoffLocation" .

schema:VoteAction  rdf:type  rdfs:Class ;
        rdfs:comment     "The act of expressing a preference from a fixed/finite/structured set of choices/options." ;
        rdfs:label       "VoteAction" ;
        rdfs:subClassOf  schema:ChooseAction .

schema:BedType  rdf:type  rdfs:Class ;
        rdfs:comment     "A type of bed. This is used for indicating the bed or beds available in an accommodation." ;
        rdfs:label       "BedType" ;
        rdfs:subClassOf  schema:QualitativeValue .

schema:cvdFacilityCounty
        rdf:type      rdf:Property ;
        rdfs:comment  "Name of the County of the NHSN facility that this data record applies to. Use [[cvdFacilityId]] to identify the facility. To provide other details, [[healthcareReportingData]] can be used on a [[Hospital]] entry." ;
        rdfs:label    "cvdFacilityCounty" .

schema:WriteAction  rdf:type  rdfs:Class ;
        rdfs:comment     "The act of authoring written creative content." ;
        rdfs:label       "WriteAction" ;
        rdfs:subClassOf  schema:CreateAction .

schema:MenuSection  rdf:type  rdfs:Class ;
        rdfs:comment     "A sub-grouping of food or drink items in a menu. E.g. courses (such as 'Dinner', 'Breakfast', etc.), specific type of dishes (such as 'Meat', 'Vegan', 'Drinks', etc.), or some other classification made by the menu provider." ;
        rdfs:label       "MenuSection" ;
        rdfs:subClassOf  schema:CreativeWork .

schema:ContactPage  rdf:type  rdfs:Class ;
        rdfs:comment     "Web page type: Contact page." ;
        rdfs:label       "ContactPage" ;
        rdfs:subClassOf  schema:WebPage .

schema:reviewCount  rdf:type  rdf:Property ;
        rdfs:comment  "The count of total number of reviews." ;
        rdfs:label    "reviewCount" .

schema:Photograph  rdf:type  rdfs:Class ;
        rdfs:comment     "A photograph." ;
        rdfs:label       "Photograph" ;
        rdfs:subClassOf  schema:CreativeWork .

schema:expectedArrivalFrom
        rdf:type      rdf:Property ;
        rdfs:comment  "The earliest date the package may arrive." ;
        rdfs:label    "expectedArrivalFrom" .

schema:recipe  rdf:type     rdf:Property ;
        rdfs:comment        "A sub property of instrument. The recipe/instructions used to perform the action." ;
        rdfs:label          "recipe" ;
        rdfs:subPropertyOf  schema:instrument .

skos:broader  rdf:type      owl:ObjectProperty ;
        rdfs:comment        "Broader concepts are typically rendered as parents in a concept hierarchy (tree)."@en ;
        rdfs:label          "has broader"@en ;
        rdfs:subPropertyOf  skos:broaderTransitive ;
        owl:inverseOf       skos:narrower .

schema:checkoutTime  rdf:type  rdf:Property ;
        rdfs:comment  "The latest someone may check out of a lodging establishment." ;
        rdfs:label    "checkoutTime" .

schema:InvestmentFund
        rdf:type         rdfs:Class ;
        rdfs:comment     "A company or fund that gathers capital from a number of investors to create a pool of money that is then re-invested into stocks, bonds and other assets." ;
        rdfs:label       "InvestmentFund" ;
        rdfs:subClassOf  schema:InvestmentOrDeposit .

schema:fuelEfficiency
        rdf:type      rdf:Property ;
        rdfs:comment  "The distance traveled per unit of fuel used; most commonly miles per gallon (mpg) or kilometers per liter (km/L).\\n\\n* Note 1: There are unfortunately no standard unit codes for miles per gallon or kilometers per liter. Use [[unitText]] to indicate the unit of measurement, e.g. mpg or km/L.\\n* Note 2: There are two ways of indicating the fuel consumption, [[fuelConsumption]] (e.g. 8 liters per 100 km) and [[fuelEfficiency]] (e.g. 30 miles per gallon). They are reciprocal.\\n* Note 3: Often, the absolute value is useful only when related to driving speed (\"at 80 km/h\") or usage pattern (\"city traffic\"). You can use [[valueReference]] to link the value for the fuel economy to another value." ;
        rdfs:label    "fuelEfficiency" .

schema:orderedItem  rdf:type  rdf:Property ;
        rdfs:comment  "The item ordered." ;
        rdfs:label    "orderedItem" .

schema:map  rdf:type  rdf:Property ;
        rdfs:comment  "A URL to a map of the place." ;
        rdfs:label    "map" .

schema:circle  rdf:type  rdf:Property ;
        rdfs:comment  "A circle is the circular region of a specified radius centered at a specified latitude and longitude. A circle is expressed as a pair followed by a radius in meters." ;
        rdfs:label    "circle" .

schema:materialExtent
        rdf:type      rdf:Property ;
        rdfs:comment  "The quantity of the materials being described or an expression of the physical space they occupy."@en ;
        rdfs:label    "materialExtent"@en .

schema:actors  rdf:type  rdf:Property ;
        rdfs:comment  "An actor, e.g. in tv, radio, movie, video games etc. Actors can be associated with individual items or with a series, episode, clip." ;
        rdfs:label    "actors" .

schema:PlayAction  rdf:type  rdfs:Class ;
        rdfs:comment     "The act of playing/exercising/training/performing for enjoyment, leisure, recreation, Competition or exercise.\\n\\nRelated actions:\\n\\n* [[ListenAction]]: Unlike ListenAction (which is under ConsumeAction), PlayAction refers to performing for an audience or at an event, rather than consuming music.\\n* [[WatchAction]]: Unlike WatchAction (which is under ConsumeAction), PlayAction refers to showing/displaying for an audience or at an event, rather than consuming visual content." ;
        rdfs:label       "PlayAction" ;
        rdfs:subClassOf  schema:Action .

schema:parents  rdf:type  rdf:Property ;
        rdfs:comment  "A parents of the person." ;
        rdfs:label    "parents" .

schema:Airline  rdf:type  rdfs:Class ;
        rdfs:comment     "An organization that provides flights for passengers." ;
        rdfs:label       "Airline" ;
        rdfs:subClassOf  schema:Organization .

schema:jobTitle  rdf:type  rdf:Property ;
        rdfs:comment  "The job title of the person (for example, Financial Manager)." ;
        rdfs:label    "jobTitle" .

schema:correctionsPolicy
        rdf:type            rdf:Property ;
        rdfs:comment        "For an [[Organization]] (e.g. [[NewsMediaOrganization]]), a statement describing (in news media, the newsroom’s) disclosure and correction policy for errors." ;
        rdfs:label          "correctionsPolicy" ;
        rdfs:subPropertyOf  schema:publishingPrinciples .

schema:legislationPassedBy
        rdf:type            rdf:Property ;
        rdfs:comment        "The person or organization that originally passed or made the law : typically parliament (for primary legislation) or government (for secondary legislation). This indicates the \"legal author\" of the law, as opposed to its physical author." ;
        rdfs:label          "legislationPassedBy" ;
        rdfs:subPropertyOf  schema:creator .

schema:BroadcastChannel
        rdf:type         rdfs:Class ;
        rdfs:comment     "A unique instance of a BroadcastService on a CableOrSatelliteService lineup." ;
        rdfs:label       "BroadcastChannel" ;
        rdfs:subClassOf  schema:Intangible .

schema:membershipPointsEarned
        rdf:type      rdf:Property ;
        rdfs:comment  "The number of membership points earned by the member. If necessary, the unitText can be used to express the units the points are issued in. (e.g. stars, miles, etc.)" ;
        rdfs:label    "membershipPointsEarned" .

schema:ConvenienceStore
        rdf:type         rdfs:Class ;
        rdfs:comment     "A convenience store." ;
        rdfs:label       "ConvenienceStore" ;
        rdfs:subClassOf  schema:Store .

schema:xpath  rdf:type  rdf:Property ;
        rdfs:comment  "An XPath, e.g. of a [[SpeakableSpecification]] or [[WebPageElement]]. In the latter case, multiple matches within a page can constitute a single conceptual \"Web page element\"." ;
        rdfs:label    "xpath" .

schema:CatholicChurch
        rdf:type         rdfs:Class ;
        rdfs:comment     "A Catholic church." ;
        rdfs:label       "CatholicChurch" ;
        rdfs:subClassOf  schema:Church .

schema:cookingMethod  rdf:type  rdf:Property ;
        rdfs:comment  "The method of cooking, such as Frying, Steaming, ..." ;
        rdfs:label    "cookingMethod" .

schema:executableLibraryName
        rdf:type      rdf:Property ;
        rdfs:comment  "Library file name e.g., mscorlib.dll, system.web.dll." ;
        rdfs:label    "executableLibraryName" .

schema:TrainTrip  rdf:type  rdfs:Class ;
        rdfs:comment     "A trip on a commercial train line." ;
        rdfs:label       "TrainTrip" ;
        rdfs:subClassOf  schema:Trip .

schema:BroadcastService
        rdf:type         rdfs:Class ;
        rdfs:comment     "A delivery service through which content is provided via broadcast over the air or online." ;
        rdfs:label       "BroadcastService" ;
        rdfs:subClassOf  schema:Service .

schema:numberOfPages  rdf:type  rdf:Property ;
        rdfs:comment  "The number of pages in the book." ;
        rdfs:label    "numberOfPages" .

schema:EmployeeRole  rdf:type  rdfs:Class ;
        rdfs:comment     "A subclass of OrganizationRole used to describe employee relationships." ;
        rdfs:label       "EmployeeRole" ;
        rdfs:subClassOf  schema:OrganizationRole .

schema:ImageObject  rdf:type  rdfs:Class ;
        rdfs:comment     "An image file." ;
        rdfs:label       "ImageObject" ;
        rdfs:subClassOf  schema:MediaObject .

schema:LegalService  rdf:type  rdfs:Class ;
        rdfs:comment     "A LegalService is a business that provides legally-oriented services, advice and representation, e.g. law firms.\\n\\nAs a [[LocalBusiness]] it can be described as a [[provider]] of one or more [[Service]]\\(s)." ;
        rdfs:label       "LegalService" ;
        rdfs:subClassOf  schema:LocalBusiness .

schema:UserCheckins  rdf:type  rdfs:Class ;
        rdfs:comment     "UserInteraction and its subtypes is an old way of talking about users interacting with pages. It is generally better to use [[Action]]-based vocabulary, alongside types such as [[Comment]]." ;
        rdfs:label       "UserCheckins" ;
        rdfs:subClassOf  schema:UserInteraction .

schema:bccRecipient  rdf:type  rdf:Property ;
        rdfs:comment        "A sub property of recipient. The recipient blind copied on a message." ;
        rdfs:label          "bccRecipient" ;
        rdfs:subPropertyOf  schema:recipient .

schema:AchieveAction  rdf:type  rdfs:Class ;
        rdfs:comment     "The act of accomplishing something via previous efforts. It is an instantaneous action rather than an ongoing process." ;
        rdfs:label       "AchieveAction" ;
        rdfs:subClassOf  schema:Action .

schema:collection  rdf:type  rdf:Property ;
        rdfs:comment        "A sub property of object. The collection target of the action." ;
        rdfs:label          "collection" ;
        rdfs:subPropertyOf  schema:object .

schema:occupancy  rdf:type  rdf:Property ;
        rdfs:comment  "The allowed total occupancy for the accommodation in persons (including infants etc). For individual accommodations, this is not necessarily the legal maximum but defines the permitted usage as per the contractual agreement (e.g. a double room used by a single person).\nTypical unit code(s): C62 for person" ;
        rdfs:label    "occupancy" .

schema:ReservationPackage
        rdf:type         rdfs:Class ;
        rdfs:comment     "A group of multiple reservations with common values for all sub-reservations." ;
        rdfs:label       "ReservationPackage" ;
        rdfs:subClassOf  schema:Reservation .

schema:faxNumber  rdf:type  rdf:Property ;
        rdfs:comment  "The fax number." ;
        rdfs:label    "faxNumber" .

schema:CheckAction  rdf:type  rdfs:Class ;
        rdfs:comment     "An agent inspects, determines, investigates, inquires, or examines an object's accuracy, quality, condition, or state." ;
        rdfs:label       "CheckAction" ;
        rdfs:subClassOf  schema:FindAction .

schema:cvdNumTotBeds  rdf:type  rdf:Property ;
        rdfs:comment  "numtotbeds - ALL HOSPITAL BEDS: Total number of all Inpatient and outpatient beds, including all staffed,ICU, licensed, and overflow (surge) beds used for inpatients or outpatients." ;
        rdfs:label    "cvdNumTotBeds" .

schema:previousItem  rdf:type  rdf:Property ;
        rdfs:comment  "A link to the ListItem that preceeds the current one." ;
        rdfs:label    "previousItem" .

schema:transmissionMethod
        rdf:type      rdf:Property ;
        rdfs:comment  "How the disease spreads, either as a route or vector, for example 'direct contact', 'Aedes aegypti', etc." ;
        rdfs:label    "transmissionMethod" .

schema:Casino  rdf:type  rdfs:Class ;
        rdfs:comment     "A casino." ;
        rdfs:label       "Casino" ;
        rdfs:subClassOf  schema:EntertainmentBusiness .

schema:track  rdf:type  rdf:Property ;
        rdfs:comment  "A music recording (track)&#x2014;usually a single song. If an ItemList is given, the list should contain items of type MusicRecording." ;
        rdfs:label    "track" .

schema:MusicStore  rdf:type  rdfs:Class ;
        rdfs:comment     "A music store." ;
        rdfs:label       "MusicStore" ;
        rdfs:subClassOf  schema:Store .

schema:requiredCollateral
        rdf:type      rdf:Property ;
        rdfs:comment  "Assets required to secure loan or credit repayments. It may take form of third party pledge, goods, financial instruments (cash, securities, etc.)" ;
        rdfs:label    "requiredCollateral" .

skos:Collection  rdf:type  rdfs:Class ;
        rdfs:label  "Collection"@en .

schema:Flight  rdf:type  rdfs:Class ;
        rdfs:comment     "An airline flight." ;
        rdfs:label       "Flight" ;
        rdfs:subClassOf  schema:Trip .

schema:Grant  rdf:type   rdfs:Class ;
        rdfs:comment     "A grant, typically financial or otherwise quantifiable, of resources. Typically a [[funder]] sponsors some [[MonetaryAmount]] to an [[Organization]] or [[Person]],\n    sometimes not necessarily via a dedicated or long-lived [[Project]], resulting in one or more outputs, or [[fundedItem]]s. For financial sponsorship, indicate the [[funder]] of a [[MonetaryGrant]]. For non-financial support, indicate [[sponsor]] of [[Grant]]s of resources (e.g. office space).\n\nGrants support  activities directed towards some agreed collective goals, often but not always organized as [[Project]]s. Long-lived projects are sometimes sponsored by a variety of grants over time, but it is also common for a project to be associated with a single grant.\n\nThe amount of a [[Grant]] is represented using [[amount]] as a [[MonetaryAmount]].\n    " ;
        rdfs:label       "Grant" ;
        rdfs:subClassOf  schema:Intangible .

schema:warrantyScope  rdf:type  rdf:Property ;
        rdfs:comment  "The scope of the warranty promise." ;
        rdfs:label    "warrantyScope" .

schema:SendAction  rdf:type  rdfs:Class ;
        rdfs:comment     "The act of physically/electronically dispatching an object for transfer from an origin to a destination.Related actions:\\n\\n* [[ReceiveAction]]: The reciprocal of SendAction.\\n* [[GiveAction]]: Unlike GiveAction, SendAction does not imply the transfer of ownership (e.g. I can send you my laptop, but I'm not necessarily giving it to you)." ;
        rdfs:label       "SendAction" ;
        rdfs:subClassOf  schema:TransferAction .

schema:ProfilePage  rdf:type  rdfs:Class ;
        rdfs:comment     "Web page type: Profile page." ;
        rdfs:label       "ProfilePage" ;
        rdfs:subClassOf  schema:WebPage .

schema:evidenceLevel  rdf:type  rdf:Property ;
        rdfs:comment  "Strength of evidence of the data used to formulate the guideline (enumerated)." ;
        rdfs:label    "evidenceLevel" .

schema:device  rdf:type  rdf:Property ;
        rdfs:comment  "Device required to run the application. Used in cases where a specific make/model is required to run the application." ;
        rdfs:label    "device" .

schema:subEvents  rdf:type  rdf:Property ;
        rdfs:comment  "Events that are a part of this event. For example, a conference event includes many presentations, each subEvents of the conference." ;
        rdfs:label    "subEvents" .

schema:schoolClosuresInfo
        rdf:type      rdf:Property ;
        rdfs:comment  "Information about school closures." ;
        rdfs:label    "schoolClosuresInfo" .

schema:utterances  rdf:type  rdf:Property ;
        rdfs:comment  "Text of an utterances (spoken words, lyrics etc.) that occurs at a certain section of a media object, represented as a [[HyperTocEntry]]." ;
        rdfs:label    "utterances" .

schema:publishedBy  rdf:type  rdf:Property ;
        rdfs:comment  "An agent associated with the publication event." ;
        rdfs:label    "publishedBy" .

schema:usedToDiagnose
        rdf:type      rdf:Property ;
        rdfs:comment  "A condition the test is used to diagnose." ;
        rdfs:label    "usedToDiagnose" .

schema:relatedAnatomy
        rdf:type      rdf:Property ;
        rdfs:comment  "Anatomical systems or structures that relate to the superficial anatomy." ;
        rdfs:label    "relatedAnatomy" .

schema:siblings  rdf:type  rdf:Property ;
        rdfs:comment  "A sibling of the person." ;
        rdfs:label    "siblings" .

schema:trackingNumber
        rdf:type      rdf:Property ;
        rdfs:comment  "Shipper tracking number." ;
        rdfs:label    "trackingNumber" .

schema:elevation  rdf:type  rdf:Property ;
        rdfs:comment  "The elevation of a location ([WGS 84](https://en.wikipedia.org/wiki/World_Geodetic_System)). Values may be of the form 'NUMBER UNIT_OF_MEASUREMENT' (e.g., '1,000 m', '3,200 ft') while numbers alone should be assumed to be a value in meters." ;
        rdfs:label    "elevation" .

schema:timeOfDay  rdf:type  rdf:Property ;
        rdfs:comment  "The time of day the program normally runs. For example, \"evenings\"." ;
        rdfs:label    "timeOfDay" .

schema:datePublished  rdf:type  rdf:Property ;
        rdfs:comment  "Date of first broadcast/publication." ;
        rdfs:label    "datePublished" .

schema:interactingDrug
        rdf:type      rdf:Property ;
        rdfs:comment  "Another drug that is known to interact with this drug in a way that impacts the effect of this drug or causes a risk to the patient. Note: disease interactions are typically captured as contraindications." ;
        rdfs:label    "interactingDrug" .

schema:gender  rdf:type  rdf:Property ;
        rdfs:comment  "Gender of something, typically a [[Person]], but possibly also fictional characters, animals, etc. While http://schema.org/Male and http://schema.org/Female may be used, text strings are also acceptable for people who do not identify as a binary gender. The [[gender]] property can also be used in an extended sense to cover e.g. the gender of sports teams. As with the gender of individuals, we do not try to enumerate all possibilities. A mixed-gender [[SportsTeam]] can be indicated with a text value of \"Mixed\"." ;
        rdfs:label    "gender" .

schema:offers  rdf:type  rdf:Property ;
        rdfs:comment  "An offer to provide this item&#x2014;for example, an offer to sell a product, rent the DVD of a movie, perform a service, or give away tickets to an event. Use [[businessFunction]] to indicate the kind of transaction offered, i.e. sell, lease, etc. This property can also be used to describe a [[Demand]]. While this property is listed as expected on a number of common types, it can be used in others. In that case, using a second type, such as Product or a subtype of Product, can clarify the nature of the offer.\n      " ;
        rdfs:label    "offers" .

schema:Bakery  rdf:type  rdfs:Class ;
        rdfs:comment     "A bakery." ;
        rdfs:label       "Bakery" ;
        rdfs:subClassOf  schema:FoodEstablishment .

schema:healthCondition
        rdf:type      rdf:Property ;
        rdfs:comment  "Specifying the health condition(s) of a patient, medical study, or other target audience." ;
        rdfs:label    "healthCondition" .

skos:historyNote  rdf:type  rdf:Property ;
        rdfs:label          "history note"@en ;
        rdfs:subPropertyOf  skos:note .

schema:isPlanForApartment
        rdf:type      rdf:Property ;
        rdfs:comment  "Indicates some accommodation that this floor plan describes." ;
        rdfs:label    "isPlanForApartment" .

schema:ExerciseGym  rdf:type  rdfs:Class ;
        rdfs:comment     "A gym." ;
        rdfs:label       "ExerciseGym" ;
        rdfs:subClassOf  schema:SportsActivityLocation .

schema:WebAPI  rdf:type  rdfs:Class ;
        rdfs:comment     "An application programming interface accessible over Web/Internet technologies." ;
        rdfs:label       "WebAPI" ;
        rdfs:subClassOf  schema:Service .

schema:genre  rdf:type  rdf:Property ;
        rdfs:comment  "Genre of the creative work, broadcast channel or group." ;
        rdfs:label    "genre" .

schema:Volcano  rdf:type  rdfs:Class ;
        rdfs:comment     "A volcano, like Fuji san." ;
        rdfs:label       "Volcano" ;
        rdfs:subClassOf  schema:Landform .

schema:geoTouches  rdf:type  rdf:Property ;
        rdfs:comment  "Represents spatial relations in which two geometries (or the places they represent) touch: they have at least one boundary point in common, but no interior points.\" (a symmetric relationship, as defined in [DE-9IM](https://en.wikipedia.org/wiki/DE-9IM) )" ;
        rdfs:label    "geoTouches" .

schema:MathSolver  rdf:type  rdfs:Class ;
        rdfs:comment     "A math solver which is capable of solving a subset of mathematical problems." ;
        rdfs:label       "MathSolver" ;
        rdfs:subClassOf  schema:CreativeWork .

schema:SizeGroupEnumeration
        rdf:type         rdfs:Class ;
        rdfs:comment     "Enumerates common size groups for various product categories." ;
        rdfs:label       "SizeGroupEnumeration" ;
        rdfs:subClassOf  schema:Enumeration .

schema:BroadcastFrequencySpecification
        rdf:type         rdfs:Class ;
        rdfs:comment     "The frequency in MHz and the modulation used for a particular BroadcastService." ;
        rdfs:label       "BroadcastFrequencySpecification" ;
        rdfs:subClassOf  schema:Intangible .

schema:Resort  rdf:type  rdfs:Class ;
        rdfs:comment     "A resort is a place used for relaxation or recreation, attracting visitors for holidays or vacations. Resorts are places, towns or sometimes commercial establishment operated by a single company (Source: Wikipedia, the free encyclopedia, see <a href=\"http://en.wikipedia.org/wiki/Resort\">http://en.wikipedia.org/wiki/Resort</a>).\n<br /><br />\nSee also the <a href=\"/docs/hotels.html\">dedicated document on the use of schema.org for marking up hotels and other forms of accommodations</a>.\n    " ;
        rdfs:label       "Resort" ;
        rdfs:subClassOf  schema:LodgingBusiness .

schema:ingredients  rdf:type  rdf:Property ;
        rdfs:comment        "A single ingredient used in the recipe, e.g. sugar, flour or garlic." ;
        rdfs:label          "ingredients" ;
        rdfs:subPropertyOf  schema:supply .

schema:maximumVirtualAttendeeCapacity
        rdf:type      rdf:Property ;
        rdfs:comment  "The maximum physical attendee capacity of an [[Event]] whose [[eventAttendanceMode]] is [[OnlineEventAttendanceMode]] (or the online aspects, in the case of a [[MixedEventAttendanceMode]]). " ;
        rdfs:label    "maximumVirtualAttendeeCapacity" .

schema:loanRepaymentForm
        rdf:type      rdf:Property ;
        rdfs:comment  "A form of paying back money previously borrowed from a lender. Repayment usually takes the form of periodic payments that normally include part principal plus interest in each payment." ;
        rdfs:label    "loanRepaymentForm" .

schema:MedicalTest  rdf:type  rdfs:Class ;
        rdfs:comment     "Any medical test, typically performed for diagnostic purposes." ;
        rdfs:label       "MedicalTest" ;
        rdfs:subClassOf  schema:MedicalEntity .

schema:PoliceStation  rdf:type  rdfs:Class ;
        rdfs:comment     "A police station." ;
        rdfs:label       "PoliceStation" ;
        rdfs:subClassOf  schema:CivicStructure , schema:EmergencyService .

schema:VisualArtsEvent
        rdf:type         rdfs:Class ;
        rdfs:comment     "Event type: Visual arts event." ;
        rdfs:label       "VisualArtsEvent" ;
        rdfs:subClassOf  schema:Event .

schema:currenciesAccepted
        rdf:type      rdf:Property ;
        rdfs:comment  "The currency accepted.\\n\\nUse standard formats: [ISO 4217 currency format](http://en.wikipedia.org/wiki/ISO_4217) e.g. \"USD\"; [Ticker symbol](https://en.wikipedia.org/wiki/List_of_cryptocurrencies) for cryptocurrencies e.g. \"BTC\"; well known names for [Local Exchange Tradings Systems](https://en.wikipedia.org/wiki/Local_exchange_trading_system) (LETS) and other currency types e.g. \"Ithaca HOUR\"." ;
        rdfs:label    "currenciesAccepted" .

schema:healthPlanCostSharing
        rdf:type      rdf:Property ;
        rdfs:comment  "Whether The costs to the patient for services under this network or formulary." ;
        rdfs:label    "healthPlanCostSharing" .

schema:DefinedTerm  rdf:type  rdfs:Class ;
        rdfs:comment     "A word, name, acronym, phrase, etc. with a formal definition. Often used in the context of category or subject classification, glossaries or dictionaries, product or creative work types, etc. Use the name property for the term being defined, use termCode if the term has an alpha-numeric code allocated, use description to provide the definition of the term." ;
        rdfs:label       "DefinedTerm" ;
        rdfs:subClassOf  schema:Intangible .

schema:administrationRoute
        rdf:type      rdf:Property ;
        rdfs:comment  "A route by which this drug may be administered, e.g. 'oral'." ;
        rdfs:label    "administrationRoute" .

schema:fileSize  rdf:type  rdf:Property ;
        rdfs:comment  "Size of the application / package (e.g. 18MB). In the absence of a unit (MB, KB etc.), KB will be assumed." ;
        rdfs:label    "fileSize" .

schema:applicationCategory
        rdf:type      rdf:Property ;
        rdfs:comment  "Type of software application, e.g. 'Game, Multimedia'." ;
        rdfs:label    "applicationCategory" .

schema:ConsumeAction  rdf:type  rdfs:Class ;
        rdfs:comment     "The act of ingesting information/resources/food." ;
        rdfs:label       "ConsumeAction" ;
        rdfs:subClassOf  schema:Action .

schema:paymentAccepted
        rdf:type      rdf:Property ;
        rdfs:comment  "Cash, Credit Card, Cryptocurrency, Local Exchange Tradings System, etc." ;
        rdfs:label    "paymentAccepted" .

schema:CompleteDataFeed
        rdf:type         rdfs:Class ;
        rdfs:comment     "A [[CompleteDataFeed]] is a [[DataFeed]] whose standard representation includes content for every item currently in the feed.\n\nThis is the equivalent of Atom's element as defined in Feed Paging and Archiving [RFC 5005](https://tools.ietf.org/html/rfc5005), For example (and as defined for Atom), when using data from a feed that represents a collection of items that varies over time (e.g. \"Top Twenty Records\") there is no need to have newer entries mixed in alongside older, obsolete entries. By marking this feed as a CompleteDataFeed, old entries can be safely discarded when the feed is refreshed, since we can assume the feed has provided descriptions for all current items." ;
        rdfs:label       "CompleteDataFeed" ;
        rdfs:subClassOf  schema:DataFeed .

schema:TouristAttraction
        rdf:type         rdfs:Class ;
        rdfs:comment     "A tourist attraction.  In principle any Thing can be a [[TouristAttraction]], from a [[Mountain]] and [[LandmarksOrHistoricalBuildings]] to a [[LocalBusiness]].  This Type can be used on its own to describe a general [[TouristAttraction]], or be used as an [[additionalType]] to add tourist attraction properties to any other type.  (See examples below)" ;
        rdfs:label       "TouristAttraction" ;
        rdfs:subClassOf  schema:Place .

schema:AudioObject  rdf:type  rdfs:Class ;
        rdfs:comment     "An audio file." ;
        rdfs:label       "AudioObject" ;
        rdfs:subClassOf  schema:MediaObject .

schema:geographicArea
        rdf:type      rdf:Property ;
        rdfs:comment  "The geographic area associated with the audience." ;
        rdfs:label    "geographicArea" .

schema:BusinessEvent  rdf:type  rdfs:Class ;
        rdfs:comment     "Event type: Business event." ;
        rdfs:label       "BusinessEvent" ;
        rdfs:subClassOf  schema:Event .

schema:noBylinesPolicy
        rdf:type            rdf:Property ;
        rdfs:comment        "For a [[NewsMediaOrganization]] or other news-related [[Organization]], a statement explaining when authors of articles are not named in bylines." ;
        rdfs:label          "noBylinesPolicy" ;
        rdfs:subPropertyOf  schema:publishingPrinciples .

schema:actionAccessibilityRequirement
        rdf:type      rdf:Property ;
        rdfs:comment  "A set of requirements that a must be fulfilled in order to perform an Action. If more than one value is specied, fulfilling one set of requirements will allow the Action to be performed." ;
        rdfs:label    "actionAccessibilityRequirement" .

schema:customer  rdf:type  rdf:Property ;
        rdfs:comment  "Party placing the order or paying the invoice." ;
        rdfs:label    "customer" .

schema:awayTeam  rdf:type   rdf:Property ;
        rdfs:comment        "The away team in a sports event." ;
        rdfs:label          "awayTeam" ;
        rdfs:subPropertyOf  schema:competitor .

schema:Otolaryngologic
        rdf:type         rdfs:Class ;
        rdfs:comment     "A specific branch of medical science that is concerned with the ear, nose and throat and their respective disease states." ;
        rdfs:label       "Otolaryngologic" ;
        rdfs:subClassOf  schema:MedicalBusiness .

schema:significantLink
        rdf:type      rdf:Property ;
        rdfs:comment  "One of the more significant URLs on the page. Typically, these are the non-navigation links that are clicked on the most." ;
        rdfs:label    "significantLink" .

schema:CoverArt  rdf:type  rdfs:Class ;
        rdfs:comment     "The artwork on the outer surface of a CreativeWork." ;
        rdfs:label       "CoverArt" ;
        rdfs:subClassOf  schema:VisualArtwork .

schema:areaServed  rdf:type  rdf:Property ;
        rdfs:comment  "The geographic area where a service or offered item is provided." ;
        rdfs:label    "areaServed" .

schema:serialNumber  rdf:type  rdf:Property ;
        rdfs:comment        "The serial number or any alphanumeric identifier of a particular product. When attached to an offer, it is a shortcut for the serial number of the product included in the offer." ;
        rdfs:label          "serialNumber" ;
        rdfs:subPropertyOf  schema:identifier .

schema:specialOpeningHoursSpecification
        rdf:type      rdf:Property ;
        rdfs:comment  "The special opening hours of a certain place.\\n\\nUse this to explicitly override general opening hours brought in scope by [[openingHoursSpecification]] or [[openingHours]].\n      " ;
        rdfs:label    "specialOpeningHoursSpecification" .

schema:Zoo  rdf:type     rdfs:Class ;
        rdfs:comment     "A zoo." ;
        rdfs:label       "Zoo" ;
        rdfs:subClassOf  schema:CivicStructure .

schema:episode  rdf:type    rdf:Property ;
        rdfs:comment        "An episode of a tv, radio or game media within a series or season." ;
        rdfs:label          "episode" ;
        rdfs:subPropertyOf  schema:hasPart .

schema:jurisdiction  rdf:type  rdf:Property ;
        rdfs:comment  "Indicates a legal jurisdiction, e.g. of some legislation, or where some government service is based." ;
        rdfs:label    "jurisdiction" .

schema:MedicalClinic  rdf:type  rdfs:Class ;
        rdfs:comment     "A facility, often associated with a hospital or medical school, that is devoted to the specific diagnosis and/or healthcare. Previously limited to outpatients but with evolution it may be open to inpatients as well." ;
        rdfs:label       "MedicalClinic" ;
        rdfs:subClassOf  schema:MedicalBusiness , schema:MedicalOrganization .

schema:CategoryCode  rdf:type  rdfs:Class ;
        rdfs:comment     "A Category Code." ;
        rdfs:label       "CategoryCode" ;
        rdfs:subClassOf  schema:DefinedTerm .

schema:DataFeedItem  rdf:type  rdfs:Class ;
        rdfs:comment     "A single item within a larger data feed." ;
        rdfs:label       "DataFeedItem" ;
        rdfs:subClassOf  schema:Intangible .

schema:warrantyPromise
        rdf:type      rdf:Property ;
        rdfs:comment  "The warranty promise(s) included in the offer." ;
        rdfs:label    "warrantyPromise" .

schema:PodcastEpisode
        rdf:type         rdfs:Class ;
        rdfs:comment     "A single episode of a podcast series." ;
        rdfs:label       "PodcastEpisode" ;
        rdfs:subClassOf  schema:Episode .

schema:sodiumContent  rdf:type  rdf:Property ;
        rdfs:comment  "The number of milligrams of sodium." ;
        rdfs:label    "sodiumContent" .

schema:bookingTime  rdf:type  rdf:Property ;
        rdfs:comment  "The date and time the reservation was booked." ;
        rdfs:label    "bookingTime" .

schema:hasHealthAspect
        rdf:type      rdf:Property ;
        rdfs:comment  "Indicates the aspect or aspects specifically addressed in some [[HealthTopicContent]]. For example, that the content is an overview, or that it talks about treatment, self-care, treatments or their side-effects." ;
        rdfs:label    "hasHealthAspect" .

schema:gameItem  rdf:type  rdf:Property ;
        rdfs:comment  "An item is an object within the game world that can be collected by a player or, occasionally, a non-player character." ;
        rdfs:label    "gameItem" .

schema:supersededBy  rdf:type  rdf:Property ;
        rdfs:comment  "Relates a term (i.e. a property, class or enumeration) to one that supersedes it." ;
        rdfs:label    "supersededBy" .

schema:printColumn  rdf:type  rdf:Property ;
        rdfs:comment  "The number of the column in which the NewsArticle appears in the print edition." ;
        rdfs:label    "printColumn" .

schema:numberOfPlayers
        rdf:type      rdf:Property ;
        rdfs:comment  "Indicate how many people can play this game (minimum, maximum, or range)." ;
        rdfs:label    "numberOfPlayers" .

schema:comment  rdf:type  rdf:Property ;
        rdfs:comment  "Comments, typically from users." ;
        rdfs:label    "comment" .

schema:Place  rdf:type   rdfs:Class ;
        rdfs:comment     "Entities that have a somewhat fixed, physical extension." ;
        rdfs:label       "Place" ;
        rdfs:subClassOf  schema:Thing .

schema:letterer  rdf:type  rdf:Property ;
        rdfs:comment  "The individual who adds lettering, including speech balloons and sound effects, to artwork." ;
        rdfs:label    "letterer" .

schema:contactPoint  rdf:type  rdf:Property ;
        rdfs:comment  "A contact point for a person or organization." ;
        rdfs:label    "contactPoint" .

schema:broker  rdf:type  rdf:Property ;
        rdfs:comment  "An entity that arranges for an exchange between a buyer and a seller.  In most cases a broker never acquires or releases ownership of a product or service involved in an exchange.  If it is not clear whether an entity is a broker, seller, or buyer, the latter two terms are preferred." ;
        rdfs:label    "broker" .

schema:MedicalRiskCalculator
        rdf:type         rdfs:Class ;
        rdfs:comment     "A complex mathematical calculation requiring an online calculator, used to assess prognosis. Note: use the url property of Thing to record any URLs for online calculators." ;
        rdfs:label       "MedicalRiskCalculator" ;
        rdfs:subClassOf  schema:MedicalRiskEstimator .

schema:appliesToDeliveryMethod
        rdf:type      rdf:Property ;
        rdfs:comment  "The delivery method(s) to which the delivery charge or payment charge specification applies." ;
        rdfs:label    "appliesToDeliveryMethod" .

schema:suggestedMeasurement
        rdf:type      rdf:Property ;
        rdfs:comment  "A suggested range of body measurements for the intended audience or person, for example inseam between 32 and 34 inches or height between 170 and 190 cm. Typically found on a size chart for wearable products." ;
        rdfs:label    "suggestedMeasurement" .

schema:UserDownloads  rdf:type  rdfs:Class ;
        rdfs:comment     "UserInteraction and its subtypes is an old way of talking about users interacting with pages. It is generally better to use [[Action]]-based vocabulary, alongside types such as [[Comment]]." ;
        rdfs:label       "UserDownloads" ;
        rdfs:subClassOf  schema:UserInteraction .

schema:dateSent  rdf:type  rdf:Property ;
        rdfs:comment  "The date/time at which the message was sent." ;
        rdfs:label    "dateSent" .

schema:SuperficialAnatomy
        rdf:type         rdfs:Class ;
        rdfs:comment     "Anatomical features that can be observed by sight (without dissection), including the form and proportions of the human body as well as surface landmarks that correspond to deeper subcutaneous structures. Superficial anatomy plays an important role in sports medicine, phlebotomy, and other medical specialties as underlying anatomical structures can be identified through surface palpation. For example, during back surgery, superficial anatomy can be used to palpate and count vertebrae to find the site of incision. Or in phlebotomy, superficial anatomy can be used to locate an underlying vein; for example, the median cubital vein can be located by palpating the borders of the cubital fossa (such as the epicondyles of the humerus) and then looking for the superficial signs of the vein, such as size, prominence, ability to refill after depression, and feel of surrounding tissue support. As another example, in a subluxation (dislocation) of the glenohumeral joint, the bony structure becomes pronounced with the deltoid muscle failing to cover the glenohumeral joint allowing the edges of the scapula to be superficially visible. Here, the superficial anatomy is the visible edges of the scapula, implying the underlying dislocation of the joint (the related anatomical structure)." ;
        rdfs:label       "SuperficialAnatomy" ;
        rdfs:subClassOf  schema:MedicalEntity .

schema:supplyTo  rdf:type  rdf:Property ;
        rdfs:comment  "The area to which the artery supplies blood." ;
        rdfs:label    "supplyTo" .

schema:game  rdf:type  rdf:Property ;
        rdfs:comment  "Video game which is played on this server." ;
        rdfs:label    "game" .

schema:MotorcycleDealer
        rdf:type         rdfs:Class ;
        rdfs:comment     "A motorcycle dealer." ;
        rdfs:label       "MotorcycleDealer" ;
        rdfs:subClassOf  schema:AutomotiveBusiness .

schema:providerMobility
        rdf:type      rdf:Property ;
        rdfs:comment  "Indicates the mobility of a provided service (e.g. 'static', 'dynamic')." ;
        rdfs:label    "providerMobility" .

schema:boardingPolicy
        rdf:type      rdf:Property ;
        rdfs:comment  "The type of boarding policy used by the airline (e.g. zone-based or group-based)." ;
        rdfs:label    "boardingPolicy" .

schema:variableMeasured
        rdf:type      rdf:Property ;
        rdfs:comment  "The variableMeasured property can indicate (repeated as necessary) the  variables that are measured in some dataset, either described as text or as pairs of identifier and description using PropertyValue." ;
        rdfs:label    "variableMeasured" .

schema:DonateAction  rdf:type  rdfs:Class ;
        rdfs:comment     "The act of providing goods, services, or money without compensation, often for philanthropic reasons." ;
        rdfs:label       "DonateAction" ;
        rdfs:subClassOf  schema:TradeAction .

schema:ProductCollection
        rdf:type         rdfs:Class ;
        rdfs:comment     "A set of products (either [[ProductGroup]]s or specific variants) that are listed together e.g. in an [[Offer]]." ;
        rdfs:label       "ProductCollection" ;
        rdfs:subClassOf  schema:Product , schema:Collection .

schema:ActionAccessSpecification
        rdf:type         rdfs:Class ;
        rdfs:comment     "A set of requirements that a must be fulfilled in order to perform an Action." ;
        rdfs:label       "ActionAccessSpecification" ;
        rdfs:subClassOf  schema:Intangible .

schema:labelDetails  rdf:type  rdf:Property ;
        rdfs:comment  "Link to the drug's label details." ;
        rdfs:label    "labelDetails" .

schema:tocContinuation
        rdf:type      rdf:Property ;
        rdfs:comment  "A [[HyperTocEntry]] can have a [[tocContinuation]] indicated, which is another [[HyperTocEntry]] that would be the default next item to play or render." ;
        rdfs:label    "tocContinuation" .

schema:OrganizationRole
        rdf:type         rdfs:Class ;
        rdfs:comment     "A subclass of Role used to describe roles within organizations." ;
        rdfs:label       "OrganizationRole" ;
        rdfs:subClassOf  schema:Role .

schema:BodyMeasurementTypeEnumeration
        rdf:type         rdfs:Class ;
        rdfs:comment     "Enumerates types (or dimensions) of a person's body measurements, for example for fitting of clothes." ;
        rdfs:label       "BodyMeasurementTypeEnumeration" ;
        rdfs:subClassOf  schema:MeasurementTypeEnumeration .

schema:SkiResort  rdf:type  rdfs:Class ;
        rdfs:comment     "A ski resort." ;
        rdfs:label       "SkiResort" ;
        rdfs:subClassOf  schema:SportsActivityLocation , schema:Resort .

schema:itinerary  rdf:type  rdf:Property ;
        rdfs:comment  "Destination(s) ( [[Place]] ) that make up a trip. For a trip where destination order is important use [[ItemList]] to specify that order (see examples)." ;
        rdfs:label    "itinerary" .

void:Dataset  rdf:type  rdfs:Class .

schema:interactionService
        rdf:type      rdf:Property ;
        rdfs:comment  "The WebSite or SoftwareApplication where the interactions took place." ;
        rdfs:label    "interactionService" .

schema:floorSize  rdf:type  rdf:Property ;
        rdfs:comment  "The size of the accommodation, e.g. in square meter or squarefoot.\nTypical unit code(s): MTK for square meter, FTK for square foot, or YDK for square yard " ;
        rdfs:label    "floorSize" .

schema:warning  rdf:type  rdf:Property ;
        rdfs:comment  "Any FDA or other warnings about the drug (text or URL)." ;
        rdfs:label    "warning" .

schema:Quiz  rdf:type    rdfs:Class ;
        rdfs:comment     "Quiz: A test of knowledge, skills and abilities." ;
        rdfs:label       "Quiz" ;
        rdfs:subClassOf  schema:LearningResource .

schema:DrugClass  rdf:type  rdfs:Class ;
        rdfs:comment     "A class of medical drugs, e.g., statins. Classes can represent general pharmacological class, common mechanisms of action, common physiological effects, etc." ;
        rdfs:label       "DrugClass" ;
        rdfs:subClassOf  schema:MedicalEntity .

schema:includedComposition
        rdf:type      rdf:Property ;
        rdfs:comment  "Smaller compositions included in this work (e.g. a movement in a symphony)." ;
        rdfs:label    "includedComposition" .

schema:costCategory  rdf:type  rdf:Property ;
        rdfs:comment  "The category of cost, such as wholesale, retail, reimbursement cap, etc." ;
        rdfs:label    "costCategory" .

schema:WPHeader  rdf:type  rdfs:Class ;
        rdfs:comment     "The header section of the page." ;
        rdfs:label       "WPHeader" ;
        rdfs:subClassOf  schema:WebPageElement .

schema:EmployerReview
        rdf:type         rdfs:Class ;
        rdfs:comment     "An [[EmployerReview]] is a review of an [[Organization]] regarding its role as an employer, written by a current or former employee of that organization." ;
        rdfs:label       "EmployerReview" ;
        rdfs:subClassOf  schema:Review .

schema:backstory  rdf:type  rdf:Property ;
        rdfs:comment  "For an [[Article]], typically a [[NewsArticle]], the backstory property provides a textual summary giving a brief explanation of why and how an article was created. In a journalistic setting this could include information about reporting process, methods, interviews, data sources, etc." ;
        rdfs:label    "backstory" .

schema:reservationId  rdf:type  rdf:Property ;
        rdfs:comment  "A unique identifier for the reservation." ;
        rdfs:label    "reservationId" .

schema:followee  rdf:type   rdf:Property ;
        rdfs:comment        "A sub property of object. The person or organization being followed." ;
        rdfs:label          "followee" ;
        rdfs:subPropertyOf  schema:object .

schema:copyrightHolder
        rdf:type      rdf:Property ;
        rdfs:comment  "The party holding the legal copyright to the CreativeWork." ;
        rdfs:label    "copyrightHolder" .

schema:targetCollection
        rdf:type            rdf:Property ;
        rdfs:comment        "A sub property of object. The collection target of the action." ;
        rdfs:label          "targetCollection" ;
        rdfs:subPropertyOf  schema:object .

schema:WorkersUnion  rdf:type  rdfs:Class ;
        rdfs:comment     "A Workers Union (also known as a Labor Union, Labour Union, or Trade Union) is an organization that promotes the interests of its worker members by collectively bargaining with management, organizing, and political lobbying." ;
        rdfs:label       "WorkersUnion" ;
        rdfs:subClassOf  schema:Organization .

schema:toLocation  rdf:type  rdf:Property ;
        rdfs:comment        "A sub property of location. The final location of the object or the agent after the action." ;
        rdfs:label          "toLocation" ;
        rdfs:subPropertyOf  schema:location .

schema:ItemPage  rdf:type  rdfs:Class ;
        rdfs:comment     "A page devoted to a single item, such as a particular product or hotel." ;
        rdfs:label       "ItemPage" ;
        rdfs:subClassOf  schema:WebPage .

schema:naics  rdf:type  rdf:Property ;
        rdfs:comment  "The North American Industry Classification System (NAICS) code for a particular organization or business person." ;
        rdfs:label    "naics" .

schema:partOfSystem  rdf:type  rdf:Property ;
        rdfs:comment  "The anatomical or organ system that this structure is part of." ;
        rdfs:label    "partOfSystem" .

schema:Notary  rdf:type  rdfs:Class ;
        rdfs:comment     "A notary." ;
        rdfs:label       "Notary" ;
        rdfs:subClassOf  schema:LegalService .

schema:birthPlace  rdf:type  rdf:Property ;
        rdfs:comment  "The place where the person was born." ;
        rdfs:label    "birthPlace" .

schema:returnFees  rdf:type  rdf:Property ;
        rdfs:comment  "Indicates (via enumerated options) the return fees policy for a MerchantReturnPolicy" ;
        rdfs:label    "returnFees" .

schema:estimatesRiskOf
        rdf:type      rdf:Property ;
        rdfs:comment  "The condition, complication, or symptom whose risk is being estimated." ;
        rdfs:label    "estimatesRiskOf" .

schema:depth  rdf:type  rdf:Property ;
        rdfs:comment  "The depth of the item." ;
        rdfs:label    "depth" .

schema:numAdults  rdf:type  rdf:Property ;
        rdfs:comment  "The number of adults staying in the unit." ;
        rdfs:label    "numAdults" .

schema:strengthValue  rdf:type  rdf:Property ;
        rdfs:comment  "The value of an active ingredient's strength, e.g. 325." ;
        rdfs:label    "strengthValue" .

schema:hasMap  rdf:type  rdf:Property ;
        rdfs:comment  "A URL to a map of the place." ;
        rdfs:label    "hasMap" .

schema:ratingExplanation
        rdf:type      rdf:Property ;
        rdfs:comment  "A short explanation (e.g. one to two sentences) providing background context and other information that led to the conclusion expressed in the rating. This is particularly applicable to ratings associated with \"fact check\" markup using [[ClaimReview]]." ;
        rdfs:label    "ratingExplanation" .

schema:eligibleRegion
        rdf:type            rdf:Property ;
        rdfs:comment        "The ISO 3166-1 (ISO 3166-1 alpha-2) or ISO 3166-2 code, the place, or the GeoShape for the geo-political region(s) for which the offer or delivery charge specification is valid.\\n\\nSee also [[ineligibleRegion]].\n    " ;
        rdfs:label          "eligibleRegion" ;
        rdfs:subPropertyOf  schema:areaServed .

schema:dietFeatures  rdf:type  rdf:Property ;
        rdfs:comment  "Nutritional information specific to the dietary plan. May include dietary recommendations on what foods to avoid, what foods to consume, and specific alterations/deviations from the USDA or other regulatory body's approved dietary guidelines." ;
        rdfs:label    "dietFeatures" .

schema:courseCode  rdf:type  rdf:Property ;
        rdfs:comment  "The identifier for the [[Course]] used by the course [[provider]] (e.g. CS101 or 6.001)." ;
        rdfs:label    "courseCode" .

schema:cvdNumC19OverflowPats
        rdf:type      rdf:Property ;
        rdfs:comment  "numc19overflowpats - ED/OVERFLOW: Patients with suspected or confirmed COVID-19 who are in the ED or any overflow location awaiting an inpatient bed." ;
        rdfs:label    "cvdNumC19OverflowPats" .

voc:ProductCategory  rdf:type  rdfs:Class ;
        rdfs:subClassOf  skos:Concept .

schema:rxcui  rdf:type  rdf:Property ;
        rdfs:comment  "The RxCUI drug identifier from RXNORM." ;
        rdfs:label    "rxcui" .

schema:Seat  rdf:type    rdfs:Class ;
        rdfs:comment     "Used to describe a seat, such as a reserved seat in an event reservation." ;
        rdfs:label       "Seat" ;
        rdfs:subClassOf  schema:Intangible .

schema:serviceUrl  rdf:type  rdf:Property ;
        rdfs:comment  "The website to access the service." ;
        rdfs:label    "serviceUrl" .

schema:percentile90  rdf:type  rdf:Property ;
        rdfs:comment  "The 90th percentile value." ;
        rdfs:label    "percentile90" .

schema:MedicalEvidenceLevel
        rdf:type         rdfs:Class ;
        rdfs:comment     "Level of evidence for a medical guideline. Enumerated type." ;
        rdfs:label       "MedicalEvidenceLevel" ;
        rdfs:subClassOf  schema:MedicalEnumeration .

schema:isAcceptingNewPatients
        rdf:type      rdf:Property ;
        rdfs:comment  "Whether the provider is accepting new patients." ;
        rdfs:label    "isAcceptingNewPatients" .

schema:ReplyAction  rdf:type  rdfs:Class ;
        rdfs:comment     "The act of responding to a question/message asked/sent by the object. Related to [[AskAction]]\\n\\nRelated actions:\\n\\n* [[AskAction]]: Appears generally as an origin of a ReplyAction." ;
        rdfs:label       "ReplyAction" ;
        rdfs:subClassOf  schema:CommunicateAction .

schema:CableOrSatelliteService
        rdf:type         rdfs:Class ;
        rdfs:comment     "A service which provides access to media programming like TV or radio. Access may be via cable or satellite." ;
        rdfs:label       "CableOrSatelliteService" ;
        rdfs:subClassOf  schema:Service .

schema:DaySpa  rdf:type  rdfs:Class ;
        rdfs:comment     "A day spa." ;
        rdfs:label       "DaySpa" ;
        rdfs:subClassOf  schema:HealthAndBeautyBusiness .

schema:GovernmentBenefitsType
        rdf:type         rdfs:Class ;
        rdfs:comment     "GovernmentBenefitsType enumerates several kinds of government benefits to support the COVID-19 situation. Note that this structure may not capture all benefits offered." ;
        rdfs:label       "GovernmentBenefitsType" ;
        rdfs:subClassOf  schema:Enumeration .

schema:CheckInAction  rdf:type  rdfs:Class ;
        rdfs:comment     "The act of an agent communicating (service provider, social media, etc) their arrival by registering/confirming for a previously reserved service (e.g. flight check in) or at a place (e.g. hotel), possibly resulting in a result (boarding pass, etc).\\n\\nRelated actions:\\n\\n* [[CheckOutAction]]: The antonym of CheckInAction.\\n* [[ArriveAction]]: Unlike ArriveAction, CheckInAction implies that the agent is informing/confirming the start of a previously reserved service.\\n* [[ConfirmAction]]: Unlike ConfirmAction, CheckInAction implies that the agent is informing/confirming the *start* of a previously reserved service rather than its validity/existence." ;
        rdfs:label       "CheckInAction" ;
        rdfs:subClassOf  schema:CommunicateAction .

schema:Taxi  rdf:type    rdfs:Class ;
        rdfs:comment     "A taxi." ;
        rdfs:label       "Taxi" ;
        rdfs:subClassOf  schema:Service .

schema:downvoteCount  rdf:type  rdf:Property ;
        rdfs:comment  "The number of downvotes this question, answer or comment has received from the community." ;
        rdfs:label    "downvoteCount" .

schema:menuAddOn  rdf:type  rdf:Property ;
        rdfs:comment  "Additional menu item(s) such as a side dish of salad or side order of fries that can be added to this menu item. Additionally it can be a menu section containing allowed add-on menu items for this menu item." ;
        rdfs:label    "menuAddOn" .

schema:relatedDrug  rdf:type  rdf:Property ;
        rdfs:comment  "Any other drug related to this one, for example commonly-prescribed alternatives." ;
        rdfs:label    "relatedDrug" .

schema:dateReceived  rdf:type  rdf:Property ;
        rdfs:comment  "The date/time the message was received if a single recipient exists." ;
        rdfs:label    "dateReceived" .

schema:partOfSeason  rdf:type  rdf:Property ;
        rdfs:comment        "The season to which this episode belongs." ;
        rdfs:label          "partOfSeason" ;
        rdfs:subPropertyOf  schema:isPartOf .

schema:offersPrescriptionByMail
        rdf:type      rdf:Property ;
        rdfs:comment  "Whether prescriptions can be delivered by mail." ;
        rdfs:label    "offersPrescriptionByMail" .

schema:LiveBlogPosting
        rdf:type         rdfs:Class ;
        rdfs:comment     "A blog post intended to provide a rolling textual coverage of an ongoing event through continuous updates." ;
        rdfs:label       "LiveBlogPosting" ;
        rdfs:subClassOf  schema:BlogPosting .

schema:object  rdf:type  rdf:Property ;
        rdfs:comment  "The object upon which the action is carried out, whose state is kept intact or changed. Also known as the semantic roles patient, affected or undergoer (which change their state) or theme (which doesn't). e.g. John read *a book*." ;
        rdfs:label    "object" .

schema:DiscoverAction
        rdf:type         rdfs:Class ;
        rdfs:comment     "The act of discovering/finding an object." ;
        rdfs:label       "DiscoverAction" ;
        rdfs:subClassOf  schema:FindAction .

schema:Play  rdf:type    rdfs:Class ;
        rdfs:comment     "A play is a form of literature, usually consisting of dialogue between characters, intended for theatrical performance rather than just reading. Note the peformance of a Play would be a [[TheaterEvent]] - the *Play* being the [[workPerformed]]." ;
        rdfs:label       "Play" ;
        rdfs:subClassOf  schema:CreativeWork .

schema:CampingPitch  rdf:type  rdfs:Class ;
        rdfs:comment     "A [[CampingPitch]] is an individual place for overnight stay in the outdoors, typically being part of a larger camping site, or [[Campground]].\\n\\n\nIn British English a campsite, or campground, is an area, usually divided into a number of pitches, where people can camp overnight using tents or camper vans or caravans; this British English use of the word is synonymous with the American English expression campground. In American English the term campsite generally means an area where an individual, family, group, or military unit can pitch a tent or park a camper; a campground may contain many campsites.\n(Source: Wikipedia see [https://en.wikipedia.org/wiki/Campsite](https://en.wikipedia.org/wiki/Campsite)).\\n\\n\nSee also the dedicated [document on the use of schema.org for marking up hotels and other forms of accommodations](/docs/hotels.html).\n" ;
        rdfs:label       "CampingPitch" ;
        rdfs:subClassOf  schema:Accommodation .

schema:healthPlanCopay
        rdf:type      rdf:Property ;
        rdfs:comment  "Whether The copay amount." ;
        rdfs:label    "healthPlanCopay" .

schema:conditionsOfAccess
        rdf:type      rdf:Property ;
        rdfs:comment  "Conditions that affect the availability of, or method(s) of access to, an item. Typically used for real world items such as an [[ArchiveComponent]] held by an [[ArchiveOrganization]]. This property is not suitable for use as a general Web access control mechanism. It is expressed only in natural language.\\n\\nFor example \"Available by appointment from the Reading Room\" or \"Accessible only from logged-in accounts \". " ;
        rdfs:label    "conditionsOfAccess" .

schema:arrivalGate  rdf:type  rdf:Property ;
        rdfs:comment  "Identifier of the flight's arrival gate." ;
        rdfs:label    "arrivalGate" .

schema:occupationLocation
        rdf:type      rdf:Property ;
        rdfs:comment  " The region/country for which this occupational description is appropriate. Note that educational requirements and qualifications can vary between jurisdictions." ;
        rdfs:label    "occupationLocation" .

schema:hasEnergyConsumptionDetails
        rdf:type      rdf:Property ;
        rdfs:comment  "Defines the energy efficiency Category (also known as \"class\" or \"rating\") for a product according to an international energy efficiency standard." ;
        rdfs:label    "hasEnergyConsumptionDetails" .

schema:salaryUponCompletion
        rdf:type      rdf:Property ;
        rdfs:comment  "The expected salary upon completing the training." ;
        rdfs:label    "salaryUponCompletion" .

schema:SportsTeam  rdf:type  rdfs:Class ;
        rdfs:comment     "Organization: Sports team." ;
        rdfs:label       "SportsTeam" ;
        rdfs:subClassOf  schema:SportsOrganization .

schema:amount  rdf:type  rdf:Property ;
        rdfs:comment  "The amount of money." ;
        rdfs:label    "amount" .

schema:ApprovedIndication
        rdf:type         rdfs:Class ;
        rdfs:comment     "An indication for a medical therapy that has been formally specified or approved by a regulatory body that regulates use of the therapy; for example, the US FDA approves indications for most drugs in the US." ;
        rdfs:label       "ApprovedIndication" ;
        rdfs:subClassOf  schema:MedicalIndication .

schema:reportNumber  rdf:type  rdf:Property ;
        rdfs:comment  "The number or other unique designator assigned to a Report by the publishing organization." ;
        rdfs:label    "reportNumber" .

schema:medicineSystem
        rdf:type      rdf:Property ;
        rdfs:comment  "The system of medicine that includes this MedicalEntity, for example 'evidence-based', 'homeopathic', 'chiropractic', etc." ;
        rdfs:label    "medicineSystem" .

schema:PaintAction  rdf:type  rdfs:Class ;
        rdfs:comment     "The act of producing a painting, typically with paint and canvas as instruments." ;
        rdfs:label       "PaintAction" ;
        rdfs:subClassOf  schema:CreateAction .

schema:CityHall  rdf:type  rdfs:Class ;
        rdfs:comment     "A city hall." ;
        rdfs:label       "CityHall" ;
        rdfs:subClassOf  schema:GovernmentBuilding .

skos:narrower  rdf:type     owl:ObjectProperty ;
        rdfs:comment        "Narrower concepts are typically rendered as children in a concept hierarchy (tree)."@en ;
        rdfs:label          "has narrower"@en ;
        rdfs:subPropertyOf  skos:narrowerTransitive ;
        owl:inverseOf       skos:broader .

schema:seatSection  rdf:type  rdf:Property ;
        rdfs:comment  "The section location of the reserved seat (e.g. Orchestra)." ;
        rdfs:label    "seatSection" .

skos:memberList  rdf:type  owl:ObjectProperty ;
        rdfs:comment  "For any resource, every item in the list given as the value of the\n      skos:memberList property is also a value of the skos:member property."@en ;
        rdfs:domain   skos:OrderedCollection ;
        rdfs:label    "has member list"@en ;
        rdfs:range    rdf:List .

schema:releaseDate  rdf:type  rdf:Property ;
        rdfs:comment  "The release date of a product or product model. This can be used to distinguish the exact variant of a product." ;
        rdfs:label    "releaseDate" .

schema:ComicStory  rdf:type  rdfs:Class ;
        rdfs:comment     "The term \"story\" is any indivisible, re-printable\n    \tunit of a comic, including the interior stories, covers, and backmatter. Most\n    \tcomics have at least two stories: a cover (ComicCoverArt) and an interior story." ;
        rdfs:label       "ComicStory" ;
        rdfs:subClassOf  schema:CreativeWork .

schema:EnergyStarEnergyEfficiencyEnumeration
        rdf:type         rdfs:Class ;
        rdfs:comment     "Used to indicate whether a product is EnergyStar certified." ;
        rdfs:label       "EnergyStarEnergyEfficiencyEnumeration" ;
        rdfs:subClassOf  schema:EnergyEfficiencyEnumeration .

schema:EventVenue  rdf:type  rdfs:Class ;
        rdfs:comment     "An event venue." ;
        rdfs:label       "EventVenue" ;
        rdfs:subClassOf  schema:CivicStructure .

schema:jobStartDate  rdf:type  rdf:Property ;
        rdfs:comment  "The date on which a successful applicant for this job would be expected to start work. Choose a specific date in the future or use the jobImmediateStart property to indicate the position is to be filled as soon as possible." ;
        rdfs:label    "jobStartDate" .

schema:isPartOf  rdf:type  rdf:Property ;
        rdfs:comment  "Indicates an item or CreativeWork that this item, or CreativeWork (in some sense), is part of." ;
        rdfs:label    "isPartOf" .

schema:DriveWheelConfigurationValue
        rdf:type         rdfs:Class ;
        rdfs:comment     "A value indicating which roadwheels will receive torque." ;
        rdfs:label       "DriveWheelConfigurationValue" ;
        rdfs:subClassOf  schema:QualitativeValue .

schema:accessMode  rdf:type  rdf:Property ;
        rdfs:comment  "The human sensory perceptual system or cognitive faculty through which a person may process or perceive information. Expected values include: auditory, tactile, textual, visual, colorDependent, chartOnVisual, chemOnVisual, diagramOnVisual, mathOnVisual, musicOnVisual, textOnVisual.\n      " ;
        rdfs:label    "accessMode" .

schema:EngineSpecification
        rdf:type         rdfs:Class ;
        rdfs:comment     "Information about the engine of the vehicle. A vehicle can have multiple engines represented by multiple engine specification entities." ;
        rdfs:label       "EngineSpecification" ;
        rdfs:subClassOf  schema:StructuredValue .

schema:nonProprietaryName
        rdf:type      rdf:Property ;
        rdfs:comment  "The generic name of this drug or supplement." ;
        rdfs:label    "nonProprietaryName" .

schema:weight  rdf:type  rdf:Property ;
        rdfs:comment  "The weight of the product or person." ;
        rdfs:label    "weight" .

schema:VirtualLocation
        rdf:type         rdfs:Class ;
        rdfs:comment     "An online or virtual location for attending events. For example, one may attend an online seminar or educational event. While a virtual location may be used as the location of an event, virtual locations should not be confused with physical locations in the real world." ;
        rdfs:label       "VirtualLocation" ;
        rdfs:subClassOf  schema:Intangible .

schema:knownVehicleDamages
        rdf:type      rdf:Property ;
        rdfs:comment  "A textual description of known damages, both repaired and unrepaired." ;
        rdfs:label    "knownVehicleDamages" .

schema:characterAttribute
        rdf:type      rdf:Property ;
        rdfs:comment  "A piece of data that represents a particular aspect of a fictional character (skill, power, character points, advantage, disadvantage)." ;
        rdfs:label    "characterAttribute" .

schema:estimatedCost  rdf:type  rdf:Property ;
        rdfs:comment  "The estimated cost of the supply or supplies consumed when performing instructions." ;
        rdfs:label    "estimatedCost" .

schema:legalName  rdf:type  rdf:Property ;
        rdfs:comment  "The official name of the organization, e.g. the registered company name." ;
        rdfs:label    "legalName" .

schema:HighSchool  rdf:type  rdfs:Class ;
        rdfs:comment     "A high school." ;
        rdfs:label       "HighSchool" ;
        rdfs:subClassOf  schema:EducationalOrganization .

schema:CategoryCodeSet
        rdf:type         rdfs:Class ;
        rdfs:comment     "A set of Category Code values." ;
        rdfs:label       "CategoryCodeSet" ;
        rdfs:subClassOf  schema:DefinedTermSet .

schema:deliveryMethod
        rdf:type            rdf:Property ;
        rdfs:comment        "A sub property of instrument. The method of delivery." ;
        rdfs:label          "deliveryMethod" ;
        rdfs:subPropertyOf  schema:instrument .

schema:PublicHealth  rdf:type  rdfs:Class ;
        rdfs:comment     "Branch of medicine that pertains to the health services to improve and protect community health, especially epidemiology, sanitation, immunization, and preventive medicine." ;
        rdfs:label       "PublicHealth" ;
        rdfs:subClassOf  schema:MedicalBusiness .

schema:infectiousAgentClass
        rdf:type      rdf:Property ;
        rdfs:comment  "The class of infectious agent (bacteria, prion, etc.) that causes the disease." ;
        rdfs:label    "infectiousAgentClass" .

schema:CancelAction  rdf:type  rdfs:Class ;
        rdfs:comment     "The act of asserting that a future event/action is no longer going to happen.\\n\\nRelated actions:\\n\\n* [[ConfirmAction]]: The antonym of CancelAction." ;
        rdfs:label       "CancelAction" ;
        rdfs:subClassOf  schema:PlanAction .

schema:audienceType  rdf:type  rdf:Property ;
        rdfs:comment  "The target group associated with a given audience (e.g. veterans, car owners, musicians, etc.)." ;
        rdfs:label    "audienceType" .

schema:MedicalStudyStatus
        rdf:type         rdfs:Class ;
        rdfs:comment     "The status of a medical study. Enumerated type." ;
        rdfs:label       "MedicalStudyStatus" ;
        rdfs:subClassOf  schema:MedicalEnumeration .

schema:citation  rdf:type  rdf:Property ;
        rdfs:comment  "A citation or reference to another creative work, such as another publication, web page, scholarly article, etc." ;
        rdfs:label    "citation" .

schema:hasMerchantReturnPolicy
        rdf:type      rdf:Property ;
        rdfs:comment  "Indicates a MerchantReturnPolicy that may be applicable." ;
        rdfs:label    "hasMerchantReturnPolicy" .

schema:primaryPrevention
        rdf:type      rdf:Property ;
        rdfs:comment  "A preventative therapy used to prevent an initial occurrence of the medical condition, such as vaccination." ;
        rdfs:label    "primaryPrevention" .

schema:PrimaryCare  rdf:type  rdfs:Class ;
        rdfs:comment     "The medical care by a physician, or other health-care professional, who is the patient's first contact with the health-care system and who may recommend a specialist if necessary." ;
        rdfs:label       "PrimaryCare" ;
        rdfs:subClassOf  schema:MedicalBusiness .

schema:ListenAction  rdf:type  rdfs:Class ;
        rdfs:comment     "The act of consuming audio content." ;
        rdfs:label       "ListenAction" ;
        rdfs:subClassOf  schema:ConsumeAction .

schema:servicePostalAddress
        rdf:type      rdf:Property ;
        rdfs:comment  "The address for accessing the service by mail." ;
        rdfs:label    "servicePostalAddress" .

schema:ClaimReview  rdf:type  rdfs:Class ;
        rdfs:comment     "A fact-checking review of claims made (or reported) in some creative work (referenced via itemReviewed)." ;
        rdfs:label       "ClaimReview" ;
        rdfs:subClassOf  schema:Review .

schema:MedicalConditionStage
        rdf:type         rdfs:Class ;
        rdfs:comment     "A stage of a medical condition, such as 'Stage IIIa'." ;
        rdfs:label       "MedicalConditionStage" ;
        rdfs:subClassOf  schema:MedicalIntangible .

schema:parentOrganization
        rdf:type      rdf:Property ;
        rdfs:comment  "The larger organization that this organization is a [[subOrganization]] of, if any." ;
        rdfs:label    "parentOrganization" .

schema:permittedUsage
        rdf:type      rdf:Property ;
        rdfs:comment  "Indications regarding the permitted usage of the accommodation." ;
        rdfs:label    "permittedUsage" .

schema:ServiceChannel
        rdf:type         rdfs:Class ;
        rdfs:comment     "A means for accessing a service, e.g. a government office location, web site, or phone number." ;
        rdfs:label       "ServiceChannel" ;
        rdfs:subClassOf  schema:Intangible .

schema:percentile10  rdf:type  rdf:Property ;
        rdfs:comment  "The 10th percentile value." ;
        rdfs:label    "percentile10" .

schema:endorsee  rdf:type   rdf:Property ;
        rdfs:comment        "A sub property of participant. The person/organization being supported." ;
        rdfs:label          "endorsee" ;
        rdfs:subPropertyOf  schema:participant .

schema:trainNumber  rdf:type  rdf:Property ;
        rdfs:comment  "The unique identifier for the train." ;
        rdfs:label    "trainNumber" .

schema:repeatFrequency
        rdf:type            rdf:Property ;
        rdfs:comment        "Defines the frequency at which [[Event]]s will occur according to a schedule [[Schedule]]. The intervals between\n      events should be defined as a [[Duration]] of time." ;
        rdfs:label          "repeatFrequency" ;
        rdfs:subPropertyOf  schema:frequency .

schema:weightTotal  rdf:type  rdf:Property ;
        rdfs:comment  "The permitted total weight of the loaded vehicle, including passengers and cargo and the weight of the empty vehicle.\\n\\nTypical unit code(s): KGM for kilogram, LBR for pound\\n\\n* Note 1: You can indicate additional information in the [[name]] of the [[QuantitativeValue]] node.\\n* Note 2: You may also link to a [[QualitativeValue]] node that provides additional information using [[valueReference]].\\n* Note 3: Note that you can use [[minValue]] and [[maxValue]] to indicate ranges." ;
        rdfs:label    "weightTotal" .

schema:remainingAttendeeCapacity
        rdf:type      rdf:Property ;
        rdfs:comment  "The number of attendee places for an event that remain unallocated." ;
        rdfs:label    "remainingAttendeeCapacity" .

schema:Canal  rdf:type   rdfs:Class ;
        rdfs:comment     "A canal, like the Panama Canal." ;
        rdfs:label       "Canal" ;
        rdfs:subClassOf  schema:BodyOfWater .

schema:PodcastSeries  rdf:type  rdfs:Class ;
        rdfs:comment     "A podcast is an episodic series of digital audio or video files which a user can download and listen to." ;
        rdfs:label       "PodcastSeries" ;
        rdfs:subClassOf  schema:CreativeWorkSeries .

schema:legislationDateVersion
        rdf:type      rdf:Property ;
        rdfs:comment  "The point-in-time at which the provided description of the legislation is valid (e.g. : when looking at the law on the 2016-04-07 (= dateVersion), I get the consolidation of 2015-04-12 of the \"National Insurance Contributions Act 2015\")" ;
        rdfs:label    "legislationDateVersion" .

schema:QualitativeValue
        rdf:type         rdfs:Class ;
        rdfs:comment     "A predefined value for a product characteristic, e.g. the power cord plug type 'US' or the garment sizes 'S', 'M', 'L', and 'XL'." ;
        rdfs:label       "QualitativeValue" ;
        rdfs:subClassOf  schema:Enumeration .

schema:applicationSuite
        rdf:type      rdf:Property ;
        rdfs:comment  "The name of the application suite to which the application belongs (e.g. Excel belongs to Office)." ;
        rdfs:label    "applicationSuite" .

schema:version  rdf:type  rdf:Property ;
        rdfs:comment  "The version of the CreativeWork embodied by a specified resource." ;
        rdfs:label    "version" .

schema:relatedStructure
        rdf:type      rdf:Property ;
        rdfs:comment  "Related anatomical structure(s) that are not part of the system but relate or connect to it, such as vascular bundles associated with an organ system." ;
        rdfs:label    "relatedStructure" .

schema:floorLimit  rdf:type  rdf:Property ;
        rdfs:comment  "A floor limit is the amount of money above which credit card transactions must be authorized." ;
        rdfs:label    "floorLimit" .

schema:MedicalCondition
        rdf:type         rdfs:Class ;
        rdfs:comment     "Any condition of the human body that affects the normal functioning of a person, whether physically or mentally. Includes diseases, injuries, disabilities, disorders, syndromes, etc." ;
        rdfs:label       "MedicalCondition" ;
        rdfs:subClassOf  schema:MedicalEntity .

schema:HowToSupply  rdf:type  rdfs:Class ;
        rdfs:comment     "A supply consumed when performing the instructions for how to achieve a result." ;
        rdfs:label       "HowToSupply" ;
        rdfs:subClassOf  schema:HowToItem .

schema:HealthPlanNetwork
        rdf:type         rdfs:Class ;
        rdfs:comment     "A US-style health insurance plan network. " ;
        rdfs:label       "HealthPlanNetwork" ;
        rdfs:subClassOf  schema:Intangible .

schema:Physiotherapy  rdf:type  rdfs:Class ;
        rdfs:comment     "The practice of treatment of disease, injury, or deformity by physical methods such as massage, heat treatment, and exercise rather than by drugs or surgery.." ;
        rdfs:label       "Physiotherapy" ;
        rdfs:subClassOf  schema:MedicalBusiness .

schema:Time  rdf:type  rdfs:Class ;
        rdfs:comment  "A point in time recurring on multiple days in the form hh:mm:ss[Z|(+|-)hh:mm] (see [XML schema for details](http://www.w3.org/TR/xmlschema-2/#time))." ;
        rdfs:label    "Time" .

schema:isBasedOnUrl  rdf:type  rdf:Property ;
        rdfs:comment  "A resource that was used in the creation of this resource. This term can be repeated for multiple sources. For example, http://example.com/great-multiplication-intro.html." ;
        rdfs:label    "isBasedOnUrl" .

schema:MoveAction  rdf:type  rdfs:Class ;
        rdfs:comment     "The act of an agent relocating to a place.\\n\\nRelated actions:\\n\\n* [[TransferAction]]: Unlike TransferAction, the subject of the move is a living Person or Organization rather than an inanimate object." ;
        rdfs:label       "MoveAction" ;
        rdfs:subClassOf  schema:Action .

schema:EventReservation
        rdf:type         rdfs:Class ;
        rdfs:comment     "A reservation for an event like a concert, sporting event, or lecture.\\n\\nNote: This type is for information about actual reservations, e.g. in confirmation emails or HTML pages with individual confirmations of reservations. For offers of tickets, use [[Offer]]." ;
        rdfs:label       "EventReservation" ;
        rdfs:subClassOf  schema:Reservation .

schema:House  rdf:type   rdfs:Class ;
        rdfs:comment     "A house is a building or structure that has the ability to be occupied for habitation by humans or other creatures (Source: Wikipedia, the free encyclopedia, see <a href=\"http://en.wikipedia.org/wiki/House\">http://en.wikipedia.org/wiki/House</a>)." ;
        rdfs:label       "House" ;
        rdfs:subClassOf  schema:Accommodation .

schema:sportsActivityLocation
        rdf:type            rdf:Property ;
        rdfs:comment        "A sub property of location. The sports activity location where this action occurred." ;
        rdfs:label          "sportsActivityLocation" ;
        rdfs:subPropertyOf  schema:location .

schema:SearchAction  rdf:type  rdfs:Class ;
        rdfs:comment     "The act of searching for an object.\\n\\nRelated actions:\\n\\n* [[FindAction]]: SearchAction generally leads to a FindAction, but not necessarily." ;
        rdfs:label       "SearchAction" ;
        rdfs:subClassOf  schema:Action .

schema:TravelAgency  rdf:type  rdfs:Class ;
        rdfs:comment     "A travel agency." ;
        rdfs:label       "TravelAgency" ;
        rdfs:subClassOf  schema:LocalBusiness .

schema:orderItemStatus
        rdf:type      rdf:Property ;
        rdfs:comment  "The current status of the order item." ;
        rdfs:label    "orderItemStatus" .

schema:netWorth  rdf:type  rdf:Property ;
        rdfs:comment  "The total financial value of the person as calculated by subtracting assets from liabilities." ;
        rdfs:label    "netWorth" .

schema:signOrSymptom  rdf:type  rdf:Property ;
        rdfs:comment  "A sign or symptom of this condition. Signs are objective or physically observable manifestations of the medical condition while symptoms are the subjective experience of the medical condition." ;
        rdfs:label    "signOrSymptom" .

schema:AccountingService
        rdf:type         rdfs:Class ;
        rdfs:comment     "Accountancy business.\\n\\nAs a [[LocalBusiness]] it can be described as a [[provider]] of one or more [[Service]]\\(s).\n      " ;
        rdfs:label       "AccountingService" ;
        rdfs:subClassOf  schema:FinancialService .

voc:reason  rdf:type  owl:ObjectProperty .

schema:serviceOperator
        rdf:type      rdf:Property ;
        rdfs:comment  "The operating organization, if different from the provider.  This enables the representation of services that are provided by an organization, but operated by another organization like a subcontractor." ;
        rdfs:label    "serviceOperator" .

schema:validFor  rdf:type  rdf:Property ;
        rdfs:comment  "The duration of validity of a permit or similar thing." ;
        rdfs:label    "validFor" .

schema:costCurrency  rdf:type  rdf:Property ;
        rdfs:comment  "The currency (in 3-letter of the drug cost. See: http://en.wikipedia.org/wiki/ISO_4217. " ;
        rdfs:label    "costCurrency" .

schema:partOfTrip  rdf:type  rdf:Property ;
        rdfs:comment  "Identifies that this [[Trip]] is a subTrip of another Trip.  For example Day 1, Day 2, etc. of a multi-day trip." ;
        rdfs:label    "partOfTrip" .

schema:slogan  rdf:type  rdf:Property ;
        rdfs:comment  "A slogan or motto associated with the item." ;
        rdfs:label    "slogan" .

schema:Review  rdf:type  rdfs:Class ;
        rdfs:comment     "A review of an item - for example, of a restaurant, movie, or store." ;
        rdfs:label       "Review" ;
        rdfs:subClassOf  schema:CreativeWork .

schema:SpreadsheetDigitalDocument
        rdf:type         rdfs:Class ;
        rdfs:comment     "A spreadsheet file." ;
        rdfs:label       "SpreadsheetDigitalDocument" ;
        rdfs:subClassOf  schema:DigitalDocument .

schema:albumReleaseType
        rdf:type      rdf:Property ;
        rdfs:comment  "The kind of release which this album is: single, EP or album." ;
        rdfs:label    "albumReleaseType" .

schema:calories  rdf:type  rdf:Property ;
        rdfs:comment  "The number of calories." ;
        rdfs:label    "calories" .

schema:Winery  rdf:type  rdfs:Class ;
        rdfs:comment     "A winery." ;
        rdfs:label       "Winery" ;
        rdfs:subClassOf  schema:FoodEstablishment .

schema:PlaceOfWorship
        rdf:type         rdfs:Class ;
        rdfs:comment     "Place of worship, such as a church, synagogue, or mosque." ;
        rdfs:label       "PlaceOfWorship" ;
        rdfs:subClassOf  schema:CivicStructure .

schema:distribution  rdf:type  rdf:Property ;
        rdfs:comment  "A downloadable form of this dataset, at a specific location, in a specific format." ;
        rdfs:label    "distribution" .

schema:alternateName  rdf:type  rdf:Property ;
        rdfs:comment  "An alias for the item." ;
        rdfs:label    "alternateName" .

schema:HVACBusiness  rdf:type  rdfs:Class ;
        rdfs:comment     "A business that provide Heating, Ventilation and Air Conditioning services." ;
        rdfs:label       "HVACBusiness" ;
        rdfs:subClassOf  schema:HomeAndConstructionBusiness .

schema:energyEfficiencyScaleMax
        rdf:type      rdf:Property ;
        rdfs:comment  "Specifies the most energy efficient class on the regulated EU energy consumption scale for the product category a product belongs to. For example, energy consumption for televisions placed on the market after January 1, 2020 is scaled from D to A+++." ;
        rdfs:label    "energyEfficiencyScaleMax" .

schema:hasMenuItem  rdf:type  rdf:Property ;
        rdfs:comment  "A food or drink item contained in a menu or menu section." ;
        rdfs:label    "hasMenuItem" .

schema:workFeatured  rdf:type  rdf:Property ;
        rdfs:comment  "A work featured in some event, e.g. exhibited in an ExhibitionEvent.\n       Specific subproperties are available for workPerformed (e.g. a play), or a workPresented (a Movie at a ScreeningEvent)." ;
        rdfs:label    "workFeatured" .

schema:TrainStation  rdf:type  rdfs:Class ;
        rdfs:comment     "A train station." ;
        rdfs:label       "TrainStation" ;
        rdfs:subClassOf  schema:CivicStructure .

schema:biomechnicalClass
        rdf:type      rdf:Property ;
        rdfs:comment  "The biomechanical properties of the bone." ;
        rdfs:label    "biomechnicalClass" .

schema:Property  rdf:type  rdfs:Class ;
        rdfs:comment     "A property, used to indicate attributes and relationships of some Thing; equivalent to rdf:Property." ;
        rdfs:label       "Property" ;
        rdfs:subClassOf  schema:Intangible .

schema:UserPageVisits
        rdf:type         rdfs:Class ;
        rdfs:comment     "UserInteraction and its subtypes is an old way of talking about users interacting with pages. It is generally better to use [[Action]]-based vocabulary, alongside types such as [[Comment]]." ;
        rdfs:label       "UserPageVisits" ;
        rdfs:subClassOf  schema:UserInteraction .

schema:howPerformed  rdf:type  rdf:Property ;
        rdfs:comment  "How the procedure is performed." ;
        rdfs:label    "howPerformed" .

schema:AdultEntertainment
        rdf:type         rdfs:Class ;
        rdfs:comment     "An adult entertainment establishment." ;
        rdfs:label       "AdultEntertainment" ;
        rdfs:subClassOf  schema:EntertainmentBusiness .

schema:priceCurrency  rdf:type  rdf:Property ;
        rdfs:comment  "The currency of the price, or a price component when attached to [[PriceSpecification]] and its subtypes.\\n\\nUse standard formats: [ISO 4217 currency format](http://en.wikipedia.org/wiki/ISO_4217) e.g. \"USD\"; [Ticker symbol](https://en.wikipedia.org/wiki/List_of_cryptocurrencies) for cryptocurrencies e.g. \"BTC\"; well known names for [Local Exchange Tradings Systems](https://en.wikipedia.org/wiki/Local_exchange_trading_system) (LETS) and other currency types e.g. \"Ithaca HOUR\"." ;
        rdfs:label    "priceCurrency" .

schema:Integer  rdf:type  rdfs:Class ;
        rdfs:comment     "Data type: Integer." ;
        rdfs:label       "Integer" ;
        rdfs:subClassOf  schema:Number .

schema:abridged  rdf:type  rdf:Property ;
        rdfs:comment  "Indicates whether the book is an abridged edition." ;
        rdfs:label    "abridged" .

schema:targetDescription
        rdf:type      rdf:Property ;
        rdfs:comment  "The description of a node in an established educational framework." ;
        rdfs:label    "targetDescription" .

schema:inPlaylist  rdf:type  rdf:Property ;
        rdfs:comment  "The playlist to which this recording belongs." ;
        rdfs:label    "inPlaylist" .

schema:InformAction  rdf:type  rdfs:Class ;
        rdfs:comment     "The act of notifying someone of information pertinent to them, with no expectation of a response." ;
        rdfs:label       "InformAction" ;
        rdfs:subClassOf  schema:CommunicateAction .

schema:replacer  rdf:type   rdf:Property ;
        rdfs:comment        "A sub property of object. The object that replaces." ;
        rdfs:label          "replacer" ;
        rdfs:subPropertyOf  schema:object .

schema:tracks  rdf:type  rdf:Property ;
        rdfs:comment  "A music recording (track)&#x2014;usually a single song." ;
        rdfs:label    "tracks" .

schema:NailSalon  rdf:type  rdfs:Class ;
        rdfs:comment     "A nail salon." ;
        rdfs:label       "NailSalon" ;
        rdfs:subClassOf  schema:HealthAndBeautyBusiness .

schema:recognizedBy  rdf:type  rdf:Property ;
        rdfs:comment  "An organization that acknowledges the validity, value or utility of a credential. Note: recognition may include a process of quality assurance or accreditation." ;
        rdfs:label    "recognizedBy" .

schema:item  rdf:type  rdf:Property ;
        rdfs:comment  "An entity represented by an entry in a list or data feed (e.g. an 'artist' in a list of 'artists')’." ;
        rdfs:label    "item" .

schema:OccupationalTherapy
        rdf:type         rdfs:Class ;
        rdfs:comment     "A treatment of people with physical, emotional, or social problems, using purposeful activity to help them overcome or learn to deal with their problems." ;
        rdfs:label       "OccupationalTherapy" ;
        rdfs:subClassOf  schema:MedicalTherapy .

schema:OwnershipInfo  rdf:type  rdfs:Class ;
        rdfs:comment     "A structured value providing information about when a certain organization or person owned a certain product." ;
        rdfs:label       "OwnershipInfo" ;
        rdfs:subClassOf  schema:StructuredValue .

schema:buyer  rdf:type      rdf:Property ;
        rdfs:comment        "A sub property of participant. The participant/person/organization that bought the object." ;
        rdfs:label          "buyer" ;
        rdfs:subPropertyOf  schema:participant .

schema:runtime  rdf:type  rdf:Property ;
        rdfs:comment  "Runtime platform or script interpreter dependencies (Example - Java v1, Python2.3, .Net Framework 3.0)." ;
        rdfs:label    "runtime" .

schema:query  rdf:type      rdf:Property ;
        rdfs:comment        "A sub property of instrument. The query used on this action." ;
        rdfs:label          "query" ;
        rdfs:subPropertyOf  schema:instrument .

schema:numberOfAccommodationUnits
        rdf:type      rdf:Property ;
        rdfs:comment  "Indicates the total (available plus unavailable) number of accommodation units in an [[ApartmentComplex]], or the number of accommodation units for a specific [[FloorPlan]] (within its specific [[ApartmentComplex]]). See also [[numberOfAvailableAccommodationUnits]]." ;
        rdfs:label    "numberOfAccommodationUnits" .

schema:encodesCreativeWork
        rdf:type      rdf:Property ;
        rdfs:comment  "The CreativeWork encoded by this media object." ;
        rdfs:label    "encodesCreativeWork" .

schema:gtin13  rdf:type     rdf:Property ;
        rdfs:comment        "The GTIN-13 code of the product, or the product to which the offer refers. This is equivalent to 13-digit ISBN codes and EAN UCC-13. Former 12-digit UPC codes can be converted into a GTIN-13 code by simply adding a preceding zero. See [GS1 GTIN Summary](http://www.gs1.org/barcodes/technical/idkeys/gtin) for more details." ;
        rdfs:label          "gtin13" ;
        rdfs:subPropertyOf  schema:identifier , schema:gtin .

schema:temporalCoverage
        rdf:type      rdf:Property ;
        rdfs:comment  "The temporalCoverage of a CreativeWork indicates the period that the content applies to, i.e. that it describes, either as a DateTime or as a textual string indicating a time period in [ISO 8601 time interval format](https://en.wikipedia.org/wiki/ISO_8601#Time_intervals). In\n      the case of a Dataset it will typically indicate the relevant time period in a precise notation (e.g. for a 2011 census dataset, the year 2011 would be written \"2011/2012\"). Other forms of content e.g. ScholarlyArticle, Book, TVSeries or TVEpisode may indicate their temporalCoverage in broader terms - textually or via well-known URL.\n      Written works such as books may sometimes have precise temporal coverage too, e.g. a work set in 1939 - 1945 can be indicated in ISO 8601 interval format format via \"1939/1945\".\n\nOpen-ended date ranges can be written with \"..\" in place of the end date. For example, \"2015-11/..\" indicates a range beginning in November 2015 and with no specified final date. This is tentative and might be updated in future when ISO 8601 is officially updated." ;
        rdfs:label    "temporalCoverage" .

schema:applicationContact
        rdf:type      rdf:Property ;
        rdfs:comment  "Contact details for further information relevant to this job posting." ;
        rdfs:label    "applicationContact" .

schema:median  rdf:type  rdf:Property ;
        rdfs:comment  "The median value." ;
        rdfs:label    "median" .

schema:3DModel  rdf:type  rdfs:Class ;
        rdfs:comment     "A 3D model represents some kind of 3D content, which may have [[encoding]]s in one or more [[MediaObject]]s. Many 3D formats are available (e.g. see [Wikipedia](https://en.wikipedia.org/wiki/Category:3D_graphics_file_formats)); specific encoding formats can be represented using the [[encodingFormat]] property applied to the relevant [[MediaObject]]. For the\ncase of a single file published after Zip compression, the convention of appending '+zip' to the [[encodingFormat]] can be used. Geospatial, AR/VR, artistic/animation, gaming, engineering and scientific content can all be represented using [[3DModel]]." ;
        rdfs:label       "3DModel" ;
        rdfs:subClassOf  schema:MediaObject .

schema:steeringPosition
        rdf:type      rdf:Property ;
        rdfs:comment  "The position of the steering wheel or similar device (mostly for cars)." ;
        rdfs:label    "steeringPosition" .

schema:postalCode  rdf:type  rdf:Property ;
        rdfs:comment  "The postal code. For example, 94043." ;
        rdfs:label    "postalCode" .

schema:healthPlanDrugOption
        rdf:type      rdf:Property ;
        rdfs:comment  "TODO." ;
        rdfs:label    "healthPlanDrugOption" .

schema:AnalysisNewsArticle
        rdf:type         rdfs:Class ;
        rdfs:comment     "An AnalysisNewsArticle is a [[NewsArticle]] that, while based on factual reporting, incorporates the expertise of the author/producer, offering interpretations and conclusions." ;
        rdfs:label       "AnalysisNewsArticle" ;
        rdfs:subClassOf  schema:NewsArticle .

schema:requiredMaxAge
        rdf:type      rdf:Property ;
        rdfs:comment  "Audiences defined by a person's maximum age." ;
        rdfs:label    "requiredMaxAge" .

schema:MedicalGuidelineContraindication
        rdf:type         rdfs:Class ;
        rdfs:comment     "A guideline contraindication that designates a process as harmful and where quality of the data supporting the contraindication is sound." ;
        rdfs:label       "MedicalGuidelineContraindication" ;
        rdfs:subClassOf  schema:MedicalGuideline .

schema:activityDuration
        rdf:type      rdf:Property ;
        rdfs:comment  "Length of time to engage in the activity." ;
        rdfs:label    "activityDuration" .

schema:hasOccupation  rdf:type  rdf:Property ;
        rdfs:comment  "The Person's occupation. For past professions, use Role for expressing dates." ;
        rdfs:label    "hasOccupation" .

schema:videoFormat  rdf:type  rdf:Property ;
        rdfs:comment  "The type of screening or video broadcast used (e.g. IMAX, 3D, SD, HD, etc.)." ;
        rdfs:label    "videoFormat" .

schema:dateVehicleFirstRegistered
        rdf:type      rdf:Property ;
        rdfs:comment  "The date of the first registration of the vehicle with the respective public authorities." ;
        rdfs:label    "dateVehicleFirstRegistered" .

schema:broadcaster  rdf:type  rdf:Property ;
        rdfs:comment  "The organization owning or operating the broadcast service." ;
        rdfs:label    "broadcaster" .

schema:members  rdf:type  rdf:Property ;
        rdfs:comment  "A member of this organization." ;
        rdfs:label    "members" .

schema:addressLocality
        rdf:type      rdf:Property ;
        rdfs:comment  "The locality in which the street address is, and which is in the region. For example, Mountain View." ;
        rdfs:label    "addressLocality" .

schema:reservationStatus
        rdf:type      rdf:Property ;
        rdfs:comment  "The current status of the reservation." ;
        rdfs:label    "reservationStatus" .

schema:license  rdf:type  rdf:Property ;
        rdfs:comment  "A license document that applies to this content, typically indicated by URL." ;
        rdfs:label    "license" .

schema:bed  rdf:type  rdf:Property ;
        rdfs:comment  "The type of bed or beds included in the accommodation. For the single case of just one bed of a certain type, you use bed directly with a text.\n      If you want to indicate the quantity of a certain kind of bed, use an instance of BedDetails. For more detailed information, use the amenityFeature property." ;
        rdfs:label    "bed" .

schema:Audiobook  rdf:type  rdfs:Class ;
        rdfs:comment     "An audiobook." ;
        rdfs:label       "Audiobook" ;
        rdfs:subClassOf  schema:Book , schema:AudioObject .

schema:recipeInstructions
        rdf:type            rdf:Property ;
        rdfs:comment        "A step in making the recipe, in the form of a single item (document, video, etc.) or an ordered list with HowToStep and/or HowToSection items." ;
        rdfs:label          "recipeInstructions" ;
        rdfs:subPropertyOf  schema:step .

schema:replyToUrl  rdf:type  rdf:Property ;
        rdfs:comment  "The URL at which a reply may be posted to the specified UserComment." ;
        rdfs:label    "replyToUrl" .

schema:additionalType
        rdf:type            rdf:Property ;
        rdfs:comment        "An additional type for the item, typically used for adding more specific types from external vocabularies in microdata syntax. This is a relationship between something and a class that the thing is in. In RDFa syntax, it is better to use the native RDFa syntax - the 'typeof' attribute - for multiple types. Schema.org tools may have only weaker understanding of extra types, in particular those defined externally." ;
        rdfs:label          "additionalType" ;
        rdfs:subPropertyOf  rdf:type .

schema:OrderAction  rdf:type  rdfs:Class ;
        rdfs:comment     "An agent orders an object/product/service to be delivered/sent." ;
        rdfs:label       "OrderAction" ;
        rdfs:subClassOf  schema:TradeAction .

schema:skills  rdf:type  rdf:Property ;
        rdfs:comment  "A statement of knowledge, skill, ability, task or any other assertion expressing a competency that is desired or required to fulfill this role or to work in this occupation." ;
        rdfs:label    "skills" .

schema:newsUpdatesAndGuidelines
        rdf:type      rdf:Property ;
        rdfs:comment  "Indicates a page with news updates and guidelines. This could often be (but is not required to be) the main page containing [[SpecialAnnouncement]] markup on a site." ;
        rdfs:label    "newsUpdatesAndGuidelines" .

schema:WorkBasedProgram
        rdf:type         rdfs:Class ;
        rdfs:comment     "A program with both an educational and employment component. Typically based at a workplace and structured around work-based learning, with the aim of instilling competencies related to an occupation. WorkBasedProgram is used to distinguish programs such as apprenticeships from school, college or other classroom based educational programs." ;
        rdfs:label       "WorkBasedProgram" ;
        rdfs:subClassOf  schema:EducationalOccupationalProgram .

schema:OfferForLease  rdf:type  rdfs:Class ;
        rdfs:comment     "An [[OfferForLease]] in Schema.org represents an [[Offer]] to lease out something, i.e. an [[Offer]] whose\n  [[businessFunction]] is [lease out](http://purl.org/goodrelations/v1#LeaseOut.). See [Good Relations](https://en.wikipedia.org/wiki/GoodRelations) for\n  background on the underlying concepts.\n  " ;
        rdfs:label       "OfferForLease" ;
        rdfs:subClassOf  schema:Offer .

schema:ScheduleAction
        rdf:type         rdfs:Class ;
        rdfs:comment     "Scheduling future actions, events, or tasks.\\n\\nRelated actions:\\n\\n* [[ReserveAction]]: Unlike ReserveAction, ScheduleAction allocates future actions (e.g. an event, a task, etc) towards a time slot / spatial allocation." ;
        rdfs:label       "ScheduleAction" ;
        rdfs:subClassOf  schema:PlanAction .

schema:boardingGroup  rdf:type  rdf:Property ;
        rdfs:comment  "The airline-specific indicator of boarding order / preference." ;
        rdfs:label    "boardingGroup" .

schema:energyEfficiencyScaleMin
        rdf:type      rdf:Property ;
        rdfs:comment  "Specifies the least energy efficient class on the regulated EU energy consumption scale for the product category a product belongs to. For example, energy consumption for televisions placed on the market after January 1, 2020 is scaled from D to A+++." ;
        rdfs:label    "energyEfficiencyScaleMin" .

schema:AnatomicalSystem
        rdf:type         rdfs:Class ;
        rdfs:comment     "An anatomical system is a group of anatomical structures that work together to perform a certain task. Anatomical systems, such as organ systems, are one organizing principle of anatomy, and can includes circulatory, digestive, endocrine, integumentary, immune, lymphatic, muscular, nervous, reproductive, respiratory, skeletal, urinary, vestibular, and other systems." ;
        rdfs:label       "AnatomicalSystem" ;
        rdfs:subClassOf  schema:MedicalEntity .

schema:assembly  rdf:type  rdf:Property ;
        rdfs:comment  "Library file name e.g., mscorlib.dll, system.web.dll." ;
        rdfs:label    "assembly" .

schema:TipAction  rdf:type  rdfs:Class ;
        rdfs:comment     "The act of giving money voluntarily to a beneficiary in recognition of services rendered." ;
        rdfs:label       "TipAction" ;
        rdfs:subClassOf  schema:TradeAction .

schema:MusicRecording
        rdf:type         rdfs:Class ;
        rdfs:comment     "A music recording (track), usually a single song." ;
        rdfs:label       "MusicRecording" ;
        rdfs:subClassOf  schema:CreativeWork .

schema:BeautySalon  rdf:type  rdfs:Class ;
        rdfs:comment     "Beauty salon." ;
        rdfs:label       "BeautySalon" ;
        rdfs:subClassOf  schema:HealthAndBeautyBusiness .

schema:hasCourseInstance
        rdf:type      rdf:Property ;
        rdfs:comment  "An offering of the course at a specific time and place or through specific media or mode of study or to a specific section of students." ;
        rdfs:label    "hasCourseInstance" .

schema:issuedBy  rdf:type  rdf:Property ;
        rdfs:comment  "The organization issuing the ticket or permit." ;
        rdfs:label    "issuedBy" .

schema:dataset  rdf:type  rdf:Property ;
        rdfs:comment  "A dataset contained in this catalog." ;
        rdfs:label    "dataset" .

schema:SatiricalArticle
        rdf:type         rdfs:Class ;
        rdfs:comment     "An [[Article]] whose content is primarily [[satirical]](https://en.wikipedia.org/wiki/Satire) in nature, i.e. unlikely to be literally true. A satirical article is sometimes but not necessarily also a [[NewsArticle]]. [[ScholarlyArticle]]s are also sometimes satirized." ;
        rdfs:label       "SatiricalArticle" ;
        rdfs:subClassOf  schema:Article .

schema:structuralClass
        rdf:type      rdf:Property ;
        rdfs:comment  "The name given to how bone physically connects to each other." ;
        rdfs:label    "structuralClass" .

schema:AutoDealer  rdf:type  rdfs:Class ;
        rdfs:comment     "An car dealership." ;
        rdfs:label       "AutoDealer" ;
        rdfs:subClassOf  schema:AutomotiveBusiness .

schema:medicalSpecialty
        rdf:type      rdf:Property ;
        rdfs:comment  "A medical specialty of the provider." ;
        rdfs:label    "medicalSpecialty" .

schema:MovieRentalStore
        rdf:type         rdfs:Class ;
        rdfs:comment     "A movie rental store." ;
        rdfs:label       "MovieRentalStore" ;
        rdfs:subClassOf  schema:Store .

schema:regionDrained  rdf:type  rdf:Property ;
        rdfs:comment  "The anatomical or organ system drained by this vessel; generally refers to a specific part of an organ." ;
        rdfs:label    "regionDrained" .

schema:postalCodeEnd  rdf:type  rdf:Property ;
        rdfs:comment  "Last postal code in the range (included). Needs to be after [[postalCodeBegin]]." ;
        rdfs:label    "postalCodeEnd" .

schema:teaches  rdf:type  rdf:Property ;
        rdfs:comment  "The item being described is intended to help a person learn the competency or learning outcome defined by the referenced term." ;
        rdfs:label    "teaches" .

schema:geo  rdf:type  rdf:Property ;
        rdfs:comment  "The geo coordinates of the place." ;
        rdfs:label    "geo" .

schema:PerformingGroup
        rdf:type         rdfs:Class ;
        rdfs:comment     "A performance group, such as a band, an orchestra, or a circus." ;
        rdfs:label       "PerformingGroup" ;
        rdfs:subClassOf  schema:Organization .

schema:SelfStorage  rdf:type  rdfs:Class ;
        rdfs:comment     "A self-storage facility." ;
        rdfs:label       "SelfStorage" ;
        rdfs:subClassOf  schema:LocalBusiness .

schema:SellAction  rdf:type  rdfs:Class ;
        rdfs:comment     "The act of taking money from a buyer in exchange for goods or services rendered. An agent sells an object, product, or service to a buyer for a price. Reciprocal of BuyAction." ;
        rdfs:label       "SellAction" ;
        rdfs:subClassOf  schema:TradeAction .

schema:tissueSample  rdf:type  rdf:Property ;
        rdfs:comment  "The type of tissue sample required for the test." ;
        rdfs:label    "tissueSample" .

schema:datasetTimeInterval
        rdf:type      rdf:Property ;
        rdfs:comment  "The range of temporal applicability of a dataset, e.g. for a 2011 census dataset, the year 2011 (in ISO 8601 time interval format)." ;
        rdfs:label    "datasetTimeInterval" .

schema:hasOfferCatalog
        rdf:type      rdf:Property ;
        rdfs:comment  "Indicates an OfferCatalog listing for this Organization, Person, or Service." ;
        rdfs:label    "hasOfferCatalog" .

schema:Locksmith  rdf:type  rdfs:Class ;
        rdfs:comment     "A locksmith." ;
        rdfs:label       "Locksmith" ;
        rdfs:subClassOf  schema:HomeAndConstructionBusiness .

schema:pregnancyCategory
        rdf:type      rdf:Property ;
        rdfs:comment  "Pregnancy category of this drug." ;
        rdfs:label    "pregnancyCategory" .

schema:Language  rdf:type  rdfs:Class ;
        rdfs:comment     "Natural languages such as Spanish, Tamil, Hindi, English, etc. Formal language code tags expressed in [BCP 47](https://en.wikipedia.org/wiki/IETF_language_tag) can be used via the [[alternateName]] property. The Language type previously also covered programming languages such as Scheme and Lisp, which are now best represented using [[ComputerLanguage]]." ;
        rdfs:label       "Language" ;
        rdfs:subClassOf  schema:Intangible .

schema:resultComment  rdf:type  rdf:Property ;
        rdfs:comment        "A sub property of result. The Comment created or sent as a result of this action." ;
        rdfs:label          "resultComment" ;
        rdfs:subPropertyOf  schema:result .

schema:FastFoodRestaurant
        rdf:type         rdfs:Class ;
        rdfs:comment     "A fast-food restaurant." ;
        rdfs:label       "FastFoodRestaurant" ;
        rdfs:subClassOf  schema:FoodEstablishment .

schema:incentives  rdf:type  rdf:Property ;
        rdfs:comment  "Description of bonus and commission compensation aspects of the job." ;
        rdfs:label    "incentives" .

schema:benefits  rdf:type  rdf:Property ;
        rdfs:comment  "Description of benefits associated with the job." ;
        rdfs:label    "benefits" .

schema:vehicleSeatingCapacity
        rdf:type      rdf:Property ;
        rdfs:comment  "The number of passengers that can be seated in the vehicle, both in terms of the physical space available, and in terms of limitations set by law.\\n\\nTypical unit code(s): C62 for persons." ;
        rdfs:label    "vehicleSeatingCapacity" .

schema:thumbnailUrl  rdf:type  rdf:Property ;
        rdfs:comment  "A thumbnail image relevant to the Thing." ;
        rdfs:label    "thumbnailUrl" .

schema:Event  rdf:type   rdfs:Class ;
        rdfs:comment     "An event happening at a certain time and location, such as a concert, lecture, or festival. Ticketing information may be added via the [[offers]] property. Repeated events may be structured as separate Event objects." ;
        rdfs:label       "Event" ;
        rdfs:subClassOf  schema:Thing .

schema:releaseNotes  rdf:type  rdf:Property ;
        rdfs:comment  "Description of what changed in this version." ;
        rdfs:label    "releaseNotes" .

schema:annualPercentageRate
        rdf:type      rdf:Property ;
        rdfs:comment  "The annual rate that is charged for borrowing (or made by investing), expressed as a single percentage number that represents the actual yearly cost of funds over the term of a loan. This includes any fees or additional costs associated with the transaction." ;
        rdfs:label    "annualPercentageRate" .

skos:Concept  rdf:type  rdfs:Class ;
        rdfs:label  "Concept"@en .

schema:IndividualProduct
        rdf:type         rdfs:Class ;
        rdfs:comment     "A single, identifiable product instance (e.g. a laptop with a particular serial number)." ;
        rdfs:label       "IndividualProduct" ;
        rdfs:subClassOf  schema:Product .

schema:gracePeriod  rdf:type  rdf:Property ;
        rdfs:comment  "The period of time after any due date that the borrower has to fulfil its obligations before a default (failure to pay) is deemed to have occurred." ;
        rdfs:label    "gracePeriod" .

schema:UserLikes  rdf:type  rdfs:Class ;
        rdfs:comment     "UserInteraction and its subtypes is an old way of talking about users interacting with pages. It is generally better to use [[Action]]-based vocabulary, alongside types such as [[Comment]]." ;
        rdfs:label       "UserLikes" ;
        rdfs:subClassOf  schema:UserInteraction .

schema:expectsAcceptanceOf
        rdf:type      rdf:Property ;
        rdfs:comment  "An Offer which must be accepted before the user can perform the Action. For example, the user may need to buy a movie before being able to watch it." ;
        rdfs:label    "expectsAcceptanceOf" .

schema:valuePattern  rdf:type  rdf:Property ;
        rdfs:comment  "Specifies a regular expression for testing literal values according to the HTML spec." ;
        rdfs:label    "valuePattern" .

schema:performerIn  rdf:type  rdf:Property ;
        rdfs:comment  "Event that this person is a performer or participant in." ;
        rdfs:label    "performerIn" .

schema:priceRange  rdf:type  rdf:Property ;
        rdfs:comment  "The price range of the business, for example ```$$$```." ;
        rdfs:label    "priceRange" .

schema:ShippingRateSettings
        rdf:type         rdfs:Class ;
        rdfs:comment     "A ShippingRateSettings represents re-usable pieces of shipping information. It is designed for publication on an URL that may be referenced via the [[shippingSettingsLink]] property of an [[OfferShippingDetails]]. Several occurrences can be published, distinguished and matched (i.e. identified/referenced) by their different values for [[shippingLabel]]." ;
        rdfs:label       "ShippingRateSettings" ;
        rdfs:subClassOf  schema:StructuredValue .

schema:WebApplication
        rdf:type         rdfs:Class ;
        rdfs:comment     "Web applications." ;
        rdfs:label       "WebApplication" ;
        rdfs:subClassOf  schema:SoftwareApplication .

schema:VideoObject  rdf:type  rdfs:Class ;
        rdfs:comment     "A video file." ;
        rdfs:label       "VideoObject" ;
        rdfs:subClassOf  schema:MediaObject .

schema:programmingLanguage
        rdf:type      rdf:Property ;
        rdfs:comment  "The computer programming language." ;
        rdfs:label    "programmingLanguage" .

schema:qualifications
        rdf:type      rdf:Property ;
        rdfs:comment  "Specific qualifications required for this role or Occupation." ;
        rdfs:label    "qualifications" .

schema:BankAccount  rdf:type  rdfs:Class ;
        rdfs:comment     "A product or service offered by a bank whereby one may deposit, withdraw or transfer money and in some cases be paid interest." ;
        rdfs:label       "BankAccount" ;
        rdfs:subClassOf  schema:FinancialProduct .

schema:postOfficeBoxNumber
        rdf:type      rdf:Property ;
        rdfs:comment  "The post office box number for PO box addresses." ;
        rdfs:label    "postOfficeBoxNumber" .

schema:Florist  rdf:type  rdfs:Class ;
        rdfs:comment     "A florist." ;
        rdfs:label       "Florist" ;
        rdfs:subClassOf  schema:Store .

schema:currentExchangeRate
        rdf:type      rdf:Property ;
        rdfs:comment  "The current price of a currency." ;
        rdfs:label    "currentExchangeRate" .

schema:flightDistance
        rdf:type      rdf:Property ;
        rdfs:comment  "The distance of the flight." ;
        rdfs:label    "flightDistance" .

schema:DigitalDocumentPermissionType
        rdf:type         rdfs:Class ;
        rdfs:comment     "A type of permission which can be granted for accessing a digital document." ;
        rdfs:label       "DigitalDocumentPermissionType" ;
        rdfs:subClassOf  schema:Enumeration .

schema:discountCode  rdf:type  rdf:Property ;
        rdfs:comment  "Code used to redeem a discount." ;
        rdfs:label    "discountCode" .

schema:quarantineGuidelines
        rdf:type      rdf:Property ;
        rdfs:comment  "Guidelines about quarantine rules, e.g. in the context of a pandemic." ;
        rdfs:label    "quarantineGuidelines" .

schema:archiveHeld  rdf:type  rdf:Property ;
        rdfs:comment  "Collection, [fonds](https://en.wikipedia.org/wiki/Fonds), or item held, kept or maintained by an [[ArchiveOrganization]]."@en ;
        rdfs:label    "archiveHeld"@en .

schema:openingHoursSpecification
        rdf:type      rdf:Property ;
        rdfs:comment  "The opening hours of a certain place." ;
        rdfs:label    "openingHoursSpecification" .

schema:BedAndBreakfast
        rdf:type         rdfs:Class ;
        rdfs:comment     "Bed and breakfast.\n<br /><br />\nSee also the <a href=\"/docs/hotels.html\">dedicated document on the use of schema.org for marking up hotels and other forms of accommodations</a>.\n" ;
        rdfs:label       "BedAndBreakfast" ;
        rdfs:subClassOf  schema:LodgingBusiness .

schema:encodingFormat
        rdf:type      rdf:Property ;
        rdfs:comment  "Media type typically expressed using a MIME format (see [IANA site](http://www.iana.org/assignments/media-types/media-types.xhtml) and [MDN reference](https://developer.mozilla.org/en-US/docs/Web/HTTP/Basics_of_HTTP/MIME_types)) e.g. application/zip for a SoftwareApplication binary, audio/mpeg for .mp3 etc.).\n\nIn cases where a [[CreativeWork]] has several media type representations, [[encoding]] can be used to indicate each [[MediaObject]] alongside particular [[encodingFormat]] information.\n\nUnregistered or niche encoding and file formats can be indicated instead via the most appropriate URL, e.g. defining Web page or a Wikipedia/Wikidata entry." ;
        rdfs:label    "encodingFormat" .

schema:numberOfPreviousOwners
        rdf:type      rdf:Property ;
        rdfs:comment  "The number of owners of the vehicle, including the current one.\\n\\nTypical unit code(s): C62" ;
        rdfs:label    "numberOfPreviousOwners" .

schema:ArriveAction  rdf:type  rdfs:Class ;
        rdfs:comment     "The act of arriving at a place. An agent arrives at a destination from a fromLocation, optionally with participants." ;
        rdfs:label       "ArriveAction" ;
        rdfs:subClassOf  schema:MoveAction .

schema:Continent  rdf:type  rdfs:Class ;
        rdfs:comment     "One of the continents (for example, Europe or Africa)." ;
        rdfs:label       "Continent" ;
        rdfs:subClassOf  schema:Landform .

schema:wheelbase  rdf:type  rdf:Property ;
        rdfs:comment  "The distance between the centers of the front and rear wheels.\\n\\nTypical unit code(s): CMT for centimeters, MTR for meters, INH for inches, FOT for foot/feet" ;
        rdfs:label    "wheelbase" .

schema:GovernmentOffice
        rdf:type         rdfs:Class ;
        rdfs:comment     "A government office&#x2014;for example, an IRS or DMV office." ;
        rdfs:label       "GovernmentOffice" ;
        rdfs:subClassOf  schema:LocalBusiness .

schema:Class  rdf:type   rdfs:Class ;
        rdfs:comment     "A class, also often called a 'Type'; equivalent to rdfs:Class." ;
        rdfs:label       "Class" ;
        rdfs:subClassOf  schema:Intangible .

schema:source  rdf:type  rdf:Property .

schema:address  rdf:type  rdf:Property ;
        rdfs:comment  "Physical address of the item." ;
        rdfs:label    "address" .

schema:CreativeWorkSeries
        rdf:type         rdfs:Class ;
        rdfs:comment     "A CreativeWorkSeries in schema.org is a group of related items, typically but not necessarily of the same kind. CreativeWorkSeries are usually organized into some order, often chronological. Unlike [[ItemList]] which is a general purpose data structure for lists of things, the emphasis with CreativeWorkSeries is on published materials (written e.g. books and periodicals, or media such as tv, radio and games).\\n\\nSpecific subtypes are available for describing [[TVSeries]], [[RadioSeries]], [[MovieSeries]], [[BookSeries]], [[Periodical]] and [[VideoGameSeries]]. In each case, the [[hasPart]] / [[isPartOf]] properties can be used to relate the CreativeWorkSeries to its parts. The general CreativeWorkSeries type serves largely just to organize these more specific and practical subtypes.\\n\\nIt is common for properties applicable to an item from the series to be usefully applied to the containing group. Schema.org attempts to anticipate some of these cases, but publishers should be free to apply properties of the series parts to the series as a whole wherever they seem appropriate.\n\t  " ;
        rdfs:label       "CreativeWorkSeries" ;
        rdfs:subClassOf  schema:Series , schema:CreativeWork .

schema:vendor  rdf:type     rdf:Property ;
        rdfs:comment        "'vendor' is an earlier term for 'seller'." ;
        rdfs:label          "vendor" ;
        rdfs:subPropertyOf  schema:participant .

schema:evidenceOrigin
        rdf:type      rdf:Property ;
        rdfs:comment  "Source of the data used to formulate the guidance, e.g. RCT, consensus opinion, etc." ;
        rdfs:label    "evidenceOrigin" .

schema:broadcastTimezone
        rdf:type      rdf:Property ;
        rdfs:comment  "The timezone in [ISO 8601 format](http://en.wikipedia.org/wiki/ISO_8601) for which the service bases its broadcasts" ;
        rdfs:label    "broadcastTimezone" .

schema:estimatedSalary
        rdf:type      rdf:Property ;
        rdfs:comment  "An estimated salary for a job posting or occupation, based on a variety of variables including, but not limited to industry, job title, and location. Estimated salaries  are often computed by outside organizations rather than the hiring organization, who may not have committed to the estimated value." ;
        rdfs:label    "estimatedSalary" .

schema:SearchResultsPage
        rdf:type         rdfs:Class ;
        rdfs:comment     "Web page type: Search results page." ;
        rdfs:label       "SearchResultsPage" ;
        rdfs:subClassOf  schema:WebPage .

schema:WebContent  rdf:type  rdfs:Class ;
        rdfs:comment     "WebContent is a type representing all [[WebPage]], [[WebSite]] and [[WebPageElement]] content. It is sometimes the case that detailed distinctions between Web pages, sites and their parts is not always important or obvious. The  [[WebContent]] type makes it easier to describe Web-addressable content without requiring such distinctions to always be stated. (The intent is that the existing types [[WebPage]], [[WebSite]] and [[WebPageElement]] will eventually be declared as subtypes of [[WebContent]])." ;
        rdfs:label       "WebContent" ;
        rdfs:subClassOf  schema:CreativeWork .

schema:HardwareStore  rdf:type  rdfs:Class ;
        rdfs:comment     "A hardware store." ;
        rdfs:label       "HardwareStore" ;
        rdfs:subClassOf  schema:Store .

schema:nerveMotor  rdf:type  rdf:Property ;
        rdfs:comment  "The neurological pathway extension that involves muscle control." ;
        rdfs:label    "nerveMotor" .

schema:size  rdf:type  rdf:Property ;
        rdfs:comment  "A standardized size of a product or creative work, specified either through a simple textual string (for example 'XL', '32Wx34L'), a  QuantitativeValue with a unitCode, or a comprehensive and structured [[SizeSpecification]]; in other cases, the [[width]], [[height]], [[depth]] and [[weight]] properties may be more applicable. " ;
        rdfs:label    "size" .

schema:albumProductionType
        rdf:type      rdf:Property ;
        rdfs:comment  "Classification of the album by it's type of content: soundtrack, live album, studio album, etc." ;
        rdfs:label    "albumProductionType" .

schema:NewsMediaOrganization
        rdf:type         rdfs:Class ;
        rdfs:comment     "A News/Media organization such as a newspaper or TV station." ;
        rdfs:label       "NewsMediaOrganization" ;
        rdfs:subClassOf  schema:Organization .

schema:SchoolDistrict
        rdf:type         rdfs:Class ;
        rdfs:comment     "A School District is an administrative area for the administration of schools." ;
        rdfs:label       "SchoolDistrict" ;
        rdfs:subClassOf  schema:AdministrativeArea .

schema:competencyRequired
        rdf:type      rdf:Property ;
        rdfs:comment  "Knowledge, skill, ability or personal attribute that must be demonstrated by a person or other entity in order to do something such as earn an Educational Occupational Credential or understand a LearningResource." ;
        rdfs:label    "competencyRequired" .

schema:Date  rdf:type  rdfs:Class ;
        rdfs:comment  "A date value in [ISO 8601 date format](http://en.wikipedia.org/wiki/ISO_8601)." ;
        rdfs:label    "Date" .

schema:ExercisePlan  rdf:type  rdfs:Class ;
        rdfs:comment     "Fitness-related activity designed for a specific health-related purpose, including defined exercise routines as well as activity prescribed by a clinician." ;
        rdfs:label       "ExercisePlan" ;
        rdfs:subClassOf  schema:PhysicalActivity , schema:CreativeWork .

schema:numChildren  rdf:type  rdf:Property ;
        rdfs:comment  "The number of children staying in the unit." ;
        rdfs:label    "numChildren" .

schema:addressCountry
        rdf:type      rdf:Property ;
        rdfs:comment  "The country. For example, USA. You can also provide the two-letter [ISO 3166-1 alpha-2 country code](http://en.wikipedia.org/wiki/ISO_3166-1)." ;
        rdfs:label    "addressCountry" .

schema:thumbnail  rdf:type  rdf:Property ;
        rdfs:comment  "Thumbnail image for an image or video." ;
        rdfs:label    "thumbnail" .

schema:eventStatus  rdf:type  rdf:Property ;
        rdfs:comment  "An eventStatus of an event represents its status; particularly useful when an event is cancelled or rescheduled." ;
        rdfs:label    "eventStatus" .

schema:BedDetails  rdf:type  rdfs:Class ;
        rdfs:comment     "An entity holding detailed information about the available bed types, e.g. the quantity of twin beds for a hotel room. For the single case of just one bed of a certain type, you can use bed directly with a text. See also [[BedType]] (under development)." ;
        rdfs:label       "BedDetails" ;
        rdfs:subClassOf  schema:Intangible .

schema:supply  rdf:type     rdf:Property ;
        rdfs:comment        "A sub-property of instrument. A supply consumed when performing instructions or a direction." ;
        rdfs:label          "supply" ;
        rdfs:subPropertyOf  schema:instrument .

schema:isProprietary  rdf:type  rdf:Property ;
        rdfs:comment  "True if this item's name is a proprietary/brand name (vs. generic name)." ;
        rdfs:label    "isProprietary" .

schema:value  rdf:type  rdf:Property ;
        rdfs:comment  "The value of the quantitative value or property value node.\\n\\n* For [[QuantitativeValue]] and [[MonetaryAmount]], the recommended type for values is 'Number'.\\n* For [[PropertyValue]], it can be 'Text;', 'Number', 'Boolean', or 'StructuredValue'.\\n* Use values from 0123456789 (Unicode 'DIGIT ZERO' (U+0030) to 'DIGIT NINE' (U+0039)) rather than superficially similiar Unicode symbols.\\n* Use '.' (Unicode 'FULL STOP' (U+002E)) rather than ',' to indicate a decimal point. Avoid using these symbols as a readability separator." ;
        rdfs:label    "value" .

schema:MedicalOrganization
        rdf:type         rdfs:Class ;
        rdfs:comment     "A medical organization (physical or not), such as hospital, institution or clinic." ;
        rdfs:label       "MedicalOrganization" ;
        rdfs:subClassOf  schema:Organization .

schema:termCode  rdf:type  rdf:Property ;
        rdfs:comment  "A code that identifies this [[DefinedTerm]] within a [[DefinedTermSet]]" ;
        rdfs:label    "termCode" .

schema:area  rdf:type  rdf:Property ;
        rdfs:comment  "The area within which users can expect to reach the broadcast service." ;
        rdfs:label    "area" .

schema:NonprofitType  rdf:type  rdfs:Class ;
        rdfs:comment     "NonprofitType enumerates several kinds of official non-profit types of which a non-profit organization can be." ;
        rdfs:label       "NonprofitType" ;
        rdfs:subClassOf  schema:Enumeration .

schema:hasDefinedTerm
        rdf:type      rdf:Property ;
        rdfs:comment  "A Defined Term contained in this term set." ;
        rdfs:label    "hasDefinedTerm" .

schema:lender  rdf:type     rdf:Property ;
        rdfs:comment        "A sub property of participant. The person that lends the object being borrowed." ;
        rdfs:label          "lender" ;
        rdfs:subPropertyOf  schema:participant .

schema:stepValue  rdf:type  rdf:Property ;
        rdfs:comment  "The stepValue attribute indicates the granularity that is expected (and required) of the value in a PropertyValueSpecification." ;
        rdfs:label    "stepValue" .

schema:inDefinedTermSet
        rdf:type            rdf:Property ;
        rdfs:comment        "A [[DefinedTermSet]] that contains this term." ;
        rdfs:label          "inDefinedTermSet" ;
        rdfs:subPropertyOf  schema:isPartOf .

schema:SocialMediaPosting
        rdf:type         rdfs:Class ;
        rdfs:comment     "A post to a social media platform, including blog posts, tweets, Facebook posts, etc." ;
        rdfs:label       "SocialMediaPosting" ;
        rdfs:subClassOf  schema:Article .

schema:itemOffered  rdf:type  rdf:Property ;
        rdfs:comment  "An item being offered (or demanded). The transactional nature of the offer or demand is documented using [[businessFunction]], e.g. sell, lease etc. While several common expected types are listed explicitly in this definition, others can be used. Using a second type, such as Product or a subtype of Product, can clarify the nature of the offer." ;
        rdfs:label    "itemOffered" .

schema:readBy  rdf:type     rdf:Property ;
        rdfs:comment        "A person who reads (performs) the audiobook." ;
        rdfs:label          "readBy" ;
        rdfs:subPropertyOf  schema:actor .

schema:City  rdf:type    rdfs:Class ;
        rdfs:comment     "A city or town." ;
        rdfs:label       "City" ;
        rdfs:subClassOf  schema:AdministrativeArea .

schema:courseWorkload
        rdf:type      rdf:Property ;
        rdfs:comment  "The amount of work expected of students taking the course, often provided as a figure per week or per month, and may be broken down by type. For example, \"2 hours of lectures, 1 hour of lab work and 3 hours of independent study per week\"." ;
        rdfs:label    "courseWorkload" .

rdf:type  rdf:type  rdf:Property .

schema:sizeSystem  rdf:type  rdf:Property ;
        rdfs:comment  "The size system used to identify a product's size. Typically either a standard (for example, \"GS1\" or \"ISO-EN13402\"), country code (for example \"US\" or \"JP\"), or a measuring system (for example \"Metric\" or \"Imperial\")." ;
        rdfs:label    "sizeSystem" .

schema:MedicalScholarlyArticle
        rdf:type         rdfs:Class ;
        rdfs:comment     "A scholarly article in the medical domain." ;
        rdfs:label       "MedicalScholarlyArticle" ;
        rdfs:subClassOf  schema:ScholarlyArticle .

schema:ArchiveComponent
        rdf:type         rdfs:Class ;
        rdfs:comment     "An intangible type to be applied to any archive content, carrying with it a set of properties required to describe archival items and collections."@en ;
        rdfs:label       "ArchiveComponent"@en ;
        rdfs:subClassOf  schema:CreativeWork .

schema:closes  rdf:type  rdf:Property ;
        rdfs:comment  "The closing hour of the place or service on the given day(s) of the week." ;
        rdfs:label    "closes" .

schema:albums  rdf:type  rdf:Property ;
        rdfs:comment  "A collection of music albums." ;
        rdfs:label    "albums" .

schema:highPrice  rdf:type  rdf:Property ;
        rdfs:comment  "The highest price of all offers available.\\n\\nUsage guidelines:\\n\\n* Use values from 0123456789 (Unicode 'DIGIT ZERO' (U+0030) to 'DIGIT NINE' (U+0039)) rather than superficially similiar Unicode symbols.\\n* Use '.' (Unicode 'FULL STOP' (U+002E)) rather than ',' to indicate a decimal point. Avoid using these symbols as a readability separator." ;
        rdfs:label    "highPrice" .

schema:Bone  rdf:type    rdfs:Class ;
        rdfs:comment     "Rigid connective tissue that comprises up the skeletal structure of the human body." ;
        rdfs:label       "Bone" ;
        rdfs:subClassOf  schema:AnatomicalStructure .

schema:Museum  rdf:type  rdfs:Class ;
        rdfs:comment     "A museum." ;
        rdfs:label       "Museum" ;
        rdfs:subClassOf  schema:CivicStructure .

schema:EndorsementRating
        rdf:type         rdfs:Class ;
        rdfs:comment     "An EndorsementRating is a rating that expresses some level of endorsement, for example inclusion in a \"critic's pick\" blog, a\n\"Like\" or \"+1\" on a social network. It can be considered the [[result]] of an [[EndorseAction]] in which the [[object]] of the action is rated positively by\nsome [[agent]]. As is common elsewhere in schema.org, it is sometimes more useful to describe the results of such an action without explicitly describing the [[Action]].\n\nAn [[EndorsementRating]] may be part of a numeric scale or organized system, but this is not required: having an explicit type for indicating a positive,\nendorsement rating is particularly useful in the absence of numeric scales as it helps consumers understand that the rating is broadly positive.\n" ;
        rdfs:label       "EndorsementRating" ;
        rdfs:subClassOf  schema:Rating .

schema:issueNumber  rdf:type  rdf:Property ;
        rdfs:comment        "Identifies the issue of publication; for example, \"iii\" or \"2\"." ;
        rdfs:label          "issueNumber" ;
        rdfs:subPropertyOf  schema:position .

schema:wordCount  rdf:type  rdf:Property ;
        rdfs:comment  "The number of words in the text of the Article." ;
        rdfs:label    "wordCount" .

schema:Claim  rdf:type   rdfs:Class ;
        rdfs:comment     "A [[Claim]] in Schema.org represents a specific, factually-oriented claim that could be the [[itemReviewed]] in a [[ClaimReview]]. The content of a claim can be summarized with the [[text]] property. Variations on well known claims can have their common identity indicated via [[sameAs]] links, and summarized with a [[name]]. Ideally, a [[Claim]] description includes enough contextual information to minimize the risk of ambiguity or inclarity. In practice, many claims are better understood in the context in which they appear or the interpretations provided by claim reviews.\n\n  Beyond [[ClaimReview]], the Claim type can be associated with related creative works - for example a [[ScholarlyArticle]] or [[Question]] might be [[about]] some [[Claim]].\n\n  At this time, Schema.org does not define any types of relationship between claims. This is a natural area for future exploration.\n  " ;
        rdfs:label       "Claim" ;
        rdfs:subClassOf  schema:CreativeWork .

schema:MiddleSchool  rdf:type  rdfs:Class ;
        rdfs:comment     "A middle school (typically for children aged around 11-14, although this varies somewhat)." ;
        rdfs:label       "MiddleSchool" ;
        rdfs:subClassOf  schema:EducationalOrganization .

schema:validIn  rdf:type  rdf:Property ;
        rdfs:comment  "The geographic area where a permit or similar thing is valid." ;
        rdfs:label    "validIn" .

schema:AgreeAction  rdf:type  rdfs:Class ;
        rdfs:comment     "The act of expressing a consistency of opinion with the object. An agent agrees to/about an object (a proposition, topic or theme) with participants." ;
        rdfs:label       "AgreeAction" ;
        rdfs:subClassOf  schema:ReactAction .

schema:vehicleConfiguration
        rdf:type      rdf:Property ;
        rdfs:comment  "A short text indicating the configuration of the vehicle, e.g. '5dr hatchback ST 2.5 MT 225 hp' or 'limited edition'." ;
        rdfs:label    "vehicleConfiguration" .

schema:artEdition  rdf:type  rdf:Property ;
        rdfs:comment  "The number of copies when multiple copies of a piece of artwork are produced - e.g. for a limited edition of 20 prints, 'artEdition' refers to the total number of copies (in this example \"20\")." ;
        rdfs:label    "artEdition" .

schema:diagnosis  rdf:type  rdf:Property ;
        rdfs:comment  "One or more alternative conditions considered in the differential diagnosis process as output of a diagnosis process." ;
        rdfs:label    "diagnosis" .

schema:duration  rdf:type  rdf:Property ;
        rdfs:comment  "The duration of the item (movie, audio recording, event, etc.) in [ISO 8601 date format](http://en.wikipedia.org/wiki/ISO_8601)." ;
        rdfs:label    "duration" .

schema:guidelineSubject
        rdf:type      rdf:Property ;
        rdfs:comment  "The medical conditions, treatments, etc. that are the subject of the guideline." ;
        rdfs:label    "guidelineSubject" .

schema:TrainReservation
        rdf:type         rdfs:Class ;
        rdfs:comment     "A reservation for train travel.\\n\\nNote: This type is for information about actual reservations, e.g. in confirmation emails or HTML pages with individual confirmations of reservations. For offers of tickets, use [[Offer]]." ;
        rdfs:label       "TrainReservation" ;
        rdfs:subClassOf  schema:Reservation .

schema:actionOption  rdf:type  rdf:Property ;
        rdfs:comment        "A sub property of object. The options subject to this action." ;
        rdfs:label          "actionOption" ;
        rdfs:subPropertyOf  schema:object .

schema:MedicalProcedureType
        rdf:type         rdfs:Class ;
        rdfs:comment     "An enumeration that describes different types of medical procedures." ;
        rdfs:label       "MedicalProcedureType" ;
        rdfs:subClassOf  schema:MedicalEnumeration .

schema:price  rdf:type  rdf:Property ;
        rdfs:comment  "The offer price of a product, or of a price component when attached to PriceSpecification and its subtypes.\\n\\nUsage guidelines:\\n\\n* Use the [[priceCurrency]] property (with standard formats: [ISO 4217 currency format](http://en.wikipedia.org/wiki/ISO_4217) e.g. \"USD\"; [Ticker symbol](https://en.wikipedia.org/wiki/List_of_cryptocurrencies) for cryptocurrencies e.g. \"BTC\"; well known names for [Local Exchange Tradings Systems](https://en.wikipedia.org/wiki/Local_exchange_trading_system) (LETS) and other currency types e.g. \"Ithaca HOUR\") instead of including [ambiguous symbols](http://en.wikipedia.org/wiki/Dollar_sign#Currencies_that_use_the_dollar_or_peso_sign) such as '$' in the value.\\n* Use '.' (Unicode 'FULL STOP' (U+002E)) rather than ',' to indicate a decimal point. Avoid using these symbols as a readability separator.\\n* Note that both [RDFa](http://www.w3.org/TR/xhtml-rdfa-primer/#using-the-content-attribute) and Microdata syntax allow the use of a \"content=\" attribute for publishing simple machine-readable values alongside more human-friendly formatting.\\n* Use values from 0123456789 (Unicode 'DIGIT ZERO' (U+0030) to 'DIGIT NINE' (U+0039)) rather than superficially similiar Unicode symbols.\n      " ;
        rdfs:label    "price" .

schema:servicePhone  rdf:type  rdf:Property ;
        rdfs:comment  "The phone number to use to access the service." ;
        rdfs:label    "servicePhone" .

schema:flightNumber  rdf:type  rdf:Property ;
        rdfs:comment        "The unique identifier for a flight including the airline IATA code. For example, if describing United flight 110, where the IATA code for United is 'UA', the flightNumber is 'UA110'." ;
        rdfs:label          "flightNumber" ;
        rdfs:subPropertyOf  schema:identifier .

schema:recognizingAuthority
        rdf:type      rdf:Property ;
        rdfs:comment  "If applicable, the organization that officially recognizes this entity as part of its endorsed system of medicine." ;
        rdfs:label    "recognizingAuthority" .

skos:note  rdf:type  rdf:Property ;
        rdfs:label  "note"@en .

schema:availableOnDevice
        rdf:type      rdf:Property ;
        rdfs:comment  "Device required to run the application. Used in cases where a specific make/model is required to run the application." ;
        rdfs:label    "availableOnDevice" .

schema:MedicalCode  rdf:type  rdfs:Class ;
        rdfs:comment     "A code for a medical entity." ;
        rdfs:label       "MedicalCode" ;
        rdfs:subClassOf  schema:CategoryCode , schema:MedicalIntangible .

schema:duringMedia  rdf:type  rdf:Property ;
        rdfs:comment  "A media object representing the circumstances while performing this direction." ;
        rdfs:label    "duringMedia" .

schema:sugarContent  rdf:type  rdf:Property ;
        rdfs:comment  "The number of grams of sugar." ;
        rdfs:label    "sugarContent" .

schema:Waterfall  rdf:type  rdfs:Class ;
        rdfs:comment     "A waterfall, like Niagara." ;
        rdfs:label       "Waterfall" ;
        rdfs:subClassOf  schema:BodyOfWater .

schema:inBroadcastLineup
        rdf:type      rdf:Property ;
        rdfs:comment  "The CableOrSatelliteService offering the channel." ;
        rdfs:label    "inBroadcastLineup" .

schema:WarrantyScope  rdf:type  rdfs:Class ;
        rdfs:comment     "A range of of services that will be provided to a customer free of charge in case of a defect or malfunction of a product.\\n\\nCommonly used values:\\n\\n* http://purl.org/goodrelations/v1#Labor-BringIn\\n* http://purl.org/goodrelations/v1#PartsAndLabor-BringIn\\n* http://purl.org/goodrelations/v1#PartsAndLabor-PickUp\n      " ;
        rdfs:label       "WarrantyScope" ;
        rdfs:subClassOf  schema:Enumeration .

schema:loanMortgageMandateAmount
        rdf:type      rdf:Property ;
        rdfs:comment  "Amount of mortgage mandate that can be converted into a proper mortgage at a later stage." ;
        rdfs:label    "loanMortgageMandateAmount" .

schema:inventoryLevel
        rdf:type      rdf:Property ;
        rdfs:comment  "The current approximate inventory level for the item or items." ;
        rdfs:label    "inventoryLevel" .

schema:Crematorium  rdf:type  rdfs:Class ;
        rdfs:comment     "A crematorium." ;
        rdfs:label       "Crematorium" ;
        rdfs:subClassOf  schema:CivicStructure .

schema:httpMethod  rdf:type  rdf:Property ;
        rdfs:comment  "An HTTP method that specifies the appropriate HTTP method for a request to an HTTP EntryPoint. Values are capitalized strings as used in HTTP." ;
        rdfs:label    "httpMethod" .

schema:LiquorStore  rdf:type  rdfs:Class ;
        rdfs:comment     "A shop that sells alcoholic drinks such as wine, beer, whisky and other spirits." ;
        rdfs:label       "LiquorStore" ;
        rdfs:subClassOf  schema:Store .

schema:yearBuilt  rdf:type  rdf:Property ;
        rdfs:comment  "The year an [[Accommodation]] was constructed. This corresponds to the [YearBuilt field in RESO](https://ddwiki.reso.org/display/DDW17/YearBuilt+Field). " ;
        rdfs:label    "yearBuilt" .

schema:seatingCapacity
        rdf:type      rdf:Property ;
        rdfs:comment  "The number of persons that can be seated (e.g. in a vehicle), both in terms of the physical space available, and in terms of limitations set by law.\\n\\nTypical unit code(s): C62 for persons " ;
        rdfs:label    "seatingCapacity" .

schema:event  rdf:type  rdf:Property ;
        rdfs:comment  "Upcoming or past event associated with this place, organization, or action." ;
        rdfs:label    "event" .

schema:tourBookingPage
        rdf:type      rdf:Property ;
        rdfs:comment  "A page providing information on how to book a tour of some [[Place]], such as an [[Accommodation]] or [[ApartmentComplex]] in a real estate setting, as well as other kinds of tours as appropriate." ;
        rdfs:label    "tourBookingPage" .

schema:exchangeRateSpread
        rdf:type      rdf:Property ;
        rdfs:comment  "The difference between the price at which a broker or other intermediary buys and sells foreign currency." ;
        rdfs:label    "exchangeRateSpread" .

schema:openingHours  rdf:type  rdf:Property ;
        rdfs:comment  "The general opening hours for a business. Opening hours can be specified as a weekly time range, starting with days, then times per day. Multiple days can be listed with commas ',' separating each day. Day or time ranges are specified using a hyphen '-'.\\n\\n* Days are specified using the following two-letter combinations: ```Mo```, ```Tu```, ```We```, ```Th```, ```Fr```, ```Sa```, ```Su```.\\n* Times are specified using 24:00 format. For example, 3pm is specified as ```15:00```, 10am as ```10:00```. \\n* Here is an example: <code>&lt;time itemprop=\"openingHours\" datetime=&quot;Tu,Th 16:00-20:00&quot;&gt;Tuesdays and Thursdays 4-8pm&lt;/time&gt;</code>.\\n* If a business is open 7 days a week, then it can be specified as <code>&lt;time itemprop=&quot;openingHours&quot; datetime=&quot;Mo-Su&quot;&gt;Monday through Sunday, all day&lt;/time&gt;</code>." ;
        rdfs:label    "openingHours" .

schema:HealthPlanCostSharingSpecification
        rdf:type         rdfs:Class ;
        rdfs:comment     "A description of costs to the patient under a given network or formulary." ;
        rdfs:label       "HealthPlanCostSharingSpecification" ;
        rdfs:subClassOf  schema:Intangible .

schema:GeospatialGeometry
        rdf:type         rdfs:Class ;
        rdfs:comment     "(Eventually to be defined as) a supertype of GeoShape designed to accommodate definitions from Geo-Spatial best practices." ;
        rdfs:label       "GeospatialGeometry" ;
        rdfs:subClassOf  schema:Intangible .

schema:accessibilitySummary
        rdf:type      rdf:Property ;
        rdfs:comment  "A human-readable summary of specific accessibility features or deficiencies, consistent with the other accessibility metadata but expressing subtleties such as \"short descriptions are present but long descriptions will be needed for non-visual users\" or \"short descriptions are present and no long descriptions are needed.\"" ;
        rdfs:label    "accessibilitySummary" .

schema:DateTime  rdf:type  rdfs:Class ;
        rdfs:comment  "A combination of date and time of day in the form [-]CCYY-MM-DDThh:mm:ss[Z|(+|-)hh:mm] (see Chapter 5.4 of ISO 8601)." ;
        rdfs:label    "DateTime" .

schema:spokenByCharacter
        rdf:type      rdf:Property ;
        rdfs:comment  "The (e.g. fictional) character, Person or Organization to whom the quotation is attributed within the containing CreativeWork." ;
        rdfs:label    "spokenByCharacter" .

schema:Festival  rdf:type  rdfs:Class ;
        rdfs:comment     "Event type: Festival." ;
        rdfs:label       "Festival" ;
        rdfs:subClassOf  schema:Event .

schema:OfferItemCondition
        rdf:type         rdfs:Class ;
        rdfs:comment     "A list of possible conditions for the item." ;
        rdfs:label       "OfferItemCondition" ;
        rdfs:subClassOf  schema:Enumeration .

schema:CompoundPriceSpecification
        rdf:type         rdfs:Class ;
        rdfs:comment     "A compound price specification is one that bundles multiple prices that all apply in combination for different dimensions of consumption. Use the name property of the attached unit price specification for indicating the dimension of a price component (e.g. \"electricity\" or \"final cleaning\")." ;
        rdfs:label       "CompoundPriceSpecification" ;
        rdfs:subClassOf  schema:PriceSpecification .

schema:sdLicense  rdf:type  rdf:Property ;
        rdfs:comment  "A license document that applies to this structured data, typically indicated by URL." ;
        rdfs:label    "sdLicense" .

schema:hasCourse  rdf:type  rdf:Property ;
        rdfs:comment  "A course or class that is one of the learning opportunities that constitute an educational / occupational program. No information is implied about whether the course is mandatory or optional; no guarantee is implied about whether the course will be available to everyone on the program." ;
        rdfs:label    "hasCourse" .

schema:hoursAvailable
        rdf:type      rdf:Property ;
        rdfs:comment  "The hours during which this service or contact is available." ;
        rdfs:label    "hoursAvailable" .

schema:GenderType  rdf:type  rdfs:Class ;
        rdfs:comment     "An enumeration of genders." ;
        rdfs:label       "GenderType" ;
        rdfs:subClassOf  schema:Enumeration .

schema:Service  rdf:type  rdfs:Class ;
        rdfs:comment     "A service provided by an organization, e.g. delivery service, print services, etc." ;
        rdfs:label       "Service" ;
        rdfs:subClassOf  schema:Intangible .

schema:interactivityType
        rdf:type      rdf:Property ;
        rdfs:comment  "The predominant mode of learning supported by the learning resource. Acceptable values are 'active', 'expositive', or 'mixed'." ;
        rdfs:label    "interactivityType" .

schema:addOn  rdf:type  rdf:Property ;
        rdfs:comment  "An additional offer that can only be obtained in combination with the first base offer (e.g. supplements and extensions that are available for a surcharge)." ;
        rdfs:label    "addOn" .

schema:streetAddress  rdf:type  rdf:Property ;
        rdfs:comment  "The street address. For example, 1600 Amphitheatre Pkwy." ;
        rdfs:label    "streetAddress" .

schema:sportsEvent  rdf:type  rdf:Property ;
        rdfs:comment        "A sub property of location. The sports event where this action occurred." ;
        rdfs:label          "sportsEvent" ;
        rdfs:subPropertyOf  schema:location .

schema:MedicalGuideline
        rdf:type         rdfs:Class ;
        rdfs:comment     "Any recommendation made by a standard society (e.g. ACC/AHA) or consensus statement that denotes how to diagnose and treat a particular condition. Note: this type should be used to tag the actual guideline recommendation; if the guideline recommendation occurs in a larger scholarly article, use MedicalScholarlyArticle to tag the overall article, not this type. Note also: the organization making the recommendation should be captured in the recognizingAuthority base property of MedicalEntity." ;
        rdfs:label       "MedicalGuideline" ;
        rdfs:subClassOf  schema:MedicalEntity .

schema:AggregateOffer
        rdf:type         rdfs:Class ;
        rdfs:comment     "When a single product is associated with multiple offers (for example, the same pair of shoes is offered by different merchants), then AggregateOffer can be used.\\n\\nNote: AggregateOffers are normally expected to associate multiple offers that all share the same defined [[businessFunction]] value, or default to http://purl.org/goodrelations/v1#Sell if businessFunction is not explicitly defined." ;
        rdfs:label       "AggregateOffer" ;
        rdfs:subClassOf  schema:Offer .

schema:fatContent  rdf:type  rdf:Property ;
        rdfs:comment  "The number of grams of fat." ;
        rdfs:label    "fatContent" .

schema:connectedTo  rdf:type  rdf:Property ;
        rdfs:comment  "Other anatomical structures to which this structure is connected." ;
        rdfs:label    "connectedTo" .

schema:yearsInOperation
        rdf:type      rdf:Property ;
        rdfs:comment  "The age of the business." ;
        rdfs:label    "yearsInOperation" .

schema:attendee  rdf:type  rdf:Property ;
        rdfs:comment  "A person or organization attending the event." ;
        rdfs:label    "attendee" .

schema:discountCurrency
        rdf:type      rdf:Property ;
        rdfs:comment  "The currency of the discount.\\n\\nUse standard formats: [ISO 4217 currency format](http://en.wikipedia.org/wiki/ISO_4217) e.g. \"USD\"; [Ticker symbol](https://en.wikipedia.org/wiki/List_of_cryptocurrencies) for cryptocurrencies e.g. \"BTC\"; well known names for [Local Exchange Tradings Systems](https://en.wikipedia.org/wiki/Local_exchange_trading_system) (LETS) and other currency types e.g. \"Ithaca HOUR\"." ;
        rdfs:label    "discountCurrency" .

schema:GameServerStatus
        rdf:type         rdfs:Class ;
        rdfs:comment     "Status of a game server." ;
        rdfs:label       "GameServerStatus" ;
        rdfs:subClassOf  schema:StatusEnumeration .

schema:benefitsSummaryUrl
        rdf:type      rdf:Property ;
        rdfs:comment  "The URL that goes directly to the summary of benefits and coverage for the specific standard plan or plan variation." ;
        rdfs:label    "benefitsSummaryUrl" .

schema:hasDriveThroughService
        rdf:type      rdf:Property ;
        rdfs:comment  "Indicates whether some facility (e.g. [[FoodEstablishment]], [[CovidTestingFacility]]) offers a service that can be used by driving through in a car. In the case of [[CovidTestingFacility]] such facilities could potentially help with social distancing from other potentially-infected users." ;
        rdfs:label    "hasDriveThroughService" .

schema:TravelAction  rdf:type  rdfs:Class ;
        rdfs:comment     "The act of traveling from an fromLocation to a destination by a specified mode of transport, optionally with participants." ;
        rdfs:label       "TravelAction" ;
        rdfs:subClassOf  schema:MoveAction .

schema:sport  rdf:type  rdf:Property ;
        rdfs:comment  "A type of sport (e.g. Baseball)." ;
        rdfs:label    "sport" .

schema:serviceSmsNumber
        rdf:type      rdf:Property ;
        rdfs:comment  "The number to access the service by text message." ;
        rdfs:label    "serviceSmsNumber" .

dcat:Catalog  rdf:type  rdfs:Class .

schema:hospitalAffiliation
        rdf:type      rdf:Property ;
        rdfs:comment  "A hospital with which the physician or office is affiliated." ;
        rdfs:label    "hospitalAffiliation" .

schema:VideoGame  rdf:type  rdfs:Class ;
        rdfs:comment     "A video game is an electronic game that involves human interaction with a user interface to generate visual feedback on a video device." ;
        rdfs:label       "VideoGame" ;
        rdfs:subClassOf  schema:Game , schema:SoftwareApplication .

schema:category  rdf:type  rdf:Property ;
        rdfs:comment  "A category for the item. Greater signs or slashes can be used to informally indicate a category hierarchy." ;
        rdfs:label    "category" .

schema:regionsAllowed
        rdf:type      rdf:Property ;
        rdfs:comment  "The regions where the media is allowed. If not specified, then it's assumed to be allowed everywhere. Specify the countries in [ISO 3166 format](http://en.wikipedia.org/wiki/ISO_3166)." ;
        rdfs:label    "regionsAllowed" .

schema:RentalCarReservation
        rdf:type         rdfs:Class ;
        rdfs:comment     "A reservation for a rental car.\\n\\nNote: This type is for information about actual reservations, e.g. in confirmation emails or HTML pages with individual confirmations of reservations." ;
        rdfs:label       "RentalCarReservation" ;
        rdfs:subClassOf  schema:Reservation .

schema:MedicalRiskScore
        rdf:type         rdfs:Class ;
        rdfs:comment     "A simple system that adds up the number of risk factors to yield a score that is associated with prognosis, e.g. CHAD score, TIMI risk score." ;
        rdfs:label       "MedicalRiskScore" ;
        rdfs:subClassOf  schema:MedicalRiskEstimator .

schema:occupationalCategory
        rdf:type      rdf:Property ;
        rdfs:comment  "A category describing the job, preferably using a term from a taxonomy such as [BLS O*NET-SOC](http://www.onetcenter.org/taxonomy.html), [ISCO-08](https://www.ilo.org/public/english/bureau/stat/isco/isco08/) or similar, with the property repeated for each applicable value. Ideally the taxonomy should be identified, and both the textual label and formal code for the category should be provided.\\n\nNote: for historical reasons, any textual label and formal code provided as a literal may be assumed to be from O*NET-SOC." ;
        rdfs:label    "occupationalCategory" .

schema:publicAccess  rdf:type  rdf:Property ;
        rdfs:comment  "A flag to signal that the [[Place]] is open to public visitors.  If this property is omitted there is no assumed default boolean value" ;
        rdfs:label    "publicAccess" .

schema:announcementLocation
        rdf:type            rdf:Property ;
        rdfs:comment        "Indicates a specific [[CivicStructure]] or [[LocalBusiness]] associated with the SpecialAnnouncement. For example, a specific testing facility or business with special opening hours. For a larger geographic region like a quarantine of an entire region, use [[spatialCoverage]]." ;
        rdfs:label          "announcementLocation" ;
        rdfs:subPropertyOf  schema:spatialCoverage .

schema:signDetected  rdf:type  rdf:Property ;
        rdfs:comment  "A sign detected by the test." ;
        rdfs:label    "signDetected" .

schema:upvoteCount  rdf:type  rdf:Property ;
        rdfs:comment  "The number of upvotes this question, answer or comment has received from the community." ;
        rdfs:label    "upvoteCount" .

schema:CDCPMDRecord  rdf:type  rdfs:Class ;
        rdfs:comment     "A CDCPMDRecord is a data structure representing a record in a CDC tabular data format\n      used for hospital data reporting. See [documentation](/docs/cdc-covid.html) for details, and the linked CDC materials for authoritative\n      definitions used as the source here.\n      " ;
        rdfs:label       "CDCPMDRecord" ;
        rdfs:subClassOf  schema:StructuredValue .

schema:branch  rdf:type  rdf:Property ;
        rdfs:comment  "The branches that delineate from the nerve bundle. Not to be confused with [[branchOf]]." ;
        rdfs:label    "branch" .

schema:clincalPharmacology
        rdf:type      rdf:Property ;
        rdfs:comment  "Description of the absorption and elimination of drugs, including their concentration (pharmacokinetics, pK) and biological effects (pharmacodynamics, pD)." ;
        rdfs:label    "clincalPharmacology" .

schema:MusicAlbumReleaseType
        rdf:type         rdfs:Class ;
        rdfs:comment     "The kind of release which this album is: single, EP or album." ;
        rdfs:label       "MusicAlbumReleaseType" ;
        rdfs:subClassOf  schema:Enumeration .

schema:MedicalObservationalStudyDesign
        rdf:type         rdfs:Class ;
        rdfs:comment     "Design models for observational medical studies. Enumerated type." ;
        rdfs:label       "MedicalObservationalStudyDesign" ;
        rdfs:subClassOf  schema:MedicalEnumeration .

schema:LymphaticVessel
        rdf:type         rdfs:Class ;
        rdfs:comment     "A type of blood vessel that specifically carries lymph fluid unidirectionally toward the heart." ;
        rdfs:label       "LymphaticVessel" ;
        rdfs:subClassOf  schema:Vessel .

schema:serverStatus  rdf:type  rdf:Property ;
        rdfs:comment  "Status of a game server." ;
        rdfs:label    "serverStatus" .

schema:offerCount  rdf:type  rdf:Property ;
        rdfs:comment  "The number of offers for the product." ;
        rdfs:label    "offerCount" .

schema:box  rdf:type  rdf:Property ;
        rdfs:comment  "A box is the area enclosed by the rectangle formed by two points. The first point is the lower corner, the second point is the upper corner. A box is expressed as two points separated by a space character." ;
        rdfs:label    "box" .

schema:vehicleEngine  rdf:type  rdf:Property ;
        rdfs:comment  "Information about the engine or engines of the vehicle." ;
        rdfs:label    "vehicleEngine" .

schema:acceptedAnswer
        rdf:type            rdf:Property ;
        rdfs:comment        "The answer(s) that has been accepted as best, typically on a Question/Answer site. Sites vary in their selection mechanisms, e.g. drawing on community opinion and/or the view of the Question author." ;
        rdfs:label          "acceptedAnswer" ;
        rdfs:subPropertyOf  schema:suggestedAnswer .

schema:Organization  rdf:type  rdfs:Class ;
        rdfs:comment     "An organization such as a school, NGO, corporation, club, etc." ;
        rdfs:label       "Organization" ;
        rdfs:subClassOf  schema:Thing .

schema:award  rdf:type  rdf:Property ;
        rdfs:comment  "An award won by or for this item." ;
        rdfs:label    "award" .

schema:actionPlatform
        rdf:type      rdf:Property ;
        rdfs:comment  "The high level platform(s) where the Action can be performed for the given URL. To specify a specific application or operating system instance, use actionApplication." ;
        rdfs:label    "actionPlatform" .

schema:specialty  rdf:type  rdf:Property ;
        rdfs:comment  "One of the domain specialities to which this web page's content applies." ;
        rdfs:label    "specialty" .

schema:WearAction  rdf:type  rdfs:Class ;
        rdfs:comment     "The act of dressing oneself in clothing." ;
        rdfs:label       "WearAction" ;
        rdfs:subClassOf  schema:UseAction .

schema:MusicEvent  rdf:type  rdfs:Class ;
        rdfs:comment     "Event type: Music event." ;
        rdfs:label       "MusicEvent" ;
        rdfs:subClassOf  schema:Event .

schema:freeShippingThreshold
        rdf:type      rdf:Property ;
        rdfs:comment  "A monetary value above which (or equal to) the shipping rate becomes free. Intended to be used via an [[OfferShippingDetails]] with [[shippingSettingsLink]] matching this [[ShippingRateSettings]]." ;
        rdfs:label    "freeShippingThreshold" .

rdfs:Class  rdf:type  rdfs:Class .

schema:merchant  rdf:type  rdf:Property ;
        rdfs:comment  "'merchant' is an out-dated term for 'seller'." ;
        rdfs:label    "merchant" .

skos:notation  rdf:type  owl:DatatypeProperty ;
        rdfs:label  "notation"@en .

schema:accountOverdraftLimit
        rdf:type      rdf:Property ;
        rdfs:comment  "An overdraft is an extension of credit from a lending institution when an account reaches zero. An overdraft allows the individual to continue withdrawing money even if the account has no funds in it. Basically the bank allows people to borrow a set amount of money." ;
        rdfs:label    "accountOverdraftLimit" .

schema:Pond  rdf:type    rdfs:Class ;
        rdfs:comment     "A pond." ;
        rdfs:label       "Pond" ;
        rdfs:subClassOf  schema:BodyOfWater .

schema:MaximumDoseSchedule
        rdf:type         rdfs:Class ;
        rdfs:comment     "The maximum dosing schedule considered safe for a drug or supplement as recommended by an authority or by the drug/supplement's manufacturer. Capture the recommending authority in the recognizingAuthority property of MedicalEntity." ;
        rdfs:label       "MaximumDoseSchedule" ;
        rdfs:subClassOf  schema:DoseSchedule .

schema:homeTeam  rdf:type   rdf:Property ;
        rdfs:comment        "The home team in a sports event." ;
        rdfs:label          "homeTeam" ;
        rdfs:subPropertyOf  schema:competitor .

schema:legislationIdentifier
        rdf:type            rdf:Property ;
        rdfs:comment        "An identifier for the legislation. This can be either a string-based identifier, like the CELEX at EU level or the NOR in France, or a web-based, URL/URI identifier, like an ELI (European Legislation Identifier) or an URN-Lex." ;
        rdfs:label          "legislationIdentifier" ;
        rdfs:subPropertyOf  schema:identifier .

schema:printPage  rdf:type  rdf:Property ;
        rdfs:comment  "If this NewsArticle appears in print, this field indicates the name of the page on which the article is found. Please note that this field is intended for the exact page name (e.g. A5, B18)." ;
        rdfs:label    "printPage" .

schema:byMonthDay  rdf:type  rdf:Property ;
        rdfs:comment  "Defines the day(s) of the month on which a recurring [[Event]] takes place. Specified as an [[Integer]] between 1-31." ;
        rdfs:label    "byMonthDay" .

schema:seatRow  rdf:type  rdf:Property ;
        rdfs:comment  "The row location of the reserved seat (e.g., B)." ;
        rdfs:label    "seatRow" .

schema:engineDisplacement
        rdf:type      rdf:Property ;
        rdfs:comment  "The volume swept by all of the pistons inside the cylinders of an internal combustion engine in a single movement. \\n\\nTypical unit code(s): CMQ for cubic centimeter, LTR for liters, INQ for cubic inches\\n* Note 1: You can link to information about how the given value has been determined using the [[valueReference]] property.\\n* Note 2: You can use [[minValue]] and [[maxValue]] to indicate ranges." ;
        rdfs:label    "engineDisplacement" .

schema:courseMode  rdf:type  rdf:Property ;
        rdfs:comment  "The medium or means of delivery of the course instance or the mode of study, either as a text label (e.g. \"online\", \"onsite\" or \"blended\"; \"synchronous\" or \"asynchronous\"; \"full-time\" or \"part-time\") or as a URL reference to a term from a controlled vocabulary (e.g. https://ceds.ed.gov/element/001311#Asynchronous )." ;
        rdfs:label    "courseMode" .

schema:artform  rdf:type  rdf:Property ;
        rdfs:comment  "e.g. Painting, Drawing, Sculpture, Print, Photograph, Assemblage, Collage, etc." ;
        rdfs:label    "artform" .

schema:financialAidEligible
        rdf:type      rdf:Property ;
        rdfs:comment  "A financial aid type or program which students may use to pay for tuition or fees associated with the program." ;
        rdfs:label    "financialAidEligible" .

schema:EnergyEfficiencyEnumeration
        rdf:type         rdfs:Class ;
        rdfs:comment     "Enumerates energy efficiency levels (also known as \"classes\" or \"ratings\") and certifications that are part of several international energy efficiency standards." ;
        rdfs:label       "EnergyEfficiencyEnumeration" ;
        rdfs:subClassOf  schema:Enumeration .

schema:bookEdition  rdf:type  rdf:Property ;
        rdfs:comment  "The edition of the book." ;
        rdfs:label    "bookEdition" .

schema:BarOrPub  rdf:type  rdfs:Class ;
        rdfs:comment     "A bar or pub." ;
        rdfs:label       "BarOrPub" ;
        rdfs:subClassOf  schema:FoodEstablishment .

schema:isVariantOf  rdf:type  rdf:Property ;
        rdfs:comment  "Indicates the kind of product that this is a variant of. In the case of [[ProductModel]], this is a pointer (from a ProductModel) to a base product from which this product is a variant. It is safe to infer that the variant inherits all product features from the base model, unless defined locally. This is not transitive. In the case of a [[ProductGroup]], the group description also serves as a template, representing a set of Products that vary on explicitly defined, specific dimensions only (so it defines both a set of variants, as well as which values distinguish amongst those variants). When used with [[ProductGroup]], this property can apply to any [[Product]] included in the group." ;
        rdfs:label    "isVariantOf" .

schema:masthead  rdf:type   rdf:Property ;
        rdfs:comment        "For a [[NewsMediaOrganization]], a link to the masthead page or a page listing top editorial management." ;
        rdfs:label          "masthead" ;
        rdfs:subPropertyOf  schema:publishingPrinciples .

schema:availabilityEnds
        rdf:type      rdf:Property ;
        rdfs:comment  "The end of the availability of the product or service included in the offer." ;
        rdfs:label    "availabilityEnds" .

schema:AmusementPark  rdf:type  rdfs:Class ;
        rdfs:comment     "An amusement park." ;
        rdfs:label       "AmusementPark" ;
        rdfs:subClassOf  schema:EntertainmentBusiness .

schema:recourseLoan  rdf:type  rdf:Property ;
        rdfs:comment  "The only way you get the money back in the event of default is the security. Recourse is where you still have the opportunity to go back to the borrower for the rest of the money." ;
        rdfs:label    "recourseLoan" .

schema:alumniOf  rdf:type  rdf:Property ;
        rdfs:comment  "An organization that the person is an alumni of." ;
        rdfs:label    "alumniOf" .

schema:reviewRating  rdf:type  rdf:Property ;
        rdfs:comment  "The rating given in this review. Note that reviews can themselves be rated. The ```reviewRating``` applies to rating given by the review. The [[aggregateRating]] property applies to the review itself, as a creative work." ;
        rdfs:label    "reviewRating" .

schema:educationalFramework
        rdf:type      rdf:Property ;
        rdfs:comment  "The framework to which the resource being described is aligned." ;
        rdfs:label    "educationalFramework" .

dcat:Distribution  rdf:type  rdfs:Class .

schema:playersOnline  rdf:type  rdf:Property ;
        rdfs:comment  "Number of players on the server." ;
        rdfs:label    "playersOnline" .

schema:HobbyShop  rdf:type  rdfs:Class ;
        rdfs:comment     "A store that sells materials useful or necessary for various hobbies." ;
        rdfs:label       "HobbyShop" ;
        rdfs:subClassOf  schema:Store .

schema:MedicalBusiness
        rdf:type         rdfs:Class ;
        rdfs:comment     "A particular physical or virtual business of an organization for medical purposes. Examples of MedicalBusiness include differents business run by health professionals." ;
        rdfs:label       "MedicalBusiness" ;
        rdfs:subClassOf  schema:LocalBusiness .

schema:PostalCodeRangeSpecification
        rdf:type         rdfs:Class ;
        rdfs:comment     "Indicates a range of postalcodes, usually defined as the set of valid codes between [[postalCodeBegin]] and [[postalCodeEnd]], inclusively." ;
        rdfs:label       "PostalCodeRangeSpecification" ;
        rdfs:subClassOf  schema:StructuredValue .

schema:BlogPosting  rdf:type  rdfs:Class ;
        rdfs:comment     "A blog post." ;
        rdfs:label       "BlogPosting" ;
        rdfs:subClassOf  schema:SocialMediaPosting .

schema:BuddhistTemple
        rdf:type         rdfs:Class ;
        rdfs:comment     "A Buddhist temple." ;
        rdfs:label       "BuddhistTemple" ;
        rdfs:subClassOf  schema:PlaceOfWorship .

schema:billingPeriod  rdf:type  rdf:Property ;
        rdfs:comment  "The time interval used to compute the invoice." ;
        rdfs:label    "billingPeriod" .

schema:RecommendedDoseSchedule
        rdf:type         rdfs:Class ;
        rdfs:comment     "A recommended dosing schedule for a drug or supplement as prescribed or recommended by an authority or by the drug/supplement's manufacturer. Capture the recommending authority in the recognizingAuthority property of MedicalEntity." ;
        rdfs:label       "RecommendedDoseSchedule" ;
        rdfs:subClassOf  schema:DoseSchedule .

schema:broadcastServiceTier
        rdf:type      rdf:Property ;
        rdfs:comment  "The type of service required to have access to the channel (e.g. Standard or Premium)." ;
        rdfs:label    "broadcastServiceTier" .

schema:fundedItem  rdf:type  rdf:Property ;
        rdfs:comment  "Indicates an item funded or sponsored through a [[Grant]]." ;
        rdfs:label    "fundedItem" .

schema:suggestedMinAge
        rdf:type      rdf:Property ;
        rdfs:comment  "Minimum recommended age in years for the audience or user." ;
        rdfs:label    "suggestedMinAge" .

schema:bookingAgent  rdf:type  rdf:Property ;
        rdfs:comment  "'bookingAgent' is an out-dated term indicating a 'broker' that serves as a booking agent." ;
        rdfs:label    "bookingAgent" .

schema:paymentMethod  rdf:type  rdf:Property ;
        rdfs:comment  "The name of the credit card or other method of payment for the order." ;
        rdfs:label    "paymentMethod" .

schema:postalCodePrefix
        rdf:type      rdf:Property ;
        rdfs:comment  "A defined range of postal codes indicated by a common textual prefix. Used for non-numeric systems such as UK." ;
        rdfs:label    "postalCodePrefix" .

schema:arrivalTime  rdf:type  rdf:Property ;
        rdfs:comment  "The expected arrival time." ;
        rdfs:label    "arrivalTime" .

schema:observationDate
        rdf:type      rdf:Property ;
        rdfs:comment  "The observationDate of an [[Observation]]." ;
        rdfs:label    "observationDate" .

schema:member  rdf:type  rdf:Property ;
        rdfs:comment  "A member of an Organization or a ProgramMembership. Organizations can be members of organizations; ProgramMembership is typically for individuals." ;
        rdfs:label    "member" .

schema:recipeCategory
        rdf:type      rdf:Property ;
        rdfs:comment  "The category of the recipe—for example, appetizer, entree, etc." ;
        rdfs:label    "recipeCategory" .

schema:loanTerm  rdf:type   rdf:Property ;
        rdfs:comment        "The duration of the loan or credit agreement." ;
        rdfs:label          "loanTerm" ;
        rdfs:subPropertyOf  schema:duration .

schema:checkinTime  rdf:type  rdf:Property ;
        rdfs:comment  "The earliest someone may check into a lodging establishment." ;
        rdfs:label    "checkinTime" .

schema:encodingType  rdf:type  rdf:Property ;
        rdfs:comment  "The supported encoding type(s) for an EntryPoint request." ;
        rdfs:label    "encodingType" .

schema:shippingSettingsLink
        rdf:type      rdf:Property ;
        rdfs:comment  "Link to a page containing [[ShippingRateSettings]] and [[DeliveryTimeSettings]] details." ;
        rdfs:label    "shippingSettingsLink" .

schema:athlete  rdf:type  rdf:Property ;
        rdfs:comment  "A person that acts as performing member of a sports team; a player as opposed to a coach." ;
        rdfs:label    "athlete" .

schema:recipeIngredient
        rdf:type            rdf:Property ;
        rdfs:comment        "A single ingredient used in the recipe, e.g. sugar, flour or garlic." ;
        rdfs:label          "recipeIngredient" ;
        rdfs:subPropertyOf  schema:supply .

schema:StatisticalPopulation
        rdf:type         rdfs:Class ;
        rdfs:comment     "A StatisticalPopulation is a set of instances of a certain given type that satisfy some set of constraints. The property [[populationType]] is used to specify the type. Any property that can be used on instances of that type can appear on the statistical population. For example, a [[StatisticalPopulation]] representing all [[Person]]s with a [[homeLocation]] of East Podunk California, would be described by applying the appropriate [[homeLocation]] and [[populationType]] properties to a [[StatisticalPopulation]] item that stands for that set of people.\nThe properties [[numConstraints]] and [[constrainingProperty]] are used to specify which of the populations properties are used to specify the population. Note that the sense of \"population\" used here is the general sense of a statistical\npopulation, and does not imply that the population consists of people. For example, a [[populationType]] of [[Event]] or [[NewsArticle]] could be used. See also [[Observation]], and the [data and datasets](/docs/data-and-datasets.html) overview for more details.\n  " ;
        rdfs:label       "StatisticalPopulation" ;
        rdfs:subClassOf  schema:Intangible .

schema:confirmationNumber
        rdf:type            rdf:Property ;
        rdfs:comment        "A number that confirms the given order or payment has been received." ;
        rdfs:label          "confirmationNumber" ;
        rdfs:subPropertyOf  schema:identifier .

schema:MedicalCause  rdf:type  rdfs:Class ;
        rdfs:comment     "The causative agent(s) that are responsible for the pathophysiologic process that eventually results in a medical condition, symptom or sign. In this schema, unless otherwise specified this is meant to be the proximate cause of the medical condition, symptom or sign. The proximate cause is defined as the causative agent that most directly results in the medical condition, symptom or sign. For example, the HIV virus could be considered a cause of AIDS. Or in a diagnostic context, if a patient fell and sustained a hip fracture and two days later sustained a pulmonary embolism which eventuated in a cardiac arrest, the cause of the cardiac arrest (the proximate cause) would be the pulmonary embolism and not the fall. Medical causes can include cardiovascular, chemical, dermatologic, endocrine, environmental, gastroenterologic, genetic, hematologic, gynecologic, iatrogenic, infectious, musculoskeletal, neurologic, nutritional, obstetric, oncologic, otolaryngologic, pharmacologic, psychiatric, pulmonary, renal, rheumatologic, toxic, traumatic, or urologic causes; medical conditions can be causes as well." ;
        rdfs:label       "MedicalCause" ;
        rdfs:subClassOf  schema:MedicalEntity .

schema:dropoffTime  rdf:type  rdf:Property ;
        rdfs:comment  "When a rental car can be dropped off." ;
        rdfs:label    "dropoffTime" .

schema:TennisComplex  rdf:type  rdfs:Class ;
        rdfs:comment     "A tennis complex." ;
        rdfs:label       "TennisComplex" ;
        rdfs:subClassOf  schema:SportsActivityLocation .

schema:MediaReview  rdf:type  rdfs:Class ;
        rdfs:comment     "A [[MediaReview]] is a more specialized form of Review dedicated to the evaluation of media content online, typically in the context of fact-checking and misinformation.\n    For more general reviews of media in the broader sense, use [[UserReview]], [[CriticReview]] or other [[Review]] types. This definition is\n    a work in progress. While the [[MediaManipulationRatingEnumeration]] list reflects significant community review amongst fact-checkers and others working\n    to combat misinformation, the specific structures for representing media objects, their versions and publication context, is still evolving. Similarly, best practices for the relationship between [[MediaReview]] and [[ClaimReview]] markup has not yet been finalized." ;
        rdfs:label       "MediaReview" ;
        rdfs:subClassOf  schema:Review .

schema:urlTemplate  rdf:type  rdf:Property ;
        rdfs:comment  "An url template (RFC6570) that will be used to construct the target of the execution of the action." ;
        rdfs:label    "urlTemplate" .

schema:videoFrameSize
        rdf:type      rdf:Property ;
        rdfs:comment  "The frame size of the video." ;
        rdfs:label    "videoFrameSize" .

schema:ReceiveAction  rdf:type  rdfs:Class ;
        rdfs:comment     "The act of physically/electronically taking delivery of an object that has been transferred from an origin to a destination. Reciprocal of SendAction.\\n\\nRelated actions:\\n\\n* [[SendAction]]: The reciprocal of ReceiveAction.\\n* [[TakeAction]]: Unlike TakeAction, ReceiveAction does not imply that the ownership has been transfered (e.g. I can receive a package, but it does not mean the package is now mine)." ;
        rdfs:label       "ReceiveAction" ;
        rdfs:subClassOf  schema:TransferAction .

schema:AboutPage  rdf:type  rdfs:Class ;
        rdfs:comment     "Web page type: About page." ;
        rdfs:label       "AboutPage" ;
        rdfs:subClassOf  schema:WebPage .

schema:trailer  rdf:type  rdf:Property ;
        rdfs:comment  "The trailer of a movie or tv/radio series, season, episode, etc." ;
        rdfs:label    "trailer" .

schema:constrainingProperty
        rdf:type      rdf:Property ;
        rdfs:comment  "Indicates a property used as a constraint to define a [[StatisticalPopulation]] with respect to the set of entities\n  corresponding to an indicated type (via [[populationType]])." ;
        rdfs:label    "constrainingProperty" .

schema:opponent  rdf:type   rdf:Property ;
        rdfs:comment        "A sub property of participant. The opponent on this action." ;
        rdfs:label          "opponent" ;
        rdfs:subPropertyOf  schema:participant .

schema:TreatmentIndication
        rdf:type         rdfs:Class ;
        rdfs:comment     "An indication for treating an underlying condition, symptom, etc." ;
        rdfs:label       "TreatmentIndication" ;
        rdfs:subClassOf  schema:MedicalIndication .

schema:grantee  rdf:type  rdf:Property ;
        rdfs:comment  "The person, organization, contact point, or audience that has been granted this permission." ;
        rdfs:label    "grantee" .

schema:applicationDeadline
        rdf:type      rdf:Property ;
        rdfs:comment  "The date at which the program stops collecting applications for the next enrollment cycle." ;
        rdfs:label    "applicationDeadline" .

schema:transFatContent
        rdf:type      rdf:Property ;
        rdfs:comment  "The number of grams of trans fat." ;
        rdfs:label    "transFatContent" .

schema:aspect  rdf:type  rdf:Property ;
        rdfs:comment  "An aspect of medical practice that is considered on the page, such as 'diagnosis', 'treatment', 'causes', 'prognosis', 'etiology', 'epidemiology', etc." ;
        rdfs:label    "aspect" .

schema:PaymentStatusType
        rdf:type         rdfs:Class ;
        rdfs:comment     "A specific payment status. For example, PaymentDue, PaymentComplete, etc." ;
        rdfs:label       "PaymentStatusType" ;
        rdfs:subClassOf  schema:StatusEnumeration .

schema:hasDeliveryMethod
        rdf:type      rdf:Property ;
        rdfs:comment  "Method used for delivery or shipping." ;
        rdfs:label    "hasDeliveryMethod" .

schema:FoodEvent  rdf:type  rdfs:Class ;
        rdfs:comment     "Event type: Food event." ;
        rdfs:label       "FoodEvent" ;
        rdfs:subClassOf  schema:Event .

schema:DeleteAction  rdf:type  rdfs:Class ;
        rdfs:comment     "The act of editing a recipient by removing one of its objects." ;
        rdfs:label       "DeleteAction" ;
        rdfs:subClassOf  schema:UpdateAction .

schema:StructuredValue
        rdf:type         rdfs:Class ;
        rdfs:comment     "Structured values are used when the value of a property has a more complex structure than simply being a textual value or a reference to another thing." ;
        rdfs:label       "StructuredValue" ;
        rdfs:subClassOf  schema:Intangible .

schema:employmentType
        rdf:type      rdf:Property ;
        rdfs:comment  "Type of employment (e.g. full-time, part-time, contract, temporary, seasonal, internship)." ;
        rdfs:label    "employmentType" .

schema:byMonth  rdf:type  rdf:Property ;
        rdfs:comment  "Defines the month(s) of the year on which a recurring [[Event]] takes place. Specified as an [[Integer]] between 1-12. January is 1." ;
        rdfs:label    "byMonth" .

schema:deliveryLeadTime
        rdf:type      rdf:Property ;
        rdfs:comment  "The typical delay between the receipt of the order and the goods either leaving the warehouse or being prepared for pickup, in case the delivery method is on site pickup." ;
        rdfs:label    "deliveryLeadTime" .

schema:Report  rdf:type  rdfs:Class ;
        rdfs:comment     "A Report generated by governmental or non-governmental organization." ;
        rdfs:label       "Report" ;
        rdfs:subClassOf  schema:Article .

schema:equal  rdf:type  rdf:Property ;
        rdfs:comment  "This ordering relation for qualitative values indicates that the subject is equal to the object." ;
        rdfs:label    "equal" .

schema:Consortium  rdf:type  rdfs:Class ;
        rdfs:comment     "A Consortium is a membership [[Organization]] whose members are typically Organizations." ;
        rdfs:label       "Consortium" ;
        rdfs:subClassOf  schema:Organization .

schema:paymentMethodId
        rdf:type      rdf:Property ;
        rdfs:comment  "An identifier for the method of payment used (e.g. the last 4 digits of the credit card)." ;
        rdfs:label    "paymentMethodId" .

schema:currency  rdf:type  rdf:Property ;
        rdfs:comment  "The currency in which the monetary amount is expressed.\\n\\nUse standard formats: [ISO 4217 currency format](http://en.wikipedia.org/wiki/ISO_4217) e.g. \"USD\"; [Ticker symbol](https://en.wikipedia.org/wiki/List_of_cryptocurrencies) for cryptocurrencies e.g. \"BTC\"; well known names for [Local Exchange Tradings Systems](https://en.wikipedia.org/wiki/Local_exchange_trading_system) (LETS) and other currency types e.g. \"Ithaca HOUR\"." ;
        rdfs:label    "currency" .

schema:Collection  rdf:type  rdfs:Class ;
        rdfs:comment     "A collection of items e.g. creative works or products." ;
        rdfs:label       "Collection" ;
        rdfs:subClassOf  schema:CreativeWork .

schema:CollegeOrUniversity
        rdf:type         rdfs:Class ;
        rdfs:comment     "A college, university, or other third-level educational institution." ;
        rdfs:label       "CollegeOrUniversity" ;
        rdfs:subClassOf  schema:EducationalOrganization .

schema:itemShipped  rdf:type  rdf:Property ;
        rdfs:comment  "Item(s) being shipped." ;
        rdfs:label    "itemShipped" .

schema:PriceSpecification
        rdf:type         rdfs:Class ;
        rdfs:comment     "A structured value representing a price or price range. Typically, only the subclasses of this type are used for markup. It is recommended to use [[MonetaryAmount]] to describe independent amounts of money such as a salary, credit card limits, etc." ;
        rdfs:label       "PriceSpecification" ;
        rdfs:subClassOf  schema:StructuredValue .

schema:dataFeedElement
        rdf:type      rdf:Property ;
        rdfs:comment  "An item within in a data feed. Data feeds may have many elements." ;
        rdfs:label    "dataFeedElement" .

schema:FoodEstablishmentReservation
        rdf:type         rdfs:Class ;
        rdfs:comment     "A reservation to dine at a food-related business.\\n\\nNote: This type is for information about actual reservations, e.g. in confirmation emails or HTML pages with individual confirmations of reservations." ;
        rdfs:label       "FoodEstablishmentReservation" ;
        rdfs:subClassOf  schema:Reservation .

schema:PostOffice  rdf:type  rdfs:Class ;
        rdfs:comment     "A post office." ;
        rdfs:label       "PostOffice" ;
        rdfs:subClassOf  schema:GovernmentOffice .

schema:gtin8  rdf:type      rdf:Property ;
        rdfs:comment        "The GTIN-8 code of the product, or the product to which the offer refers. This code is also known as EAN/UCC-8 or 8-digit EAN. See [GS1 GTIN Summary](http://www.gs1.org/barcodes/technical/idkeys/gtin) for more details." ;
        rdfs:label          "gtin8" ;
        rdfs:subPropertyOf  schema:identifier , schema:gtin .

schema:drugUnit  rdf:type  rdf:Property ;
        rdfs:comment  "The unit in which the drug is measured, e.g. '5 mg tablet'." ;
        rdfs:label    "drugUnit" .

schema:episodeNumber  rdf:type  rdf:Property ;
        rdfs:comment        "Position of the episode within an ordered group of episodes." ;
        rdfs:label          "episodeNumber" ;
        rdfs:subPropertyOf  schema:position .

schema:healthPlanDrugTier
        rdf:type      rdf:Property ;
        rdfs:comment  "The tier(s) of drugs offered by this formulary or insurance plan." ;
        rdfs:label    "healthPlanDrugTier" .

schema:lowPrice  rdf:type  rdf:Property ;
        rdfs:comment  "The lowest price of all offers available.\\n\\nUsage guidelines:\\n\\n* Use values from 0123456789 (Unicode 'DIGIT ZERO' (U+0030) to 'DIGIT NINE' (U+0039)) rather than superficially similiar Unicode symbols.\\n* Use '.' (Unicode 'FULL STOP' (U+002E)) rather than ',' to indicate a decimal point. Avoid using these symbols as a readability separator." ;
        rdfs:label    "lowPrice" .

schema:DatedMoneySpecification
        rdf:type         rdfs:Class ;
        rdfs:comment     "A DatedMoneySpecification represents monetary values with optional start and end dates. For example, this could represent an employee's salary over a specific period of time. __Note:__ This type has been superseded by [[MonetaryAmount]] use of that type is recommended" ;
        rdfs:label       "DatedMoneySpecification" ;
        rdfs:subClassOf  schema:StructuredValue .

schema:inStoreReturnsOffered
        rdf:type      rdf:Property ;
        rdfs:comment  "Are in-store returns offered?" ;
        rdfs:label    "inStoreReturnsOffered" .

schema:bodyType  rdf:type  rdf:Property ;
        rdfs:comment  "Indicates the design and body style of the vehicle (e.g. station wagon, hatchback, etc.)." ;
        rdfs:label    "bodyType" .

schema:acquiredFrom  rdf:type  rdf:Property ;
        rdfs:comment  "The organization or person from which the product was acquired." ;
        rdfs:label    "acquiredFrom" .

schema:supportingData
        rdf:type      rdf:Property ;
        rdfs:comment  "Supporting data for a SoftwareApplication." ;
        rdfs:label    "supportingData" .

schema:childMinAge  rdf:type  rdf:Property ;
        rdfs:comment  "Minimal age of the child." ;
        rdfs:label    "childMinAge" .

schema:Article  rdf:type  rdfs:Class ;
        rdfs:comment     "An article, such as a news article or piece of investigative report. Newspapers and magazines have articles of many different types and this is intended to cover them all.\\n\\nSee also [blog post](http://blog.schema.org/2014/09/schemaorg-support-for-bibliographic_2.html)." ;
        rdfs:label       "Article" ;
        rdfs:subClassOf  schema:CreativeWork .

schema:translationOfWork
        rdf:type      rdf:Property ;
        rdfs:comment  "The work that this work has been translated from. e.g. 物种起源 is a translationOf “On the Origin of Species”" ;
        rdfs:label    "translationOfWork" .

schema:monthlyMinimumRepaymentAmount
        rdf:type      rdf:Property ;
        rdfs:comment  "The minimum payment is the lowest amount of money that one is required to pay on a credit card statement each month." ;
        rdfs:label    "monthlyMinimumRepaymentAmount" .

schema:superEvent  rdf:type  rdf:Property ;
        rdfs:comment  "An event that this event is a part of. For example, a collection of individual music performances might each have a music festival as their superEvent." ;
        rdfs:label    "superEvent" .

schema:AuthorizeAction
        rdf:type         rdfs:Class ;
        rdfs:comment     "The act of granting permission to an object." ;
        rdfs:label       "AuthorizeAction" ;
        rdfs:subClassOf  schema:AllocateAction .

schema:accessibilityFeature
        rdf:type      rdf:Property ;
        rdfs:comment  "Content features of the resource, such as accessible media, alternatives and supported enhancements for accessibility ([WebSchemas wiki lists possible values](http://www.w3.org/wiki/WebSchemas/Accessibility))." ;
        rdfs:label    "accessibilityFeature" .

schema:Electrician  rdf:type  rdfs:Class ;
        rdfs:comment     "An electrician." ;
        rdfs:label       "Electrician" ;
        rdfs:subClassOf  schema:HomeAndConstructionBusiness .

schema:DanceGroup  rdf:type  rdfs:Class ;
        rdfs:comment     "A dance group&#x2014;for example, the Alvin Ailey Dance Theater or Riverdance." ;
        rdfs:label       "DanceGroup" ;
        rdfs:subClassOf  schema:PerformingGroup .

schema:requiredQuantity
        rdf:type      rdf:Property ;
        rdfs:comment  "The required quantity of the item(s)." ;
        rdfs:label    "requiredQuantity" .

schema:securityScreening
        rdf:type      rdf:Property ;
        rdfs:comment  "The type of security screening the passenger is subject to." ;
        rdfs:label    "securityScreening" .

schema:AdvertiserContentArticle
        rdf:type         rdfs:Class ;
        rdfs:comment     "An [[Article]] that an external entity has paid to place or to produce to its specifications. Includes [advertorials](https://en.wikipedia.org/wiki/Advertorial), sponsored content, native advertising and other paid content." ;
        rdfs:label       "AdvertiserContentArticle" ;
        rdfs:subClassOf  schema:Article .

schema:eventAttendanceMode
        rdf:type      rdf:Property ;
        rdfs:comment  "The eventAttendanceMode of an event indicates whether it occurs online, offline, or a mix." ;
        rdfs:label    "eventAttendanceMode" .

schema:DisagreeAction
        rdf:type         rdfs:Class ;
        rdfs:comment     "The act of expressing a difference of opinion with the object. An agent disagrees to/about an object (a proposition, topic or theme) with participants." ;
        rdfs:label       "DisagreeAction" ;
        rdfs:subClassOf  schema:ReactAction .

schema:minimumPaymentDue
        rdf:type      rdf:Property ;
        rdfs:comment  "The minimum payment required at this time." ;
        rdfs:label    "minimumPaymentDue" .

schema:QAPage  rdf:type  rdfs:Class ;
        rdfs:comment     "A QAPage is a WebPage focussed on a specific Question and its Answer(s), e.g. in a question answering site or documenting Frequently Asked Questions (FAQs)." ;
        rdfs:label       "QAPage" ;
        rdfs:subClassOf  schema:WebPage .

schema:orderDate  rdf:type  rdf:Property ;
        rdfs:comment  "Date order was placed." ;
        rdfs:label    "orderDate" .

schema:maximumPhysicalAttendeeCapacity
        rdf:type      rdf:Property ;
        rdfs:comment  "The maximum physical attendee capacity of an [[Event]] whose [[eventAttendanceMode]] is [[OfflineEventAttendanceMode]] (or the offline aspects, in the case of a [[MixedEventAttendanceMode]]). " ;
        rdfs:label    "maximumPhysicalAttendeeCapacity" .

schema:Painting  rdf:type  rdfs:Class ;
        rdfs:comment     "A painting." ;
        rdfs:label       "Painting" ;
        rdfs:subClassOf  schema:CreativeWork .

schema:orderStatus  rdf:type  rdf:Property ;
        rdfs:comment  "The current status of the order." ;
        rdfs:label    "orderStatus" .

schema:HowToStep  rdf:type  rdfs:Class ;
        rdfs:comment     "A step in the instructions for how to achieve a result. It is an ordered list with HowToDirection and/or HowToTip items." ;
        rdfs:label       "HowToStep" ;
        rdfs:subClassOf  schema:ListItem , schema:ItemList , schema:CreativeWork .

schema:memberOf  rdf:type  rdf:Property ;
        rdfs:comment  "An Organization (or ProgramMembership) to which this Person or Organization belongs." ;
        rdfs:label    "memberOf" .

schema:HotelRoom  rdf:type  rdfs:Class ;
        rdfs:comment     "A hotel room is a single room in a hotel.\n<br /><br />\nSee also the <a href=\"/docs/hotels.html\">dedicated document on the use of schema.org for marking up hotels and other forms of accommodations</a>.\n" ;
        rdfs:label       "HotelRoom" ;
        rdfs:subClassOf  schema:Room .

schema:PsychologicalTreatment
        rdf:type         rdfs:Class ;
        rdfs:comment     "A process of care relying upon counseling, dialogue and communication  aimed at improving a mental health condition without use of drugs." ;
        rdfs:label       "PsychologicalTreatment" ;
        rdfs:subClassOf  schema:TherapeuticProcedure .

schema:blogPosts  rdf:type  rdf:Property ;
        rdfs:comment  "The postings that are part of this blog." ;
        rdfs:label    "blogPosts" .

schema:telephone  rdf:type  rdf:Property ;
        rdfs:comment  "The telephone number." ;
        rdfs:label    "telephone" .

skos:exactMatch  rdf:type   owl:ObjectProperty ;
        rdfs:comment        "skos:exactMatch is disjoint with each of the properties skos:broadMatch and skos:relatedMatch."@en ;
        rdfs:label          "has exact match"@en ;
        rdfs:subPropertyOf  skos:closeMatch .

schema:founder  rdf:type  rdf:Property ;
        rdfs:comment  "A person who founded this organization." ;
        rdfs:label    "founder" .

schema:produces  rdf:type  rdf:Property ;
        rdfs:comment  "The tangible thing generated by the service, e.g. a passport, permit, etc." ;
        rdfs:label    "produces" .

schema:coach  rdf:type  rdf:Property ;
        rdfs:comment  "A person that acts in a coaching role for a sports team." ;
        rdfs:label    "coach" .

schema:QuantitativeValueDistribution
        rdf:type         rdfs:Class ;
        rdfs:comment     "A statistical distribution of values." ;
        rdfs:label       "QuantitativeValueDistribution" ;
        rdfs:subClassOf  schema:StructuredValue .

schema:UnitPriceSpecification
        rdf:type         rdfs:Class ;
        rdfs:comment     "The price asked for a given offer by the respective organization or person." ;
        rdfs:label       "UnitPriceSpecification" ;
        rdfs:subClassOf  schema:PriceSpecification .

schema:composer  rdf:type  rdf:Property ;
        rdfs:comment  "The person or organization who wrote a composition, or who is the composer of a work performed at some event." ;
        rdfs:label    "composer" .

schema:Action  rdf:type  rdfs:Class ;
        rdfs:comment     "An action performed by a direct agent and indirect participants upon a direct object. Optionally happens at a location with the help of an inanimate instrument. The execution of the action may produce a result. Specific action sub-type documentation specifies the exact expectation of each argument/role.\\n\\nSee also [blog post](http://blog.schema.org/2014/04/announcing-schemaorg-actions.html) and [Actions overview document](http://schema.org/docs/actions.html)." ;
        rdfs:label       "Action" ;
        rdfs:subClassOf  schema:Thing .

schema:missionCoveragePrioritiesPolicy
        rdf:type            rdf:Property ;
        rdfs:comment        "For a [[NewsMediaOrganization]], a statement on coverage priorities, including any public agenda or stance on issues." ;
        rdfs:label          "missionCoveragePrioritiesPolicy" ;
        rdfs:subPropertyOf  schema:publishingPrinciples .

schema:imagingTechnique
        rdf:type      rdf:Property ;
        rdfs:comment  "Imaging technique used." ;
        rdfs:label    "imagingTechnique" .

schema:steps  rdf:type  rdf:Property ;
        rdfs:comment  "A single step item (as HowToStep, text, document, video, etc.) or a HowToSection (originally misnamed 'steps'; 'step' is preferred)." ;
        rdfs:label    "steps" .

schema:line  rdf:type  rdf:Property ;
        rdfs:comment  "A line is a point-to-point path consisting of two or more points. A line is expressed as a series of two or more point objects separated by space." ;
        rdfs:label    "line" .

schema:jobBenefits  rdf:type  rdf:Property ;
        rdfs:comment  "Description of benefits associated with the job." ;
        rdfs:label    "jobBenefits" .

schema:spatialCoverage
        rdf:type            rdf:Property ;
        rdfs:comment        "The spatialCoverage of a CreativeWork indicates the place(s) which are the focus of the content. It is a subproperty of\n      contentLocation intended primarily for more technical and detailed materials. For example with a Dataset, it indicates\n      areas that the dataset describes: a dataset of New York weather would have spatialCoverage which was the place: the state of New York." ;
        rdfs:label          "spatialCoverage" ;
        rdfs:subPropertyOf  schema:contentLocation .

schema:DiagnosticProcedure
        rdf:type         rdfs:Class ;
        rdfs:comment     "A medical procedure intended primarily for diagnostic, as opposed to therapeutic, purposes." ;
        rdfs:label       "DiagnosticProcedure" ;
        rdfs:subClassOf  schema:MedicalProcedure .

schema:ProductModel  rdf:type  rdfs:Class ;
        rdfs:comment     "A datasheet or vendor specification of a product (in the sense of a prototypical description)." ;
        rdfs:label       "ProductModel" ;
        rdfs:subClassOf  schema:Product .

schema:location  rdf:type  rdf:Property ;
        rdfs:comment  "The location of, for example, where an event is happening, where an organization is located, or where an action takes place." ;
        rdfs:label    "location" .

schema:creditText  rdf:type  rdf:Property ;
        rdfs:comment  "Text that can be used to credit person(s) and/or organization(s) associated with a published Creative Work." ;
        rdfs:label    "creditText" .

schema:EntertainmentBusiness
        rdf:type         rdfs:Class ;
        rdfs:comment     "A business providing entertainment." ;
        rdfs:label       "EntertainmentBusiness" ;
        rdfs:subClassOf  schema:LocalBusiness .

schema:PodcastSeason  rdf:type  rdfs:Class ;
        rdfs:comment     "A single season of a podcast. Many podcasts do not break down into separate seasons. In that case, PodcastSeries should be used." ;
        rdfs:label       "PodcastSeason" ;
        rdfs:subClassOf  schema:CreativeWorkSeason .

schema:TVSeries  rdf:type  rdfs:Class ;
        rdfs:comment     "CreativeWorkSeries dedicated to TV broadcast and associated online delivery." ;
        rdfs:label       "TVSeries" ;
        rdfs:subClassOf  schema:CreativeWorkSeries , schema:CreativeWork .

schema:WPAdBlock  rdf:type  rdfs:Class ;
        rdfs:comment     "An advertising section of the page." ;
        rdfs:label       "WPAdBlock" ;
        rdfs:subClassOf  schema:WebPageElement .

schema:proprietaryName
        rdf:type      rdf:Property ;
        rdfs:comment  "Proprietary name given to the diet plan, typically by its originator or creator." ;
        rdfs:label    "proprietaryName" .

schema:epidemiology  rdf:type  rdf:Property ;
        rdfs:comment  "The characteristics of associated patients, such as age, gender, race etc." ;
        rdfs:label    "epidemiology" .

rdf:Property  rdf:type  rdfs:Class .

schema:HowTo  rdf:type   rdfs:Class ;
        rdfs:comment     "Instructions that explain how to achieve a result by performing a sequence of steps." ;
        rdfs:label       "HowTo" ;
        rdfs:subClassOf  schema:CreativeWork .

schema:fuelCapacity  rdf:type  rdf:Property ;
        rdfs:comment  "The capacity of the fuel tank or in the case of electric cars, the battery. If there are multiple components for storage, this should indicate the total of all storage of the same type.\\n\\nTypical unit code(s): LTR for liters, GLL of US gallons, GLI for UK / imperial gallons, AMH for ampere-hours (for electrical vehicles)." ;
        rdfs:label    "fuelCapacity" .

schema:starRating  rdf:type  rdf:Property ;
        rdfs:comment  "An official rating for a lodging business or food establishment, e.g. from national associations or standards bodies. Use the author property to indicate the rating organization, e.g. as an Organization with name such as (e.g. HOTREC, DEHOGA, WHR, or Hotelstars)." ;
        rdfs:label    "starRating" .

schema:InternetCafe  rdf:type  rdfs:Class ;
        rdfs:comment     "An internet cafe." ;
        rdfs:label       "InternetCafe" ;
        rdfs:subClassOf  schema:LocalBusiness .

schema:LodgingBusiness
        rdf:type         rdfs:Class ;
        rdfs:comment     "A lodging business, such as a motel, hotel, or inn." ;
        rdfs:label       "LodgingBusiness" ;
        rdfs:subClassOf  schema:LocalBusiness .

schema:BookFormatType
        rdf:type         rdfs:Class ;
        rdfs:comment     "The publication format of the book." ;
        rdfs:label       "BookFormatType" ;
        rdfs:subClassOf  schema:Enumeration .

schema:branchCode  rdf:type  rdf:Property ;
        rdfs:comment  "A short textual code (also called \"store code\") that uniquely identifies a place of business. The code is typically assigned by the parentOrganization and used in structured URLs.\\n\\nFor example, in the URL http://www.starbucks.co.uk/store-locator/etc/detail/3047 the code \"3047\" is a branchCode for a particular branch.\n      " ;
        rdfs:label    "branchCode" .

schema:participant  rdf:type  rdf:Property ;
        rdfs:comment  "Other co-agents that participated in the action indirectly. e.g. John wrote a book with *Steve*." ;
        rdfs:label    "participant" .

schema:discussionUrl  rdf:type  rdf:Property ;
        rdfs:comment  "A link to the page containing the comments of the CreativeWork." ;
        rdfs:label    "discussionUrl" .

schema:PawnShop  rdf:type  rdfs:Class ;
        rdfs:comment     "A shop that will buy, or lend money against the security of, personal possessions." ;
        rdfs:label       "PawnShop" ;
        rdfs:subClassOf  schema:Store .

schema:isUnlabelledFallback
        rdf:type      rdf:Property ;
        rdfs:comment  "This can be marked 'true' to indicate that some published [[DeliveryTimeSettings]] or [[ShippingRateSettings]] are intended to apply to all [[OfferShippingDetails]] published by the same merchant, when referenced by a [[shippingSettingsLink]] in those settings. It is not meaningful to use a 'true' value for this property alongside a transitTimeLabel (for [[DeliveryTimeSettings]]) or shippingLabel (for [[ShippingRateSettings]]), since this property is for use with unlabelled settings." ;
        rdfs:label    "isUnlabelledFallback" .

schema:DigitalDocument
        rdf:type         rdfs:Class ;
        rdfs:comment     "An electronic file or document." ;
        rdfs:label       "DigitalDocument" ;
        rdfs:subClassOf  schema:CreativeWork .

schema:inker  rdf:type  rdf:Property ;
        rdfs:comment  "The individual who traces over the pencil drawings in ink after pencils are complete." ;
        rdfs:label    "inker" .

schema:antagonist  rdf:type  rdf:Property ;
        rdfs:comment  "The muscle whose action counteracts the specified muscle." ;
        rdfs:label    "antagonist" .

schema:BodyOfWater  rdf:type  rdfs:Class ;
        rdfs:comment     "A body of water, such as a sea, ocean, or lake." ;
        rdfs:label       "BodyOfWater" ;
        rdfs:subClassOf  schema:Landform .

schema:AppendAction  rdf:type  rdfs:Class ;
        rdfs:comment     "The act of inserting at the end if an ordered collection." ;
        rdfs:label       "AppendAction" ;
        rdfs:subClassOf  schema:InsertAction .

schema:GamePlayMode  rdf:type  rdfs:Class ;
        rdfs:comment     "Indicates whether this game is multi-player, co-op or single-player." ;
        rdfs:label       "GamePlayMode" ;
        rdfs:subClassOf  schema:Enumeration .

schema:audio  rdf:type  rdf:Property ;
        rdfs:comment  "An embedded audio object." ;
        rdfs:label    "audio" .

schema:accountId  rdf:type  rdf:Property ;
        rdfs:comment        "The identifier for the account the payment will be applied to." ;
        rdfs:label          "accountId" ;
        rdfs:subPropertyOf  schema:identifier .

schema:SolveMathAction
        rdf:type         rdfs:Class ;
        rdfs:comment     "The action that takes in a math expression and directs users to a page potentially capable of solving/simplifying that expression." ;
        rdfs:label       "SolveMathAction" ;
        rdfs:subClassOf  schema:Action .

schema:ticketedSeat  rdf:type  rdf:Property ;
        rdfs:comment  "The seat associated with the ticket." ;
        rdfs:label    "ticketedSeat" .

schema:creativeWorkStatus
        rdf:type      rdf:Property ;
        rdfs:comment  "The status of a creative work in terms of its stage in a lifecycle. Example terms include Incomplete, Draft, Published, Obsolete. Some organizations define a set of terms for the stages of their publication lifecycle." ;
        rdfs:label    "creativeWorkStatus" .

schema:messageAttachment
        rdf:type      rdf:Property ;
        rdfs:comment  "A CreativeWork attached to the message." ;
        rdfs:label    "messageAttachment" .

schema:unitText  rdf:type  rdf:Property ;
        rdfs:comment  "A string or text indicating the unit of measurement. Useful if you cannot provide a standard unit code for\n<a href='unitCode'>unitCode</a>." ;
        rdfs:label    "unitText" .

schema:underName  rdf:type  rdf:Property ;
        rdfs:comment  "The person or organization the reservation or ticket is for." ;
        rdfs:label    "underName" .

schema:NoteDigitalDocument
        rdf:type         rdfs:Class ;
        rdfs:comment     "A file containing a note, primarily for the author." ;
        rdfs:label       "NoteDigitalDocument" ;
        rdfs:subClassOf  schema:DigitalDocument .

schema:cargoVolume  rdf:type  rdf:Property ;
        rdfs:comment  "The available volume for cargo or luggage. For automobiles, this is usually the trunk volume.\\n\\nTypical unit code(s): LTR for liters, FTQ for cubic foot/feet\\n\\nNote: You can use [[minValue]] and [[maxValue]] to indicate ranges." ;
        rdfs:label    "cargoVolume" .

schema:CheckoutPage  rdf:type  rdfs:Class ;
        rdfs:comment     "Web page type: Checkout page." ;
        rdfs:label       "CheckoutPage" ;
        rdfs:subClassOf  schema:WebPage .

schema:ChooseAction  rdf:type  rdfs:Class ;
        rdfs:comment     "The act of expressing a preference from a set of options or a large or unbounded set of choices/options." ;
        rdfs:label       "ChooseAction" ;
        rdfs:subClassOf  schema:AssessAction .

schema:postalCodeRange
        rdf:type      rdf:Property ;
        rdfs:comment  "A defined range of postal codes." ;
        rdfs:label    "postalCodeRange" .

schema:fuelType  rdf:type  rdf:Property ;
        rdfs:comment  "The type of fuel suitable for the engine or engines of the vehicle. If the vehicle has only one engine, this property can be attached directly to the vehicle." ;
        rdfs:label    "fuelType" .

schema:MedicalObservationalStudy
        rdf:type         rdfs:Class ;
        rdfs:comment     "An observational study is a type of medical study that attempts to infer the possible effect of a treatment through observation of a cohort of subjects over a period of time. In an observational study, the assignment of subjects into treatment groups versus control groups is outside the control of the investigator. This is in contrast with controlled studies, such as the randomized controlled trials represented by MedicalTrial, where each subject is randomly assigned to a treatment group or a control group before the start of the treatment." ;
        rdfs:label       "MedicalObservationalStudy" ;
        rdfs:subClassOf  schema:MedicalStudy .

schema:totalPaymentDue
        rdf:type      rdf:Property ;
        rdfs:comment  "The total amount due." ;
        rdfs:label    "totalPaymentDue" .

schema:LibrarySystem  rdf:type  rdfs:Class ;
        rdfs:comment     "A [[LibrarySystem]] is a collaborative system amongst several libraries." ;
        rdfs:label       "LibrarySystem" ;
        rdfs:subClassOf  schema:Organization .

schema:model  rdf:type  rdf:Property ;
        rdfs:comment  "The model of the product. Use with the URL of a ProductModel or a textual representation of the model identifier. The URL of the ProductModel can be from an external source. It is recommended to additionally provide strong product identifiers via the gtin8/gtin13/gtin14 and mpn properties." ;
        rdfs:label    "model" .

schema:InsertAction  rdf:type  rdfs:Class ;
        rdfs:comment     "The act of adding at a specific location in an ordered collection." ;
        rdfs:label       "InsertAction" ;
        rdfs:subClassOf  schema:AddAction .

schema:subjectOf  rdf:type  rdf:Property ;
        rdfs:comment  "A CreativeWork or Event about this Thing." ;
        rdfs:label    "subjectOf" .

schema:provider  rdf:type  rdf:Property ;
        rdfs:comment  "The service provider, service operator, or service performer; the goods producer. Another party (a seller) may offer those services or goods on behalf of the provider. A provider may also serve as the seller." ;
        rdfs:label    "provider" .

schema:MedicalWebPage
        rdf:type         rdfs:Class ;
        rdfs:comment     "A web page that provides medical information." ;
        rdfs:label       "MedicalWebPage" ;
        rdfs:subClassOf  schema:WebPage .

schema:lodgingUnitType
        rdf:type      rdf:Property ;
        rdfs:comment  "Textual description of the unit type (including suite vs. room, size of bed, etc.)." ;
        rdfs:label    "lodgingUnitType" .

schema:Motorcycle  rdf:type  rdfs:Class ;
        rdfs:comment     "A motorcycle or motorbike is a single-track, two-wheeled motor vehicle." ;
        rdfs:label       "Motorcycle" ;
        rdfs:subClassOf  schema:Vehicle .

schema:priceType  rdf:type  rdf:Property ;
        rdfs:comment  "Defines the type of a price specified for an offered product, for example a list price, a (temporary) sale price or a manufacturer suggested retail price. If multiple prices are specified for an offer the [[priceType]] property can be used to identify the type of each such specified price. The value of priceType can be specified as a value from enumeration PriceTypeEnumeration or as a free form text string for price types that are not already predefined in PriceTypeEnumeration." ;
        rdfs:label    "priceType" .

schema:answerCount  rdf:type  rdf:Property ;
        rdfs:comment  "The number of answers this question has received." ;
        rdfs:label    "answerCount" .

schema:DepartmentStore
        rdf:type         rdfs:Class ;
        rdfs:comment     "A department store." ;
        rdfs:label       "DepartmentStore" ;
        rdfs:subClassOf  schema:Store .

schema:SubscribeAction
        rdf:type         rdfs:Class ;
        rdfs:comment     "The act of forming a personal connection with someone/something (object) unidirectionally/asymmetrically to get updates pushed to.\\n\\nRelated actions:\\n\\n* [[FollowAction]]: Unlike FollowAction, SubscribeAction implies that the subscriber acts as a passive agent being constantly/actively pushed for updates.\\n* [[RegisterAction]]: Unlike RegisterAction, SubscribeAction implies that the agent is interested in continuing receiving updates from the object.\\n* [[JoinAction]]: Unlike JoinAction, SubscribeAction implies that the agent is interested in continuing receiving updates from the object." ;
        rdfs:label       "SubscribeAction" ;
        rdfs:subClassOf  schema:InteractAction .

schema:proficiencyLevel
        rdf:type      rdf:Property ;
        rdfs:comment  "Proficiency needed for this content; expected values: 'Beginner', 'Expert'." ;
        rdfs:label    "proficiencyLevel" .

schema:UpdateAction  rdf:type  rdfs:Class ;
        rdfs:comment     "The act of managing by changing/editing the state of the object." ;
        rdfs:label       "UpdateAction" ;
        rdfs:subClassOf  schema:Action .

dcmitype:Event  rdf:type  rdfs:Class .

schema:geoCrosses  rdf:type  rdf:Property ;
        rdfs:comment  "Represents a relationship between two geometries (or the places they represent), relating a geometry to another that crosses it: \"a crosses b: they have some but not all interior points in common, and the dimension of the intersection is less than that of at least one of them\". As defined in [DE-9IM](https://en.wikipedia.org/wiki/DE-9IM)." ;
        rdfs:label    "geoCrosses" .

schema:musicCompositionForm
        rdf:type      rdf:Property ;
        rdfs:comment  "The type of composition (e.g. overture, sonata, symphony, etc.)." ;
        rdfs:label    "musicCompositionForm" .

schema:entertainmentBusiness
        rdf:type            rdf:Property ;
        rdfs:comment        "A sub property of location. The entertainment business where the action occurred." ;
        rdfs:label          "entertainmentBusiness" ;
        rdfs:subPropertyOf  schema:location .

schema:speed  rdf:type  rdf:Property ;
        rdfs:comment  "The speed range of the vehicle. If the vehicle is powered by an engine, the upper limit of the speed range (indicated by [[maxValue]] should be the maximum speed achievable under regular conditions.\\n\\nTypical unit code(s): KMH for km/h, HM for mile per hour (0.447 04 m/s), KNT for knot\\n\\n*Note 1: Use [[minValue]] and [[maxValue]] to indicate the range. Typically, the minimal value is zero.\\n* Note 2: There are many different ways of measuring the speed range. You can link to information about how the given value has been determined using the [[valueReference]] property." ;
        rdfs:label    "speed" .

schema:minValue  rdf:type  rdf:Property ;
        rdfs:comment  "The lower value of some characteristic or property." ;
        rdfs:label    "minValue" .

schema:interactionStatistic
        rdf:type      rdf:Property ;
        rdfs:comment  "The number of interactions for the CreativeWork using the WebSite or SoftwareApplication. The most specific child type of InteractionCounter should be used." ;
        rdfs:label    "interactionStatistic" .

schema:RadioEpisode  rdf:type  rdfs:Class ;
        rdfs:comment     "A radio episode which can be part of a series or season." ;
        rdfs:label       "RadioEpisode" ;
        rdfs:subClassOf  schema:Episode .

schema:makesOffer  rdf:type  rdf:Property ;
        rdfs:comment  "A pointer to products or services offered by the organization or person." ;
        rdfs:label    "makesOffer" .

schema:arrivalAirport
        rdf:type      rdf:Property ;
        rdfs:comment  "The airport where the flight terminates." ;
        rdfs:label    "arrivalAirport" .

schema:gtin12  rdf:type     rdf:Property ;
        rdfs:comment        "The GTIN-12 code of the product, or the product to which the offer refers. The GTIN-12 is the 12-digit GS1 Identification Key composed of a U.P.C. Company Prefix, Item Reference, and Check Digit used to identify trade items. See [GS1 GTIN Summary](http://www.gs1.org/barcodes/technical/idkeys/gtin) for more details." ;
        rdfs:label          "gtin12" ;
        rdfs:subPropertyOf  schema:identifier , schema:gtin .

schema:FireStation  rdf:type  rdfs:Class ;
        rdfs:comment     "A fire station. With firemen." ;
        rdfs:label       "FireStation" ;
        rdfs:subClassOf  schema:CivicStructure , schema:EmergencyService .

schema:byDay  rdf:type  rdf:Property ;
        rdfs:comment  "Defines the day(s) of the week on which a recurring [[Event]] takes place. May be specified using either [[DayOfWeek]], or alternatively [[Text]] conforming to iCal's syntax for byDay recurrence rules." ;
        rdfs:label    "byDay" .

schema:printSection  rdf:type  rdf:Property ;
        rdfs:comment  "If this NewsArticle appears in print, this field indicates the print section in which the article appeared." ;
        rdfs:label    "printSection" .

schema:liveBlogUpdate
        rdf:type      rdf:Property ;
        rdfs:comment  "An update to the LiveBlog." ;
        rdfs:label    "liveBlogUpdate" .

schema:alternativeHeadline
        rdf:type      rdf:Property ;
        rdfs:comment  "A secondary title of the CreativeWork." ;
        rdfs:label    "alternativeHeadline" .

schema:PublicationVolume
        rdf:type         rdfs:Class ;
        rdfs:comment     "A part of a successively published publication such as a periodical or multi-volume work, often numbered. It may represent a time span, such as a year.\\n\\nSee also [blog post](http://blog.schema.org/2014/09/schemaorg-support-for-bibliographic_2.html)." ;
        rdfs:label       "PublicationVolume" ;
        rdfs:subClassOf  schema:CreativeWork .

schema:amountOfThisGood
        rdf:type      rdf:Property ;
        rdfs:comment  "The quantity of the goods included in the offer." ;
        rdfs:label    "amountOfThisGood" .

schema:OpinionNewsArticle
        rdf:type         rdfs:Class ;
        rdfs:comment     "An [[OpinionNewsArticle]] is a [[NewsArticle]] that primarily expresses opinions rather than journalistic reporting of news and events. For example, a [[NewsArticle]] consisting of a column or [[Blog]]/[[BlogPosting]] entry in the Opinions section of a news publication. " ;
        rdfs:label       "OpinionNewsArticle" ;
        rdfs:subClassOf  schema:NewsArticle .

schema:containsPlace  rdf:type  rdf:Property ;
        rdfs:comment  "The basic containment relation between a place and another that it contains." ;
        rdfs:label    "containsPlace" .

schema:fileFormat  rdf:type  rdf:Property ;
        rdfs:comment  "Media type, typically MIME format (see [IANA site](http://www.iana.org/assignments/media-types/media-types.xhtml)) of the content e.g. application/zip of a SoftwareApplication binary. In cases where a CreativeWork has several media type representations, 'encoding' can be used to indicate each MediaObject alongside particular fileFormat information. Unregistered or niche file formats can be indicated instead via the most appropriate URL, e.g. defining Web page or a Wikipedia entry." ;
        rdfs:label    "fileFormat" .

schema:mealService  rdf:type  rdf:Property ;
        rdfs:comment  "Description of the meals that will be provided or available for purchase." ;
        rdfs:label    "mealService" .

schema:pathophysiology
        rdf:type      rdf:Property ;
        rdfs:comment  "Changes in the normal mechanical, physical, and biochemical functions that are associated with this activity or condition." ;
        rdfs:label    "pathophysiology" .

schema:Invoice  rdf:type  rdfs:Class ;
        rdfs:comment     "A statement of the money due for goods or services; a bill." ;
        rdfs:label       "Invoice" ;
        rdfs:subClassOf  schema:Intangible .

schema:mediaAuthenticityCategory
        rdf:type      rdf:Property ;
        rdfs:comment  "Indicates a MediaManipulationRatingEnumeration classification of a media object (in the context of how it was published or shared)." ;
        rdfs:label    "mediaAuthenticityCategory" .

schema:ApplyAction  rdf:type  rdfs:Class ;
        rdfs:comment     "The act of registering to an organization/service without the guarantee to receive it.\\n\\nRelated actions:\\n\\n* [[RegisterAction]]: Unlike RegisterAction, ApplyAction has no guarantees that the application will be accepted." ;
        rdfs:label       "ApplyAction" ;
        rdfs:subClassOf  schema:OrganizeAction .

schema:ComicIssue  rdf:type  rdfs:Class ;
        rdfs:comment     "Individual comic issues are serially published as\n    \tpart of a larger series. For the sake of consistency, even one-shot issues\n    \tbelong to a series comprised of a single issue. All comic issues can be\n    \tuniquely identified by: the combination of the name and volume number of the\n    \tseries to which the issue belongs; the issue number; and the variant\n    \tdescription of the issue (if any)." ;
        rdfs:label       "ComicIssue" ;
        rdfs:subClassOf  schema:PublicationIssue .

schema:breadcrumb  rdf:type  rdf:Property ;
        rdfs:comment  "A set of links that can help a user understand and navigate a website hierarchy." ;
        rdfs:label    "breadcrumb" .

schema:Geriatric  rdf:type  rdfs:Class ;
        rdfs:comment     "A specific branch of medical science that is concerned with the diagnosis and treatment of diseases, debilities and provision of care to the aged." ;
        rdfs:label       "Geriatric" ;
        rdfs:subClassOf  schema:MedicalBusiness .

schema:priceComponent
        rdf:type      rdf:Property ;
        rdfs:comment  "This property links to all [[UnitPriceSpecification]] nodes that apply in parallel for the [[CompoundPriceSpecification]] node." ;
        rdfs:label    "priceComponent" .

schema:contentSize  rdf:type  rdf:Property ;
        rdfs:comment  "File size in (mega/kilo) bytes." ;
        rdfs:label    "contentSize" .

schema:attendees  rdf:type  rdf:Property ;
        rdfs:comment  "A person attending the event." ;
        rdfs:label    "attendees" .

schema:webFeed  rdf:type  rdf:Property ;
        rdfs:comment  "The URL for a feed, e.g. associated with a podcast series, blog, or series of date-stamped updates. This is usually RSS or Atom." ;
        rdfs:label    "webFeed" .

schema:pattern  rdf:type  rdf:Property ;
        rdfs:comment  "A pattern that something has, for example 'polka dot', 'striped', 'Canadian flag'. Values are typically expressed as text, although links to controlled value schemes are also supported." ;
        rdfs:label    "pattern" .

schema:availableService
        rdf:type      rdf:Property ;
        rdfs:comment  "A medical service available from this provider." ;
        rdfs:label    "availableService" .

schema:MovieTheater  rdf:type  rdfs:Class ;
        rdfs:comment     "A movie theater." ;
        rdfs:label       "MovieTheater" ;
        rdfs:subClassOf  schema:EntertainmentBusiness , schema:CivicStructure .

schema:lyricist  rdf:type  rdf:Property ;
        rdfs:comment  "The person who wrote the words." ;
        rdfs:label    "lyricist" .

schema:PlanAction  rdf:type  rdfs:Class ;
        rdfs:comment     "The act of planning the execution of an event/task/action/reservation/plan to a future date." ;
        rdfs:label       "PlanAction" ;
        rdfs:subClassOf  schema:OrganizeAction .

schema:minPrice  rdf:type  rdf:Property ;
        rdfs:comment  "The lowest price if the price is a range." ;
        rdfs:label    "minPrice" .

schema:cvdNumVentUse  rdf:type  rdf:Property ;
        rdfs:comment  "numventuse - MECHANICAL VENTILATORS IN USE: Total number of ventilators in use." ;
        rdfs:label    "cvdNumVentUse" .

schema:UserComments  rdf:type  rdfs:Class ;
        rdfs:comment     "UserInteraction and its subtypes is an old way of talking about users interacting with pages. It is generally better to use [[Action]]-based vocabulary, alongside types such as [[Comment]]." ;
        rdfs:label       "UserComments" ;
        rdfs:subClassOf  schema:UserInteraction .

schema:PublicationIssue
        rdf:type         rdfs:Class ;
        rdfs:comment     "A part of a successively published publication such as a periodical or publication volume, often numbered, usually containing a grouping of works such as articles.\\n\\nSee also [blog post](http://blog.schema.org/2014/09/schemaorg-support-for-bibliographic_2.html)." ;
        rdfs:label       "PublicationIssue" ;
        rdfs:subClassOf  schema:CreativeWork .

schema:XPathType  rdf:type  rdfs:Class ;
        rdfs:comment     "Text representing an XPath (typically but not necessarily version 1.0)." ;
        rdfs:label       "XPathType" ;
        rdfs:subClassOf  schema:Text .

skos:editorialNote  rdf:type  rdf:Property ;
        rdfs:label          "editorial note"@en ;
        rdfs:subPropertyOf  skos:note .

schema:Distance  rdf:type  rdfs:Class ;
        rdfs:comment     "Properties that take Distances as values are of the form '&lt;Number&gt; &lt;Length unit of measure&gt;'. E.g., '7 ft'." ;
        rdfs:label       "Distance" ;
        rdfs:subClassOf  schema:Quantity .

schema:valueRequired  rdf:type  rdf:Property ;
        rdfs:comment  "Whether the property must be filled in to complete the action.  Default is false." ;
        rdfs:label    "valueRequired" .

schema:studyDesign  rdf:type  rdf:Property ;
        rdfs:comment  "Specifics about the observational study design (enumerated)." ;
        rdfs:label    "studyDesign" .

schema:publishingPrinciples
        rdf:type      rdf:Property ;
        rdfs:comment  "The publishingPrinciples property indicates (typically via [[URL]]) a document describing the editorial principles of an [[Organization]] (or individual e.g. a [[Person]] writing a blog) that relate to their activities as a publisher, e.g. ethics or diversity policies. When applied to a [[CreativeWork]] (e.g. [[NewsArticle]]) the principles are those of the party primarily responsible for the creation of the [[CreativeWork]].\n\nWhile such policies are most typically expressed in natural language, sometimes related information (e.g. indicating a [[funder]]) can be expressed using schema.org terminology.\n" ;
        rdfs:label    "publishingPrinciples" .

schema:HousePainter  rdf:type  rdfs:Class ;
        rdfs:comment     "A house painting service." ;
        rdfs:label       "HousePainter" ;
        rdfs:subClassOf  schema:HomeAndConstructionBusiness .

schema:GovernmentPermit
        rdf:type         rdfs:Class ;
        rdfs:comment     "A permit issued by a government agency." ;
        rdfs:label       "GovernmentPermit" ;
        rdfs:subClassOf  schema:Permit .

schema:mileageFromOdometer
        rdf:type      rdf:Property ;
        rdfs:comment  "The total distance travelled by the particular vehicle since its initial production, as read from its odometer.\\n\\nTypical unit code(s): KMT for kilometers, SMI for statute miles" ;
        rdfs:label    "mileageFromOdometer" .

schema:vehicleInteriorType
        rdf:type      rdf:Property ;
        rdfs:comment  "The type or material of the interior of the vehicle (e.g. synthetic fabric, leather, wood, etc.). While most interior types are characterized by the material used, an interior type can also be based on vehicle usage or target audience." ;
        rdfs:label    "vehicleInteriorType" .

schema:AcceptAction  rdf:type  rdfs:Class ;
        rdfs:comment     "The act of committing to/adopting an object.\\n\\nRelated actions:\\n\\n* [[RejectAction]]: The antonym of AcceptAction." ;
        rdfs:label       "AcceptAction" ;
        rdfs:subClassOf  schema:AllocateAction .

schema:geoIntersects  rdf:type  rdf:Property ;
        rdfs:comment  "Represents spatial relations in which two geometries (or the places they represent) have at least one point in common. As defined in [DE-9IM](https://en.wikipedia.org/wiki/DE-9IM)." ;
        rdfs:label    "geoIntersects" .

schema:dateRead  rdf:type  rdf:Property ;
        rdfs:comment  "The date/time at which the message has been read by the recipient if a single recipient exists." ;
        rdfs:label    "dateRead" .

schema:Podiatric  rdf:type  rdfs:Class ;
        rdfs:comment     "Podiatry is the care of the human foot, especially the diagnosis and treatment of foot disorders." ;
        rdfs:label       "Podiatric" ;
        rdfs:subClassOf  schema:MedicalBusiness .

schema:sender  rdf:type     rdf:Property ;
        rdfs:comment        "A sub property of participant. The participant who is at the sending end of the action." ;
        rdfs:label          "sender" ;
        rdfs:subPropertyOf  schema:participant .

schema:Hospital  rdf:type  rdfs:Class ;
        rdfs:comment     "A hospital." ;
        rdfs:label       "Hospital" ;
        rdfs:subClassOf  schema:CivicStructure , schema:MedicalOrganization , schema:EmergencyService .

schema:comprisedOf  rdf:type  rdf:Property ;
        rdfs:comment  "Specifying something physically contained by something else. Typically used here for the underlying anatomical structures, such as organs, that comprise the anatomical system." ;
        rdfs:label    "comprisedOf" .

schema:priceSpecification
        rdf:type      rdf:Property ;
        rdfs:comment  "One or more detailed price specifications, indicating the unit price and delivery or payment charges." ;
        rdfs:label    "priceSpecification" .

schema:Artery  rdf:type  rdfs:Class ;
        rdfs:comment     "A type of blood vessel that specifically carries blood away from the heart." ;
        rdfs:label       "Artery" ;
        rdfs:subClassOf  schema:Vessel .

schema:MonetaryAmountDistribution
        rdf:type         rdfs:Class ;
        rdfs:comment     "A statistical distribution of monetary amounts." ;
        rdfs:label       "MonetaryAmountDistribution" ;
        rdfs:subClassOf  schema:QuantitativeValueDistribution .

schema:UserPlusOnes  rdf:type  rdfs:Class ;
        rdfs:comment     "UserInteraction and its subtypes is an old way of talking about users interacting with pages. It is generally better to use [[Action]]-based vocabulary, alongside types such as [[Comment]]." ;
        rdfs:label       "UserPlusOnes" ;
        rdfs:subClassOf  schema:UserInteraction .

schema:tool  rdf:type       rdf:Property ;
        rdfs:comment        "A sub property of instrument. An object used (but not consumed) when performing instructions or a direction." ;
        rdfs:label          "tool" ;
        rdfs:subPropertyOf  schema:instrument .

schema:answerExplanation
        rdf:type      rdf:Property ;
        rdfs:comment  "A step-by-step or full explanation about Answer. Can outline how this Answer was achieved or contain more broad clarification or statement about it. " ;
        rdfs:label    "answerExplanation" .

schema:publishedOn  rdf:type  rdf:Property ;
        rdfs:comment  "A broadcast service associated with the publication event." ;
        rdfs:label    "publishedOn" .

schema:numberOfBeds  rdf:type  rdf:Property ;
        rdfs:comment  "The quantity of the given bed type available in the HotelRoom, Suite, House, or Apartment." ;
        rdfs:label    "numberOfBeds" .

schema:endTime  rdf:type  rdf:Property ;
        rdfs:comment  "The endTime of something. For a reserved event or service (e.g. FoodEstablishmentReservation), the time that it is expected to end. For actions that span a period of time, when the action was performed. e.g. John wrote a book from January to *December*. For media, including audio and video, it's the time offset of the end of a clip within a larger file.\\n\\nNote that Event uses startDate/endDate instead of startTime/endTime, even when describing dates with times. This situation may be clarified in future revisions." ;
        rdfs:label    "endTime" .

schema:lyrics  rdf:type  rdf:Property ;
        rdfs:comment  "The words in the song." ;
        rdfs:label    "lyrics" .

schema:RejectAction  rdf:type  rdfs:Class ;
        rdfs:comment     "The act of rejecting to/adopting an object.\\n\\nRelated actions:\\n\\n* [[AcceptAction]]: The antonym of RejectAction." ;
        rdfs:label       "RejectAction" ;
        rdfs:subClassOf  schema:AllocateAction .

schema:Motel  rdf:type   rdfs:Class ;
        rdfs:comment     "A motel.\n<br /><br />\nSee also the <a href=\"/docs/hotels.html\">dedicated document on the use of schema.org for marking up hotels and other forms of accommodations</a>.\n" ;
        rdfs:label       "Motel" ;
        rdfs:subClassOf  schema:LodgingBusiness .

schema:BookSeries  rdf:type  rdfs:Class ;
        rdfs:comment     "A series of books. Included books can be indicated with the hasPart property." ;
        rdfs:label       "BookSeries" ;
        rdfs:subClassOf  schema:CreativeWorkSeries .

schema:issn  rdf:type       rdf:Property ;
        rdfs:comment        "The International Standard Serial Number (ISSN) that identifies this serial publication. You can repeat this property to identify different formats of, or the linking ISSN (ISSN-L) for, this serial publication." ;
        rdfs:label          "issn" ;
        rdfs:subPropertyOf  schema:identifier .

schema:expectedArrivalUntil
        rdf:type      rdf:Property ;
        rdfs:comment  "The latest date the package may arrive." ;
        rdfs:label    "expectedArrivalUntil" .

schema:measuredProperty
        rdf:type      rdf:Property ;
        rdfs:comment  "The measuredProperty of an [[Observation]], either a schema.org property, a property from other RDF-compatible systems e.g. W3C RDF Data Cube, or schema.org extensions such as [GS1's](https://www.gs1.org/voc/?show=properties)." ;
        rdfs:label    "measuredProperty" .

schema:educationalAlignment
        rdf:type      rdf:Property ;
        rdfs:comment  "An alignment to an established educational framework.\n\nThis property should not be used where the nature of the alignment can be described using a simple property, for example to express that a resource [[teaches]] or [[assesses]] a competency." ;
        rdfs:label    "educationalAlignment" .

schema:resultReview  rdf:type  rdf:Property ;
        rdfs:comment        "A sub property of result. The review that resulted in the performing of the action." ;
        rdfs:label          "resultReview" ;
        rdfs:subPropertyOf  schema:result .

schema:arrivalTerminal
        rdf:type      rdf:Property ;
        rdfs:comment  "Identifier of the flight's arrival terminal." ;
        rdfs:label    "arrivalTerminal" .

schema:providesService
        rdf:type      rdf:Property ;
        rdfs:comment  "The service provided by this channel." ;
        rdfs:label    "providesService" .

schema:eventSchedule  rdf:type  rdf:Property ;
        rdfs:comment  "Associates an [[Event]] with a [[Schedule]]. There are circumstances where it is preferable to share a schedule for a series of\n      repeating events rather than data on the individual events themselves. For example, a website or application might prefer to publish a schedule for a weekly\n      gym class rather than provide data on every event. A schedule could be processed by applications to add forthcoming events to a calendar. An [[Event]] that\n      is associated with a [[Schedule]] using this property should not have [[startDate]] or [[endDate]] properties. These are instead defined within the associated\n      [[Schedule]], this avoids any ambiguity for clients using the data. The property might have repeated values to specify different schedules, e.g. for different months\n      or seasons." ;
        rdfs:label    "eventSchedule" .

schema:assemblyVersion
        rdf:type      rdf:Property ;
        rdfs:comment  "Associated product/technology version. e.g., .NET Framework 4.5." ;
        rdfs:label    "assemblyVersion" .

schema:videoQuality  rdf:type  rdf:Property ;
        rdfs:comment  "The quality of the video." ;
        rdfs:label    "videoQuality" .

schema:worstRating  rdf:type  rdf:Property ;
        rdfs:comment  "The lowest value allowed in this rating system. If worstRating is omitted, 1 is assumed." ;
        rdfs:label    "worstRating" .

schema:PaymentCard  rdf:type  rdfs:Class ;
        rdfs:comment     "A payment method using a credit, debit, store or other card to associate the payment with an account." ;
        rdfs:label       "PaymentCard" ;
        rdfs:subClassOf  schema:PaymentMethod , schema:FinancialProduct .

foaf:Person  rdf:type  rdfs:Class .

schema:ChildrensEvent
        rdf:type         rdfs:Class ;
        rdfs:comment     "Event type: Children's event." ;
        rdfs:label       "ChildrensEvent" ;
        rdfs:subClassOf  schema:Event .

schema:hasMenu  rdf:type  rdf:Property ;
        rdfs:comment  "Either the actual menu as a structured representation, as text, or a URL of the menu." ;
        rdfs:label    "hasMenu" .

schema:HyperToc  rdf:type  rdfs:Class ;
        rdfs:comment     "A HyperToc represents a hypertext table of contents for complex media objects, such as [[VideoObject]], [[AudioObject]]. Items in the table of contents are indicated using the [[tocEntry]] property, and typed [[HyperTocEntry]]. For cases where the same larger work is split into multiple files, [[associatedMedia]] can be used on individual [[HyperTocEntry]] items." ;
        rdfs:label       "HyperToc" ;
        rdfs:subClassOf  schema:CreativeWork .

schema:recordedAt  rdf:type  rdf:Property ;
        rdfs:comment  "The Event where the CreativeWork was recorded. The CreativeWork may capture all or part of the event." ;
        rdfs:label    "recordedAt" .

schema:arrivalBoatTerminal
        rdf:type      rdf:Property ;
        rdfs:comment  "The terminal or port from which the boat arrives." ;
        rdfs:label    "arrivalBoatTerminal" .

schema:mainContentOfPage
        rdf:type      rdf:Property ;
        rdfs:comment  "Indicates if this web page element is the main subject of the page." ;
        rdfs:label    "mainContentOfPage" .

schema:Attorney  rdf:type  rdfs:Class ;
        rdfs:comment     "Professional service: Attorney. \\n\\nThis type is deprecated - [[LegalService]] is more inclusive and less ambiguous." ;
        rdfs:label       "Attorney" ;
        rdfs:subClassOf  schema:LegalService .

schema:spouse  rdf:type  rdf:Property ;
        rdfs:comment  "The person's spouse." ;
        rdfs:label    "spouse" .

schema:recordLabel  rdf:type  rdf:Property ;
        rdfs:comment  "The label that issued the release." ;
        rdfs:label    "recordLabel" .

schema:numberOfSeasons
        rdf:type      rdf:Property ;
        rdfs:comment  "The number of seasons in this series." ;
        rdfs:label    "numberOfSeasons" .

schema:MobileApplication
        rdf:type         rdfs:Class ;
        rdfs:comment     "A software application designed specifically to work well on a mobile device such as a telephone." ;
        rdfs:label       "MobileApplication" ;
        rdfs:subClassOf  schema:SoftwareApplication .

schema:ContactPoint  rdf:type  rdfs:Class ;
        rdfs:comment     "A contact point&#x2014;for example, a Customer Complaints department." ;
        rdfs:label       "ContactPoint" ;
        rdfs:subClassOf  schema:StructuredValue .

schema:nextItem  rdf:type  rdf:Property ;
        rdfs:comment  "A link to the ListItem that follows the current one." ;
        rdfs:label    "nextItem" .

schema:InteractAction
        rdf:type         rdfs:Class ;
        rdfs:comment     "The act of interacting with another person or organization." ;
        rdfs:label       "InteractAction" ;
        rdfs:subClassOf  schema:Action .

schema:costOrigin  rdf:type  rdf:Property ;
        rdfs:comment  "Additional details to capture the origin of the cost data. For example, 'Medicare Part B'." ;
        rdfs:label    "costOrigin" .

schema:cutoffTime  rdf:type  rdf:Property ;
        rdfs:comment  "Order cutoff time allows merchants to describe the time after which they will no longer process orders received on that day. For orders processed after cutoff time, one day gets added to the delivery time estimate. This property is expected to be most typically used via the [[ShippingRateSettings]] publication pattern. The time is indicated using the ISO-8601 Time format, e.g. \"23:30:00-05:00\" would represent 6:30 pm Eastern Standard Time (EST) which is 5 hours behind Coordinated Universal Time (UTC)." ;
        rdfs:label    "cutoffTime" .

schema:deliveryAddress
        rdf:type      rdf:Property ;
        rdfs:comment  "Destination address." ;
        rdfs:label    "deliveryAddress" .

schema:MedicalAudienceType
        rdf:type         rdfs:Class ;
        rdfs:comment     "Target audiences types for medical web pages. Enumerated type." ;
        rdfs:label       "MedicalAudienceType" ;
        rdfs:subClassOf  schema:MedicalEnumeration .

schema:DrugLegalStatus
        rdf:type         rdfs:Class ;
        rdfs:comment     "The legal availability status of a medical drug." ;
        rdfs:label       "DrugLegalStatus" ;
        rdfs:subClassOf  schema:MedicalIntangible .

schema:softwareHelp  rdf:type  rdf:Property ;
        rdfs:comment  "Software application help." ;
        rdfs:label    "softwareHelp" .

schema:SubwayStation  rdf:type  rdfs:Class ;
        rdfs:comment     "A subway station." ;
        rdfs:label       "SubwayStation" ;
        rdfs:subClassOf  schema:CivicStructure .

schema:valueMinLength
        rdf:type      rdf:Property ;
        rdfs:comment  "Specifies the minimum allowed range for number of characters in a literal value." ;
        rdfs:label    "valueMinLength" .

schema:FollowAction  rdf:type  rdfs:Class ;
        rdfs:comment     "The act of forming a personal connection with someone/something (object) unidirectionally/asymmetrically to get updates polled from.\\n\\nRelated actions:\\n\\n* [[BefriendAction]]: Unlike BefriendAction, FollowAction implies that the connection is *not* necessarily reciprocal.\\n* [[SubscribeAction]]: Unlike SubscribeAction, FollowAction implies that the follower acts as an active agent constantly/actively polling for updates.\\n* [[RegisterAction]]: Unlike RegisterAction, FollowAction implies that the agent is interested in continuing receiving updates from the object.\\n* [[JoinAction]]: Unlike JoinAction, FollowAction implies that the agent is interested in getting updates from the object.\\n* [[TrackAction]]: Unlike TrackAction, FollowAction refers to the polling of updates of all aspects of animate objects rather than the location of inanimate objects (e.g. you track a package, but you don't follow it)." ;
        rdfs:label       "FollowAction" ;
        rdfs:subClassOf  schema:InteractAction .

schema:speakable  rdf:type  rdf:Property ;
        rdfs:comment  "Indicates sections of a Web page that are particularly 'speakable' in the sense of being highlighted as being especially appropriate for text-to-speech conversion. Other sections of a page may also be usefully spoken in particular circumstances; the 'speakable' property serves to indicate the parts most likely to be generally useful for speech.\n\nThe *speakable* property can be repeated an arbitrary number of times, with three kinds of possible 'content-locator' values:\n\n1.) *id-value* URL references - uses *id-value* of an element in the page being annotated. The simplest use of *speakable* has (potentially relative) URL values, referencing identified sections of the document concerned.\n\n2.) CSS Selectors - addresses content in the annotated page, eg. via class attribute. Use the [[cssSelector]] property.\n\n3.)  XPaths - addresses content via XPaths (assuming an XML view of the content). Use the [[xpath]] property.\n\n\nFor more sophisticated markup of speakable sections beyond simple ID references, either CSS selectors or XPath expressions to pick out document section(s) as speakable. For this\nwe define a supporting type, [[SpeakableSpecification]]  which is defined to be a possible value of the *speakable* property.\n         " ;
        rdfs:label    "speakable" .

schema:includedRiskFactor
        rdf:type      rdf:Property ;
        rdfs:comment  "A modifiable or non-modifiable risk factor included in the calculation, e.g. age, coexisting condition." ;
        rdfs:label    "includedRiskFactor" .

schema:typicalTest  rdf:type  rdf:Property ;
        rdfs:comment  "A medical test typically performed given this condition." ;
        rdfs:label    "typicalTest" .

schema:material  rdf:type  rdf:Property ;
        rdfs:comment  "A material that something is made from, e.g. leather, wool, cotton, paper." ;
        rdfs:label    "material" .

schema:editEIDR  rdf:type   rdf:Property ;
        rdfs:comment        "An [EIDR](https://eidr.org/) (Entertainment Identifier Registry) [[identifier]] representing a specific edit / edition for a work of film or television.\n\nFor example, the motion picture known as \"Ghostbusters\" whose [[titleEIDR]] is \"10.5240/7EC7-228A-510A-053E-CBB8-J\", has several edits e.g. \"10.5240/1F2A-E1C5-680A-14C6-E76B-I\" and \"10.5240/8A35-3BEE-6497-5D12-9E4F-3\".\n\nSince schema.org types like [[Movie]] and [[TVEpisode]] can be used for both works and their multiple expressions, it is possible to use [[titleEIDR]] alone (for a general description), or alongside [[editEIDR]] for a more edit-specific description.\n" ;
        rdfs:label          "editEIDR" ;
        rdfs:subPropertyOf  schema:identifier .

schema:Oncologic  rdf:type  rdfs:Class ;
        rdfs:comment     "A specific branch of medical science that deals with benign and malignant tumors, including the study of their development, diagnosis, treatment and prevention." ;
        rdfs:label       "Oncologic" ;
        rdfs:subClassOf  schema:MedicalBusiness .

schema:Product  rdf:type  rdfs:Class ;
        rdfs:comment     "Any offered product or service. For example: a pair of shoes; a concert ticket; the rental of a car; a haircut; or an episode of a TV show streamed online." ;
        rdfs:label       "Product" ;
        rdfs:subClassOf  schema:Thing .

schema:unitCode  rdf:type  rdf:Property ;
        rdfs:comment  "The unit of measurement given using the UN/CEFACT Common Code (3 characters) or a URL. Other codes than the UN/CEFACT Common Code may be used with a prefix followed by a colon." ;
        rdfs:label    "unitCode" .

schema:subStageSuffix
        rdf:type      rdf:Property ;
        rdfs:comment  "The substage, e.g. 'a' for Stage IIIa." ;
        rdfs:label    "subStageSuffix" .

schema:isConsumableFor
        rdf:type      rdf:Property ;
        rdfs:comment  "A pointer to another product (or multiple products) for which this product is a consumable." ;
        rdfs:label    "isConsumableFor" .

schema:DataFeed  rdf:type  rdfs:Class ;
        rdfs:comment     "A single feed providing structured information about one or more entities or topics." ;
        rdfs:label       "DataFeed" ;
        rdfs:subClassOf  schema:Dataset .

schema:productSupported
        rdf:type      rdf:Property ;
        rdfs:comment  "The product or service this support contact point is related to (such as product support for a particular product line). This can be a specific product or product line (e.g. \"iPhone\") or a general category of products or services (e.g. \"smartphones\")." ;
        rdfs:label    "productSupported" .

schema:exerciseRelatedDiet
        rdf:type            rdf:Property ;
        rdfs:comment        "A sub property of instrument. The diet used in this action." ;
        rdfs:label          "exerciseRelatedDiet" ;
        rdfs:subPropertyOf  schema:instrument .

schema:RealEstateListing
        rdf:type         rdfs:Class ;
        rdfs:comment     "A [[RealEstateListing]] is a listing that describes one or more real-estate [[Offer]]s (whose [[businessFunction]] is typically to lease out, or to sell).\n  The [[RealEstateListing]] type itself represents the overall listing, as manifested in some [[WebPage]].\n  " ;
        rdfs:label       "RealEstateListing" ;
        rdfs:subClassOf  schema:WebPage .

schema:DietarySupplement
        rdf:type         rdfs:Class ;
        rdfs:comment     "A product taken by mouth that contains a dietary ingredient intended to supplement the diet. Dietary ingredients may include vitamins, minerals, herbs or other botanicals, amino acids, and substances such as enzymes, organ tissues, glandulars and metabolites." ;
        rdfs:label       "DietarySupplement" ;
        rdfs:subClassOf  schema:Substance .

schema:instrument  rdf:type  rdf:Property ;
        rdfs:comment  "The object that helped the agent perform the action. e.g. John wrote a book with *a pen*." ;
        rdfs:label    "instrument" .

schema:PeopleAudience
        rdf:type         rdfs:Class ;
        rdfs:comment     "A set of characteristics belonging to people, e.g. who compose an item's target audience." ;
        rdfs:label       "PeopleAudience" ;
        rdfs:subClassOf  schema:Audience .

schema:ccRecipient  rdf:type  rdf:Property ;
        rdfs:comment        "A sub property of recipient. The recipient copied on a message." ;
        rdfs:label          "ccRecipient" ;
        rdfs:subPropertyOf  schema:recipient .

schema:MedicalIndication
        rdf:type         rdfs:Class ;
        rdfs:comment     "A condition or factor that indicates use of a medical therapy, including signs, symptoms, risk factors, anatomical states, etc." ;
        rdfs:label       "MedicalIndication" ;
        rdfs:subClassOf  schema:MedicalEntity .

schema:UserTweets  rdf:type  rdfs:Class ;
        rdfs:comment     "UserInteraction and its subtypes is an old way of talking about users interacting with pages. It is generally better to use [[Action]]-based vocabulary, alongside types such as [[Comment]]." ;
        rdfs:label       "UserTweets" ;
        rdfs:subClassOf  schema:UserInteraction .

skos:narrowerTransitive
        rdf:type            owl:ObjectProperty ;
        rdfs:label          "has narrower transitive"@en ;
        rdfs:subPropertyOf  skos:semanticRelation ;
        owl:inverseOf       skos:broaderTransitive .

schema:Question  rdf:type  rdfs:Class ;
        rdfs:comment     "A specific question - e.g. from a user seeking answers online, or collected in a Frequently Asked Questions (FAQ) document." ;
        rdfs:label       "Question" ;
        rdfs:subClassOf  schema:Comment .

schema:ownedThrough  rdf:type  rdf:Property ;
        rdfs:comment  "The date and time of giving up ownership on the product." ;
        rdfs:label    "ownedThrough" .

schema:acceptsReservations
        rdf:type      rdf:Property ;
        rdfs:comment  "Indicates whether a FoodEstablishment accepts reservations. Values can be Boolean, an URL at which reservations can be made or (for backwards compatibility) the strings ```Yes``` or ```No```." ;
        rdfs:label    "acceptsReservations" .

schema:MusicReleaseFormatType
        rdf:type         rdfs:Class ;
        rdfs:comment     "Format of this release (the type of recording media used, ie. compact disc, digital media, LP, etc.)." ;
        rdfs:label       "MusicReleaseFormatType" ;
        rdfs:subClassOf  schema:Enumeration .

schema:SingleFamilyResidence
        rdf:type         rdfs:Class ;
        rdfs:comment     "Residence type: Single-family home." ;
        rdfs:label       "SingleFamilyResidence" ;
        rdfs:subClassOf  schema:House .

schema:gettingTestedInfo
        rdf:type      rdf:Property ;
        rdfs:comment  "Information about getting tested (for a [[MedicalCondition]]), e.g. in the context of a pandemic." ;
        rdfs:label    "gettingTestedInfo" .

schema:acrissCode  rdf:type  rdf:Property ;
        rdfs:comment  "The ACRISS Car Classification Code is a code used by many car rental companies, for classifying vehicles. ACRISS stands for Association of Car Rental Industry Systems and Standards." ;
        rdfs:label    "acrissCode" .

schema:duplicateTherapy
        rdf:type      rdf:Property ;
        rdfs:comment  "A therapy that duplicates or overlaps this one." ;
        rdfs:label    "duplicateTherapy" .

schema:MedicalSpecialty
        rdf:type         rdfs:Class ;
        rdfs:comment     "Any specific branch of medical science or practice. Medical specialities include clinical specialties that pertain to particular organ systems and their respective disease states, as well as allied health specialties. Enumerated type." ;
        rdfs:label       "MedicalSpecialty" ;
        rdfs:subClassOf  schema:MedicalEnumeration , schema:Specialty .

schema:healthPlanId  rdf:type  rdf:Property ;
        rdfs:comment  "The 14-character, HIOS-generated Plan ID number. (Plan IDs must be unique, even across different markets.)" ;
        rdfs:label    "healthPlanId" .

schema:releasedEvent  rdf:type  rdf:Property ;
        rdfs:comment  "The place and time the release was issued, expressed as a PublicationEvent." ;
        rdfs:label    "releasedEvent" .

schema:Intangible  rdf:type  rdfs:Class ;
        rdfs:comment     "A utility class that serves as the umbrella for a number of 'intangible' things such as quantities, structured values, etc." ;
        rdfs:label       "Intangible" ;
        rdfs:subClassOf  schema:Thing .

schema:cvdFacilityId  rdf:type  rdf:Property ;
        rdfs:comment  "Identifier of the NHSN facility that this data record applies to. Use [[cvdFacilityCounty]] to indicate the county. To provide other details, [[healthcareReportingData]] can be used on a [[Hospital]] entry." ;
        rdfs:label    "cvdFacilityId" .

schema:Reservoir  rdf:type  rdfs:Class ;
        rdfs:comment     "A reservoir of water, typically an artificially created lake, like the Lake Kariba reservoir." ;
        rdfs:label       "Reservoir" ;
        rdfs:subClassOf  schema:BodyOfWater .

schema:InstallAction  rdf:type  rdfs:Class ;
        rdfs:comment     "The act of installing an application." ;
        rdfs:label       "InstallAction" ;
        rdfs:subClassOf  schema:ConsumeAction .

schema:adverseOutcome
        rdf:type      rdf:Property ;
        rdfs:comment  "A possible complication and/or side effect of this therapy. If it is known that an adverse outcome is serious (resulting in death, disability, or permanent damage; requiring hospitalization; or is otherwise life-threatening or requires immediate medical attention), tag it as a seriouseAdverseOutcome instead." ;
        rdfs:label    "adverseOutcome" .

schema:language  rdf:type   rdf:Property ;
        rdfs:comment        "A sub property of instrument. The language used on this action." ;
        rdfs:label          "language" ;
        rdfs:subPropertyOf  schema:instrument .

schema:ComputerStore  rdf:type  rdfs:Class ;
        rdfs:comment     "A computer store." ;
        rdfs:label       "ComputerStore" ;
        rdfs:subClassOf  schema:Store .

schema:MusicVenue  rdf:type  rdfs:Class ;
        rdfs:comment     "A music venue." ;
        rdfs:label       "MusicVenue" ;
        rdfs:subClassOf  schema:CivicStructure .

schema:layoutImage  rdf:type  rdf:Property ;
        rdfs:comment        "A schematic image showing the floorplan layout." ;
        rdfs:label          "layoutImage" ;
        rdfs:subPropertyOf  schema:image .

schema:BoatTrip  rdf:type  rdfs:Class ;
        rdfs:comment     "A trip on a commercial ferry line." ;
        rdfs:label       "BoatTrip" ;
        rdfs:subClassOf  schema:Trip .

schema:Specialty  rdf:type  rdfs:Class ;
        rdfs:comment     "Any branch of a field in which people typically develop specific expertise, usually after significant study, time, and effort." ;
        rdfs:label       "Specialty" ;
        rdfs:subClassOf  schema:Enumeration .

schema:Joint  rdf:type   rdfs:Class ;
        rdfs:comment     "The anatomical location at which two or more bones make contact." ;
        rdfs:label       "Joint" ;
        rdfs:subClassOf  schema:AnatomicalStructure .

schema:sdDatePublished
        rdf:type      rdf:Property ;
        rdfs:comment  "Indicates the date on which the current structured data was generated / published. Typically used alongside [[sdPublisher]]" ;
        rdfs:label    "sdDatePublished" .

schema:DislikeAction  rdf:type  rdfs:Class ;
        rdfs:comment     "The act of expressing a negative sentiment about the object. An agent dislikes an object (a proposition, topic or theme) with participants." ;
        rdfs:label       "DislikeAction" ;
        rdfs:subClassOf  schema:ReactAction .

schema:broadcastDisplayName
        rdf:type      rdf:Property ;
        rdfs:comment  "The name displayed in the channel guide. For many US affiliates, it is the network name." ;
        rdfs:label    "broadcastDisplayName" .

schema:Mountain  rdf:type  rdfs:Class ;
        rdfs:comment     "A mountain, like Mount Whitney or Mount Everest." ;
        rdfs:label       "Mountain" ;
        rdfs:subClassOf  schema:Landform .

schema:OfficeEquipmentStore
        rdf:type         rdfs:Class ;
        rdfs:comment     "An office equipment store." ;
        rdfs:label       "OfficeEquipmentStore" ;
        rdfs:subClassOf  schema:Store .

schema:TattooParlor  rdf:type  rdfs:Class ;
        rdfs:comment     "A tattoo parlor." ;
        rdfs:label       "TattooParlor" ;
        rdfs:subClassOf  schema:HealthAndBeautyBusiness .

schema:ownershipFundingInfo
        rdf:type            rdf:Property ;
        rdfs:comment        "For an [[Organization]] (often but not necessarily a [[NewsMediaOrganization]]), a description of organizational ownership structure; funding and grants. In a news/media setting, this is with particular reference to editorial independence.   Note that the [[funder]] is also available and can be used to make basic funder information machine-readable." ;
        rdfs:label          "ownershipFundingInfo" ;
        rdfs:subPropertyOf  schema:publishingPrinciples .

schema:encodings  rdf:type  rdf:Property ;
        rdfs:comment  "A media object that encodes this CreativeWork." ;
        rdfs:label    "encodings" .

schema:photos  rdf:type  rdf:Property ;
        rdfs:comment  "Photographs of this place." ;
        rdfs:label    "photos" .

schema:requiredGender
        rdf:type      rdf:Property ;
        rdfs:comment  "Audiences defined by a person's gender." ;
        rdfs:label    "requiredGender" .

schema:cvdNumC19HOPats
        rdf:type      rdf:Property ;
        rdfs:comment  "numc19hopats - HOSPITAL ONSET: Patients hospitalized in an NHSN inpatient care location with onset of suspected or confirmed COVID-19 14 or more days after hospitalization." ;
        rdfs:label    "cvdNumC19HOPats" .

schema:SurgicalProcedure
        rdf:type         rdfs:Class ;
        rdfs:comment     "A medical procedure involving an incision with instruments; performed for diagnose, or therapeutic purposes." ;
        rdfs:label       "SurgicalProcedure" ;
        rdfs:subClassOf  schema:MedicalProcedure .

schema:SpecialAnnouncement
        rdf:type         rdfs:Class ;
        rdfs:comment     "A SpecialAnnouncement combines a simple date-stamped textual information update\n      with contextualized Web links and other structured data.  It represents an information update made by a\n      locally-oriented organization, for example schools, pharmacies, healthcare providers,  community groups, police,\n      local government.\n\nFor work in progress guidelines on Coronavirus-related markup see [this doc](https://docs.google.com/document/d/14ikaGCKxo50rRM7nvKSlbUpjyIk2WMQd3IkB1lItlrM/edit#).\n\nThe motivating scenario for SpecialAnnouncement is the [Coronavirus pandemic](https://en.wikipedia.org/wiki/2019%E2%80%9320_coronavirus_pandemic), and the initial vocabulary is oriented to this urgent situation. Schema.org\nexpect to improve the markup iteratively as it is deployed and as feedback emerges from use. In addition to our\nusual [Github entry](https://github.com/schemaorg/schemaorg/issues/2490), feedback comments can also be provided in [this document](https://docs.google.com/document/d/1fpdFFxk8s87CWwACs53SGkYv3aafSxz_DTtOQxMrBJQ/edit#).\n\n\nWhile this schema is designed to communicate urgent crisis-related information, it is not the same as an emergency warning technology like [CAP](https://en.wikipedia.org/wiki/Common_Alerting_Protocol), although there may be overlaps. The intent is to cover\nthe kinds of everyday practical information being posted to existing websites during an emergency situation.\n\nSeveral kinds of information can be provided:\n\nWe encourage the provision of \"name\", \"text\", \"datePosted\", \"expires\" (if appropriate), \"category\" and\n\"url\" as a simple baseline. It is important to provide a value for \"category\" where possible, most ideally as a well known\nURL from Wikipedia or Wikidata. In the case of the 2019-2020 Coronavirus pandemic, this should be \"https://en.wikipedia.org/w/index.php?title=2019-20\\_coronavirus\\_pandemic\" or \"https://www.wikidata.org/wiki/Q81068910\".\n\nFor many of the possible properties, values can either be simple links or an inline description, depending on whether a summary is available. For a link, provide just the URL of the appropriate page as the property's value. For an inline description, use a [[WebContent]] type, and provide the url as a property of that, alongside at least a simple \"[[text]]\" summary of the page. It is\nunlikely that a single SpecialAnnouncement will need all of the possible properties simultaneously.\n\nWe expect that in many cases the page referenced might contain more specialized structured data, e.g. contact info, [[openingHours]], [[Event]], [[FAQPage]] etc. By linking to those pages from a [[SpecialAnnouncement]] you can help make it clearer that the events are related to the situation (e.g. Coronavirus) indicated by the [[category]] property of the [[SpecialAnnouncement]].\n\nMany [[SpecialAnnouncement]]s will relate to particular regions and to identifiable local organizations. Use [[spatialCoverage]] for the region, and [[announcementLocation]] to indicate specific [[LocalBusiness]]es and [[CivicStructure]]s. If the announcement affects both a particular region and a specific location (for example, a library closure that serves an entire region), use both [[spatialCoverage]] and [[announcementLocation]].\n\nThe [[about]] property can be used to indicate entities that are the focus of the announcement. We now recommend using [[about]] only\nfor representing non-location entities (e.g. a [[Course]] or a [[RadioStation]]). For places, use [[announcementLocation]] and [[spatialCoverage]]. Consumers of this markup should be aware that the initial design encouraged the use of /about for locations too.\n\nThe basic content of [[SpecialAnnouncement]] is similar to that of an [RSS](https://en.wikipedia.org/wiki/RSS) or [Atom](https://en.wikipedia.org/wiki/Atom_(Web_standard)) feed. For publishers without such feeds, basic feed-like information can be shared by posting\n[[SpecialAnnouncement]] updates in a page, e.g. using JSON-LD. For sites with Atom/RSS functionality, you can point to a feed\nwith the [[webFeed]] property. This can be a simple URL, or an inline [[DataFeed]] object, with [[encodingFormat]] providing\nmedia type information e.g. \"application/rss+xml\" or \"application/atom+xml\".\n" ;
        rdfs:label       "SpecialAnnouncement" ;
        rdfs:subClassOf  schema:CreativeWork .

schema:TouristInformationCenter
        rdf:type         rdfs:Class ;
        rdfs:comment     "A tourist information center." ;
        rdfs:label       "TouristInformationCenter" ;
        rdfs:subClassOf  schema:LocalBusiness .

schema:mentions  rdf:type  rdf:Property ;
        rdfs:comment  "Indicates that the CreativeWork contains a reference to, but is not necessarily about a concept." ;
        rdfs:label    "mentions" .

schema:stageAsNumber  rdf:type  rdf:Property ;
        rdfs:comment  "The stage represented as a number, e.g. 3." ;
        rdfs:label    "stageAsNumber" .

schema:ExchangeRateSpecification
        rdf:type         rdfs:Class ;
        rdfs:comment     "A structured value representing exchange rate." ;
        rdfs:label       "ExchangeRateSpecification" ;
        rdfs:subClassOf  schema:StructuredValue .

schema:SportsClub  rdf:type  rdfs:Class ;
        rdfs:comment     "A sports club." ;
        rdfs:label       "SportsClub" ;
        rdfs:subClassOf  schema:SportsActivityLocation .

schema:accountablePerson
        rdf:type      rdf:Property ;
        rdfs:comment  "Specifies the Person that is legally accountable for the CreativeWork." ;
        rdfs:label    "accountablePerson" .

schema:DepartAction  rdf:type  rdfs:Class ;
        rdfs:comment     "The act of  departing from a place. An agent departs from an fromLocation for a destination, optionally with participants." ;
        rdfs:label       "DepartAction" ;
        rdfs:subClassOf  schema:MoveAction .

schema:follows  rdf:type  rdf:Property ;
        rdfs:comment  "The most generic uni-directional social relation." ;
        rdfs:label    "follows" .

schema:cholesterolContent
        rdf:type      rdf:Property ;
        rdfs:comment  "The number of milligrams of cholesterol." ;
        rdfs:label    "cholesterolContent" .

schema:Hackathon  rdf:type  rdfs:Class ;
        rdfs:comment     "A [hackathon](https://en.wikipedia.org/wiki/Hackathon) event." ;
        rdfs:label       "Hackathon" ;
        rdfs:subClassOf  schema:Event .

schema:knows  rdf:type  rdf:Property ;
        rdfs:comment  "The most generic bi-directional social/work relation." ;
        rdfs:label    "knows" .

schema:acceptedPaymentMethod
        rdf:type      rdf:Property ;
        rdfs:comment  "The payment method(s) accepted by seller for this offer." ;
        rdfs:label    "acceptedPaymentMethod" .

schema:BrainStructure
        rdf:type         rdfs:Class ;
        rdfs:comment     "Any anatomical structure which pertains to the soft nervous tissue functioning as the coordinating center of sensation and intellectual and nervous activity." ;
        rdfs:label       "BrainStructure" ;
        rdfs:subClassOf  schema:AnatomicalStructure .

schema:webCheckinTime
        rdf:type      rdf:Property ;
        rdfs:comment  "The time when a passenger can check into the flight online." ;
        rdfs:label    "webCheckinTime" .

schema:Season  rdf:type  rdfs:Class ;
        rdfs:comment     "A media season e.g. tv, radio, video game etc." ;
        rdfs:label       "Season" ;
        rdfs:subClassOf  schema:CreativeWork .

schema:validThrough  rdf:type  rdf:Property ;
        rdfs:comment  "The date after when the item is not valid. For example the end of an offer, salary period, or a period of opening hours." ;
        rdfs:label    "validThrough" .

schema:headline  rdf:type  rdf:Property ;
        rdfs:comment  "Headline of the article." ;
        rdfs:label    "headline" .

schema:BowlingAlley  rdf:type  rdfs:Class ;
        rdfs:comment     "A bowling alley." ;
        rdfs:label       "BowlingAlley" ;
        rdfs:subClassOf  schema:SportsActivityLocation .

schema:petsAllowed  rdf:type  rdf:Property ;
        rdfs:comment  "Indicates whether pets are allowed to enter the accommodation or lodging business. More detailed information can be put in a text value." ;
        rdfs:label    "petsAllowed" .

schema:readonlyValue  rdf:type  rdf:Property ;
        rdfs:comment  "Whether or not a property is mutable.  Default is false. Specifying this for a property that also has a value makes it act similar to a \"hidden\" input in an HTML form." ;
        rdfs:label    "readonlyValue" .

schema:album  rdf:type  rdf:Property ;
        rdfs:comment  "A music album." ;
        rdfs:label    "album" .

schema:volumeNumber  rdf:type  rdf:Property ;
        rdfs:comment        "Identifies the volume of publication or multi-part work; for example, \"iii\" or \"2\"." ;
        rdfs:label          "volumeNumber" ;
        rdfs:subPropertyOf  schema:position .

schema:Patient  rdf:type  rdfs:Class ;
        rdfs:comment     "A patient is any person recipient of health care services." ;
        rdfs:label       "Patient" ;
        rdfs:subClassOf  schema:MedicalAudience , schema:Person .

schema:DeliveryChargeSpecification
        rdf:type         rdfs:Class ;
        rdfs:comment     "The price for the delivery of an offer using a particular delivery method." ;
        rdfs:label       "DeliveryChargeSpecification" ;
        rdfs:subClassOf  schema:PriceSpecification .

schema:hiringOrganization
        rdf:type      rdf:Property ;
        rdfs:comment  "Organization offering the job position." ;
        rdfs:label    "hiringOrganization" .

schema:RefundTypeEnumeration
        rdf:type         rdfs:Class ;
        rdfs:comment     "RefundTypeEnumeration enumerates several kinds of product return refund types." ;
        rdfs:label       "RefundTypeEnumeration" ;
        rdfs:subClassOf  schema:Enumeration .

schema:Campground  rdf:type  rdfs:Class ;
        rdfs:comment     "A camping site, campsite, or [[Campground]] is a place used for overnight stay in the outdoors, typically containing individual [[CampingPitch]] locations. \\n\\n\nIn British English a campsite is an area, usually divided into a number of pitches, where people can camp overnight using tents or camper vans or caravans; this British English use of the word is synonymous with the American English expression campground. In American English the term campsite generally means an area where an individual, family, group, or military unit can pitch a tent or park a camper; a campground may contain many campsites (Source: Wikipedia see [https://en.wikipedia.org/wiki/Campsite](https://en.wikipedia.org/wiki/Campsite)).\\n\\n\n\nSee also the dedicated [document on the use of schema.org for marking up hotels and other forms of accommodations](/docs/hotels.html).\n" ;
        rdfs:label       "Campground" ;
        rdfs:subClassOf  schema:CivicStructure , schema:LodgingBusiness .

schema:exercisePlan  rdf:type  rdf:Property ;
        rdfs:comment        "A sub property of instrument. The exercise plan used on this action." ;
        rdfs:label          "exercisePlan" ;
        rdfs:subPropertyOf  schema:instrument .

schema:educationalLevel
        rdf:type      rdf:Property ;
        rdfs:comment  "The level in terms of progression through an educational or training context. Examples of educational levels include 'beginner', 'intermediate' or 'advanced', and formal sets of level indicators." ;
        rdfs:label    "educationalLevel" .

schema:firstAppearance
        rdf:type            rdf:Property ;
        rdfs:comment        "Indicates the first known occurence of a [[Claim]] in some [[CreativeWork]]." ;
        rdfs:label          "firstAppearance" ;
        rdfs:subPropertyOf  schema:workExample .

schema:availableLanguage
        rdf:type      rdf:Property ;
        rdfs:comment  "A language someone may use with or at the item, service or place. Please use one of the language codes from the [IETF BCP 47 standard](http://tools.ietf.org/html/bcp47). See also [[inLanguage]]" ;
        rdfs:label    "availableLanguage" .

schema:Restaurant  rdf:type  rdfs:Class ;
        rdfs:comment     "A restaurant." ;
        rdfs:label       "Restaurant" ;
        rdfs:subClassOf  schema:FoodEstablishment .

schema:accessibilityAPI
        rdf:type      rdf:Property ;
        rdfs:comment  "Indicates that the resource is compatible with the referenced accessibility API ([WebSchemas wiki lists possible values](http://www.w3.org/wiki/WebSchemas/Accessibility))." ;
        rdfs:label    "accessibilityAPI" .

schema:LocationFeatureSpecification
        rdf:type         rdfs:Class ;
        rdfs:comment     "Specifies a location feature by providing a structured value representing a feature of an accommodation as a property-value pair of varying degrees of formality." ;
        rdfs:label       "LocationFeatureSpecification" ;
        rdfs:subClassOf  schema:PropertyValue .

schema:url  rdf:type  rdf:Property ;
        rdfs:comment  "URL of the item." ;
        rdfs:label    "url" .

schema:catalog  rdf:type  rdf:Property ;
        rdfs:comment  "A data catalog which contains this dataset." ;
        rdfs:label    "catalog" .

schema:bookFormat  rdf:type  rdf:Property ;
        rdfs:comment  "The format of the book." ;
        rdfs:label    "bookFormat" .

schema:usesDevice  rdf:type  rdf:Property ;
        rdfs:comment  "Device used to perform the test." ;
        rdfs:label    "usesDevice" .

schema:Country  rdf:type  rdfs:Class ;
        rdfs:comment     "A country." ;
        rdfs:label       "Country" ;
        rdfs:subClassOf  schema:AdministrativeArea .

schema:FilmAction  rdf:type  rdfs:Class ;
        rdfs:comment     "The act of capturing sound and moving images on film, video, or digitally." ;
        rdfs:label       "FilmAction" ;
        rdfs:subClassOf  schema:CreateAction .

skos:semanticRelation
        rdf:type     owl:ObjectProperty ;
        rdfs:domain  skos:Concept ;
        rdfs:label   "is in semantic relation with"@en ;
        rdfs:range   skos:Concept .

schema:InviteAction  rdf:type  rdfs:Class ;
        rdfs:comment     "The act of asking someone to attend an event. Reciprocal of RsvpAction." ;
        rdfs:label       "InviteAction" ;
        rdfs:subClassOf  schema:CommunicateAction .

schema:serviceType  rdf:type  rdf:Property ;
        rdfs:comment  "The type of service being offered, e.g. veterans' benefits, emergency relief, etc." ;
        rdfs:label    "serviceType" .

schema:programPrerequisites
        rdf:type      rdf:Property ;
        rdfs:comment  "Prerequisites for enrolling in the program." ;
        rdfs:label    "programPrerequisites" .

schema:position  rdf:type  rdf:Property ;
        rdfs:comment  "The position of an item in a series or sequence of items." ;
        rdfs:label    "position" .

schema:vehicleTransmission
        rdf:type      rdf:Property ;
        rdfs:comment  "The type of component used for transmitting the power from a rotating power source to the wheels or other relevant component(s) (\"gearbox\" for cars)." ;
        rdfs:label    "vehicleTransmission" .

schema:cookTime  rdf:type   rdf:Property ;
        rdfs:comment        "The time it takes to actually cook the dish, in [ISO 8601 duration format](http://en.wikipedia.org/wiki/ISO_8601)." ;
        rdfs:label          "cookTime" ;
        rdfs:subPropertyOf  schema:performTime .

schema:endDate  rdf:type  rdf:Property ;
        rdfs:comment  "The end date and time of the item (in [ISO 8601 date format](http://en.wikipedia.org/wiki/ISO_8601))." ;
        rdfs:label    "endDate" .

schema:codeValue  rdf:type  rdf:Property ;
        rdfs:comment        "A short textual code that uniquely identifies the value." ;
        rdfs:label          "codeValue" ;
        rdfs:subPropertyOf  schema:termCode .

schema:LeaveAction  rdf:type  rdfs:Class ;
        rdfs:comment     "An agent leaves an event / group with participants/friends at a location.\\n\\nRelated actions:\\n\\n* [[JoinAction]]: The antonym of LeaveAction.\\n* [[UnRegisterAction]]: Unlike UnRegisterAction, LeaveAction implies leaving a group/team of people rather than a service." ;
        rdfs:label       "LeaveAction" ;
        rdfs:subClassOf  schema:InteractAction .

schema:Pediatric  rdf:type  rdfs:Class ;
        rdfs:comment     "A specific branch of medical science that specializes in the care of infants, children and adolescents." ;
        rdfs:label       "Pediatric" ;
        rdfs:subClassOf  schema:MedicalBusiness .

schema:userInteractionCount
        rdf:type      rdf:Property ;
        rdfs:comment  "The number of interactions for the CreativeWork using the WebSite or SoftwareApplication." ;
        rdfs:label    "userInteractionCount" .

schema:programmingModel
        rdf:type      rdf:Property ;
        rdfs:comment  "Indicates whether API is managed or unmanaged." ;
        rdfs:label    "programmingModel" .

schema:TelevisionChannel
        rdf:type         rdfs:Class ;
        rdfs:comment     "A unique instance of a television BroadcastService on a CableOrSatelliteService lineup." ;
        rdfs:label       "TelevisionChannel" ;
        rdfs:subClassOf  schema:BroadcastChannel .

schema:PlasticSurgery
        rdf:type         rdfs:Class ;
        rdfs:comment     "A specific branch of medical science that pertains to therapeutic or cosmetic repair or re-formation of missing, injured or malformed tissues or body parts by manual and instrumental means." ;
        rdfs:label       "PlasticSurgery" ;
        rdfs:subClassOf  schema:MedicalBusiness .

schema:UserPlays  rdf:type  rdfs:Class ;
        rdfs:comment     "UserInteraction and its subtypes is an old way of talking about users interacting with pages. It is generally better to use [[Action]]-based vocabulary, alongside types such as [[Comment]]." ;
        rdfs:label       "UserPlays" ;
        rdfs:subClassOf  schema:UserInteraction .

schema:UnRegisterAction
        rdf:type         rdfs:Class ;
        rdfs:comment     "The act of un-registering from a service.\\n\\nRelated actions:\\n\\n* [[RegisterAction]]: antonym of UnRegisterAction.\\n* [[LeaveAction]]: Unlike LeaveAction, UnRegisterAction implies that you are unregistering from a service you werer previously registered, rather than leaving a team/group of people." ;
        rdfs:label       "UnRegisterAction" ;
        rdfs:subClassOf  schema:InteractAction .

schema:iswcCode  rdf:type  rdf:Property ;
        rdfs:comment  "The International Standard Musical Work Code for the composition." ;
        rdfs:label    "iswcCode" .

schema:mainEntityOfPage
        rdf:type      rdf:Property ;
        rdfs:comment  "Indicates a page (or other CreativeWork) for which this thing is the main entity being described. See [background notes](/docs/datamodel.html#mainEntityBackground) for details." ;
        rdfs:label    "mainEntityOfPage" .

schema:requiresSubscription
        rdf:type      rdf:Property ;
        rdfs:comment  "Indicates if use of the media require a subscription  (either paid or free). Allowed values are ```true``` or ```false``` (note that an earlier version had 'yes', 'no')." ;
        rdfs:label    "requiresSubscription" .

schema:logo  rdf:type       rdf:Property ;
        rdfs:comment        "An associated logo." ;
        rdfs:label          "logo" ;
        rdfs:subPropertyOf  schema:image .

schema:pickupLocation
        rdf:type      rdf:Property ;
        rdfs:comment  "Where a taxi will pick up a passenger or a rental car can be picked up." ;
        rdfs:label    "pickupLocation" .

schema:transcript  rdf:type  rdf:Property ;
        rdfs:comment  "If this MediaObject is an AudioObject or VideoObject, the transcript of that object." ;
        rdfs:label    "transcript" .

schema:returnPolicyCategory
        rdf:type      rdf:Property ;
        rdfs:comment  "A returnPolicyCategory expresses at most one of several enumerated kinds of return." ;
        rdfs:label    "returnPolicyCategory" .

schema:vehicleModelDate
        rdf:type      rdf:Property ;
        rdfs:comment  "The release date of a vehicle model (often used to differentiate versions of the same make and model)." ;
        rdfs:label    "vehicleModelDate" .

schema:successorOf  rdf:type  rdf:Property ;
        rdfs:comment  "A pointer from a newer variant of a product  to its previous, often discontinued predecessor." ;
        rdfs:label    "successorOf" .

schema:physiologicalBenefits
        rdf:type      rdf:Property ;
        rdfs:comment  "Specific physiologic benefits associated to the plan." ;
        rdfs:label    "physiologicalBenefits" .

schema:title  rdf:type  rdf:Property ;
        rdfs:comment  "The title of the job." ;
        rdfs:label    "title" .

schema:GasStation  rdf:type  rdfs:Class ;
        rdfs:comment     "A gas station." ;
        rdfs:label       "GasStation" ;
        rdfs:subClassOf  schema:AutomotiveBusiness .

schema:DrinkAction  rdf:type  rdfs:Class ;
        rdfs:comment     "The act of swallowing liquids." ;
        rdfs:label       "DrinkAction" ;
        rdfs:subClassOf  schema:ConsumeAction .

schema:CarUsageType  rdf:type  rdfs:Class ;
        rdfs:comment     "A value indicating a special usage of a car, e.g. commercial rental, driving school, or as a taxi." ;
        rdfs:label       "CarUsageType" ;
        rdfs:subClassOf  schema:Enumeration .

schema:VideoGallery  rdf:type  rdfs:Class ;
        rdfs:comment     "Web page type: Video gallery page." ;
        rdfs:label       "VideoGallery" ;
        rdfs:subClassOf  schema:MediaGallery .

schema:primaryImageOfPage
        rdf:type      rdf:Property ;
        rdfs:comment  "Indicates the main image on the page." ;
        rdfs:label    "primaryImageOfPage" .

schema:businessFunction
        rdf:type      rdf:Property ;
        rdfs:comment  "The business function (e.g. sell, lease, repair, dispose) of the offer or component of a bundle (TypeAndQuantityNode). The default is http://purl.org/goodrelations/v1#Sell." ;
        rdfs:label    "businessFunction" .

schema:FoodEstablishment
        rdf:type         rdfs:Class ;
        rdfs:comment     "A food-related business." ;
        rdfs:label       "FoodEstablishment" ;
        rdfs:subClassOf  schema:LocalBusiness .

schema:LakeBodyOfWater
        rdf:type         rdfs:Class ;
        rdfs:comment     "A lake (for example, Lake Pontrachain)." ;
        rdfs:label       "LakeBodyOfWater" ;
        rdfs:subClassOf  schema:BodyOfWater .

schema:employees  rdf:type  rdf:Property ;
        rdfs:comment  "People working for this organization." ;
        rdfs:label    "employees" .

schema:partOfSeries  rdf:type  rdf:Property ;
        rdfs:comment        "The series to which this episode or season belongs." ;
        rdfs:label          "partOfSeries" ;
        rdfs:subPropertyOf  schema:isPartOf .

schema:ShortStory  rdf:type  rdfs:Class ;
        rdfs:comment     "Short story or tale. A brief work of literature, usually written in narrative prose." ;
        rdfs:label       "ShortStory" ;
        rdfs:subClassOf  schema:CreativeWork .

schema:Vehicle  rdf:type  rdfs:Class ;
        rdfs:comment     "A vehicle is a device that is designed or used to transport people or cargo over land, water, air, or through space." ;
        rdfs:label       "Vehicle" ;
        rdfs:subClassOf  schema:Product .

schema:educationalRole
        rdf:type      rdf:Property ;
        rdfs:comment  "An educationalRole of an EducationalAudience." ;
        rdfs:label    "educationalRole" .

schema:trainingSalary
        rdf:type      rdf:Property ;
        rdfs:comment  "The estimated salary earned while in the program." ;
        rdfs:label    "trainingSalary" .

schema:Menu  rdf:type    rdfs:Class ;
        rdfs:comment     "A structured representation of food or drink items available from a FoodEstablishment." ;
        rdfs:label       "Menu" ;
        rdfs:subClassOf  schema:CreativeWork .

schema:birthDate  rdf:type  rdf:Property ;
        rdfs:comment  "Date of birth." ;
        rdfs:label    "birthDate" .

schema:dateDeleted  rdf:type  rdf:Property ;
        rdfs:comment  "The datetime the item was removed from the DataFeed." ;
        rdfs:label    "dateDeleted" .

schema:significantLinks
        rdf:type      rdf:Property ;
        rdfs:comment  "The most significant URLs on the page. Typically, these are the non-navigation links that are clicked on the most." ;
        rdfs:label    "significantLinks" .

schema:review  rdf:type  rdf:Property ;
        rdfs:comment  "A review of the item." ;
        rdfs:label    "review" .

schema:loanPaymentAmount
        rdf:type      rdf:Property ;
        rdfs:comment  "The amount of money to pay in a single payment." ;
        rdfs:label    "loanPaymentAmount" .

schema:DepositAccount
        rdf:type         rdfs:Class ;
        rdfs:comment     "A type of Bank Account with a main purpose of depositing funds to gain interest or other benefits." ;
        rdfs:label       "DepositAccount" ;
        rdfs:subClassOf  schema:InvestmentOrDeposit , schema:BankAccount .

schema:actor  rdf:type  rdf:Property ;
        rdfs:comment  "An actor, e.g. in tv, radio, movie, video games etc., or in an event. Actors can be associated with individual items or with a series, episode, clip." ;
        rdfs:label    "actor" .

schema:carbohydrateContent
        rdf:type      rdf:Property ;
        rdfs:comment  "The number of grams of carbohydrates." ;
        rdfs:label    "carbohydrateContent" .

schema:downloadUrl  rdf:type  rdf:Property ;
        rdfs:comment  "If the file can be downloaded, URL to download the binary." ;
        rdfs:label    "downloadUrl" .

schema:documentation  rdf:type  rdf:Property ;
        rdfs:comment  "Further documentation describing the Web API in more detail." ;
        rdfs:label    "documentation" .

schema:PreventionIndication
        rdf:type         rdfs:Class ;
        rdfs:comment     "An indication for preventing an underlying condition, symptom, etc." ;
        rdfs:label       "PreventionIndication" ;
        rdfs:subClassOf  schema:MedicalIndication .

schema:DrugCost  rdf:type  rdfs:Class ;
        rdfs:comment     "The cost per unit of a medical drug. Note that this type is not meant to represent the price in an offer of a drug for sale; see the Offer type for that. This type will typically be used to tag wholesale or average retail cost of a drug, or maximum reimbursable cost. Costs of medical drugs vary widely depending on how and where they are paid for, so while this type captures some of the variables, costs should be used with caution by consumers of this schema's markup." ;
        rdfs:label       "DrugCost" ;
        rdfs:subClassOf  schema:MedicalEntity .

schema:propertyID  rdf:type  rdf:Property ;
        rdfs:comment  "A commonly used identifier for the characteristic represented by the property, e.g. a manufacturer or a standard code for a property. propertyID can be\n(1) a prefixed string, mainly meant to be used with standards for product properties; (2) a site-specific, non-prefixed string (e.g. the primary key of the property or the vendor-specific id of the property), or (3)\na URL indicating the type of the property, either pointing to an external vocabulary, or a Web resource that describes the property (e.g. a glossary entry).\nStandards bodies should promote a standard prefix for the identifiers of properties from their standards." ;
        rdfs:label    "propertyID" .

schema:option  rdf:type     rdf:Property ;
        rdfs:comment        "A sub property of object. The options subject to this action." ;
        rdfs:label          "option" ;
        rdfs:subPropertyOf  schema:object .

schema:PublicationEvent
        rdf:type         rdfs:Class ;
        rdfs:comment     "A PublicationEvent corresponds indifferently to the event of publication for a CreativeWork of any type e.g. a broadcast event, an on-demand event, a book/journal publication via a variety of delivery media." ;
        rdfs:label       "PublicationEvent" ;
        rdfs:subClassOf  schema:Event .

schema:MusicAlbum  rdf:type  rdfs:Class ;
        rdfs:comment     "A collection of music tracks." ;
        rdfs:label       "MusicAlbum" ;
        rdfs:subClassOf  schema:MusicPlaylist .

schema:Boolean  rdf:type  rdfs:Class ;
        rdfs:comment  "Boolean: True or False." ;
        rdfs:label    "Boolean" .

schema:transitTimeLabel
        rdf:type      rdf:Property ;
        rdfs:comment  "Label to match an [[OfferShippingDetails]] with a [[DeliveryTimeSettings]] (within the context of a [[shippingSettingsLink]] cross-reference)." ;
        rdfs:label    "transitTimeLabel" .

schema:contactlessPayment
        rdf:type      rdf:Property ;
        rdfs:comment  "A secure method for consumers to purchase products or services via debit, credit or smartcards by using RFID or NFC technology." ;
        rdfs:label    "contactlessPayment" .

schema:greaterOrEqual
        rdf:type      rdf:Property ;
        rdfs:comment  "This ordering relation for qualitative values indicates that the subject is greater than or equal to the object." ;
        rdfs:label    "greaterOrEqual" .

schema:softwareRequirements
        rdf:type      rdf:Property ;
        rdfs:comment  "Component dependency requirements for application. This includes runtime environments and shared libraries that are not included in the application distribution package, but required to run the application (Examples: DirectX, Java or .NET runtime)." ;
        rdfs:label    "softwareRequirements" .

schema:valueAddedTaxIncluded
        rdf:type      rdf:Property ;
        rdfs:comment  "Specifies whether the applicable value-added tax (VAT) is included in the price specification or not." ;
        rdfs:label    "valueAddedTaxIncluded" .

schema:associatedMedia
        rdf:type      rdf:Property ;
        rdfs:comment  "A media object that encodes this CreativeWork. This property is a synonym for encoding." ;
        rdfs:label    "associatedMedia" .

schema:hostingOrganization
        rdf:type      rdf:Property ;
        rdfs:comment  "The organization (airline, travelers' club, etc.) the membership is made with." ;
        rdfs:label    "hostingOrganization" .

schema:interestRate  rdf:type  rdf:Property ;
        rdfs:comment  "The interest rate, charged or paid, applicable to the financial product. Note: This is different from the calculated annualPercentageRate." ;
        rdfs:label    "interestRate" .

schema:penciler  rdf:type  rdf:Property ;
        rdfs:comment  "The individual who draws the primary narrative artwork." ;
        rdfs:label    "penciler" .

schema:yield  rdf:type  rdf:Property ;
        rdfs:comment  "The quantity that results by performing instructions. For example, a paper airplane, 10 personalized candles." ;
        rdfs:label    "yield" .

schema:geoCovers  rdf:type  rdf:Property ;
        rdfs:comment  "Represents a relationship between two geometries (or the places they represent), relating a covering geometry to a covered geometry. \"Every point of b is a point of (the interior or boundary of) a\". As defined in [DE-9IM](https://en.wikipedia.org/wiki/DE-9IM)." ;
        rdfs:label    "geoCovers" .

schema:potentialAction
        rdf:type      rdf:Property ;
        rdfs:comment  "Indicates a potential Action, which describes an idealized action in which this thing would play an 'object' role." ;
        rdfs:label    "potentialAction" .

schema:WantAction  rdf:type  rdfs:Class ;
        rdfs:comment     "The act of expressing a desire about the object. An agent wants an object." ;
        rdfs:label       "WantAction" ;
        rdfs:subClassOf  schema:ReactAction .

schema:gamePlatform  rdf:type  rdf:Property ;
        rdfs:comment  "The electronic systems used to play <a href=\"http://en.wikipedia.org/wiki/Category:Video_game_platforms\">video games</a>." ;
        rdfs:label    "gamePlatform" .

schema:discusses  rdf:type  rdf:Property ;
        rdfs:comment  "Specifies the CreativeWork associated with the UserComment." ;
        rdfs:label    "discusses" .

schema:artworkSurface
        rdf:type      rdf:Property ;
        rdfs:comment  "The supporting materials for the artwork, e.g. Canvas, Paper, Wood, Board, etc." ;
        rdfs:label    "artworkSurface" .

schema:targetUrl  rdf:type  rdf:Property ;
        rdfs:comment  "The URL of a node in an established educational framework." ;
        rdfs:label    "targetUrl" .

schema:diseaseSpreadStatistics
        rdf:type      rdf:Property ;
        rdfs:comment  "Statistical information about the spread of a disease, either as [[WebContent]], or\n  described directly as a [[Dataset]], or the specific [[Observation]]s in the dataset. When a [[WebContent]] URL is\n  provided, the page indicated might also contain more such markup." ;
        rdfs:label    "diseaseSpreadStatistics" .

schema:Library  rdf:type  rdfs:Class ;
        rdfs:comment     "A library." ;
        rdfs:label       "Library" ;
        rdfs:subClassOf  schema:LocalBusiness .

schema:credentialCategory
        rdf:type      rdf:Property ;
        rdfs:comment  "The category or type of credential being described, for example \"degree”, “certificate”, “badge”, or more specific term." ;
        rdfs:label    "credentialCategory" .

schema:accessModeSufficient
        rdf:type      rdf:Property ;
        rdfs:comment  "A list of single or combined accessModes that are sufficient to understand all the intellectual content of a resource. Expected values include:  auditory, tactile, textual, visual.\n      " ;
        rdfs:label    "accessModeSufficient" .

schema:PaymentMethod  rdf:type  rdfs:Class ;
        rdfs:comment     "A payment method is a standardized procedure for transferring the monetary amount for a purchase. Payment methods are characterized by the legal and technical structures used, and by the organization or group carrying out the transaction.\\n\\nCommonly used values:\\n\\n* http://purl.org/goodrelations/v1#ByBankTransferInAdvance\\n* http://purl.org/goodrelations/v1#ByInvoice\\n* http://purl.org/goodrelations/v1#Cash\\n* http://purl.org/goodrelations/v1#CheckInAdvance\\n* http://purl.org/goodrelations/v1#COD\\n* http://purl.org/goodrelations/v1#DirectDebit\\n* http://purl.org/goodrelations/v1#GoogleCheckout\\n* http://purl.org/goodrelations/v1#PayPal\\n* http://purl.org/goodrelations/v1#PaySwarm\n        " ;
        rdfs:label       "PaymentMethod" ;
        rdfs:subClassOf  schema:Enumeration .

schema:servingSize  rdf:type  rdf:Property ;
        rdfs:comment  "The serving size, in terms of the number of volume or mass." ;
        rdfs:label    "servingSize" .

schema:availability  rdf:type  rdf:Property ;
        rdfs:comment  "The availability of this item&#x2014;for example In stock, Out of stock, Pre-order, etc." ;
        rdfs:label    "availability" .

schema:MovieSeries  rdf:type  rdfs:Class ;
        rdfs:comment     "A series of movies. Included movies can be indicated with the hasPart property." ;
        rdfs:label       "MovieSeries" ;
        rdfs:subClassOf  schema:CreativeWorkSeries .

schema:events  rdf:type  rdf:Property ;
        rdfs:comment  "Upcoming or past events associated with this place or organization." ;
        rdfs:label    "events" .

schema:MensClothingStore
        rdf:type         rdfs:Class ;
        rdfs:comment     "A men's clothing store." ;
        rdfs:label       "MensClothingStore" ;
        rdfs:subClassOf  schema:Store .

schema:exerciseCourse
        rdf:type            rdf:Property ;
        rdfs:comment        "A sub property of location. The course where this action was taken." ;
        rdfs:label          "exerciseCourse" ;
        rdfs:subPropertyOf  schema:location .

schema:LodgingReservation
        rdf:type         rdfs:Class ;
        rdfs:comment     "A reservation for lodging at a hotel, motel, inn, etc.\\n\\nNote: This type is for information about actual reservations, e.g. in confirmation emails or HTML pages with individual confirmations of reservations." ;
        rdfs:label       "LodgingReservation" ;
        rdfs:subClassOf  schema:Reservation .

schema:diagram  rdf:type  rdf:Property ;
        rdfs:comment  "An image containing a diagram that illustrates the structure and/or its component substructures and/or connections with other structures." ;
        rdfs:label    "diagram" .

schema:WearableSizeSystemEnumeration
        rdf:type         rdfs:Class ;
        rdfs:comment     "Enumerates common size systems specific for wearable products" ;
        rdfs:label       "WearableSizeSystemEnumeration" ;
        rdfs:subClassOf  schema:SizeSystemEnumeration .

schema:MedicalEnumeration
        rdf:type         rdfs:Class ;
        rdfs:comment     "Enumerations related to health and the practice of medicine: A concept that is used to attribute a quality to another concept, as a qualifier, a collection of items or a listing of all of the elements of a set in medicine practice." ;
        rdfs:label       "MedicalEnumeration" ;
        rdfs:subClassOf  schema:Enumeration .

schema:DefinedRegion  rdf:type  rdfs:Class ;
        rdfs:comment     "A DefinedRegion is a geographic area defined by potentially arbitrary (rather than political, administrative or natural geographical) criteria. Properties are provided for defining a region by reference to sets of postal codes.\n\nExamples: a delivery destination when shopping. Region where regional pricing is configured.\n\nRequirement 1:\nCountry: US\nStates: \"NY\", \"CA\"\n\nRequirement 2:\nCountry: US\nPostalCode Set: { [94000-94585], [97000, 97999], [13000, 13599]}\n{ [12345, 12345], [78945, 78945], }\nRegion = state, canton, prefecture, autonomous community...\n" ;
        rdfs:label       "DefinedRegion" ;
        rdfs:subClassOf  schema:StructuredValue .

schema:legislationApplies
        rdf:type      rdf:Property ;
        rdfs:comment  "Indicates that this legislation (or part of a legislation) somehow transfers another legislation in a different legislative context. This is an informative link, and it has no legal value. For legally-binding links of transposition, use the <a href=\"/legislationTransposes\">legislationTransposes</a> property. For example an informative consolidated law of a European Union's member state \"applies\" the consolidated version of the European Directive implemented in it." ;
        rdfs:label    "legislationApplies" .

schema:FindAction  rdf:type  rdfs:Class ;
        rdfs:comment     "The act of finding an object.\\n\\nRelated actions:\\n\\n* [[SearchAction]]: FindAction is generally lead by a SearchAction, but not necessarily." ;
        rdfs:label       "FindAction" ;
        rdfs:subClassOf  schema:Action .

schema:NewsArticle  rdf:type  rdfs:Class ;
        rdfs:comment     "A NewsArticle is an article whose content reports news, or provides background context and supporting materials for understanding the news.\n\nA more detailed overview of [schema.org News markup](/docs/news.html) is also available.\n" ;
        rdfs:label       "NewsArticle" ;
        rdfs:subClassOf  schema:Article .

schema:productionDate
        rdf:type      rdf:Property ;
        rdfs:comment  "The date of production of the item, e.g. vehicle." ;
        rdfs:label    "productionDate" .

schema:Permit  rdf:type  rdfs:Class ;
        rdfs:comment     "A permit issued by an organization, e.g. a parking pass." ;
        rdfs:label       "Permit" ;
        rdfs:subClassOf  schema:Intangible .

schema:PhysicalActivity
        rdf:type         rdfs:Class ;
        rdfs:comment     "Any bodily activity that enhances or maintains physical fitness and overall health and wellness. Includes activity that is part of daily living and routine, structured exercise, and exercise prescribed as part of a medical treatment or recovery plan." ;
        rdfs:label       "PhysicalActivity" ;
        rdfs:subClassOf  schema:LifestyleModification .

schema:RsvpAction  rdf:type  rdfs:Class ;
        rdfs:comment     "The act of notifying an event organizer as to whether you expect to attend the event." ;
        rdfs:label       "RsvpAction" ;
        rdfs:subClassOf  schema:InformAction .

schema:uploadDate  rdf:type  rdf:Property ;
        rdfs:comment  "Date when this media object was uploaded to this site." ;
        rdfs:label    "uploadDate" .

schema:Number  rdf:type  rdfs:Class ;
        rdfs:comment  "Data type: Number.\\n\\nUsage guidelines:\\n\\n* Use values from 0123456789 (Unicode 'DIGIT ZERO' (U+0030) to 'DIGIT NINE' (U+0039)) rather than superficially similiar Unicode symbols.\\n* Use '.' (Unicode 'FULL STOP' (U+002E)) rather than ',' to indicate a decimal point. Avoid using these symbols as a readability separator." ;
        rdfs:label    "Number" .

schema:specialCommitments
        rdf:type      rdf:Property ;
        rdfs:comment  "Any special commitments associated with this job posting. Valid entries include VeteranCommit, MilitarySpouseCommit, etc." ;
        rdfs:label    "specialCommitments" .

schema:claimReviewed  rdf:type  rdf:Property ;
        rdfs:comment  "A short summary of the specific claims reviewed in a ClaimReview." ;
        rdfs:label    "claimReviewed" .

schema:Float  rdf:type   rdfs:Class ;
        rdfs:comment     "Data type: Floating number." ;
        rdfs:label       "Float" ;
        rdfs:subClassOf  schema:Number .

skos:OrderedCollection
        rdf:type         rdfs:Class ;
        rdfs:label       "Ordered Collection"@en ;
        rdfs:subClassOf  skos:Collection .

schema:legislationTransposes
        rdf:type            rdf:Property ;
        rdfs:comment        "Indicates that this legislation (or part of legislation) fulfills the objectives set by another legislation, by passing appropriate implementation measures. Typically, some legislations of European Union's member states or regions transpose European Directives. This indicates a legally binding link between the 2 legislations." ;
        rdfs:label          "legislationTransposes" ;
        rdfs:subPropertyOf  schema:legislationApplies .

schema:prepTime  rdf:type  rdf:Property ;
        rdfs:comment  "The length of time it takes to prepare the items to be used in instructions or a direction, in [ISO 8601 duration format](http://en.wikipedia.org/wiki/ISO_8601)." ;
        rdfs:label    "prepTime" .

schema:availableAtOrFrom
        rdf:type            rdf:Property ;
        rdfs:comment        "The place(s) from which the offer can be obtained (e.g. store locations)." ;
        rdfs:label          "availableAtOrFrom" ;
        rdfs:subPropertyOf  schema:areaServed .

schema:textValue  rdf:type  rdf:Property ;
        rdfs:comment  "Text value being annotated." ;
        rdfs:label    "textValue" .

schema:CommentAction  rdf:type  rdfs:Class ;
        rdfs:comment     "The act of generating a comment about a subject." ;
        rdfs:label       "CommentAction" ;
        rdfs:subClassOf  schema:CommunicateAction .

schema:verificationFactCheckingPolicy
        rdf:type            rdf:Property ;
        rdfs:comment        "Disclosure about verification and fact-checking processes for a [[NewsMediaOrganization]] or other fact-checking [[Organization]]." ;
        rdfs:label          "verificationFactCheckingPolicy" ;
        rdfs:subPropertyOf  schema:publishingPrinciples .

schema:RentAction  rdf:type  rdfs:Class ;
        rdfs:comment     "The act of giving money in return for temporary use, but not ownership, of an object such as a vehicle or property. For example, an agent rents a property from a landlord in exchange for a periodic payment." ;
        rdfs:label       "RentAction" ;
        rdfs:subClassOf  schema:TradeAction .

schema:sensoryRequirement
        rdf:type      rdf:Property ;
        rdfs:comment  "A description of any sensory requirements and levels necessary to function on the job, including hearing and vision. Defined terms such as those in O*net may be used, but note that there is no way to specify the level of ability as well as its nature when using a defined term." ;
        rdfs:label    "sensoryRequirement" .

schema:numberOfAxles  rdf:type  rdf:Property ;
        rdfs:comment  "The number of axles.\\n\\nTypical unit code(s): C62" ;
        rdfs:label    "numberOfAxles" .

schema:embedUrl  rdf:type  rdf:Property ;
        rdfs:comment  "A URL pointing to a player for a specific video. In general, this is the information in the ```src``` element of an ```embed``` tag and should not be the same as the content of the ```loc``` tag." ;
        rdfs:label    "embedUrl" .

schema:permissions  rdf:type  rdf:Property ;
        rdfs:comment  "Permission(s) required to run the app (for example, a mobile app may require full internet access or may run only on wifi)." ;
        rdfs:label    "permissions" .

schema:parentItem  rdf:type  rdf:Property ;
        rdfs:comment  "The parent of a question, answer or item in general." ;
        rdfs:label    "parentItem" .

schema:Manuscript  rdf:type  rdfs:Class ;
        rdfs:comment     "A book, document, or piece of music written by hand rather than typed or printed." ;
        rdfs:label       "Manuscript" ;
        rdfs:subClassOf  schema:CreativeWork .

schema:riskFactor  rdf:type  rdf:Property ;
        rdfs:comment  "A modifiable or non-modifiable factor that increases the risk of a patient contracting this condition, e.g. age,  coexisting condition." ;
        rdfs:label    "riskFactor" .

schema:observedNode  rdf:type  rdf:Property ;
        rdfs:comment  "The observedNode of an [[Observation]], often a [[StatisticalPopulation]]." ;
        rdfs:label    "observedNode" .

schema:PublicSwimmingPool
        rdf:type         rdfs:Class ;
        rdfs:comment     "A public swimming pool." ;
        rdfs:label       "PublicSwimmingPool" ;
        rdfs:subClassOf  schema:SportsActivityLocation .

schema:authenticator  rdf:type  rdf:Property ;
        rdfs:comment  "The Organization responsible for authenticating the user's subscription. For example, many media apps require a cable/satellite provider to authenticate your subscription before playing media." ;
        rdfs:label    "authenticator" .

schema:OutletStore  rdf:type  rdfs:Class ;
        rdfs:comment     "An outlet store." ;
        rdfs:label       "OutletStore" ;
        rdfs:subClassOf  schema:Store .

schema:screenCount  rdf:type  rdf:Property ;
        rdfs:comment  "The number of screens in the movie theater." ;
        rdfs:label    "screenCount" .

schema:organizer  rdf:type  rdf:Property ;
        rdfs:comment  "An organizer of an Event." ;
        rdfs:label    "organizer" .

schema:ExerciseAction
        rdf:type         rdfs:Class ;
        rdfs:comment     "The act of participating in exertive activity for the purposes of improving health and fitness." ;
        rdfs:label       "ExerciseAction" ;
        rdfs:subClassOf  schema:PlayAction .

schema:Psychiatric  rdf:type  rdfs:Class ;
        rdfs:comment     "A specific branch of medical science that is concerned with the study, treatment, and prevention of mental illness, using both medical and psychological therapies." ;
        rdfs:label       "Psychiatric" ;
        rdfs:subClassOf  schema:MedicalBusiness .

schema:Accommodation  rdf:type  rdfs:Class ;
        rdfs:comment     "An accommodation is a place that can accommodate human beings, e.g. a hotel room, a camping pitch, or a meeting room. Many accommodations are for overnight stays, but this is not a mandatory requirement.\nFor more specific types of accommodations not defined in schema.org, one can use additionalType with external vocabularies.\n<br /><br />\nSee also the <a href=\"/docs/hotels.html\">dedicated document on the use of schema.org for marking up hotels and other forms of accommodations</a>.\n" ;
        rdfs:label       "Accommodation" ;
        rdfs:subClassOf  schema:Place .

schema:mapType  rdf:type  rdf:Property ;
        rdfs:comment  "Indicates the kind of Map, from the MapCategoryType Enumeration." ;
        rdfs:label    "mapType" .

schema:departureAirport
        rdf:type      rdf:Property ;
        rdfs:comment  "The airport where the flight originates." ;
        rdfs:label    "departureAirport" .

schema:bloodSupply  rdf:type  rdf:Property ;
        rdfs:comment  "The blood vessel that carries blood from the heart to the muscle." ;
        rdfs:label    "bloodSupply" .

schema:numberOfAvailableAccommodationUnits
        rdf:type      rdf:Property ;
        rdfs:comment  "Indicates the number of available accommodation units in an [[ApartmentComplex]], or the number of accommodation units for a specific [[FloorPlan]] (within its specific [[ApartmentComplex]]). See also [[numberOfAccommodationUnits]]." ;
        rdfs:label    "numberOfAvailableAccommodationUnits" .

schema:AutoRepair  rdf:type  rdfs:Class ;
        rdfs:comment     "Car repair business." ;
        rdfs:label       "AutoRepair" ;
        rdfs:subClassOf  schema:AutomotiveBusiness .

schema:unsaturatedFatContent
        rdf:type      rdf:Property ;
        rdfs:comment  "The number of grams of unsaturated fat." ;
        rdfs:label    "unsaturatedFatContent" .

schema:durationOfWarranty
        rdf:type      rdf:Property ;
        rdfs:comment  "The duration of the warranty promise. Common unitCode values are ANN for year, MON for months, or DAY for days." ;
        rdfs:label    "durationOfWarranty" .

schema:department  rdf:type  rdf:Property ;
        rdfs:comment  "A relationship between an organization and a department of that organization, also described as an organization (allowing different urls, logos, opening hours). For example: a store with a pharmacy, or a bakery with a cafe." ;
        rdfs:label    "department" .

schema:CourseInstance
        rdf:type         rdfs:Class ;
        rdfs:comment     "An instance of a [[Course]] which is distinct from other instances because it is offered at a different time or location or through different media or modes of study or to a specific section of students." ;
        rdfs:label       "CourseInstance" ;
        rdfs:subClassOf  schema:Event .

schema:email  rdf:type  rdf:Property ;
        rdfs:comment  "Email address." ;
        rdfs:label    "email" .

schema:copyrightYear  rdf:type  rdf:Property ;
        rdfs:comment  "The year during which the claimed copyright for the CreativeWork was first asserted." ;
        rdfs:label    "copyrightYear" .

schema:contactOption  rdf:type  rdf:Property ;
        rdfs:comment  "An option available on this contact point (e.g. a toll-free number or support for hearing-impaired callers)." ;
        rdfs:label    "contactOption" .

schema:representativeOfPage
        rdf:type      rdf:Property ;
        rdfs:comment  "Indicates whether this image is representative of the content of the page." ;
        rdfs:label    "representativeOfPage" .

schema:MedicalRiskEstimator
        rdf:type         rdfs:Class ;
        rdfs:comment     "Any rule set or interactive tool for estimating the risk of developing a complication or condition." ;
        rdfs:label       "MedicalRiskEstimator" ;
        rdfs:subClassOf  schema:MedicalEntity .

schema:name  rdf:type       rdf:Property ;
        rdfs:comment        "The name of the item." ;
        rdfs:label          "name" ;
        rdfs:subPropertyOf  rdfs:label .

schema:usageInfo  rdf:type  rdf:Property ;
        rdfs:comment  "The schema.org [[usageInfo]] property indicates further information about a [[CreativeWork]]. This property is applicable both to works that are freely available and to those that require payment or other transactions. It can reference additional information e.g. community expectations on preferred linking and citation conventions, as well as purchasing details. For something that can be commercially licensed, usageInfo can provide detailed, resource-specific information about licensing options.\n\nThis property can be used alongside the license property which indicates license(s) applicable to some piece of content. The usageInfo property can provide information about other licensing options, e.g. acquiring commercial usage rights for an image that is also available under non-commercial creative commons licenses." ;
        rdfs:label    "usageInfo" .

schema:subEvent  rdf:type  rdf:Property ;
        rdfs:comment  "An Event that is part of this event. For example, a conference event includes many presentations, each of which is a subEvent of the conference." ;
        rdfs:label    "subEvent" .

schema:Thesis  rdf:type  rdfs:Class ;
        rdfs:comment     "A thesis or dissertation document submitted in support of candidature for an academic degree or professional qualification." ;
        rdfs:label       "Thesis" ;
        rdfs:subClassOf  schema:CreativeWork .

schema:MedicalRiskFactor
        rdf:type         rdfs:Class ;
        rdfs:comment     "A risk factor is anything that increases a person's likelihood of developing or contracting a disease, medical condition, or complication." ;
        rdfs:label       "MedicalRiskFactor" ;
        rdfs:subClassOf  schema:MedicalEntity .

schema:diversityStaffingReport
        rdf:type            rdf:Property ;
        rdfs:comment        "For an [[Organization]] (often but not necessarily a [[NewsMediaOrganization]]), a report on staffing diversity issues. In a news context this might be for example ASNE or RTDNA (US) reports, or self-reported." ;
        rdfs:label          "diversityStaffingReport" ;
        rdfs:subPropertyOf  schema:publishingPrinciples .

schema:healthcareReportingData
        rdf:type      rdf:Property ;
        rdfs:comment  "Indicates data describing a hospital, e.g. a CDC [[CDCPMDRecord]] or as some kind of [[Dataset]]." ;
        rdfs:label    "healthcareReportingData" .

skos:inScheme  rdf:type  owl:ObjectProperty ;
        rdfs:label  "is in scheme"@en ;
        rdfs:range  skos:ConceptScheme .

schema:HomeAndConstructionBusiness
        rdf:type         rdfs:Class ;
        rdfs:comment     "A construction business.\\n\\nA HomeAndConstructionBusiness is a [[LocalBusiness]] that provides services around homes and buildings.\\n\\nAs a [[LocalBusiness]] it can be described as a [[provider]] of one or more [[Service]]\\(s)." ;
        rdfs:label       "HomeAndConstructionBusiness" ;
        rdfs:subClassOf  schema:LocalBusiness .

schema:icaoCode  rdf:type  rdf:Property ;
        rdfs:comment  "ICAO identifier for an airport." ;
        rdfs:label    "icaoCode" .

schema:actionStatus  rdf:type  rdf:Property ;
        rdfs:comment  "Indicates the current disposition of the Action." ;
        rdfs:label    "actionStatus" .

schema:itemCondition  rdf:type  rdf:Property ;
        rdfs:comment  "A predefined value from OfferItemCondition or a textual description of the condition of the product or service, or the products or services included in the offer." ;
        rdfs:label    "itemCondition" .

schema:sameAs  rdf:type  rdf:Property ;
        rdfs:comment  "URL of a reference Web page that unambiguously indicates the item's identity. E.g. the URL of the item's Wikipedia page, Wikidata entry, or official website." ;
        rdfs:label    "sameAs" .

schema:AlignmentObject
        rdf:type         rdfs:Class ;
        rdfs:comment     "An intangible item that describes an alignment between a learning resource and a node in an educational framework.\n\nShould not be used where the nature of the alignment can be described using a simple property, for example to express that a resource [[teaches]] or [[assesses]] a competency." ;
        rdfs:label       "AlignmentObject" ;
        rdfs:subClassOf  schema:Intangible .

schema:VideoGameSeries
        rdf:type         rdfs:Class ;
        rdfs:comment     "A video game series." ;
        rdfs:label       "VideoGameSeries" ;
        rdfs:subClassOf  schema:CreativeWorkSeries .

schema:safetyConsideration
        rdf:type      rdf:Property ;
        rdfs:comment  "Any potential safety concern associated with the supplement. May include interactions with other drugs and foods, pregnancy, breastfeeding, known adverse reactions, and documented efficacy of the supplement." ;
        rdfs:label    "safetyConsideration" .

schema:permissionType
        rdf:type      rdf:Property ;
        rdfs:comment  "The type of permission granted the person, organization, or audience." ;
        rdfs:label    "permissionType" .

schema:associatedAnatomy
        rdf:type      rdf:Property ;
        rdfs:comment  "The anatomy of the underlying organ system or structures associated with this entity." ;
        rdfs:label    "associatedAnatomy" .

schema:RadiationTherapy
        rdf:type         rdfs:Class ;
        rdfs:comment     "A process of care using radiation aimed at improving a health condition." ;
        rdfs:label       "RadiationTherapy" ;
        rdfs:subClassOf  schema:MedicalTherapy .

schema:legislationType
        rdf:type            rdf:Property ;
        rdfs:comment        "The type of the legislation. Examples of values are \"law\", \"act\", \"directive\", \"decree\", \"regulation\", \"statutory instrument\", \"loi organique\", \"règlement grand-ducal\", etc., depending on the country." ;
        rdfs:label          "legislationType" ;
        rdfs:subPropertyOf  schema:genre .

schema:Episode  rdf:type  rdfs:Class ;
        rdfs:comment     "A media episode (e.g. TV, radio, video game) which can be part of a series or season." ;
        rdfs:label       "Episode" ;
        rdfs:subClassOf  schema:CreativeWork .

schema:Reservation  rdf:type  rdfs:Class ;
        rdfs:comment     "Describes a reservation for travel, dining or an event. Some reservations require tickets. \\n\\nNote: This type is for information about actual reservations, e.g. in confirmation emails or HTML pages with individual confirmations of reservations. For offers of tickets, restaurant reservations, flights, or rental cars, use [[Offer]]." ;
        rdfs:label       "Reservation" ;
        rdfs:subClassOf  schema:Intangible .

schema:SiteNavigationElement
        rdf:type         rdfs:Class ;
        rdfs:comment     "A navigation element of the page." ;
        rdfs:label       "SiteNavigationElement" ;
        rdfs:subClassOf  schema:WebPageElement .

schema:legislationResponsible
        rdf:type      rdf:Property ;
        rdfs:comment  "An individual or organization that has some kind of responsibility for the legislation. Typically the ministry who is/was in charge of elaborating the legislation, or the adressee for potential questions about the legislation once it is published." ;
        rdfs:label    "legislationResponsible" .

schema:UseAction  rdf:type  rdfs:Class ;
        rdfs:comment     "The act of applying an object to its intended purpose." ;
        rdfs:label       "UseAction" ;
        rdfs:subClassOf  schema:ConsumeAction .

schema:workPresented  rdf:type  rdf:Property ;
        rdfs:comment        "The movie presented during this event." ;
        rdfs:label          "workPresented" ;
        rdfs:subPropertyOf  schema:workFeatured .

skos:broadMatch  rdf:type   owl:ObjectProperty ;
        rdfs:label          "has broader match"@en ;
        rdfs:subPropertyOf  skos:broader , skos:mappingRelation ;
        owl:inverseOf       skos:narrowMatch .

schema:originatesFrom
        rdf:type      rdf:Property ;
        rdfs:comment  "The vasculature the lymphatic structure originates, or afferents, from." ;
        rdfs:label    "originatesFrom" .

schema:WearableSizeGroupEnumeration
        rdf:type         rdfs:Class ;
        rdfs:comment     "Enumerates common size groups (also known as \"size types\") for wearable products." ;
        rdfs:label       "WearableSizeGroupEnumeration" ;
        rdfs:subClassOf  schema:SizeGroupEnumeration .

schema:Comment  rdf:type  rdfs:Class ;
        rdfs:comment     "A comment on an item - for example, a comment on a blog post. The comment's content is expressed via the [[text]] property, and its topic via [[about]], properties shared with all CreativeWorks." ;
        rdfs:label       "Comment" ;
        rdfs:subClassOf  schema:CreativeWork .

schema:video  rdf:type  rdf:Property ;
        rdfs:comment  "An embedded video object." ;
        rdfs:label    "video" .

schema:MedicalSymptom
        rdf:type         rdfs:Class ;
        rdfs:comment     "Any complaint sensed and expressed by the patient (therefore defined as subjective)  like stomachache, lower-back pain, or fatigue." ;
        rdfs:label       "MedicalSymptom" ;
        rdfs:subClassOf  schema:MedicalSignOrSymptom .

schema:PaymentService
        rdf:type         rdfs:Class ;
        rdfs:comment     "A Service to transfer funds from a person or organization to a beneficiary person or organization." ;
        rdfs:label       "PaymentService" ;
        rdfs:subClassOf  schema:FinancialProduct .

schema:legalStatus  rdf:type  rdf:Property ;
        rdfs:comment  "The drug or supplement's legal status, including any controlled substance schedules that apply." ;
        rdfs:label    "legalStatus" .

schema:Thing  rdf:type  rdfs:Class ;
        rdfs:comment  "The most generic type of item." ;
        rdfs:label    "Thing" .

schema:affiliation  rdf:type  rdf:Property ;
        rdfs:comment        "An organization that this person is affiliated with. For example, a school/university, a club, or a team." ;
        rdfs:label          "affiliation" ;
        rdfs:subPropertyOf  schema:memberOf .

schema:recommendationStrength
        rdf:type      rdf:Property ;
        rdfs:comment  "Strength of the guideline's recommendation (e.g. 'class I')." ;
        rdfs:label    "recommendationStrength" .

schema:ItemAvailability
        rdf:type         rdfs:Class ;
        rdfs:comment     "A list of possible product availability options." ;
        rdfs:label       "ItemAvailability" ;
        rdfs:subClassOf  schema:Enumeration .

schema:numberOfLoanPayments
        rdf:type      rdf:Property ;
        rdfs:comment  "The number of payments contractually required at origination to repay the loan. For monthly paying loans this is the number of months from the contractual first payment date to the maturity date." ;
        rdfs:label    "numberOfLoanPayments" .

schema:HowToDirection
        rdf:type         rdfs:Class ;
        rdfs:comment     "A direction indicating a single action to do in the instructions for how to achieve a result." ;
        rdfs:label       "HowToDirection" ;
        rdfs:subClassOf  schema:ListItem , schema:CreativeWork .

schema:MobilePhoneStore
        rdf:type         rdfs:Class ;
        rdfs:comment     "A store that sells mobile phones and related accessories." ;
        rdfs:label       "MobilePhoneStore" ;
        rdfs:subClassOf  schema:Store .

schema:PhysicalExam  rdf:type  rdfs:Class ;
        rdfs:comment     "A type of physical examination of a patient performed by a physician. " ;
        rdfs:label       "PhysicalExam" ;
        rdfs:subClassOf  schema:MedicalEnumeration , schema:MedicalProcedure .

skos:topConceptOf  rdf:type  owl:ObjectProperty ;
        rdfs:domain         skos:Concept ;
        rdfs:label          "is top concept in scheme"@en ;
        rdfs:range          skos:ConceptScheme ;
        rdfs:subPropertyOf  skos:inScheme ;
        owl:inverseOf       skos:hasTopConcept .

schema:associatedArticle
        rdf:type      rdf:Property ;
        rdfs:comment  "A NewsArticle associated with the Media Object." ;
        rdfs:label    "associatedArticle" .

schema:PerformingArtsTheater
        rdf:type         rdfs:Class ;
        rdfs:comment     "A theater or other performing art center." ;
        rdfs:label       "PerformingArtsTheater" ;
        rdfs:subClassOf  schema:CivicStructure .

schema:SteeringPositionValue
        rdf:type         rdfs:Class ;
        rdfs:comment     "A value indicating a steering position." ;
        rdfs:label       "SteeringPositionValue" ;
        rdfs:subClassOf  schema:QualitativeValue .

schema:securityClearanceRequirement
        rdf:type      rdf:Property ;
        rdfs:comment  "A description of any security clearance requirements of the job." ;
        rdfs:label    "securityClearanceRequirement" .

schema:latitude  rdf:type  rdf:Property ;
        rdfs:comment  "The latitude of a location. For example ```37.42242``` ([WGS 84](https://en.wikipedia.org/wiki/World_Geodetic_System))." ;
        rdfs:label    "latitude" .

schema:WebPageElement
        rdf:type         rdfs:Class ;
        rdfs:comment     "A web page element, like a table or an image." ;
        rdfs:label       "WebPageElement" ;
        rdfs:subClassOf  schema:CreativeWork .

schema:Church  rdf:type  rdfs:Class ;
        rdfs:comment     "A church." ;
        rdfs:label       "Church" ;
        rdfs:subClassOf  schema:PlaceOfWorship .

schema:preOp  rdf:type  rdf:Property ;
        rdfs:comment  "A description of the workup, testing, and other preparations required before implanting this device." ;
        rdfs:label    "preOp" .

schema:EventSeries  rdf:type  rdfs:Class ;
        rdfs:comment     "A series of [[Event]]s. Included events can relate with the series using the [[superEvent]] property.\n\nAn EventSeries is a collection of events that share some unifying characteristic. For example, \"The Olympic Games\" is a series, which\nis repeated regularly. The \"2012 London Olympics\" can be presented both as an [[Event]] in the series \"Olympic Games\", and as an\n[[EventSeries]] that included a number of sporting competitions as Events.\n\nThe nature of the association between the events in an [[EventSeries]] can vary, but typical examples could\ninclude a thematic event series (e.g. topical meetups or classes), or a series of regular events that share a location, attendee group and/or organizers.\n\nEventSeries has been defined as a kind of Event to make it easy for publishers to use it in an Event context without\nworrying about which kinds of series are really event-like enough to call an Event. In general an EventSeries\nmay seem more Event-like when the period of time is compact and when aspects such as location are fixed, but\nit may also sometimes prove useful to describe a longer-term series as an Event.\n   " ;
        rdfs:label       "EventSeries" ;
        rdfs:subClassOf  schema:Event , schema:Series .

schema:Substance  rdf:type  rdfs:Class ;
        rdfs:comment     "Any matter of defined composition that has discrete existence, whose origin may be biological, mineral or chemical." ;
        rdfs:label       "Substance" ;
        rdfs:subClassOf  schema:MedicalEntity .

schema:TieAction  rdf:type  rdfs:Class ;
        rdfs:comment     "The act of reaching a draw in a competitive activity." ;
        rdfs:label       "TieAction" ;
        rdfs:subClassOf  schema:AchieveAction .

schema:pageEnd  rdf:type  rdf:Property ;
        rdfs:comment  "The page on which the work ends; for example \"138\" or \"xvi\"." ;
        rdfs:label    "pageEnd" .

schema:intensity  rdf:type  rdf:Property ;
        rdfs:comment  "Quantitative measure gauging the degree of force involved in the exercise, for example, heartbeats per minute. May include the velocity of the movement." ;
        rdfs:label    "intensity" .

schema:healthPlanNetworkId
        rdf:type      rdf:Property ;
        rdfs:comment  "Name or unique ID of network. (Networks are often reused across different insurance plans)." ;
        rdfs:label    "healthPlanNetworkId" .

schema:Cemetery  rdf:type  rdfs:Class ;
        rdfs:comment     "A graveyard." ;
        rdfs:label       "Cemetery" ;
        rdfs:subClassOf  schema:CivicStructure .

schema:relatedTo  rdf:type  rdf:Property ;
        rdfs:comment  "The most generic familial relation." ;
        rdfs:label    "relatedTo" .

schema:HyperTocEntry  rdf:type  rdfs:Class ;
        rdfs:comment     "A HyperToEntry is an item within a [[HyperToc]], which represents a hypertext table of contents for complex media objects, such as [[VideoObject]], [[AudioObject]]. The media object itself is indicated using [[associatedMedia]]. Each section of interest within that content can be described with a [[HyperTocEntry]], with associated [[startOffset]] and [[endOffset]]. When several entries are all from the same file, [[associatedMedia]] is used on the overarching [[HyperTocEntry]]; if the content has been split into multiple files, they can be referenced using [[associatedMedia]] on each [[HyperTocEntry]]." ;
        rdfs:label       "HyperTocEntry" ;
        rdfs:subClassOf  schema:CreativeWork .

schema:Periodical  rdf:type  rdfs:Class ;
        rdfs:comment     "A publication in any medium issued in successive parts bearing numerical or chronological designations and intended, such as a magazine, scholarly journal, or newspaper to continue indefinitely.\\n\\nSee also [blog post](http://blog.schema.org/2014/09/schemaorg-support-for-bibliographic_2.html)." ;
        rdfs:label       "Periodical" ;
        rdfs:subClassOf  schema:CreativeWorkSeries .

schema:toRecipient  rdf:type  rdf:Property ;
        rdfs:comment        "A sub property of recipient. The recipient who was directly sent the message." ;
        rdfs:label          "toRecipient" ;
        rdfs:subPropertyOf  schema:recipient .

schema:pickupTime  rdf:type  rdf:Property ;
        rdfs:comment  "When a taxi will pickup a passenger or a rental car can be picked up." ;
        rdfs:label    "pickupTime" .

schema:bestRating  rdf:type  rdf:Property ;
        rdfs:comment  "The highest value allowed in this rating system. If bestRating is omitted, 5 is assumed." ;
        rdfs:label    "bestRating" .

schema:FundingAgency  rdf:type  rdfs:Class ;
        rdfs:comment     "A FundingAgency is an organization that implements one or more [[FundingScheme]]s and manages\n    the granting process (via [[Grant]]s, typically [[MonetaryGrant]]s).\n    A funding agency is not always required for grant funding, e.g. philanthropic giving, corporate sponsorship etc.\n    \nExamples of funding agencies include ERC, REA, NIH, Bill and Melinda Gates Foundation...\n    " ;
        rdfs:label       "FundingAgency" ;
        rdfs:subClassOf  schema:Project .

schema:OfferCatalog  rdf:type  rdfs:Class ;
        rdfs:comment     "An OfferCatalog is an ItemList that contains related Offers and/or further OfferCatalogs that are offeredBy the same provider." ;
        rdfs:label       "OfferCatalog" ;
        rdfs:subClassOf  schema:ItemList .

schema:WholesaleStore
        rdf:type         rdfs:Class ;
        rdfs:comment     "A wholesale store." ;
        rdfs:label       "WholesaleStore" ;
        rdfs:subClassOf  schema:Store .

schema:BreadcrumbList
        rdf:type         rdfs:Class ;
        rdfs:comment     "A BreadcrumbList is an ItemList consisting of a chain of linked Web pages, typically described using at least their URL and their name, and typically ending with the current page.\\n\\nThe [[position]] property is used to reconstruct the order of the items in a BreadcrumbList The convention is that a breadcrumb list has an [[itemListOrder]] of [[ItemListOrderAscending]] (lower values listed first), and that the first items in this list correspond to the \"top\" or beginning of the breadcrumb trail, e.g. with a site or section homepage. The specific values of 'position' are not assigned meaning for a BreadcrumbList, but they should be integers, e.g. beginning with '1' for the first item in the list.\n      " ;
        rdfs:label       "BreadcrumbList" ;
        rdfs:subClassOf  schema:ItemList .

schema:BusTrip  rdf:type  rdfs:Class ;
        rdfs:comment     "A trip on a commercial bus line." ;
        rdfs:label       "BusTrip" ;
        rdfs:subClassOf  schema:Trip .

schema:gameTip  rdf:type  rdf:Property ;
        rdfs:comment  "Links to tips, tactics, etc." ;
        rdfs:label    "gameTip" .

schema:worksFor  rdf:type  rdf:Property ;
        rdfs:comment  "Organizations that the person works for." ;
        rdfs:label    "worksFor" .

schema:emissionsCO2  rdf:type  rdf:Property ;
        rdfs:comment  "The CO2 emissions in g/km. When used in combination with a QuantitativeValue, put \"g/km\" into the unitText property of that value, since there is no UN/CEFACT Common Code for \"g/km\"." ;
        rdfs:label    "emissionsCO2" .

schema:photo  rdf:type      rdf:Property ;
        rdfs:comment        "A photograph of this place." ;
        rdfs:label          "photo" ;
        rdfs:subPropertyOf  schema:image .

schema:RadioChannel  rdf:type  rdfs:Class ;
        rdfs:comment     "A unique instance of a radio BroadcastService on a CableOrSatelliteService lineup." ;
        rdfs:label       "RadioChannel" ;
        rdfs:subClassOf  schema:BroadcastChannel .

schema:partySize  rdf:type  rdf:Property ;
        rdfs:comment  "Number of people the reservation should accommodate." ;
        rdfs:label    "partySize" .

schema:EmailMessage  rdf:type  rdfs:Class ;
        rdfs:comment     "An email message." ;
        rdfs:label       "EmailMessage" ;
        rdfs:subClassOf  schema:Message .

schema:CollectionPage
        rdf:type         rdfs:Class ;
        rdfs:comment     "Web page type: Collection page." ;
        rdfs:label       "CollectionPage" ;
        rdfs:subClassOf  schema:WebPage .

schema:EmploymentAgency
        rdf:type         rdfs:Class ;
        rdfs:comment     "An employment agency." ;
        rdfs:label       "EmploymentAgency" ;
        rdfs:subClassOf  schema:LocalBusiness .

schema:Pharmacy  rdf:type  rdfs:Class ;
        rdfs:comment     "A pharmacy or drugstore." ;
        rdfs:label       "Pharmacy" ;
        rdfs:subClassOf  schema:MedicalBusiness , schema:MedicalOrganization .

schema:color  rdf:type  rdf:Property ;
        rdfs:comment  "The color of the product." ;
        rdfs:label    "color" .

schema:producer  rdf:type  rdf:Property ;
        rdfs:comment  "The person or organization who produced the work (e.g. music album, movie, tv/radio series etc.)." ;
        rdfs:label    "producer" .

schema:Landform  rdf:type  rdfs:Class ;
        rdfs:comment     "A landform or physical feature.  Landform elements include mountains, plains, lakes, rivers, seascape and oceanic waterbody interface features such as bays, peninsulas, seas and so forth, including sub-aqueous terrain features such as submersed mountain ranges, volcanoes, and the great ocean basins." ;
        rdfs:label       "Landform" ;
        rdfs:subClassOf  schema:Place .

schema:hasVariant  rdf:type  rdf:Property ;
        rdfs:comment  "Indicates a [[Product]] that is a member of this [[ProductGroup]] (or [[ProductModel]])." ;
        rdfs:label    "hasVariant" .

schema:free  rdf:type  rdf:Property ;
        rdfs:comment  "A flag to signal that the item, event, or place is accessible for free." ;
        rdfs:label    "free" .

schema:acquireLicensePage
        rdf:type            rdf:Property ;
        rdfs:comment        "Indicates a page documenting how licenses can be purchased or otherwise acquired, for the current item." ;
        rdfs:label          "acquireLicensePage" ;
        rdfs:subPropertyOf  schema:usageInfo .

schema:MoneyTransfer  rdf:type  rdfs:Class ;
        rdfs:comment     "The act of transferring money from one place to another place. This may occur electronically or physically." ;
        rdfs:label       "MoneyTransfer" ;
        rdfs:subClassOf  schema:TransferAction .

schema:startOffset  rdf:type  rdf:Property ;
        rdfs:comment  "The start time of the clip expressed as the number of seconds from the beginning of the work." ;
        rdfs:label    "startOffset" .

schema:cheatCode  rdf:type  rdf:Property ;
        rdfs:comment  "Cheat codes to the game." ;
        rdfs:label    "cheatCode" .

schema:GardenStore  rdf:type  rdfs:Class ;
        rdfs:comment     "A garden store." ;
        rdfs:label       "GardenStore" ;
        rdfs:subClassOf  schema:Store .

schema:MediaGallery  rdf:type  rdfs:Class ;
        rdfs:comment     "Web page type: Media gallery page. A mixed-media page that can contains media such as images, videos, and other multimedia." ;
        rdfs:label       "MediaGallery" ;
        rdfs:subClassOf  schema:CollectionPage .

schema:GiveAction  rdf:type  rdfs:Class ;
        rdfs:comment     "The act of transferring ownership of an object to a destination. Reciprocal of TakeAction.\\n\\nRelated actions:\\n\\n* [[TakeAction]]: Reciprocal of GiveAction.\\n* [[SendAction]]: Unlike SendAction, GiveAction implies that ownership is being transferred (e.g. I may send my laptop to you, but that doesn't mean I'm giving it to you)." ;
        rdfs:label       "GiveAction" ;
        rdfs:subClassOf  schema:TransferAction .

schema:blogPost  rdf:type  rdf:Property ;
        rdfs:comment  "A posting that is part of this blog." ;
        rdfs:label    "blogPost" .

schema:USNonprofitType
        rdf:type         rdfs:Class ;
        rdfs:comment     "USNonprofitType: Non-profit organization type originating from the United States." ;
        rdfs:label       "USNonprofitType" ;
        rdfs:subClassOf  schema:NonprofitType .

schema:Audience  rdf:type  rdfs:Class ;
        rdfs:comment     "Intended audience for an item, i.e. the group for whom the item was created." ;
        rdfs:label       "Audience" ;
        rdfs:subClassOf  schema:Intangible .

schema:contributor  rdf:type  rdf:Property ;
        rdfs:comment  "A secondary contributor to the CreativeWork or Event." ;
        rdfs:label    "contributor" .

schema:application  rdf:type  rdf:Property ;
        rdfs:comment  "An application that can complete the request." ;
        rdfs:label    "application" .

skos:relatedMatch  rdf:type  owl:ObjectProperty ;
        rdfs:label          "has related match"@en ;
        rdfs:subPropertyOf  skos:related , skos:mappingRelation .

schema:educationRequirements
        rdf:type      rdf:Property ;
        rdfs:comment  "Educational background needed for the position or Occupation." ;
        rdfs:label    "educationRequirements" .

schema:DataType  rdf:type  rdfs:Class ;
        rdfs:comment     "The basic data types such as Integers, Strings, etc." ;
        rdfs:label       "DataType" ;
        rdfs:subClassOf  rdfs:Class .

schema:Rating  rdf:type  rdfs:Class ;
        rdfs:comment     "A rating is an evaluation on a numeric scale, such as 1 to 5 stars." ;
        rdfs:label       "Rating" ;
        rdfs:subClassOf  schema:Intangible .

schema:instructor  rdf:type  rdf:Property ;
        rdfs:comment  "A person assigned to instruct or provide instructional assistance for the [[CourseInstance]]." ;
        rdfs:label    "instructor" .

schema:experienceRequirements
        rdf:type      rdf:Property ;
        rdfs:comment  "Description of skills and experience needed for the position or Occupation." ;
        rdfs:label    "experienceRequirements" .

schema:Plumber  rdf:type  rdfs:Class ;
        rdfs:comment     "A plumbing service." ;
        rdfs:label       "Plumber" ;
        rdfs:subClassOf  schema:HomeAndConstructionBusiness .

schema:TouristTrip  rdf:type  rdfs:Class ;
        rdfs:comment     "A tourist trip. A created itinerary of visits to one or more places of interest ([[TouristAttraction]]/[[TouristDestination]]) often linked by a similar theme, geographic area, or interest to a particular [[touristType]]. The [UNWTO](http://www2.unwto.org/) defines tourism trip as the Trip taken by visitors.\n  (See examples below)." ;
        rdfs:label       "TouristTrip" ;
        rdfs:subClassOf  schema:Trip .

schema:paymentDueDate
        rdf:type      rdf:Property ;
        rdfs:comment  "The date that payment is due." ;
        rdfs:label    "paymentDueDate" .

schema:shippingLabel  rdf:type  rdf:Property ;
        rdfs:comment  "Label to match an [[OfferShippingDetails]] with a [[ShippingRateSettings]] (within the context of a [[shippingSettingsLink]] cross-reference)." ;
        rdfs:label    "shippingLabel" .

schema:competitor  rdf:type  rdf:Property ;
        rdfs:comment  "A competitor in a sports event." ;
        rdfs:label    "competitor" .

schema:increasesRiskOf
        rdf:type      rdf:Property ;
        rdfs:comment  "The condition, complication, etc. influenced by this factor." ;
        rdfs:label    "increasesRiskOf" .

schema:RadioSeason  rdf:type  rdfs:Class ;
        rdfs:comment     "Season dedicated to radio broadcast and associated online delivery." ;
        rdfs:label       "RadioSeason" ;
        rdfs:subClassOf  schema:CreativeWorkSeason .

schema:performers  rdf:type  rdf:Property ;
        rdfs:comment  "The main performer or performers of the event&#x2014;for example, a presenter, musician, or actor." ;
        rdfs:label    "performers" .

schema:numberOfEmployees
        rdf:type      rdf:Property ;
        rdfs:comment  "The number of employees in an organization e.g. business." ;
        rdfs:label    "numberOfEmployees" .

schema:endOffset  rdf:type  rdf:Property ;
        rdfs:comment  "The end time of the clip expressed as the number of seconds from the beginning of the work." ;
        rdfs:label    "endOffset" .

schema:suggestedGender
        rdf:type      rdf:Property ;
        rdfs:comment  "The suggested gender of the intended person or audience, for example \"male\", \"female\", or \"unisex\"." ;
        rdfs:label    "suggestedGender" .

schema:LearningResource
        rdf:type         rdfs:Class ;
        rdfs:comment     "The LearningResource type can be used to indicate [[CreativeWork]]s (whether physical or digital) that have a particular and explicit orientation towards learning, education, skill acquisition, and other educational purposes.\n\n[[LearningResource]] is expected to be used as an addition to a primary type such as [[Book]], [[VideoObject]], [[Product]] etc.\n\n[[EducationEvent]] serves a similar purpose for event-like things (e.g. a [[Trip]]). A [[LearningResource]] may be created as a result of an [[EducationEvent]], for example by recording one." ;
        rdfs:label       "LearningResource" ;
        rdfs:subClassOf  schema:CreativeWork .

schema:AutoPartsStore
        rdf:type         rdfs:Class ;
        rdfs:comment     "An auto parts store." ;
        rdfs:label       "AutoPartsStore" ;
        rdfs:subClassOf  schema:Store , schema:AutomotiveBusiness .

schema:UKNonprofitType
        rdf:type         rdfs:Class ;
        rdfs:comment     "UKNonprofitType: Non-profit organization type originating from the United Kingdom." ;
        rdfs:label       "UKNonprofitType" ;
        rdfs:subClassOf  schema:NonprofitType .

schema:MusicComposition
        rdf:type         rdfs:Class ;
        rdfs:comment     "A musical composition." ;
        rdfs:label       "MusicComposition" ;
        rdfs:subClassOf  schema:CreativeWork .

schema:DrugCostCategory
        rdf:type         rdfs:Class ;
        rdfs:comment     "Enumerated categories of medical drug costs." ;
        rdfs:label       "DrugCostCategory" ;
        rdfs:subClassOf  schema:MedicalEnumeration .

schema:algorithm  rdf:type  rdf:Property ;
        rdfs:comment  "The algorithm or rules to follow to compute the score." ;
        rdfs:label    "algorithm" .

schema:Beach  rdf:type   rdfs:Class ;
        rdfs:comment     "Beach." ;
        rdfs:label       "Beach" ;
        rdfs:subClassOf  schema:CivicStructure .

schema:hasEnergyEfficiencyCategory
        rdf:type      rdf:Property ;
        rdfs:comment  "Defines the energy efficiency Category (which could be either a rating out of range of values or a yes/no certification) for a product according to an international energy efficiency standard." ;
        rdfs:label    "hasEnergyEfficiencyCategory" .

schema:locationCreated
        rdf:type      rdf:Property ;
        rdfs:comment  "The location where the CreativeWork was created, which may not be the same as the location depicted in the CreativeWork." ;
        rdfs:label    "locationCreated" .

schema:CivicStructure
        rdf:type         rdfs:Class ;
        rdfs:comment     "A public structure, such as a town hall or concert hall." ;
        rdfs:label       "CivicStructure" ;
        rdfs:subClassOf  schema:Place .

schema:targetName  rdf:type  rdf:Property ;
        rdfs:comment  "The name of a node in an established educational framework." ;
        rdfs:label    "targetName" .

schema:validFrom  rdf:type  rdf:Property ;
        rdfs:comment  "The date when the item becomes valid." ;
        rdfs:label    "validFrom" .

schema:DoseSchedule  rdf:type  rdfs:Class ;
        rdfs:comment     "A specific dosing schedule for a drug or supplement." ;
        rdfs:label       "DoseSchedule" ;
        rdfs:subClassOf  schema:MedicalIntangible .

schema:PostalAddress  rdf:type  rdfs:Class ;
        rdfs:comment     "The mailing address." ;
        rdfs:label       "PostalAddress" ;
        rdfs:subClassOf  schema:ContactPoint .

schema:arrivalStation
        rdf:type      rdf:Property ;
        rdfs:comment  "The station where the train trip ends." ;
        rdfs:label    "arrivalStation" .

schema:MovieClip  rdf:type  rdfs:Class ;
        rdfs:comment     "A short segment/part of a movie." ;
        rdfs:label       "MovieClip" ;
        rdfs:subClassOf  schema:Clip .

schema:ParcelDelivery
        rdf:type         rdfs:Class ;
        rdfs:comment     "The delivery of a parcel either via the postal service or a commercial service." ;
        rdfs:label       "ParcelDelivery" ;
        rdfs:subClassOf  schema:Intangible .

schema:MerchantReturnEnumeration
        rdf:type         rdfs:Class ;
        rdfs:comment     "MerchantReturnEnumeration enumerates several kinds of product return policy. Note that this structure may not capture all aspects of the policy." ;
        rdfs:label       "MerchantReturnEnumeration" ;
        rdfs:subClassOf  schema:Enumeration .

schema:VeterinaryCare
        rdf:type         rdfs:Class ;
        rdfs:comment     "A vet's office." ;
        rdfs:label       "VeterinaryCare" ;
        rdfs:subClassOf  schema:MedicalOrganization .

schema:ReportageNewsArticle
        rdf:type         rdfs:Class ;
        rdfs:comment     "The [[ReportageNewsArticle]] type is a subtype of [[NewsArticle]] representing\n news articles which are the result of journalistic news reporting conventions.\n\nIn practice many news publishers produce a wide variety of article types, many of which might be considered a [[NewsArticle]] but not a [[ReportageNewsArticle]]. For example, opinion pieces, reviews, analysis, sponsored or satirical articles, or articles that combine several of these elements.\n\nThe [[ReportageNewsArticle]] type is based on a stricter ideal for \"news\" as a work of journalism, with articles based on factual information either observed or verified by the author, or reported and verified from knowledgeable sources.  This often includes perspectives from multiple viewpoints on a particular issue (distinguishing news reports from public relations or propaganda).  News reports in the [[ReportageNewsArticle]] sense de-emphasize the opinion of the author, with commentary and value judgements typically expressed elsewhere.\n\nA [[ReportageNewsArticle]] which goes deeper into analysis can also be marked with an additional type of [[AnalysisNewsArticle]].\n" ;
        rdfs:label       "ReportageNewsArticle" ;
        rdfs:subClassOf  schema:NewsArticle .

schema:HowToTip  rdf:type  rdfs:Class ;
        rdfs:comment     "An explanation in the instructions for how to achieve a result. It provides supplementary information about a technique, supply, author's preference, etc. It can explain what could be done, or what should not be done, but doesn't specify what should be done (see HowToDirection)." ;
        rdfs:label       "HowToTip" ;
        rdfs:subClassOf  schema:ListItem , schema:CreativeWork .

schema:employerOverview
        rdf:type      rdf:Property ;
        rdfs:comment  "A description of the employer, career opportunities and work environment for this position." ;
        rdfs:label    "employerOverview" .

schema:maps  rdf:type  rdf:Property ;
        rdfs:comment  "A URL to a map of the place." ;
        rdfs:label    "maps" .

schema:CommunicateAction
        rdf:type         rdfs:Class ;
        rdfs:comment     "The act of conveying information to another person via a communication medium (instrument) such as speech, email, or telephone conversation." ;
        rdfs:label       "CommunicateAction" ;
        rdfs:subClassOf  schema:InteractAction .

schema:ImageGallery  rdf:type  rdfs:Class ;
        rdfs:comment     "Web page type: Image gallery page." ;
        rdfs:label       "ImageGallery" ;
        rdfs:subClassOf  schema:MediaGallery .

schema:touristType  rdf:type  rdf:Property ;
        rdfs:comment  "Attraction suitable for type(s) of tourist. eg. Children, visitors from a particular country, etc. " ;
        rdfs:label    "touristType" .

schema:breastfeedingWarning
        rdf:type      rdf:Property ;
        rdfs:comment  "Any precaution, guidance, contraindication, etc. related to this drug's use by breastfeeding mothers." ;
        rdfs:label    "breastfeedingWarning" .

schema:GatedResidenceCommunity
        rdf:type         rdfs:Class ;
        rdfs:comment     "Residence type: Gated community." ;
        rdfs:label       "GatedResidenceCommunity" ;
        rdfs:subClassOf  schema:Residence .

schema:subOrganization
        rdf:type      rdf:Property ;
        rdfs:comment  "A relationship between two organizations where the first includes the second, e.g., as a subsidiary. See also: the more specific 'department' property." ;
        rdfs:label    "subOrganization" .

schema:ClothingStore  rdf:type  rdfs:Class ;
        rdfs:comment     "A clothing store." ;
        rdfs:label       "ClothingStore" ;
        rdfs:subClassOf  schema:Store .

schema:CssSelectorType
        rdf:type         rdfs:Class ;
        rdfs:comment     "Text representing a CSS selector." ;
        rdfs:label       "CssSelectorType" ;
        rdfs:subClassOf  schema:Text .

schema:accommodationCategory
        rdf:type            rdf:Property ;
        rdfs:comment        "Category of an [[Accommodation]], following real estate conventions e.g. RESO (see [PropertySubType](https://ddwiki.reso.org/display/DDW17/PropertySubType+Field), and [PropertyType](https://ddwiki.reso.org/display/DDW17/PropertyType+Field) fields  for suggested values)." ;
        rdfs:label          "accommodationCategory" ;
        rdfs:subPropertyOf  schema:category .

schema:actionApplication
        rdf:type      rdf:Property ;
        rdfs:comment  "An application that can complete the request." ;
        rdfs:label    "actionApplication" .

schema:termsOfService
        rdf:type      rdf:Property ;
        rdfs:comment  "Human-readable terms of service documentation." ;
        rdfs:label    "termsOfService" .

schema:billingIncrement
        rdf:type      rdf:Property ;
        rdfs:comment  "This property specifies the minimal quantity and rounding increment that will be the basis for the billing. The unit of measurement is specified by the unitCode property." ;
        rdfs:label    "billingIncrement" .

bibo:Periodical  rdf:type  rdfs:Class .

schema:seatNumber  rdf:type  rdf:Property ;
        rdfs:comment  "The location of the reserved seat (e.g., 27)." ;
        rdfs:label    "seatNumber" .

schema:mathExpression
        rdf:type      rdf:Property ;
        rdfs:comment  "A mathematical expression (e.g. 'x^2-3x=0') that may be solved for a specific variable, simplified, or transformed. This can take many formats, e.g. LaTeX, Ascii-Math, or math as you would write with a keyboard." ;
        rdfs:label    "mathExpression" .

schema:PriceComponentTypeEnumeration
        rdf:type         rdfs:Class ;
        rdfs:comment     "Enumerates different price components that together make up the total price for an offered product." ;
        rdfs:label       "PriceComponentTypeEnumeration" ;
        rdfs:subClassOf  schema:Enumeration .

schema:numberOfAirbags
        rdf:type      rdf:Property ;
        rdfs:comment  "The number or type of airbags in the vehicle." ;
        rdfs:label    "numberOfAirbags" .

schema:ReadAction  rdf:type  rdfs:Class ;
        rdfs:comment     "The act of consuming written content." ;
        rdfs:label       "ReadAction" ;
        rdfs:subClassOf  schema:ConsumeAction .

schema:numberOfPartialBathrooms
        rdf:type      rdf:Property ;
        rdfs:comment  "Number of partial bathrooms - The total number of half and ¼ bathrooms in an [[Accommodation]]. This corresponds to the [BathroomsPartial field in RESO](https://ddwiki.reso.org/display/DDW17/BathroomsPartial+Field). " ;
        rdfs:label    "numberOfPartialBathrooms" .

schema:Energy  rdf:type  rdfs:Class ;
        rdfs:comment     "Properties that take Energy as values are of the form '&lt;Number&gt; &lt;Energy unit of measure&gt;'." ;
        rdfs:label       "Energy" ;
        rdfs:subClassOf  schema:Quantity .

schema:funder  rdf:type     rdf:Property ;
        rdfs:comment        "A person or organization that supports (sponsors) something through some kind of financial contribution." ;
        rdfs:label          "funder" ;
        rdfs:subPropertyOf  schema:sponsor .

schema:legislationLegalForce
        rdf:type      rdf:Property ;
        rdfs:comment  "Whether the legislation is currently in force, not in force, or partially in force." ;
        rdfs:label    "legislationLegalForce" .

schema:episodes  rdf:type  rdf:Property ;
        rdfs:comment  "An episode of a TV/radio series or season." ;
        rdfs:label    "episodes" .

schema:reviewBody  rdf:type  rdf:Property ;
        rdfs:comment  "The actual body of the review." ;
        rdfs:label    "reviewBody" .

schema:AutoBodyShop  rdf:type  rdfs:Class ;
        rdfs:comment     "Auto body shop." ;
        rdfs:label       "AutoBodyShop" ;
        rdfs:subClassOf  schema:AutomotiveBusiness .

schema:typeOfGood  rdf:type  rdf:Property ;
        rdfs:comment  "The product that this structured value is referring to." ;
        rdfs:label    "typeOfGood" .

schema:billingAddress
        rdf:type      rdf:Property ;
        rdfs:comment  "The billing address for the order." ;
        rdfs:label    "billingAddress" .

schema:BuyAction  rdf:type  rdfs:Class ;
        rdfs:comment     "The act of giving money to a seller in exchange for goods or services rendered. An agent buys an object, product, or service from a seller for a price. Reciprocal of SellAction." ;
        rdfs:label       "BuyAction" ;
        rdfs:subClassOf  schema:TradeAction .

schema:DataCatalog  rdf:type  rdfs:Class ;
        rdfs:comment     "A collection of datasets." ;
        rdfs:label       "DataCatalog" ;
        rdfs:subClassOf  schema:CreativeWork .

schema:postOp  rdf:type  rdf:Property ;
        rdfs:comment  "A description of the postoperative procedures, care, and/or followups for this device." ;
        rdfs:label    "postOp" .

schema:lastReviewed  rdf:type  rdf:Property ;
        rdfs:comment  "Date on which the content on this web page was last reviewed for accuracy and/or completeness." ;
        rdfs:label    "lastReviewed" .

schema:contentReferenceTime
        rdf:type      rdf:Property ;
        rdfs:comment  "The specific time described by a creative work, for works (e.g. articles, video objects etc.) that emphasise a particular moment within an Event." ;
        rdfs:label    "contentReferenceTime" .

schema:parentService  rdf:type  rdf:Property ;
        rdfs:comment  "A broadcast service to which the broadcast service may belong to such as regional variations of a national channel." ;
        rdfs:label    "parentService" .

schema:caption  rdf:type  rdf:Property ;
        rdfs:comment  "The caption for this object. For downloadable machine formats (closed caption, subtitles etc.) use MediaObject and indicate the [[encodingFormat]]." ;
        rdfs:label    "caption" .

schema:possibleTreatment
        rdf:type      rdf:Property ;
        rdfs:comment  "A possible treatment to address this condition, sign or symptom." ;
        rdfs:label    "possibleTreatment" .

schema:contactType  rdf:type  rdf:Property ;
        rdfs:comment  "A person or organization can have different contact points, for different purposes. For example, a sales contact point, a PR contact point and so on. This property is used to specify the kind of contact point." ;
        rdfs:label    "contactType" .

schema:sourceOrganization
        rdf:type      rdf:Property ;
        rdfs:comment  "The Organization on whose behalf the creator was working." ;
        rdfs:label    "sourceOrganization" .

schema:musicReleaseFormat
        rdf:type      rdf:Property ;
        rdfs:comment  "Format of this release (the type of recording media used, ie. compact disc, digital media, LP, etc.)." ;
        rdfs:label    "musicReleaseFormat" .

schema:cvdCollectionDate
        rdf:type      rdf:Property ;
        rdfs:comment  "collectiondate - Date for which patient counts are reported." ;
        rdfs:label    "cvdCollectionDate" .

schema:sibling  rdf:type  rdf:Property ;
        rdfs:comment  "A sibling of the person." ;
        rdfs:label    "sibling" .

schema:PresentationDigitalDocument
        rdf:type         rdfs:Class ;
        rdfs:comment     "A file containing slides or used for a presentation." ;
        rdfs:label       "PresentationDigitalDocument" ;
        rdfs:subClassOf  schema:DigitalDocument .

schema:nutrition  rdf:type  rdf:Property ;
        rdfs:comment  "Nutrition information about the recipe or menu item." ;
        rdfs:label    "nutrition" .

schema:Suite  rdf:type   rdfs:Class ;
        rdfs:comment     "A suite in a hotel or other public accommodation, denotes a class of luxury accommodations, the key feature of which is multiple rooms (Source: Wikipedia, the free encyclopedia, see <a href=\"http://en.wikipedia.org/wiki/Suite_(hotel)\">http://en.wikipedia.org/wiki/Suite_(hotel)</a>).\n<br /><br />\nSee also the <a href=\"/docs/hotels.html\">dedicated document on the use of schema.org for marking up hotels and other forms of accommodations</a>.\n" ;
        rdfs:label       "Suite" ;
        rdfs:subClassOf  schema:Accommodation .

schema:ControlAction  rdf:type  rdfs:Class ;
        rdfs:comment     "An agent controls a device or application." ;
        rdfs:label       "ControlAction" ;
        rdfs:subClassOf  schema:Action .

schema:InteractionCounter
        rdf:type         rdfs:Class ;
        rdfs:comment     "A summary of how users have interacted with this CreativeWork. In most cases, authors will use a subtype to specify the specific type of interaction." ;
        rdfs:label       "InteractionCounter" ;
        rdfs:subClassOf  schema:StructuredValue .

schema:CheckOutAction
        rdf:type         rdfs:Class ;
        rdfs:comment     "The act of an agent communicating (service provider, social media, etc) their departure of a previously reserved service (e.g. flight check in) or place (e.g. hotel).\\n\\nRelated actions:\\n\\n* [[CheckInAction]]: The antonym of CheckOutAction.\\n* [[DepartAction]]: Unlike DepartAction, CheckOutAction implies that the agent is informing/confirming the end of a previously reserved service.\\n* [[CancelAction]]: Unlike CancelAction, CheckOutAction implies that the agent is informing/confirming the end of a previously reserved service." ;
        rdfs:label       "CheckOutAction" ;
        rdfs:subClassOf  schema:CommunicateAction .

schema:PayAction  rdf:type  rdfs:Class ;
        rdfs:comment     "An agent pays a price to a participant." ;
        rdfs:label       "PayAction" ;
        rdfs:subClassOf  schema:TradeAction .

schema:MedicalAudience
        rdf:type         rdfs:Class ;
        rdfs:comment     "Target audiences for medical web pages." ;
        rdfs:label       "MedicalAudience" ;
        rdfs:subClassOf  schema:PeopleAudience , schema:Audience .

schema:workTranslation
        rdf:type      rdf:Property ;
        rdfs:comment  "A work that is a translation of the content of this work. e.g. 西遊記 has an English workTranslation “Journey to the West”,a German workTranslation “Monkeys Pilgerfahrt” and a Vietnamese  translation Tây du ký bình khảo." ;
        rdfs:label    "workTranslation" .

schema:subtitleLanguage
        rdf:type      rdf:Property ;
        rdfs:comment  "Languages in which subtitles/captions are available, in [IETF BCP 47 standard format](http://tools.ietf.org/html/bcp47)." ;
        rdfs:label    "subtitleLanguage" .

schema:ProfessionalService
        rdf:type         rdfs:Class ;
        rdfs:comment     "Original definition: \"provider of professional services.\"\\n\\nThe general [[ProfessionalService]] type for local businesses was deprecated due to confusion with [[Service]]. For reference, the types that it included were: [[Dentist]],\n        [[AccountingService]], [[Attorney]], [[Notary]], as well as types for several kinds of [[HomeAndConstructionBusiness]]: [[Electrician]], [[GeneralContractor]],\n        [[HousePainter]], [[Locksmith]], [[Plumber]], [[RoofingContractor]]. [[LegalService]] was introduced as a more inclusive supertype of [[Attorney]]." ;
        rdfs:label       "ProfessionalService" ;
        rdfs:subClassOf  schema:LocalBusiness .

schema:artMedium  rdf:type  rdf:Property ;
        rdfs:comment        "The material used. (e.g. Oil, Watercolour, Acrylic, Linoprint, Marble, Cyanotype, Digital, Lithograph, DryPoint, Intaglio, Pastel, Woodcut, Pencil, Mixed Media, etc.)" ;
        rdfs:label          "artMedium" ;
        rdfs:subPropertyOf  schema:material .

schema:purchaseDate  rdf:type  rdf:Property ;
        rdfs:comment  "The date the item e.g. vehicle was purchased by the current owner." ;
        rdfs:label    "purchaseDate" .

schema:seller  rdf:type     rdf:Property ;
        rdfs:comment        "An entity which offers (sells / leases / lends / loans) the services / goods.  A seller may also be a provider." ;
        rdfs:label          "seller" ;
        rdfs:subPropertyOf  schema:participant .

schema:arrivalBusStop
        rdf:type      rdf:Property ;
        rdfs:comment  "The stop or station from which the bus arrives." ;
        rdfs:label    "arrivalBusStop" .

schema:about  rdf:type  rdf:Property ;
        rdfs:comment  "The subject matter of the content." ;
        rdfs:label    "about" .

schema:eduQuestionType
        rdf:type      rdf:Property ;
        rdfs:comment  "For questions that are part of learning resources (e.g. Quiz), eduQuestionType indicates the format of question being given. Example: \"Multiple choice\", \"Open ended\", \"Flashcard\"." ;
        rdfs:label    "eduQuestionType" .

schema:inSupportOf  rdf:type  rdf:Property ;
        rdfs:comment  "Qualification, candidature, degree, application that Thesis supports." ;
        rdfs:label    "inSupportOf" .

schema:typicalAgeRange
        rdf:type      rdf:Property ;
        rdfs:comment  "The typical expected age range, e.g. '7-9', '11-'." ;
        rdfs:label    "typicalAgeRange" .

schema:shippingRate  rdf:type  rdf:Property ;
        rdfs:comment  "The shipping rate is the cost of shipping to the specified destination. Typically, the maxValue and currency values (of the [[MonetaryAmount]]) are most appropriate." ;
        rdfs:label    "shippingRate" .

schema:SoftwareSourceCode
        rdf:type         rdfs:Class ;
        rdfs:comment     "Computer programming source code. Example: Full (compile ready) solutions, code snippet samples, scripts, templates." ;
        rdfs:label       "SoftwareSourceCode" ;
        rdfs:subClassOf  schema:CreativeWork .

schema:WinAction  rdf:type  rdfs:Class ;
        rdfs:comment     "The act of achieving victory in a competitive activity." ;
        rdfs:label       "WinAction" ;
        rdfs:subClassOf  schema:AchieveAction .

schema:sharedContent  rdf:type  rdf:Property ;
        rdfs:comment  "A CreativeWork such as an image, video, or audio clip shared as part of this posting." ;
        rdfs:label    "sharedContent" .

schema:providesBroadcastService
        rdf:type      rdf:Property ;
        rdfs:comment  "The BroadcastService offered on this channel." ;
        rdfs:label    "providesBroadcastService" .

schema:LoseAction  rdf:type  rdfs:Class ;
        rdfs:comment     "The act of being defeated in a competitive activity." ;
        rdfs:label       "LoseAction" ;
        rdfs:subClassOf  schema:AchieveAction .

schema:IgnoreAction  rdf:type  rdfs:Class ;
        rdfs:comment     "The act of intentionally disregarding the object. An agent ignores an object." ;
        rdfs:label       "IgnoreAction" ;
        rdfs:subClassOf  schema:AssessAction .

schema:fromLocation  rdf:type  rdf:Property ;
        rdfs:comment        "A sub property of location. The original location of the object or the agent before the action." ;
        rdfs:label          "fromLocation" ;
        rdfs:subPropertyOf  schema:location .

schema:postalCodeBegin
        rdf:type      rdf:Property ;
        rdfs:comment  "First postal code in a range (included)." ;
        rdfs:label    "postalCodeBegin" .

schema:BroadcastEvent
        rdf:type         rdfs:Class ;
        rdfs:comment     "An over the air or online broadcast event." ;
        rdfs:label       "BroadcastEvent" ;
        rdfs:subClassOf  schema:PublicationEvent .

schema:inProductGroupWithID
        rdf:type      rdf:Property ;
        rdfs:comment  "Indicates the [[productGroupID]] for a [[ProductGroup]] that this product [[isVariantOf]]. " ;
        rdfs:label    "inProductGroupWithID" .

schema:Residence  rdf:type  rdfs:Class ;
        rdfs:comment     "The place where a person lives." ;
        rdfs:label       "Residence" ;
        rdfs:subClassOf  schema:Place .

schema:TelevisionStation
        rdf:type         rdfs:Class ;
        rdfs:comment     "A television station." ;
        rdfs:label       "TelevisionStation" ;
        rdfs:subClassOf  schema:LocalBusiness .

schema:ShippingDeliveryTime
        rdf:type         rdfs:Class ;
        rdfs:comment     "ShippingDeliveryTime provides various pieces of information about delivery times for shipping." ;
        rdfs:label       "ShippingDeliveryTime" ;
        rdfs:subClassOf  schema:StructuredValue .

schema:gtin  rdf:type       rdf:Property ;
        rdfs:comment        "A Global Trade Item Number ([GTIN](https://www.gs1.org/standards/id-keys/gtin)). GTINs identify trade items, including products and services, using numeric identification codes. The [[gtin]] property generalizes the earlier [[gtin8]], [[gtin12]], [[gtin13]], and [[gtin14]] properties. The GS1 [digital link specifications](https://www.gs1.org/standards/Digital-Link/) express GTINs as URLs. A correct [[gtin]] value should be a valid GTIN, which means that it should be an all-numeric string of either 8, 12, 13 or 14 digits, or a \"GS1 Digital Link\" URL based on such a string. The numeric component should also have a [valid GS1 check digit](https://www.gs1.org/services/check-digit-calculator) and meet the other rules for valid GTINs. See also [GS1's GTIN Summary](http://www.gs1.org/barcodes/technical/idkeys/gtin) and [Wikipedia](https://en.wikipedia.org/wiki/Global_Trade_Item_Number) for more details. Left-padding of the gtin values is not required or encouraged.\n   " ;
        rdfs:label          "gtin" ;
        rdfs:subPropertyOf  schema:identifier .

schema:QuoteAction  rdf:type  rdfs:Class ;
        rdfs:comment     "An agent quotes/estimates/appraises an object/product/service with a price at a location/store." ;
        rdfs:label       "QuoteAction" ;
        rdfs:subClassOf  schema:TradeAction .

schema:recordedIn  rdf:type  rdf:Property ;
        rdfs:comment  "The CreativeWork that captured all or part of this Event." ;
        rdfs:label    "recordedIn" .

schema:givenName  rdf:type  rdf:Property ;
        rdfs:comment  "Given name. In the U.S., the first name of a Person." ;
        rdfs:label    "givenName" .

schema:affectedBy  rdf:type  rdf:Property ;
        rdfs:comment  "Drugs that affect the test's results." ;
        rdfs:label    "affectedBy" .

schema:stage  rdf:type  rdf:Property ;
        rdfs:comment  "The stage of the condition, if applicable." ;
        rdfs:label    "stage" .

schema:recordedAs  rdf:type  rdf:Property ;
        rdfs:comment  "An audio recording of the work." ;
        rdfs:label    "recordedAs" .

schema:arterialBranch
        rdf:type      rdf:Property ;
        rdfs:comment  "The branches that comprise the arterial structure." ;
        rdfs:label    "arterialBranch" .

schema:meetsEmissionStandard
        rdf:type      rdf:Property ;
        rdfs:comment  "Indicates that the vehicle meets the respective emission standard." ;
        rdfs:label    "meetsEmissionStandard" .

schema:ComicCoverArt  rdf:type  rdfs:Class ;
        rdfs:comment     "The artwork on the cover of a comic." ;
        rdfs:label       "ComicCoverArt" ;
        rdfs:subClassOf  schema:CoverArt , schema:ComicStory .

schema:seriousAdverseOutcome
        rdf:type      rdf:Property ;
        rdfs:comment  "A possible serious complication and/or serious side effect of this therapy. Serious adverse outcomes include those that are life-threatening; result in death, disability, or permanent damage; require hospitalization or prolong existing hospitalization; cause congenital anomalies or birth defects; or jeopardize the patient and may require medical or surgical intervention to prevent one of the outcomes in this definition." ;
        rdfs:label    "seriousAdverseOutcome" .

schema:studySubject  rdf:type  rdf:Property ;
        rdfs:comment  "A subject of the study, i.e. one of the medical conditions, therapies, devices, drugs, etc. investigated by the study." ;
        rdfs:label    "studySubject" .

schema:secondaryPrevention
        rdf:type      rdf:Property ;
        rdfs:comment  "A preventative therapy used to prevent reoccurrence of the medical condition after an initial episode of the condition." ;
        rdfs:label    "secondaryPrevention" .

schema:issuedThrough  rdf:type  rdf:Property ;
        rdfs:comment  "The service through with the permit was granted." ;
        rdfs:label    "issuedThrough" .

schema:NLNonprofitType
        rdf:type         rdfs:Class ;
        rdfs:comment     "NLNonprofitType: Non-profit organization type originating from the Netherlands." ;
        rdfs:label       "NLNonprofitType" ;
        rdfs:subClassOf  schema:NonprofitType .

schema:risks  rdf:type  rdf:Property ;
        rdfs:comment  "Specific physiologic risks associated to the diet plan." ;
        rdfs:label    "risks" .

schema:ScreeningEvent
        rdf:type         rdfs:Class ;
        rdfs:comment     "A screening of a movie or other video." ;
        rdfs:label       "ScreeningEvent" ;
        rdfs:subClassOf  schema:Event .

schema:exerciseType  rdf:type  rdf:Property ;
        rdfs:comment  "Type(s) of exercise or activity, such as strength training, flexibility training, aerobics, cardiac rehabilitation, etc." ;
        rdfs:label    "exerciseType" .

schema:aggregateRating
        rdf:type      rdf:Property ;
        rdfs:comment  "The overall rating, based on a collection of reviews or ratings, of the item." ;
        rdfs:label    "aggregateRating" .

schema:orderDelivery  rdf:type  rdf:Property ;
        rdfs:comment  "The delivery of the parcel related to this order or order item." ;
        rdfs:label    "orderDelivery" .

schema:totalTime  rdf:type  rdf:Property ;
        rdfs:comment  "The total time required to perform instructions or a direction (including time to prepare the supplies), in [ISO 8601 duration format](http://en.wikipedia.org/wiki/ISO_8601)." ;
        rdfs:label    "totalTime" .

schema:MeetingRoom  rdf:type  rdfs:Class ;
        rdfs:comment     "A meeting room, conference room, or conference hall is a room provided for singular events such as business conferences and meetings (Source: Wikipedia, the free encyclopedia, see <a href=\"http://en.wikipedia.org/wiki/Conference_hall\">http://en.wikipedia.org/wiki/Conference_hall</a>).\n<br /><br />\nSee also the <a href=\"/docs/hotels.html\">dedicated document on the use of schema.org for marking up hotels and other forms of accommodations</a>.\n" ;
        rdfs:label       "MeetingRoom" ;
        rdfs:subClassOf  schema:Room .

schema:AnimalShelter  rdf:type  rdfs:Class ;
        rdfs:comment     "Animal shelter." ;
        rdfs:label       "AnimalShelter" ;
        rdfs:subClassOf  schema:LocalBusiness .

schema:directors  rdf:type  rdf:Property ;
        rdfs:comment  "A director of e.g. tv, radio, movie, video games etc. content. Directors can be associated with individual items or with a series, episode, clip." ;
        rdfs:label    "directors" .

schema:EventAttendanceModeEnumeration
        rdf:type         rdfs:Class ;
        rdfs:comment     "An EventAttendanceModeEnumeration value is one of potentially several modes of organising an event, relating to whether it is online or offline." ;
        rdfs:label       "EventAttendanceModeEnumeration" ;
        rdfs:subClassOf  schema:Enumeration .

schema:includedInDataCatalog
        rdf:type      rdf:Property ;
        rdfs:comment  "A data catalog which contains this dataset." ;
        rdfs:label    "includedInDataCatalog" .

schema:valueReference
        rdf:type      rdf:Property ;
        rdfs:comment  "A secondary value that provides additional information on the original value, e.g. a reference temperature or a type of measurement." ;
        rdfs:label    "valueReference" .

schema:DeliveryTimeSettings
        rdf:type         rdfs:Class ;
        rdfs:comment     "A DeliveryTimeSettings represents re-usable pieces of shipping information, relating to timing. It is designed for publication on an URL that may be referenced via the [[shippingSettingsLink]] property of a [[OfferShippingDetails]]. Several occurrences can be published, distinguished (and identified/referenced) by their different values for [[transitTimeLabel]]." ;
        rdfs:label       "DeliveryTimeSettings" ;
        rdfs:subClassOf  schema:StructuredValue .

schema:causeOf  rdf:type  rdf:Property ;
        rdfs:comment  "The condition, complication, symptom, sign, etc. caused." ;
        rdfs:label    "causeOf" .

schema:eligibleTransactionVolume
        rdf:type      rdf:Property ;
        rdfs:comment  "The transaction volume, in a monetary unit, for which the offer or price specification is valid, e.g. for indicating a minimal purchasing volume, to express free shipping above a certain order volume, or to limit the acceptance of credit cards to purchases to a certain minimal amount." ;
        rdfs:label    "eligibleTransactionVolume" .

schema:Book  rdf:type    rdfs:Class ;
        rdfs:comment     "A book." ;
        rdfs:label       "Book" ;
        rdfs:subClassOf  schema:CreativeWork .

schema:characterName  rdf:type  rdf:Property ;
        rdfs:comment  "The name of a character played in some acting or performing role, i.e. in a PerformanceRole." ;
        rdfs:label    "characterName" .

schema:illustrator  rdf:type  rdf:Property ;
        rdfs:comment  "The illustrator of the book." ;
        rdfs:label    "illustrator" .

schema:SeaBodyOfWater
        rdf:type         rdfs:Class ;
        rdfs:comment     "A sea (for example, the Caspian sea)." ;
        rdfs:label       "SeaBodyOfWater" ;
        rdfs:subClassOf  schema:BodyOfWater .

schema:hasDigitalDocumentPermission
        rdf:type      rdf:Property ;
        rdfs:comment  "A permission related to the access to this document (e.g. permission to read or write an electronic document). For a public document, specify a grantee with an Audience with audienceType equal to \"public\"." ;
        rdfs:label    "hasDigitalDocumentPermission" .

schema:geoMidpoint  rdf:type  rdf:Property ;
        rdfs:comment  "Indicates the GeoCoordinates at the centre of a GeoShape e.g. GeoCircle." ;
        rdfs:label    "geoMidpoint" .

schema:performer  rdf:type  rdf:Property ;
        rdfs:comment  "A performer at the event&#x2014;for example, a presenter, musician, musical group or actor." ;
        rdfs:label    "performer" .

schema:suggestedAnswer
        rdf:type      rdf:Property ;
        rdfs:comment  "An answer (possibly one of several, possibly incorrect) to a Question, e.g. on a Question/Answer site." ;
        rdfs:label    "suggestedAnswer" .

schema:isSimilarTo  rdf:type  rdf:Property ;
        rdfs:comment  "A pointer to another, functionally similar product (or multiple products)." ;
        rdfs:label    "isSimilarTo" .

schema:numberOfDoors  rdf:type  rdf:Property ;
        rdfs:comment  "The number of doors.\\n\\nTypical unit code(s): C62" ;
        rdfs:label    "numberOfDoors" .

schema:procedureType  rdf:type  rdf:Property ;
        rdfs:comment  "The type of procedure, for example Surgical, Noninvasive, or Percutaneous." ;
        rdfs:label    "procedureType" .

schema:Game  rdf:type    rdfs:Class ;
        rdfs:comment     "The Game type represents things which are games. These are typically rule-governed recreational activities, e.g. role-playing games in which players assume the role of characters in a fictional setting." ;
        rdfs:label       "Game" ;
        rdfs:subClassOf  schema:CreativeWork .

schema:Dataset  rdf:type  rdfs:Class ;
        rdfs:comment     "A body of structured information describing some topic(s) of interest." ;
        rdfs:label       "Dataset" ;
        rdfs:subClassOf  schema:CreativeWork .

schema:hasMenuSection
        rdf:type      rdf:Property ;
        rdfs:comment  "A subgrouping of the menu (by dishes, course, serving time period, etc.)." ;
        rdfs:label    "hasMenuSection" .

dcmitype:Dataset  rdf:type  rdfs:Class .

schema:transitTime  rdf:type  rdf:Property ;
        rdfs:comment  "The typical delay the order has been sent for delivery and the goods reach the final customer. Typical properties: minValue, maxValue, unitCode (d for DAY)." ;
        rdfs:label    "transitTime" .

schema:Vein  rdf:type    rdfs:Class ;
        rdfs:comment     "A type of blood vessel that specifically carries blood to the heart." ;
        rdfs:label       "Vein" ;
        rdfs:subClassOf  schema:Vessel .

schema:drainsTo  rdf:type  rdf:Property ;
        rdfs:comment  "The vasculature that the vein drains into." ;
        rdfs:label    "drainsTo" .

schema:busNumber  rdf:type  rdf:Property ;
        rdfs:comment  "The unique identifier for the bus." ;
        rdfs:label    "busNumber" .

schema:SuspendAction  rdf:type  rdfs:Class ;
        rdfs:comment     "The act of momentarily pausing a device or application (e.g. pause music playback or pause a timer)." ;
        rdfs:label       "SuspendAction" ;
        rdfs:subClassOf  schema:ControlAction .

schema:passengerPriorityStatus
        rdf:type      rdf:Property ;
        rdfs:comment  "The priority status assigned to a passenger for security or boarding (e.g. FastTrack or Priority)." ;
        rdfs:label    "passengerPriorityStatus" .

schema:TaxiReservation
        rdf:type         rdfs:Class ;
        rdfs:comment     "A reservation for a taxi.\\n\\nNote: This type is for information about actual reservations, e.g. in confirmation emails or HTML pages with individual confirmations of reservations. For offers of tickets, use [[Offer]]." ;
        rdfs:label       "TaxiReservation" ;
        rdfs:subClassOf  schema:Reservation .

schema:interactionType
        rdf:type      rdf:Property ;
        rdfs:comment  "The Action representing the type of interaction. For up votes, +1s, etc. use [[LikeAction]]. For down votes use [[DislikeAction]]. Otherwise, use the most specific Action." ;
        rdfs:label    "interactionType" .

schema:Obstetric  rdf:type  rdfs:Class ;
        rdfs:comment     "A specific branch of medical science that specializes in the care of women during the prenatal and postnatal care and with the delivery of the child." ;
        rdfs:label       "Obstetric" ;
        rdfs:subClassOf  schema:MedicalBusiness .

schema:MedicineSystem
        rdf:type         rdfs:Class ;
        rdfs:comment     "Systems of medical practice." ;
        rdfs:label       "MedicineSystem" ;
        rdfs:subClassOf  schema:MedicalEnumeration .

schema:additionalProperty
        rdf:type      rdf:Property ;
        rdfs:comment  "A property-value pair representing an additional characteristics of the entitity, e.g. a product feature or another characteristic for which there is no matching property in schema.org.\\n\\nNote: Publishers should be aware that applications designed to use specific schema.org properties (e.g. http://schema.org/width, http://schema.org/color, http://schema.org/gtin13, ...) will typically expect such data to be provided using those properties, rather than using the generic property/value mechanism.\n" ;
        rdfs:label    "additionalProperty" .

schema:distance  rdf:type  rdf:Property ;
        rdfs:comment  "The distance travelled, e.g. exercising or travelling." ;
        rdfs:label    "distance" .

schema:AMRadioChannel
        rdf:type         rdfs:Class ;
        rdfs:comment     "A radio channel that uses AM." ;
        rdfs:label       "AMRadioChannel" ;
        rdfs:subClassOf  schema:RadioChannel .

schema:dateCreated  rdf:type  rdf:Property ;
        rdfs:comment  "The date on which the CreativeWork was created or the item was added to a DataFeed." ;
        rdfs:label    "dateCreated" .

schema:BusinessEntityType
        rdf:type         rdfs:Class ;
        rdfs:comment     "A business entity type is a conceptual entity representing the legal form, the size, the main line of business, the position in the value chain, or any combination thereof, of an organization or business person.\\n\\nCommonly used values:\\n\\n* http://purl.org/goodrelations/v1#Business\\n* http://purl.org/goodrelations/v1#Enduser\\n* http://purl.org/goodrelations/v1#PublicInstitution\\n* http://purl.org/goodrelations/v1#Reseller\n\t  " ;
        rdfs:label       "BusinessEntityType" ;
        rdfs:subClassOf  schema:Enumeration .

schema:ElectronicsStore
        rdf:type         rdfs:Class ;
        rdfs:comment     "An electronics store." ;
        rdfs:label       "ElectronicsStore" ;
        rdfs:subClassOf  schema:Store .

schema:CommunityHealth
        rdf:type         rdfs:Class ;
        rdfs:comment     "A field of public health focusing on improving health characteristics of a defined population in relation with their geographical or environment areas." ;
        rdfs:label       "CommunityHealth" ;
        rdfs:subClassOf  schema:MedicalBusiness .

schema:duns  rdf:type       rdf:Property ;
        rdfs:comment        "The Dun & Bradstreet DUNS number for identifying an organization or business person." ;
        rdfs:label          "duns" ;
        rdfs:subPropertyOf  schema:identifier .

schema:byArtist  rdf:type  rdf:Property ;
        rdfs:comment  "The artist that performed this album or recording." ;
        rdfs:label    "byArtist" .

schema:geoDisjoint  rdf:type  rdf:Property ;
        rdfs:comment  "Represents spatial relations in which two geometries (or the places they represent) are topologically disjoint: they have no point in common. They form a set of disconnected geometries.\" (a symmetric relationship, as defined in [DE-9IM](https://en.wikipedia.org/wiki/DE-9IM))" ;
        rdfs:label    "geoDisjoint" .

schema:businessDays  rdf:type  rdf:Property ;
        rdfs:comment  "Days of the week when the merchant typically operates, indicated via opening hours markup." ;
        rdfs:label    "businessDays" .

schema:recipeCuisine  rdf:type  rdf:Property ;
        rdfs:comment  "The cuisine of the recipe (for example, French or Ethiopian)." ;
        rdfs:label    "recipeCuisine" .

schema:countriesSupported
        rdf:type      rdf:Property ;
        rdfs:comment  "Countries for which the application is supported. You can also provide the two-letter ISO 3166-1 alpha-2 country code." ;
        rdfs:label    "countriesSupported" .

schema:includedDataCatalog
        rdf:type      rdf:Property ;
        rdfs:comment  "A data catalog which contains this dataset (this property was previously 'catalog', preferred name is now 'includedInDataCatalog')." ;
        rdfs:label    "includedDataCatalog" .

schema:ethicsPolicy  rdf:type  rdf:Property ;
        rdfs:comment  "Statement about ethics policy, e.g. of a [[NewsMediaOrganization]] regarding journalistic and publishing practices, or of a [[Restaurant]], a page describing food source policies. In the case of a [[NewsMediaOrganization]], an ethicsPolicy is typically a statement describing the personal, organizational, and corporate standards of behavior expected by the organization." ;
        rdfs:label    "ethicsPolicy" .

schema:Airport  rdf:type  rdfs:Class ;
        rdfs:comment     "An airport." ;
        rdfs:label       "Airport" ;
        rdfs:subClassOf  schema:CivicStructure .

schema:Aquarium  rdf:type  rdfs:Class ;
        rdfs:comment     "Aquarium." ;
        rdfs:label       "Aquarium" ;
        rdfs:subClassOf  schema:CivicStructure .

schema:departurePlatform
        rdf:type      rdf:Property ;
        rdfs:comment  "The platform from which the train departs." ;
        rdfs:label    "departurePlatform" .

schema:State  rdf:type   rdfs:Class ;
        rdfs:comment     "A state or province of a country." ;
        rdfs:label       "State" ;
        rdfs:subClassOf  schema:AdministrativeArea .

schema:Atlas  rdf:type   rdfs:Class ;
        rdfs:comment     "A collection or bound volume of maps, charts, plates or tables, physical or in media form illustrating any subject." ;
        rdfs:label       "Atlas" ;
        rdfs:subClassOf  schema:CreativeWork .

schema:DeliveryMethod
        rdf:type         rdfs:Class ;
        rdfs:comment     "A delivery method is a standardized procedure for transferring the product or service to the destination of fulfillment chosen by the customer. Delivery methods are characterized by the means of transportation used, and by the organization or group that is the contracting party for the sending organization or person.\\n\\nCommonly used values:\\n\\n* http://purl.org/goodrelations/v1#DeliveryModeDirectDownload\\n* http://purl.org/goodrelations/v1#DeliveryModeFreight\\n* http://purl.org/goodrelations/v1#DeliveryModeMail\\n* http://purl.org/goodrelations/v1#DeliveryModeOwnFleet\\n* http://purl.org/goodrelations/v1#DeliveryModePickUp\\n* http://purl.org/goodrelations/v1#DHL\\n* http://purl.org/goodrelations/v1#FederalExpress\\n* http://purl.org/goodrelations/v1#UPS\n        " ;
        rdfs:label       "DeliveryMethod" ;
        rdfs:subClassOf  schema:Enumeration .

schema:ContactPointOption
        rdf:type         rdfs:Class ;
        rdfs:comment     "Enumerated options related to a ContactPoint." ;
        rdfs:label       "ContactPointOption" ;
        rdfs:subClassOf  schema:Enumeration .

schema:multipleValues
        rdf:type      rdf:Property ;
        rdfs:comment  "Whether multiple values are allowed for the property.  Default is false." ;
        rdfs:label    "multipleValues" .

schema:featureList  rdf:type  rdf:Property ;
        rdfs:comment  "Features or modules provided by this application (and possibly required by other applications)." ;
        rdfs:label    "featureList" .

schema:InsuranceAgency
        rdf:type         rdfs:Class ;
        rdfs:comment     "An Insurance agency." ;
        rdfs:label       "InsuranceAgency" ;
        rdfs:subClassOf  schema:FinancialService .

schema:SportsEvent  rdf:type  rdfs:Class ;
        rdfs:comment     "Event type: Sports event." ;
        rdfs:label       "SportsEvent" ;
        rdfs:subClassOf  schema:Event .

schema:branchOf  rdf:type  rdf:Property ;
        rdfs:comment  "The larger organization that this local business is a branch of, if any. Not to be confused with (anatomical)[[branch]]." ;
        rdfs:label    "branchOf" .

schema:EmployerAggregateRating
        rdf:type         rdfs:Class ;
        rdfs:comment     "An aggregate rating of an Organization related to its role as an employer." ;
        rdfs:label       "EmployerAggregateRating" ;
        rdfs:subClassOf  schema:AggregateRating .

schema:coverageEndTime
        rdf:type      rdf:Property ;
        rdfs:comment  "The time when the live blog will stop covering the Event. Note that coverage may continue after the Event concludes." ;
        rdfs:label    "coverageEndTime" .

schema:musicGroupMember
        rdf:type      rdf:Property ;
        rdfs:comment  "A member of a music group&#x2014;for example, John, Paul, George, or Ringo." ;
        rdfs:label    "musicGroupMember" .

schema:collectionSize
        rdf:type      rdf:Property ;
        rdfs:comment  "The number of items in the [[Collection]]."@en ;
        rdfs:label    "collectionSize"@en .

schema:legislationDate
        rdf:type            rdf:Property ;
        rdfs:comment        "The date of adoption or signature of the legislation. This is the date at which the text is officially aknowledged to be a legislation, even though it might not even be published or in force." ;
        rdfs:label          "legislationDate" ;
        rdfs:subPropertyOf  schema:dateCreated .

schema:GolfCourse  rdf:type  rdfs:Class ;
        rdfs:comment     "A golf course." ;
        rdfs:label       "GolfCourse" ;
        rdfs:subClassOf  schema:SportsActivityLocation .

schema:serviceOutput  rdf:type  rdf:Property ;
        rdfs:comment  "The tangible thing generated by the service, e.g. a passport, permit, etc." ;
        rdfs:label    "serviceOutput" .

schema:OfferShippingDetails
        rdf:type         rdfs:Class ;
        rdfs:comment     "OfferShippingDetails represents information about shipping destinations.\n\nMultiple of these entities can be used to represent different shipping rates for different destinations:\n\nOne entity for Alaska/Hawaii. A different one for continental US.A different one for all France.\n\nMultiple of these entities can be used to represent different shipping costs and delivery times.\n\nTwo entities that are identical but differ in rate and time:\n\ne.g. Cheaper and slower: $5 in 5-7days\nor Fast and expensive: $15 in 1-2 days." ;
        rdfs:label       "OfferShippingDetails" ;
        rdfs:subClassOf  schema:StructuredValue .

schema:LegalValueLevel
        rdf:type         rdfs:Class ;
        rdfs:comment     "A list of possible levels for the legal validity of a legislation." ;
        rdfs:label       "LegalValueLevel" ;
        rdfs:subClassOf  schema:Enumeration .

schema:EducationalOrganization
        rdf:type         rdfs:Class ;
        rdfs:comment     "An educational organization." ;
        rdfs:label       "EducationalOrganization" ;
        rdfs:subClassOf  schema:CivicStructure , schema:Organization .

schema:InfectiousDisease
        rdf:type         rdfs:Class ;
        rdfs:comment     "An infectious disease is a clinically evident human disease resulting from the presence of pathogenic microbial agents, like pathogenic viruses, pathogenic bacteria, fungi, protozoa, multicellular parasites, and prions. To be considered an infectious disease, such pathogens are known to be able to cause this disease." ;
        rdfs:label       "InfectiousDisease" ;
        rdfs:subClassOf  schema:MedicalCondition .

schema:EducationalOccupationalCredential
        rdf:type         rdfs:Class ;
        rdfs:comment     "An educational or occupational credential. A diploma, academic degree, certification, qualification, badge, etc., that may be awarded to a person or other entity that meets the requirements defined by the credentialer." ;
        rdfs:label       "EducationalOccupationalCredential" ;
        rdfs:subClassOf  schema:CreativeWork .

schema:ratingValue  rdf:type  rdf:Property ;
        rdfs:comment  "The rating for the content.\\n\\nUsage guidelines:\\n\\n* Use values from 0123456789 (Unicode 'DIGIT ZERO' (U+0030) to 'DIGIT NINE' (U+0039)) rather than superficially similiar Unicode symbols.\\n* Use '.' (Unicode 'FULL STOP' (U+002E)) rather than ',' to indicate a decimal point. Avoid using these symbols as a readability separator." ;
        rdfs:label    "ratingValue" .

schema:CorrectionComment
        rdf:type         rdfs:Class ;
        rdfs:comment     "A [[comment]] that corrects [[CreativeWork]]." ;
        rdfs:label       "CorrectionComment" ;
        rdfs:subClassOf  schema:Comment .

schema:lesser  rdf:type  rdf:Property ;
        rdfs:comment  "This ordering relation for qualitative values indicates that the subject is lesser than the object." ;
        rdfs:label    "lesser" .

schema:itemListElement
        rdf:type      rdf:Property ;
        rdfs:comment  "For itemListElement values, you can use simple strings (e.g. \"Peter\", \"Paul\", \"Mary\"), existing entities, or use ListItem.\\n\\nText values are best if the elements in the list are plain strings. Existing entities are best for a simple, unordered list of existing things in your data. ListItem is used with ordered lists when you want to provide additional context about the element in that list or when the same item might be in different places in different lists.\\n\\nNote: The order of elements in your mark-up is not sufficient for indicating the order or elements.  Use ListItem with a 'position' property in such cases." ;
        rdfs:label    "itemListElement" .

schema:GameServer  rdf:type  rdfs:Class ;
        rdfs:comment     "Server that provides game interaction in a multiplayer game." ;
        rdfs:label       "GameServer" ;
        rdfs:subClassOf  schema:Intangible .

schema:Brewery  rdf:type  rdfs:Class ;
        rdfs:comment     "Brewery." ;
        rdfs:label       "Brewery" ;
        rdfs:subClassOf  schema:FoodEstablishment .

schema:handlingTime  rdf:type  rdf:Property ;
        rdfs:comment  "The typical delay between the receipt of the order and the goods either leaving the warehouse or being prepared for pickup, in case the delivery method is on site pickup. Typical properties: minValue, maxValue, unitCode (d for DAY).  This is by common convention assumed to mean business days (if a unitCode is used, coded as \"d\"), i.e. only counting days when the business normally operates." ;
        rdfs:label    "handlingTime" .

schema:includesAttraction
        rdf:type      rdf:Property ;
        rdfs:comment  "Attraction located at destination." ;
        rdfs:label    "includesAttraction" .

schema:FMRadioChannel
        rdf:type         rdfs:Class ;
        rdfs:comment     "A radio channel that uses FM." ;
        rdfs:label       "FMRadioChannel" ;
        rdfs:subClassOf  schema:RadioChannel .

schema:SportingGoodsStore
        rdf:type         rdfs:Class ;
        rdfs:comment     "A sporting goods store." ;
        rdfs:label       "SportingGoodsStore" ;
        rdfs:subClassOf  schema:Store .

skos:closeMatch  rdf:type   owl:ObjectProperty ;
        rdfs:label          "has close match"@en ;
        rdfs:subPropertyOf  skos:mappingRelation .

schema:beforeMedia  rdf:type  rdf:Property ;
        rdfs:comment  "A media object representing the circumstances before performing this direction." ;
        rdfs:label    "beforeMedia" .

schema:taxID  rdf:type      rdf:Property ;
        rdfs:comment        "The Tax / Fiscal ID of the organization or person, e.g. the TIN in the US or the CIF/NIF in Spain." ;
        rdfs:label          "taxID" ;
        rdfs:subPropertyOf  schema:identifier .

schema:healthPlanPharmacyCategory
        rdf:type      rdf:Property ;
        rdfs:comment  "The category or type of pharmacy associated with this cost sharing." ;
        rdfs:label    "healthPlanPharmacyCategory" .

schema:temporal  rdf:type  rdf:Property ;
        rdfs:comment  "The \"temporal\" property can be used in cases where more specific properties\n(e.g. [[temporalCoverage]], [[dateCreated]], [[dateModified]], [[datePublished]]) are not known to be appropriate." ;
        rdfs:label    "temporal" .

schema:departureGate  rdf:type  rdf:Property ;
        rdfs:comment  "Identifier of the flight's departure gate." ;
        rdfs:label    "departureGate" .

schema:MenuItem  rdf:type  rdfs:Class ;
        rdfs:comment     "A food or drink item listed in a menu or menu section." ;
        rdfs:label       "MenuItem" ;
        rdfs:subClassOf  schema:Intangible .

schema:geoOverlaps  rdf:type  rdf:Property ;
        rdfs:comment  "Represents a relationship between two geometries (or the places they represent), relating a geometry to another that geospatially overlaps it, i.e. they have some but not all points in common. As defined in [DE-9IM](https://en.wikipedia.org/wiki/DE-9IM)." ;
        rdfs:label    "geoOverlaps" .

schema:appearance  rdf:type  rdf:Property ;
        rdfs:comment        "Indicates an occurence of a [[Claim]] in some [[CreativeWork]]." ;
        rdfs:label          "appearance" ;
        rdfs:subPropertyOf  schema:workExample .

schema:coverageStartTime
        rdf:type      rdf:Property ;
        rdfs:comment  "The time when the live blog will begin covering the Event. Note that coverage may begin before the Event's start time. The LiveBlogPosting may also be created before coverage begins." ;
        rdfs:label    "coverageStartTime" .

schema:hasMeasurement
        rdf:type      rdf:Property ;
        rdfs:comment  "A product measurement, for example the inseam of pants, the wheel size of a bicycle, or the gauge of a screw. Usually an exact measurement, but can also be a range of measurements for adjustable products, for example belts and ski bindings." ;
        rdfs:label    "hasMeasurement" .

schema:relatedCondition
        rdf:type      rdf:Property ;
        rdfs:comment  "A medical condition associated with this anatomy." ;
        rdfs:label    "relatedCondition" .

schema:RVPark  rdf:type  rdfs:Class ;
        rdfs:comment     "A place offering space for \"Recreational Vehicles\", Caravans, mobile homes and the like." ;
        rdfs:label       "RVPark" ;
        rdfs:subClassOf  schema:CivicStructure .

schema:MusicPlaylist  rdf:type  rdfs:Class ;
        rdfs:comment     "A collection of music tracks in playlist form." ;
        rdfs:label       "MusicPlaylist" ;
        rdfs:subClassOf  schema:CreativeWork .

schema:BorrowAction  rdf:type  rdfs:Class ;
        rdfs:comment     "The act of obtaining an object under an agreement to return it at a later date. Reciprocal of LendAction.\\n\\nRelated actions:\\n\\n* [[LendAction]]: Reciprocal of BorrowAction." ;
        rdfs:label       "BorrowAction" ;
        rdfs:subClassOf  schema:TransferAction .

schema:ComputerLanguage
        rdf:type         rdfs:Class ;
        rdfs:comment     "This type covers computer programming languages such as Scheme and Lisp, as well as other language-like computer representations. Natural languages are best represented with the [[Language]] type." ;
        rdfs:label       "ComputerLanguage" ;
        rdfs:subClassOf  schema:Intangible .

schema:typicalCreditsPerTerm
        rdf:type      rdf:Property ;
        rdfs:comment  "The number of credits or units a full-time student would be expected to take in 1 term however 'term' is defined by the institution." ;
        rdfs:label    "typicalCreditsPerTerm" .

schema:SportsOrganization
        rdf:type         rdfs:Class ;
        rdfs:comment     "Represents the collection of all sports organizations, including sports teams, governing bodies, and sports associations." ;
        rdfs:label       "SportsOrganization" ;
        rdfs:subClassOf  schema:Organization .

schema:BrokerageAccount
        rdf:type         rdfs:Class ;
        rdfs:comment     "An account that allows an investor to deposit funds and place investment orders with a licensed broker or brokerage firm." ;
        rdfs:label       "BrokerageAccount" ;
        rdfs:subClassOf  schema:InvestmentOrDeposit .

schema:ReportedDoseSchedule
        rdf:type         rdfs:Class ;
        rdfs:comment     "A patient-reported or observed dosing schedule for a drug or supplement." ;
        rdfs:label       "ReportedDoseSchedule" ;
        rdfs:subClassOf  schema:DoseSchedule .

schema:realEstateAgent
        rdf:type            rdf:Property ;
        rdfs:comment        "A sub property of participant. The real estate agent involved in the action." ;
        rdfs:label          "realEstateAgent" ;
        rdfs:subPropertyOf  schema:participant .

schema:overdosage  rdf:type  rdf:Property ;
        rdfs:comment  "Any information related to overdose on a drug, including signs or symptoms, treatments, contact information for emergency response." ;
        rdfs:label    "overdosage" .

schema:TouristDestination
        rdf:type         rdfs:Class ;
        rdfs:comment     "A tourist destination. In principle any [[Place]] can be a [[TouristDestination]] from a [[City]], Region or [[Country]] to an [[AmusementPark]] or [[Hotel]]. This Type can be used on its own to describe a general [[TouristDestination]], or be used as an [[additionalType]] to add tourist relevant properties to any other [[Place]].  A [[TouristDestination]] is defined as a [[Place]] that contains, or is colocated with, one or more [[TouristAttraction]]s, often linked by a similar theme or interest to a particular [[touristType]]. The [UNWTO](http://www2.unwto.org/) defines Destination (main destination of a tourism trip) as the place visited that is central to the decision to take the trip.\n  (See examples below)." ;
        rdfs:label       "TouristDestination" ;
        rdfs:subClassOf  schema:Place .

schema:bankAccountType
        rdf:type      rdf:Property ;
        rdfs:comment  "The type of a bank account." ;
        rdfs:label    "bankAccountType" .

schema:cvdNumVent  rdf:type  rdf:Property ;
        rdfs:comment  "numvent - MECHANICAL VENTILATORS: Total number of ventilators available." ;
        rdfs:label    "cvdNumVent" .

schema:TypeAndQuantityNode
        rdf:type         rdfs:Class ;
        rdfs:comment     "A structured value indicating the quantity, unit of measurement, and business function of goods included in a bundle offer." ;
        rdfs:label       "TypeAndQuantityNode" ;
        rdfs:subClassOf  schema:StructuredValue .

schema:shippingDestination
        rdf:type      rdf:Property ;
        rdfs:comment  "indicates (possibly multiple) shipping destinations. These can be defined in several ways e.g. postalCode ranges." ;
        rdfs:label    "shippingDestination" .

schema:codeSampleType
        rdf:type      rdf:Property ;
        rdfs:comment  "What type of code sample: full (compile ready) solution, code snippet, inline code, scripts, template." ;
        rdfs:label    "codeSampleType" .

schema:usesHealthPlanIdStandard
        rdf:type      rdf:Property ;
        rdfs:comment  "The standard for interpreting thePlan ID. The preferred is \"HIOS\". See the Centers for Medicare & Medicaid Services for more details." ;
        rdfs:label    "usesHealthPlanIdStandard" .

schema:guideline  rdf:type  rdf:Property ;
        rdfs:comment  "A medical guideline related to this entity." ;
        rdfs:label    "guideline" .

schema:geoWithin  rdf:type  rdf:Property ;
        rdfs:comment  "Represents a relationship between two geometries (or the places they represent), relating a geometry to one that contains it, i.e. it is inside (i.e. within) its interior. As defined in [DE-9IM](https://en.wikipedia.org/wiki/DE-9IM)." ;
        rdfs:label    "geoWithin" .

schema:BloodTest  rdf:type  rdfs:Class ;
        rdfs:comment     "A medical test performed on a sample of a patient's blood." ;
        rdfs:label       "BloodTest" ;
        rdfs:subClassOf  schema:MedicalTest .

schema:Legislation  rdf:type  rdfs:Class ;
        rdfs:comment     "A legal document such as an act, decree, bill, etc. (enforceable or not) or a component of a legal act (like an article)." ;
        rdfs:label       "Legislation" ;
        rdfs:subClassOf  schema:CreativeWork .

schema:knowsAbout  rdf:type  rdf:Property ;
        rdfs:comment  "Of a [[Person]], and less typically of an [[Organization]], to indicate a topic that is known about - suggesting possible expertise but not implying it. We do not distinguish skill levels here, or relate this to educational content, events, objectives or [[JobPosting]] descriptions." ;
        rdfs:label    "knowsAbout" .

schema:JewelryStore  rdf:type  rdfs:Class ;
        rdfs:comment     "A jewelry store." ;
        rdfs:label       "JewelryStore" ;
        rdfs:subClassOf  schema:Store .

schema:hasPOS  rdf:type  rdf:Property ;
        rdfs:comment  "Points-of-Sales operated by the organization or person." ;
        rdfs:label    "hasPOS" .

schema:includesHealthPlanFormulary
        rdf:type      rdf:Property ;
        rdfs:comment  "Formularies covered by this plan." ;
        rdfs:label    "includesHealthPlanFormulary" .

schema:rangeIncludes  rdf:type  rdf:Property ;
        rdfs:comment  "Relates a property to a class that constitutes (one of) the expected type(s) for values of the property." ;
        rdfs:label    "rangeIncludes" .

schema:PalliativeProcedure
        rdf:type         rdfs:Class ;
        rdfs:comment     "A medical procedure intended primarily for palliative purposes, aimed at relieving the symptoms of an underlying health condition." ;
        rdfs:label       "PalliativeProcedure" ;
        rdfs:subClassOf  schema:MedicalTherapy , schema:MedicalProcedure .

schema:inAlbum  rdf:type  rdf:Property ;
        rdfs:comment  "The album to which this recording belongs." ;
        rdfs:label    "inAlbum" .

schema:cvdNumC19HospPats
        rdf:type      rdf:Property ;
        rdfs:comment  "numc19hosppats - HOSPITALIZED: Patients currently hospitalized in an inpatient care location who have suspected or confirmed COVID-19." ;
        rdfs:label    "cvdNumC19HospPats" .

schema:editor  rdf:type  rdf:Property ;
        rdfs:comment  "Specifies the Person who edited the CreativeWork." ;
        rdfs:label    "editor" .

schema:honorificPrefix
        rdf:type      rdf:Property ;
        rdfs:comment  "An honorific prefix preceding a Person's name such as Dr/Mrs/Mr." ;
        rdfs:label    "honorificPrefix" .

schema:mainEntity  rdf:type  rdf:Property ;
        rdfs:comment        "Indicates the primary entity described in some page or other CreativeWork." ;
        rdfs:label          "mainEntity" ;
        rdfs:subPropertyOf  schema:about .

schema:DiagnosticLab  rdf:type  rdfs:Class ;
        rdfs:comment     "A medical laboratory that offers on-site or off-site diagnostic services." ;
        rdfs:label       "DiagnosticLab" ;
        rdfs:subClassOf  schema:MedicalOrganization .

schema:DietNutrition  rdf:type  rdfs:Class ;
        rdfs:comment     "Dietetic and nutrition as a medical specialty." ;
        rdfs:label       "DietNutrition" ;
        rdfs:subClassOf  schema:MedicalBusiness .

schema:musicBy  rdf:type  rdf:Property ;
        rdfs:comment  "The composer of the soundtrack." ;
        rdfs:label    "musicBy" .

schema:question  rdf:type   rdf:Property ;
        rdfs:comment        "A sub property of object. A question." ;
        rdfs:label          "question" ;
        rdfs:subPropertyOf  schema:object .

schema:cvdNumC19MechVentPats
        rdf:type      rdf:Property ;
        rdfs:comment  "numc19mechventpats - HOSPITALIZED and VENTILATED: Patients hospitalized in an NHSN inpatient care location who have suspected or confirmed COVID-19 and are on a mechanical ventilator." ;
        rdfs:label    "cvdNumC19MechVentPats" .

schema:LegislativeBuilding
        rdf:type         rdfs:Class ;
        rdfs:comment     "A legislative building&#x2014;for example, the state capitol." ;
        rdfs:label       "LegislativeBuilding" ;
        rdfs:subClassOf  schema:GovernmentBuilding .

schema:articleSection
        rdf:type      rdf:Property ;
        rdfs:comment  "Articles may belong to one or more 'sections' in a magazine or newspaper, such as Sports, Lifestyle, etc." ;
        rdfs:label    "articleSection" .

schema:expertConsiderations
        rdf:type      rdf:Property ;
        rdfs:comment  "Medical expert advice related to the plan." ;
        rdfs:label    "expertConsiderations" .

schema:Role  rdf:type    rdfs:Class ;
        rdfs:comment     "Represents additional information about a relationship or property. For example a Role can be used to say that a 'member' role linking some SportsTeam to a player occurred during a particular time period. Or that a Person's 'actor' role in a Movie was for some particular characterName. Such properties can be attached to a Role entity, which is then associated with the main entities using ordinary properties like 'member' or 'actor'.\\n\\nSee also [blog post](http://blog.schema.org/2014/06/introducing-role.html)." ;
        rdfs:label       "Role" ;
        rdfs:subClassOf  schema:Intangible .

schema:eligibilityToWorkRequirement
        rdf:type      rdf:Property ;
        rdfs:comment  "The legal requirements such as citizenship, visa and other documentation required for an applicant to this job." ;
        rdfs:label    "eligibilityToWorkRequirement" .

schema:HealthAndBeautyBusiness
        rdf:type         rdfs:Class ;
        rdfs:comment     "Health and beauty." ;
        rdfs:label       "HealthAndBeautyBusiness" ;
        rdfs:subClassOf  schema:LocalBusiness .

schema:FundingScheme  rdf:type  rdfs:Class ;
        rdfs:comment     "A FundingScheme combines organizational, project and policy aspects of grant-based funding\n    that sets guidelines, principles and mechanisms to support other kinds of projects and activities.\n    Funding is typically organized via [[Grant]] funding. Examples of funding schemes: Swiss Priority Programmes (SPPs); EU Framework 7 (FP7); Horizon 2020; the NIH-R01 Grant Program; Wellcome institutional strategic support fund. For large scale public sector funding, the management and administration of grant awards is often handled by other, dedicated, organizations - [[FundingAgency]]s such as ERC, REA, ..." ;
        rdfs:label       "FundingScheme" ;
        rdfs:subClassOf  schema:Organization .

schema:HealthPlanFormulary
        rdf:type         rdfs:Class ;
        rdfs:comment     "For a given health insurance plan, the specification for costs and coverage of prescription drugs. " ;
        rdfs:label       "HealthPlanFormulary" ;
        rdfs:subClassOf  schema:Intangible .

schema:TherapeuticProcedure
        rdf:type         rdfs:Class ;
        rdfs:comment     "A medical procedure intended primarily for therapeutic purposes, aimed at improving a health condition." ;
        rdfs:label       "TherapeuticProcedure" ;
        rdfs:subClassOf  schema:MedicalProcedure .

schema:healthPlanNetworkTier
        rdf:type      rdf:Property ;
        rdfs:comment  "The tier(s) for this network." ;
        rdfs:label    "healthPlanNetworkTier" .

schema:WearableMeasurementTypeEnumeration
        rdf:type         rdfs:Class ;
        rdfs:comment     "Enumerates common types of measurement for wearables products." ;
        rdfs:label       "WearableMeasurementTypeEnumeration" ;
        rdfs:subClassOf  schema:MeasurementTypeEnumeration .

schema:UserBlocks  rdf:type  rdfs:Class ;
        rdfs:comment     "UserInteraction and its subtypes is an old way of talking about users interacting with pages. It is generally better to use [[Action]]-based vocabulary, alongside types such as [[Comment]]." ;
        rdfs:label       "UserBlocks" ;
        rdfs:subClassOf  schema:UserInteraction .

schema:merchantReturnDays
        rdf:type      rdf:Property ;
        rdfs:comment  "The merchantReturnDays property indicates the number of days (from purchase) within which relevant merchant return policy is applicable." ;
        rdfs:label    "merchantReturnDays" .

schema:BookStore  rdf:type  rdfs:Class ;
        rdfs:comment     "A bookstore." ;
        rdfs:label       "BookStore" ;
        rdfs:subClassOf  schema:Store .

schema:recommendedIntake
        rdf:type      rdf:Property ;
        rdfs:comment  "Recommended intake of this supplement for a given population as defined by a specific recommending authority." ;
        rdfs:label    "recommendedIntake" .

schema:Dentist  rdf:type  rdfs:Class ;
        rdfs:comment     "A dentist." ;
        rdfs:label       "Dentist" ;
        rdfs:subClassOf  schema:MedicalBusiness , schema:LocalBusiness , schema:MedicalOrganization .

schema:inLanguage  rdf:type  rdf:Property ;
        rdfs:comment  "The language of the content or performance or used in an action. Please use one of the language codes from the [IETF BCP 47 standard](http://tools.ietf.org/html/bcp47). See also [[availableLanguage]]." ;
        rdfs:label    "inLanguage" .

schema:ProgramMembership
        rdf:type         rdfs:Class ;
        rdfs:comment     "Used to describe membership in a loyalty programs (e.g. \"StarAliance\"), traveler clubs (e.g. \"AAA\"), purchase clubs (\"Safeway Club\"), etc." ;
        rdfs:label       "ProgramMembership" ;
        rdfs:subClassOf  schema:Intangible .

schema:doesNotShip  rdf:type  rdf:Property ;
        rdfs:comment  "Indicates when shipping to a particular [[shippingDestination]] is not available." ;
        rdfs:label    "doesNotShip" .

schema:targetProduct  rdf:type  rdf:Property ;
        rdfs:comment  "Target Operating System / Product to which the code applies.  If applies to several versions, just the product name can be used." ;
        rdfs:label    "targetProduct" .

schema:reservationFor
        rdf:type      rdf:Property ;
        rdfs:comment  "The thing -- flight, event, restaurant,etc. being reserved." ;
        rdfs:label    "reservationFor" .

schema:reviews  rdf:type  rdf:Property ;
        rdfs:comment  "Review of the item." ;
        rdfs:label    "reviews" .

schema:playMode  rdf:type  rdf:Property ;
        rdfs:comment  "Indicates whether this game is multi-player, co-op or single-player.  The game can be marked as multi-player, co-op and single-player at the same time." ;
        rdfs:label    "playMode" .

schema:Nursing  rdf:type  rdfs:Class ;
        rdfs:comment     "A health profession of a person formally educated and trained in the care of the sick or infirm person." ;
        rdfs:label       "Nursing" ;
        rdfs:subClassOf  schema:MedicalBusiness .

schema:numberOfBedrooms
        rdf:type      rdf:Property ;
        rdfs:comment  "The total integer number of bedrooms in a some [[Accommodation]], [[ApartmentComplex]] or [[FloorPlan]]." ;
        rdfs:label    "numberOfBedrooms" .

schema:ComedyEvent  rdf:type  rdfs:Class ;
        rdfs:comment     "Event type: Comedy event." ;
        rdfs:label       "ComedyEvent" ;
        rdfs:subClassOf  schema:Event .

schema:Blog  rdf:type    rdfs:Class ;
        rdfs:comment     "A blog." ;
        rdfs:label       "Blog" ;
        rdfs:subClassOf  schema:CreativeWork .

schema:addressRegion  rdf:type  rdf:Property ;
        rdfs:comment  "The region in which the locality is, and which is in the country. For example, California or another appropriate first-level [Administrative division](https://en.wikipedia.org/wiki/List_of_administrative_divisions_by_country) " ;
        rdfs:label    "addressRegion" .

schema:publicationType
        rdf:type      rdf:Property ;
        rdfs:comment  "The type of the medical article, taken from the US NLM MeSH publication type catalog. See also [MeSH documentation](http://www.nlm.nih.gov/mesh/pubtypes.html)." ;
        rdfs:label    "publicationType" .

schema:serviceArea  rdf:type  rdf:Property ;
        rdfs:comment  "The geographic area where the service is provided." ;
        rdfs:label    "serviceArea" .

schema:AnatomicalStructure
        rdf:type         rdfs:Class ;
        rdfs:comment     "Any part of the human body, typically a component of an anatomical system. Organs, tissues, and cells are all anatomical structures." ;
        rdfs:label       "AnatomicalStructure" ;
        rdfs:subClassOf  schema:MedicalEntity .

schema:DeactivateAction
        rdf:type         rdfs:Class ;
        rdfs:comment     "The act of stopping or deactivating a device or application (e.g. stopping a timer or turning off a flashlight)." ;
        rdfs:label       "DeactivateAction" ;
        rdfs:subClassOf  schema:ControlAction .

schema:DrugPrescriptionStatus
        rdf:type         rdfs:Class ;
        rdfs:comment     "Indicates whether this drug is available by prescription or over-the-counter." ;
        rdfs:label       "DrugPrescriptionStatus" ;
        rdfs:subClassOf  schema:MedicalEnumeration .

schema:ResearchProject
        rdf:type         rdfs:Class ;
        rdfs:comment     "A Research project." ;
        rdfs:label       "ResearchProject" ;
        rdfs:subClassOf  schema:Project .

schema:permitAudience
        rdf:type      rdf:Property ;
        rdfs:comment  "The target audience for this permit." ;
        rdfs:label    "permitAudience" .

schema:drug  rdf:type  rdf:Property ;
        rdfs:comment  "Specifying a drug or medicine used in a medication procedure." ;
        rdfs:label    "drug" .

schema:knowsLanguage  rdf:type  rdf:Property ;
        rdfs:comment  "Of a [[Person]], and less typically of an [[Organization]], to indicate a known language. We do not distinguish skill levels or reading/writing/speaking/signing here. Use language codes from the [IETF BCP 47 standard](http://tools.ietf.org/html/bcp47)." ;
        rdfs:label    "knowsLanguage" .

schema:activeIngredient
        rdf:type      rdf:Property ;
        rdfs:comment  "An active ingredient, typically chemical compounds and/or biologic substances." ;
        rdfs:label    "activeIngredient" .

schema:additionalName
        rdf:type      rdf:Property ;
        rdfs:comment  "An additional name for a Person, can be used for a middle name." ;
        rdfs:label    "additionalName" .

schema:CovidTestingFacility
        rdf:type         rdfs:Class ;
        rdfs:comment     "A CovidTestingFacility is a [[MedicalClinic]] where testing for the COVID-19 Coronavirus\n      disease is available. If the facility is being made available from an established [[Pharmacy]], [[Hotel]], or other\n      non-medical organization, multiple types can be listed. This makes it easier to re-use existing schema.org information\n      about that place e.g. contact info, address, opening hours. Note that in an emergency, such information may not always be reliable.\n      " ;
        rdfs:label       "CovidTestingFacility" ;
        rdfs:subClassOf  schema:MedicalClinic .

schema:EatAction  rdf:type  rdfs:Class ;
        rdfs:comment     "The act of swallowing solid objects." ;
        rdfs:label       "EatAction" ;
        rdfs:subClassOf  schema:ConsumeAction .

schema:RadioStation  rdf:type  rdfs:Class ;
        rdfs:comment     "A radio station." ;
        rdfs:label       "RadioStation" ;
        rdfs:subClassOf  schema:LocalBusiness .

schema:publication  rdf:type  rdf:Property ;
        rdfs:comment  "A publication event associated with the item." ;
        rdfs:label    "publication" .

schema:HairSalon  rdf:type  rdfs:Class ;
        rdfs:comment     "A hair salon." ;
        rdfs:label       "HairSalon" ;
        rdfs:subClassOf  schema:HealthAndBeautyBusiness .

schema:contentUrl  rdf:type  rdf:Property ;
        rdfs:comment  "Actual bytes of the media object, for example the image file or video file." ;
        rdfs:label    "contentUrl" .

schema:titleEIDR  rdf:type  rdf:Property ;
        rdfs:comment        "An [EIDR](https://eidr.org/) (Entertainment Identifier Registry) [[identifier]] representing at the most general/abstract level, a work of film or television.\n\nFor example, the motion picture known as \"Ghostbusters\" has a titleEIDR of  \"10.5240/7EC7-228A-510A-053E-CBB8-J\". This title (or work) may have several variants, which EIDR calls \"edits\". See [[editEIDR]].\n\nSince schema.org types like [[Movie]] and [[TVEpisode]] can be used for both works and their multiple expressions, it is possible to use [[titleEIDR]] alone (for a general description), or alongside [[editEIDR]] for a more edit-specific description.\n" ;
        rdfs:label          "titleEIDR" ;
        rdfs:subPropertyOf  schema:identifier .

schema:dateline  rdf:type  rdf:Property ;
        rdfs:comment  "A [dateline](https://en.wikipedia.org/wiki/Dateline) is a brief piece of text included in news articles that describes where and when the story was written or filed though the date is often omitted. Sometimes only a placename is provided.\n\nStructured representations of dateline-related information can also be expressed more explicitly using [[locationCreated]] (which represents where a work was created e.g. where a news report was written).  For location depicted or described in the content, use [[contentLocation]].\n\nDateline summaries are oriented more towards human readers than towards automated processing, and can vary substantially. Some examples: \"BEIRUT, Lebanon, June 2.\", \"Paris, France\", \"December 19, 2017 11:43AM Reporting from Washington\", \"Beijing/Moscow\", \"QUEZON CITY, Philippines\".\n      " ;
        rdfs:label    "dateline" .

schema:OccupationalExperienceRequirements
        rdf:type         rdfs:Class ;
        rdfs:comment     "Indicates employment-related experience requirements, e.g. [[monthsOfExperience]]." ;
        rdfs:label       "OccupationalExperienceRequirements" ;
        rdfs:subClassOf  schema:Intangible .

schema:differentialDiagnosis
        rdf:type      rdf:Property ;
        rdfs:comment  "One of a set of differential diagnoses for the condition. Specifically, a closely-related or competing diagnosis typically considered later in the cognitive process whereby this medical condition is distinguished from others most likely responsible for a similar collection of signs and symptoms to reach the most parsimonious diagnosis or diagnoses in a patient." ;
        rdfs:label    "differentialDiagnosis" .

schema:cvdNumICUBeds  rdf:type  rdf:Property ;
        rdfs:comment  "numicubeds - ICU BEDS: Total number of staffed inpatient intensive care unit (ICU) beds." ;
        rdfs:label    "cvdNumICUBeds" .

schema:BusOrCoach  rdf:type  rdfs:Class ;
        rdfs:comment     "A bus (also omnibus or autobus) is a road vehicle designed to carry passengers. Coaches are luxury busses, usually in service for long distance travel." ;
        rdfs:label       "BusOrCoach" ;
        rdfs:subClassOf  schema:Vehicle .

schema:TradeAction  rdf:type  rdfs:Class ;
        rdfs:comment     "The act of participating in an exchange of goods and services for monetary compensation. An agent trades an object, product or service with a participant in exchange for a one time or periodic payment." ;
        rdfs:label       "TradeAction" ;
        rdfs:subClassOf  schema:Action .

schema:ResumeAction  rdf:type  rdfs:Class ;
        rdfs:comment     "The act of resuming a device or application which was formerly paused (e.g. resume music playback or resume a timer)." ;
        rdfs:label       "ResumeAction" ;
        rdfs:subClassOf  schema:ControlAction .

schema:recordingOf  rdf:type  rdf:Property ;
        rdfs:comment  "The composition this track is a recording of." ;
        rdfs:label    "recordingOf" .

schema:MusicRelease  rdf:type  rdfs:Class ;
        rdfs:comment     "A MusicRelease is a specific release of a music album." ;
        rdfs:label       "MusicRelease" ;
        rdfs:subClassOf  schema:MusicPlaylist .

schema:codeRepository
        rdf:type      rdf:Property ;
        rdfs:comment  "Link to the repository where the un-compiled, human readable code and related code is located (SVN, github, CodePlex)." ;
        rdfs:label    "codeRepository" .

schema:AggregateRating
        rdf:type         rdfs:Class ;
        rdfs:comment     "The average rating based on multiple ratings or reviews." ;
        rdfs:label       "AggregateRating" ;
        rdfs:subClassOf  schema:Rating .

schema:isGift  rdf:type  rdf:Property ;
        rdfs:comment  "Was the offer accepted as a gift for someone other than the buyer." ;
        rdfs:label    "isGift" .

schema:MeasurementTypeEnumeration
        rdf:type         rdfs:Class ;
        rdfs:comment     "Enumeration of common measurement types (or dimensions), for example \"chest\" for a person, \"inseam\" for pants, \"gauge\" for screws, or \"wheel\" for bicycles." ;
        rdfs:label       "MeasurementTypeEnumeration" ;
        rdfs:subClassOf  schema:Enumeration .

schema:MarryAction  rdf:type  rdfs:Class ;
        rdfs:comment     "The act of marrying a person." ;
        rdfs:label       "MarryAction" ;
        rdfs:subClassOf  schema:InteractAction .

schema:subTrip  rdf:type  rdf:Property ;
        rdfs:comment  "Identifies a [[Trip]] that is a subTrip of this Trip.  For example Day 1, Day 2, etc. of a multi-day trip." ;
        rdfs:label    "subTrip" .

schema:departureTerminal
        rdf:type      rdf:Property ;
        rdfs:comment  "Identifier of the flight's departure terminal." ;
        rdfs:label    "departureTerminal" .

schema:isicV4  rdf:type  rdf:Property ;
        rdfs:comment  "The International Standard of Industrial Classification of All Economic Activities (ISIC), Revision 4 code for a particular organization, business person, or place." ;
        rdfs:label    "isicV4" .

schema:loanPaymentFrequency
        rdf:type      rdf:Property ;
        rdfs:comment  "Frequency of payments due, i.e. number of months between payments. This is defined as a frequency, i.e. the reciprocal of a period of time." ;
        rdfs:label    "loanPaymentFrequency" .

schema:gameLocation  rdf:type  rdf:Property ;
        rdfs:comment  "Real or fictional location of the game (or part of game)." ;
        rdfs:label    "gameLocation" .

schema:renegotiableLoan
        rdf:type      rdf:Property ;
        rdfs:comment  "Whether the terms for payment of interest can be renegotiated during the life of the loan." ;
        rdfs:label    "renegotiableLoan" .

schema:driveWheelConfiguration
        rdf:type      rdf:Property ;
        rdfs:comment  "The drive wheel configuration, i.e. which roadwheels will receive torque from the vehicle's engine via the drivetrain." ;
        rdfs:label    "driveWheelConfiguration" .

schema:Trip  rdf:type    rdfs:Class ;
        rdfs:comment     "A trip or journey. An itinerary of visits to one or more places." ;
        rdfs:label       "Trip" ;
        rdfs:subClassOf  schema:Intangible .

schema:Researcher  rdf:type  rdfs:Class ;
        rdfs:comment     "Researchers." ;
        rdfs:label       "Researcher" ;
        rdfs:subClassOf  schema:Audience .

schema:marginOfError  rdf:type  rdf:Property ;
        rdfs:comment  "A marginOfError for an [[Observation]]." ;
        rdfs:label    "marginOfError" .

schema:landlord  rdf:type   rdf:Property ;
        rdfs:comment        "A sub property of participant. The owner of the real estate property." ;
        rdfs:label          "landlord" ;
        rdfs:subPropertyOf  schema:participant .

schema:identifyingExam
        rdf:type      rdf:Property ;
        rdfs:comment  "A physical examination that can identify this sign." ;
        rdfs:label    "identifyingExam" .

schema:broadcastAffiliateOf
        rdf:type      rdf:Property ;
        rdfs:comment  "The media network(s) whose content is broadcast on this station." ;
        rdfs:label    "broadcastAffiliateOf" .

schema:additionalVariable
        rdf:type      rdf:Property ;
        rdfs:comment  "Any additional component of the exercise prescription that may need to be articulated to the patient. This may include the order of exercises, the number of repetitions of movement, quantitative distance, progressions over time, etc." ;
        rdfs:label    "additionalVariable" .

schema:subReservation
        rdf:type      rdf:Property ;
        rdfs:comment  "The individual reservations included in the package. Typically a repeated property." ;
        rdfs:label    "subReservation" .

schema:winner  rdf:type     rdf:Property ;
        rdfs:comment        "A sub property of participant. The winner of the action." ;
        rdfs:label          "winner" ;
        rdfs:subPropertyOf  schema:participant .

schema:datePosted  rdf:type  rdf:Property ;
        rdfs:comment  "Publication date of an online listing." ;
        rdfs:label    "datePosted" .
